@prefix cci: <http://vocab.ceda.ac.uk/ontology/cci#> .
@prefix cci-collection: <http://vocab.ceda.ac.uk/collection/cci/> .
@prefix cci-scheme: <http://vocab.ceda.ac.uk/scheme/cci/> .
@prefix dc: <http://purl.org/dc/elements/1.1/> .
@prefix owl: <http://www.w3.org/2002/07/owl#> .
@prefix rdfs: <http://www.w3.org/2000/01/rdf-schema#> .
@prefix skos: <http://www.w3.org/2004/02/skos/core#> .
@prefix vann: <http://purl.org/vocab/vann/> .

cci-collection:dataType a skos:Collection ;
    dc:creator "Science and Technology Facilities Council" ;
    dc:date "2025-01-23" ;
    dc:description "The main data type in a data set used by the ESA Climate Change Initiative (CCI)." ;
    dc:publisher "STFC"@en ;
    dc:title "Geophysical Quantity" ;
    rdfs:comment "This collection represents the data types used by the CCI project" ;
    owl:versionInfo "0.0.1" ;
    skos:definition "The main data type in a data set used by the ESA Climate Change Initiative (CCI)."@en ;
    skos:member <http://vocab.ceda.ac.uk/collection/cci/dataType/dtype_aai>,
        <http://vocab.ceda.ac.uk/collection/cci/dataType/dtype_adg>,
        <http://vocab.ceda.ac.uk/collection/cci/dataType/dtype_adt>,
        <http://vocab.ceda.ac.uk/collection/cci/dataType/dtype_aerProd>,
        <http://vocab.ceda.ac.uk/collection/cci/dataType/dtype_aex>,
        <http://vocab.ceda.ac.uk/collection/cci/dataType/dtype_agb>,
        <http://vocab.ceda.ac.uk/collection/cci/dataType/dtype_alb>,
        <http://vocab.ceda.ac.uk/collection/cci/dataType/dtype_all>,
        <http://vocab.ceda.ac.uk/collection/cci/dataType/dtype_alt>,
        <http://vocab.ceda.ac.uk/collection/cci/dataType/dtype_aod>,
        <http://vocab.ceda.ac.uk/collection/cci/dataType/dtype_aph>,
        <http://vocab.ceda.ac.uk/collection/cci/dataType/dtype_atot>,
        <http://vocab.ceda.ac.uk/collection/cci/dataType/dtype_aty>,
        <http://vocab.ceda.ac.uk/collection/cci/dataType/dtype_ba>,
        <http://vocab.ceda.ac.uk/collection/cci/dataType/dtype_bb>,
        <http://vocab.ceda.ac.uk/collection/cci/dataType/dtype_cer>,
        <http://vocab.ceda.ac.uk/collection/cci/dataType/dtype_cfc>,
        <http://vocab.ceda.ac.uk/collection/cci/dataType/dtype_cfl>,
        <http://vocab.ceda.ac.uk/collection/cci/dataType/dtype_ch4>,
        <http://vocab.ceda.ac.uk/collection/cci/dataType/dtype_chlorA>,
        <http://vocab.ceda.ac.uk/collection/cci/dataType/dtype_cldProd>,
        <http://vocab.ceda.ac.uk/collection/cci/dataType/dtype_co2>,
        <http://vocab.ceda.ac.uk/collection/cci/dataType/dtype_cot>,
        <http://vocab.ceda.ac.uk/collection/cci/dataType/dtype_cth>,
        <http://vocab.ceda.ac.uk/collection/cci/dataType/dtype_ctp>,
        <http://vocab.ceda.ac.uk/collection/cci/dataType/dtype_ctt>,
        <http://vocab.ceda.ac.uk/collection/cci/dataType/dtype_ga>,
        <http://vocab.ceda.ac.uk/collection/cci/dataType/dtype_gll>,
        <http://vocab.ceda.ac.uk/collection/cci/dataType/dtype_gmb>,
        <http://vocab.ceda.ac.uk/collection/cci/dataType/dtype_gtd>,
        <http://vocab.ceda.ac.uk/collection/cci/dataType/dtype_iop>,
        <http://vocab.ceda.ac.uk/collection/cci/dataType/dtype_iv>,
        <http://vocab.ceda.ac.uk/collection/cci/dataType/dtype_iwp>,
        <http://vocab.ceda.ac.uk/collection/cci/dataType/dtype_jch>,
        <http://vocab.ceda.ac.uk/collection/cci/dataType/dtype_k_490>,
        <http://vocab.ceda.ac.uk/collection/cci/dataType/dtype_lai>,
        <http://vocab.ceda.ac.uk/collection/cci/dataType/dtype_lcchange>,
        <http://vocab.ceda.ac.uk/collection/cci/dataType/dtype_lccs>,
        <http://vocab.ceda.ac.uk/collection/cci/dataType/dtype_lkProds>,
        <http://vocab.ceda.ac.uk/collection/cci/dataType/dtype_lp>,
        <http://vocab.ceda.ac.uk/collection/cci/dataType/dtype_lst>,
        <http://vocab.ceda.ac.uk/collection/cci/dataType/dtype_lwp>,
        <http://vocab.ceda.ac.uk/collection/cci/dataType/dtype_map>,
        <http://vocab.ceda.ac.uk/collection/cci/dataType/dtype_msl>,
        <http://vocab.ceda.ac.uk/collection/cci/dataType/dtype_msla>,
        <http://vocab.ceda.ac.uk/collection/cci/dataType/dtype_mslamph>,
        <http://vocab.ceda.ac.uk/collection/cci/dataType/dtype_msltr>,
        <http://vocab.ceda.ac.uk/collection/cci/dataType/dtype_ndvi>,
        <http://vocab.ceda.ac.uk/collection/cci/dataType/dtype_nlw>,
        <http://vocab.ceda.ac.uk/collection/cci/dataType/dtype_np>,
        <http://vocab.ceda.ac.uk/collection/cci/dataType/dtype_ocProd>,
        <http://vocab.ceda.ac.uk/collection/cci/dataType/dtype_pfr>,
        <http://vocab.ceda.ac.uk/collection/cci/dataType/dtype_pft>,
        <http://vocab.ceda.ac.uk/collection/cci/dataType/dtype_rrs>,
        <http://vocab.ceda.ac.uk/collection/cci/dataType/dtype_scfg>,
        <http://vocab.ceda.ac.uk/collection/cci/dataType/dtype_scfv>,
        <http://vocab.ceda.ac.uk/collection/cci/dataType/dtype_sec>,
        <http://vocab.ceda.ac.uk/collection/cci/dataType/dtype_sic>,
        <http://vocab.ceda.ac.uk/collection/cci/dataType/dtype_sie>,
        <http://vocab.ceda.ac.uk/collection/cci/dataType/dtype_sit>,
        <http://vocab.ceda.ac.uk/collection/cci/dataType/dtype_sla>,
        <http://vocab.ceda.ac.uk/collection/cci/dataType/dtype_snow>,
        <http://vocab.ceda.ac.uk/collection/cci/dataType/dtype_sr>,
        <http://vocab.ceda.ac.uk/collection/cci/dataType/dtype_ssh>,
        <http://vocab.ceda.ac.uk/collection/cci/dataType/dtype_ssms>,
        <http://vocab.ceda.ac.uk/collection/cci/dataType/dtype_ssmsa>,
        <http://vocab.ceda.ac.uk/collection/cci/dataType/dtype_ssmv>,
        <http://vocab.ceda.ac.uk/collection/cci/dataType/dtype_ssmva>,
        <http://vocab.ceda.ac.uk/collection/cci/dataType/dtype_sss>,
        <http://vocab.ceda.ac.uk/collection/cci/dataType/dtype_sstDepth>,
        <http://vocab.ceda.ac.uk/collection/cci/dataType/dtype_sstFnd>,
        <http://vocab.ceda.ac.uk/collection/cci/dataType/dtype_sstInt>,
        <http://vocab.ceda.ac.uk/collection/cci/dataType/dtype_sstSkin>,
        <http://vocab.ceda.ac.uk/collection/cci/dataType/dtype_sstSubsk>,
        <http://vocab.ceda.ac.uk/collection/cci/dataType/dtype_swe>,
        <http://vocab.ceda.ac.uk/collection/cci/dataType/dtype_swh>,
        <http://vocab.ceda.ac.uk/collection/cci/dataType/dtype_swis>,
        <http://vocab.ceda.ac.uk/collection/cci/dataType/dtype_swisa>,
        <http://vocab.ceda.ac.uk/collection/cci/dataType/dtype_swiv>,
        <http://vocab.ceda.ac.uk/collection/cci/dataType/dtype_swiva>,
        <http://vocab.ceda.ac.uk/collection/cci/dataType/dtype_tc>,
        <http://vocab.ceda.ac.uk/collection/cci/dataType/dtype_tcwv>,
        <http://vocab.ceda.ac.uk/collection/cci/dataType/dtype_uncert>,
        <http://vocab.ceda.ac.uk/collection/cci/dataType/dtype_unspecified>,
        <http://vocab.ceda.ac.uk/collection/cci/dataType/dtype_v>,
        <http://vocab.ceda.ac.uk/collection/cci/dataType/dtype_vp>,
        <http://vocab.ceda.ac.uk/collection/cci/dataType/dtype_wb>,
        <http://vocab.ceda.ac.uk/collection/cci/dataType/dtype_wl> ;
    skos:prefLabel "Geophysical Quantity"@en .

cci-collection:ecv a skos:Collection ;
    dc:creator "Science and Technology Facilities Council" ;
    dc:date "2025-01-23" ;
    dc:description "The Essential Climate Variable (ECVs) in the ESA Climate Change Initiative (CCI)." ;
    dc:publisher "STFC"@en ;
    dc:title "ECV" ;
    rdfs:comment "This collection represents the ECVs used by the CCI project" ;
    owl:versionInfo "0.0.1" ;
    skos:definition "The Essential Climate Variable (ECVs) in the ESA Climate Change Initiative (CCI)."@en ;
    skos:member <http://vocab.ceda.ac.uk/collection/cci/ecv/cciecv_aerosol>,
        <http://vocab.ceda.ac.uk/collection/cci/ecv/cciecv_biomass>,
        <http://vocab.ceda.ac.uk/collection/cci/ecv/cciecv_cloud>,
        <http://vocab.ceda.ac.uk/collection/cci/ecv/cciecv_fire>,
        <http://vocab.ceda.ac.uk/collection/cci/ecv/cciecv_ghg>,
        <http://vocab.ceda.ac.uk/collection/cci/ecv/cciecv_glaciers>,
        <http://vocab.ceda.ac.uk/collection/cci/ecv/cciecv_iceSheet>,
        <http://vocab.ceda.ac.uk/collection/cci/ecv/cciecv_lakes>,
        <http://vocab.ceda.ac.uk/collection/cci/ecv/cciecv_landCov>,
        <http://vocab.ceda.ac.uk/collection/cci/ecv/cciecv_landSurfTemp>,
        <http://vocab.ceda.ac.uk/collection/cci/ecv/cciecv_oceanCol>,
        <http://vocab.ceda.ac.uk/collection/cci/ecv/cciecv_ozone>,
        <http://vocab.ceda.ac.uk/collection/cci/ecv/cciecv_permafrost>,
        <http://vocab.ceda.ac.uk/collection/cci/ecv/cciecv_riverDischarge>,
        <http://vocab.ceda.ac.uk/collection/cci/ecv/cciecv_salinity>,
        <http://vocab.ceda.ac.uk/collection/cci/ecv/cciecv_seaIce>,
        <http://vocab.ceda.ac.uk/collection/cci/ecv/cciecv_seaLevel>,
        <http://vocab.ceda.ac.uk/collection/cci/ecv/cciecv_seaState>,
        <http://vocab.ceda.ac.uk/collection/cci/ecv/cciecv_snow>,
        <http://vocab.ceda.ac.uk/collection/cci/ecv/cciecv_soilMst>,
        <http://vocab.ceda.ac.uk/collection/cci/ecv/cciecv_sst>,
        <http://vocab.ceda.ac.uk/collection/cci/ecv/cciecv_vegParam>,
        <http://vocab.ceda.ac.uk/collection/cci/ecv/cciecv_waterVapour> ;
    skos:prefLabel "ECV"@en .

cci-collection:freq a skos:Collection ;
    dc:creator "Science and Technology Facilities Council" ;
    dc:date "2025-01-23" ;
    dc:description "Temporal frequencies of data from the ESA Climate Change Initiative (CCI)." ;
    dc:publisher "STFC"@en ;
    dc:title "Frequency" ;
    rdfs:comment "This collection represents the frequencies used by the CCI project" ;
    owl:versionInfo "0.0.1" ;
    skos:definition "Temporal frequencies of data from the ESA Climate Change Initiative (CCI)."@en ;
    skos:member <http://vocab.ceda.ac.uk/collection/cci/freq/feq_min>,
        <http://vocab.ceda.ac.uk/collection/cci/freq/freq_10day>,
        <http://vocab.ceda.ac.uk/collection/cci/freq/freq_13yr>,
        <http://vocab.ceda.ac.uk/collection/cci/freq/freq_15day>,
        <http://vocab.ceda.ac.uk/collection/cci/freq/freq_3hr>,
        <http://vocab.ceda.ac.uk/collection/cci/freq/freq_5day>,
        <http://vocab.ceda.ac.uk/collection/cci/freq/freq_5yr>,
        <http://vocab.ceda.ac.uk/collection/cci/freq/freq_8day>,
        <http://vocab.ceda.ac.uk/collection/cci/freq/freq_clim>,
        <http://vocab.ceda.ac.uk/collection/cci/freq/freq_day>,
        <http://vocab.ceda.ac.uk/collection/cci/freq/freq_hr>,
        <http://vocab.ceda.ac.uk/collection/cci/freq/freq_mon>,
        <http://vocab.ceda.ac.uk/collection/cci/freq/freq_sat_orb>,
        <http://vocab.ceda.ac.uk/collection/cci/freq/freq_sec>,
        <http://vocab.ceda.ac.uk/collection/cci/freq/freq_unspecified>,
        <http://vocab.ceda.ac.uk/collection/cci/freq/freq_week>,
        <http://vocab.ceda.ac.uk/collection/cci/freq/freq_yr> ;
    skos:prefLabel "Frequency"@en .

cci-collection:org a skos:Collection ;
    dc:creator "Science and Technology Facilities Council" ;
    dc:date "2025-01-23" ;
    dc:description "Organisations (institutions) that are involved in production of data for the ESA Climate Change Initiative (CCI)." ;
    dc:publisher "STFC"@en ;
    dc:title "Institute" ;
    rdfs:comment "This collection represents the organisations in the CCI project" ;
    owl:versionInfo "0.0.1" ;
    skos:definition "Organisations (institutions) that are involved in production of data for the ESA Climate Change Initiative (CCI)."@en ;
    skos:member <http://vocab.ceda.ac.uk/collection/cci/org/org01>,
        <http://vocab.ceda.ac.uk/collection/cci/org/org02>,
        <http://vocab.ceda.ac.uk/collection/cci/org/org03>,
        <http://vocab.ceda.ac.uk/collection/cci/org/org04>,
        <http://vocab.ceda.ac.uk/collection/cci/org/org05>,
        <http://vocab.ceda.ac.uk/collection/cci/org/org06>,
        <http://vocab.ceda.ac.uk/collection/cci/org/org07>,
        <http://vocab.ceda.ac.uk/collection/cci/org/org08>,
        <http://vocab.ceda.ac.uk/collection/cci/org/org09>,
        <http://vocab.ceda.ac.uk/collection/cci/org/org10>,
        <http://vocab.ceda.ac.uk/collection/cci/org/org100>,
        <http://vocab.ceda.ac.uk/collection/cci/org/org101>,
        <http://vocab.ceda.ac.uk/collection/cci/org/org102>,
        <http://vocab.ceda.ac.uk/collection/cci/org/org103>,
        <http://vocab.ceda.ac.uk/collection/cci/org/org104>,
        <http://vocab.ceda.ac.uk/collection/cci/org/org105>,
        <http://vocab.ceda.ac.uk/collection/cci/org/org106>,
        <http://vocab.ceda.ac.uk/collection/cci/org/org107>,
        <http://vocab.ceda.ac.uk/collection/cci/org/org11>,
        <http://vocab.ceda.ac.uk/collection/cci/org/org12>,
        <http://vocab.ceda.ac.uk/collection/cci/org/org13>,
        <http://vocab.ceda.ac.uk/collection/cci/org/org14>,
        <http://vocab.ceda.ac.uk/collection/cci/org/org15>,
        <http://vocab.ceda.ac.uk/collection/cci/org/org16>,
        <http://vocab.ceda.ac.uk/collection/cci/org/org17>,
        <http://vocab.ceda.ac.uk/collection/cci/org/org18>,
        <http://vocab.ceda.ac.uk/collection/cci/org/org19>,
        <http://vocab.ceda.ac.uk/collection/cci/org/org20>,
        <http://vocab.ceda.ac.uk/collection/cci/org/org21>,
        <http://vocab.ceda.ac.uk/collection/cci/org/org22>,
        <http://vocab.ceda.ac.uk/collection/cci/org/org23>,
        <http://vocab.ceda.ac.uk/collection/cci/org/org24>,
        <http://vocab.ceda.ac.uk/collection/cci/org/org25>,
        <http://vocab.ceda.ac.uk/collection/cci/org/org26>,
        <http://vocab.ceda.ac.uk/collection/cci/org/org27>,
        <http://vocab.ceda.ac.uk/collection/cci/org/org28>,
        <http://vocab.ceda.ac.uk/collection/cci/org/org29>,
        <http://vocab.ceda.ac.uk/collection/cci/org/org30>,
        <http://vocab.ceda.ac.uk/collection/cci/org/org31>,
        <http://vocab.ceda.ac.uk/collection/cci/org/org32>,
        <http://vocab.ceda.ac.uk/collection/cci/org/org33>,
        <http://vocab.ceda.ac.uk/collection/cci/org/org34>,
        <http://vocab.ceda.ac.uk/collection/cci/org/org35>,
        <http://vocab.ceda.ac.uk/collection/cci/org/org36>,
        <http://vocab.ceda.ac.uk/collection/cci/org/org37>,
        <http://vocab.ceda.ac.uk/collection/cci/org/org38>,
        <http://vocab.ceda.ac.uk/collection/cci/org/org39>,
        <http://vocab.ceda.ac.uk/collection/cci/org/org40>,
        <http://vocab.ceda.ac.uk/collection/cci/org/org41>,
        <http://vocab.ceda.ac.uk/collection/cci/org/org42>,
        <http://vocab.ceda.ac.uk/collection/cci/org/org43>,
        <http://vocab.ceda.ac.uk/collection/cci/org/org44>,
        <http://vocab.ceda.ac.uk/collection/cci/org/org45>,
        <http://vocab.ceda.ac.uk/collection/cci/org/org46>,
        <http://vocab.ceda.ac.uk/collection/cci/org/org47>,
        <http://vocab.ceda.ac.uk/collection/cci/org/org48>,
        <http://vocab.ceda.ac.uk/collection/cci/org/org49>,
        <http://vocab.ceda.ac.uk/collection/cci/org/org50>,
        <http://vocab.ceda.ac.uk/collection/cci/org/org51>,
        <http://vocab.ceda.ac.uk/collection/cci/org/org52>,
        <http://vocab.ceda.ac.uk/collection/cci/org/org53>,
        <http://vocab.ceda.ac.uk/collection/cci/org/org54>,
        <http://vocab.ceda.ac.uk/collection/cci/org/org55>,
        <http://vocab.ceda.ac.uk/collection/cci/org/org56>,
        <http://vocab.ceda.ac.uk/collection/cci/org/org57>,
        <http://vocab.ceda.ac.uk/collection/cci/org/org58>,
        <http://vocab.ceda.ac.uk/collection/cci/org/org59>,
        <http://vocab.ceda.ac.uk/collection/cci/org/org60>,
        <http://vocab.ceda.ac.uk/collection/cci/org/org61>,
        <http://vocab.ceda.ac.uk/collection/cci/org/org62>,
        <http://vocab.ceda.ac.uk/collection/cci/org/org63>,
        <http://vocab.ceda.ac.uk/collection/cci/org/org64>,
        <http://vocab.ceda.ac.uk/collection/cci/org/org65>,
        <http://vocab.ceda.ac.uk/collection/cci/org/org66>,
        <http://vocab.ceda.ac.uk/collection/cci/org/org67>,
        <http://vocab.ceda.ac.uk/collection/cci/org/org68>,
        <http://vocab.ceda.ac.uk/collection/cci/org/org69>,
        <http://vocab.ceda.ac.uk/collection/cci/org/org70>,
        <http://vocab.ceda.ac.uk/collection/cci/org/org71>,
        <http://vocab.ceda.ac.uk/collection/cci/org/org72>,
        <http://vocab.ceda.ac.uk/collection/cci/org/org73>,
        <http://vocab.ceda.ac.uk/collection/cci/org/org74>,
        <http://vocab.ceda.ac.uk/collection/cci/org/org75>,
        <http://vocab.ceda.ac.uk/collection/cci/org/org76>,
        <http://vocab.ceda.ac.uk/collection/cci/org/org77>,
        <http://vocab.ceda.ac.uk/collection/cci/org/org78>,
        <http://vocab.ceda.ac.uk/collection/cci/org/org79>,
        <http://vocab.ceda.ac.uk/collection/cci/org/org80>,
        <http://vocab.ceda.ac.uk/collection/cci/org/org81>,
        <http://vocab.ceda.ac.uk/collection/cci/org/org82>,
        <http://vocab.ceda.ac.uk/collection/cci/org/org83>,
        <http://vocab.ceda.ac.uk/collection/cci/org/org84>,
        <http://vocab.ceda.ac.uk/collection/cci/org/org85>,
        <http://vocab.ceda.ac.uk/collection/cci/org/org86>,
        <http://vocab.ceda.ac.uk/collection/cci/org/org87>,
        <http://vocab.ceda.ac.uk/collection/cci/org/org88>,
        <http://vocab.ceda.ac.uk/collection/cci/org/org89>,
        <http://vocab.ceda.ac.uk/collection/cci/org/org90>,
        <http://vocab.ceda.ac.uk/collection/cci/org/org91>,
        <http://vocab.ceda.ac.uk/collection/cci/org/org92>,
        <http://vocab.ceda.ac.uk/collection/cci/org/org93>,
        <http://vocab.ceda.ac.uk/collection/cci/org/org94>,
        <http://vocab.ceda.ac.uk/collection/cci/org/org95>,
        <http://vocab.ceda.ac.uk/collection/cci/org/org96>,
        <http://vocab.ceda.ac.uk/collection/cci/org/org97>,
        <http://vocab.ceda.ac.uk/collection/cci/org/org98>,
        <http://vocab.ceda.ac.uk/collection/cci/org/org99> ;
    skos:prefLabel "Institute"@en .

cci-collection:platform a skos:Collection ;
    dc:creator "Science and Technology Facilities Council" ;
    dc:date "2025-01-23" ;
    dc:description "The platforms that have been used in the collection of data for the ESA Climate Change Initiative (CCI)." ;
    dc:publisher "STFC"@en ;
    dc:title "Platform" ;
    rdfs:comment "This collection represents the platforms used by the CCI project" ;
    owl:versionInfo "0.0.1" ;
    skos:definition "The platforms that have been used in the collection of data for the ESA Climate Change Initiative (CCI)."@en ;
    skos:member <http://vocab.ceda.ac.uk/collection/cci/platform/plat_FY-3A>,
        <http://vocab.ceda.ac.uk/collection/cci/platform/plat_FY-3B>,
        <http://vocab.ceda.ac.uk/collection/cci/platform/plat_FY-3C>,
        <http://vocab.ceda.ac.uk/collection/cci/platform/plat_FY-3D>,
        <http://vocab.ceda.ac.uk/collection/cci/platform/plat_FY-3E>,
        <http://vocab.ceda.ac.uk/collection/cci/platform/plat_FY-3F>,
        <http://vocab.ceda.ac.uk/collection/cci/platform/plat_FY-3G>,
        <http://vocab.ceda.ac.uk/collection/cci/platform/plat_alos>,
        <http://vocab.ceda.ac.uk/collection/cci/platform/plat_alos-2>,
        <http://vocab.ceda.ac.uk/collection/cci/platform/plat_alos-3>,
        <http://vocab.ceda.ac.uk/collection/cci/platform/plat_aqua>,
        <http://vocab.ceda.ac.uk/collection/cci/platform/plat_aura>,
        <http://vocab.ceda.ac.uk/collection/cci/platform/plat_coriolis>,
        <http://vocab.ceda.ac.uk/collection/cci/platform/plat_cryosat2>,
        <http://vocab.ceda.ac.uk/collection/cci/platform/plat_csk1>,
        <http://vocab.ceda.ac.uk/collection/cci/platform/plat_csk2>,
        <http://vocab.ceda.ac.uk/collection/cci/platform/plat_csk3>,
        <http://vocab.ceda.ac.uk/collection/cci/platform/plat_csk4>,
        <http://vocab.ceda.ac.uk/collection/cci/platform/plat_dmsp_F01>,
        <http://vocab.ceda.ac.uk/collection/cci/platform/plat_dmsp_F02>,
        <http://vocab.ceda.ac.uk/collection/cci/platform/plat_dmsp_F03>,
        <http://vocab.ceda.ac.uk/collection/cci/platform/plat_dmsp_F04>,
        <http://vocab.ceda.ac.uk/collection/cci/platform/plat_dmsp_F05>,
        <http://vocab.ceda.ac.uk/collection/cci/platform/plat_dmsp_F06>,
        <http://vocab.ceda.ac.uk/collection/cci/platform/plat_dmsp_F07>,
        <http://vocab.ceda.ac.uk/collection/cci/platform/plat_dmsp_F08>,
        <http://vocab.ceda.ac.uk/collection/cci/platform/plat_dmsp_F09>,
        <http://vocab.ceda.ac.uk/collection/cci/platform/plat_dmsp_F10>,
        <http://vocab.ceda.ac.uk/collection/cci/platform/plat_dmsp_F11>,
        <http://vocab.ceda.ac.uk/collection/cci/platform/plat_dmsp_F12>,
        <http://vocab.ceda.ac.uk/collection/cci/platform/plat_dmsp_F13>,
        <http://vocab.ceda.ac.uk/collection/cci/platform/plat_dmsp_F14>,
        <http://vocab.ceda.ac.uk/collection/cci/platform/plat_dmsp_F15>,
        <http://vocab.ceda.ac.uk/collection/cci/platform/plat_dmsp_F16>,
        <http://vocab.ceda.ac.uk/collection/cci/platform/plat_dmsp_F17>,
        <http://vocab.ceda.ac.uk/collection/cci/platform/plat_dmsp_F18>,
        <http://vocab.ceda.ac.uk/collection/cci/platform/plat_dmsp_F19>,
        <http://vocab.ceda.ac.uk/collection/cci/platform/plat_dmsp_S20>,
        <http://vocab.ceda.ac.uk/collection/cci/platform/plat_envisat>,
        <http://vocab.ceda.ac.uk/collection/cci/platform/plat_ers1>,
        <http://vocab.ceda.ac.uk/collection/cci/platform/plat_ers2>,
        <http://vocab.ceda.ac.uk/collection/cci/platform/plat_gcomW1>,
        <http://vocab.ceda.ac.uk/collection/cci/platform/plat_gcomW2>,
        <http://vocab.ceda.ac.uk/collection/cci/platform/plat_gcomW3>,
        <http://vocab.ceda.ac.uk/collection/cci/platform/plat_geosat>,
        <http://vocab.ceda.ac.uk/collection/cci/platform/plat_gfo>,
        <http://vocab.ceda.ac.uk/collection/cci/platform/plat_goes_01>,
        <http://vocab.ceda.ac.uk/collection/cci/platform/plat_goes_02>,
        <http://vocab.ceda.ac.uk/collection/cci/platform/plat_goes_03>,
        <http://vocab.ceda.ac.uk/collection/cci/platform/plat_goes_04>,
        <http://vocab.ceda.ac.uk/collection/cci/platform/plat_goes_05>,
        <http://vocab.ceda.ac.uk/collection/cci/platform/plat_goes_06>,
        <http://vocab.ceda.ac.uk/collection/cci/platform/plat_goes_07>,
        <http://vocab.ceda.ac.uk/collection/cci/platform/plat_goes_08>,
        <http://vocab.ceda.ac.uk/collection/cci/platform/plat_goes_09>,
        <http://vocab.ceda.ac.uk/collection/cci/platform/plat_goes_09_bk>,
        <http://vocab.ceda.ac.uk/collection/cci/platform/plat_goes_10>,
        <http://vocab.ceda.ac.uk/collection/cci/platform/plat_goes_10_SA>,
        <http://vocab.ceda.ac.uk/collection/cci/platform/plat_goes_11>,
        <http://vocab.ceda.ac.uk/collection/cci/platform/plat_goes_12>,
        <http://vocab.ceda.ac.uk/collection/cci/platform/plat_goes_12_SA>,
        <http://vocab.ceda.ac.uk/collection/cci/platform/plat_goes_13>,
        <http://vocab.ceda.ac.uk/collection/cci/platform/plat_goes_14>,
        <http://vocab.ceda.ac.uk/collection/cci/platform/plat_goes_15>,
        <http://vocab.ceda.ac.uk/collection/cci/platform/plat_goes_16>,
        <http://vocab.ceda.ac.uk/collection/cci/platform/plat_goes_17>,
        <http://vocab.ceda.ac.uk/collection/cci/platform/plat_goes_T>,
        <http://vocab.ceda.ac.uk/collection/cci/platform/plat_goes_U>,
        <http://vocab.ceda.ac.uk/collection/cci/platform/plat_gosat>,
        <http://vocab.ceda.ac.uk/collection/cci/platform/plat_gosat-2>,
        <http://vocab.ceda.ac.uk/collection/cci/platform/plat_gpm>,
        <http://vocab.ceda.ac.uk/collection/cci/platform/plat_grace>,
        <http://vocab.ceda.ac.uk/collection/cci/platform/plat_himawari-6>,
        <http://vocab.ceda.ac.uk/collection/cci/platform/plat_himawari-7>,
        <http://vocab.ceda.ac.uk/collection/cci/platform/plat_hrws_sar>,
        <http://vocab.ceda.ac.uk/collection/cci/platform/plat_icesat>,
        <http://vocab.ceda.ac.uk/collection/cci/platform/plat_icesat-2>,
        <http://vocab.ceda.ac.uk/collection/cci/platform/plat_jason1>,
        <http://vocab.ceda.ac.uk/collection/cci/platform/plat_jason2>,
        <http://vocab.ceda.ac.uk/collection/cci/platform/plat_jason3>,
        <http://vocab.ceda.ac.uk/collection/cci/platform/plat_landsat_1>,
        <http://vocab.ceda.ac.uk/collection/cci/platform/plat_landsat_2>,
        <http://vocab.ceda.ac.uk/collection/cci/platform/plat_landsat_3>,
        <http://vocab.ceda.ac.uk/collection/cci/platform/plat_landsat_4>,
        <http://vocab.ceda.ac.uk/collection/cci/platform/plat_landsat_5>,
        <http://vocab.ceda.ac.uk/collection/cci/platform/plat_landsat_6>,
        <http://vocab.ceda.ac.uk/collection/cci/platform/plat_landsat_7>,
        <http://vocab.ceda.ac.uk/collection/cci/platform/plat_landsat_8>,
        <http://vocab.ceda.ac.uk/collection/cci/platform/plat_metOpA>,
        <http://vocab.ceda.ac.uk/collection/cci/platform/plat_metOpB>,
        <http://vocab.ceda.ac.uk/collection/cci/platform/plat_metOpC>,
        <http://vocab.ceda.ac.uk/collection/cci/platform/plat_meteosat_1>,
        <http://vocab.ceda.ac.uk/collection/cci/platform/plat_meteosat_10>,
        <http://vocab.ceda.ac.uk/collection/cci/platform/plat_meteosat_11>,
        <http://vocab.ceda.ac.uk/collection/cci/platform/plat_meteosat_2>,
        <http://vocab.ceda.ac.uk/collection/cci/platform/plat_meteosat_3>,
        <http://vocab.ceda.ac.uk/collection/cci/platform/plat_meteosat_3_adc>,
        <http://vocab.ceda.ac.uk/collection/cci/platform/plat_meteosat_3_xadc>,
        <http://vocab.ceda.ac.uk/collection/cci/platform/plat_meteosat_4>,
        <http://vocab.ceda.ac.uk/collection/cci/platform/plat_meteosat_5>,
        <http://vocab.ceda.ac.uk/collection/cci/platform/plat_meteosat_5_iodc>,
        <http://vocab.ceda.ac.uk/collection/cci/platform/plat_meteosat_6>,
        <http://vocab.ceda.ac.uk/collection/cci/platform/plat_meteosat_6_iodc>,
        <http://vocab.ceda.ac.uk/collection/cci/platform/plat_meteosat_7>,
        <http://vocab.ceda.ac.uk/collection/cci/platform/plat_meteosat_7_iodc>,
        <http://vocab.ceda.ac.uk/collection/cci/platform/plat_meteosat_8>,
        <http://vocab.ceda.ac.uk/collection/cci/platform/plat_meteosat_9>,
        <http://vocab.ceda.ac.uk/collection/cci/platform/plat_nimbus1>,
        <http://vocab.ceda.ac.uk/collection/cci/platform/plat_nimbus2>,
        <http://vocab.ceda.ac.uk/collection/cci/platform/plat_nimbus3>,
        <http://vocab.ceda.ac.uk/collection/cci/platform/plat_nimbus4>,
        <http://vocab.ceda.ac.uk/collection/cci/platform/plat_nimbus5>,
        <http://vocab.ceda.ac.uk/collection/cci/platform/plat_nimbus6>,
        <http://vocab.ceda.ac.uk/collection/cci/platform/plat_nimbus7>,
        <http://vocab.ceda.ac.uk/collection/cci/platform/plat_noaa_1>,
        <http://vocab.ceda.ac.uk/collection/cci/platform/plat_noaa_10>,
        <http://vocab.ceda.ac.uk/collection/cci/platform/plat_noaa_11>,
        <http://vocab.ceda.ac.uk/collection/cci/platform/plat_noaa_12>,
        <http://vocab.ceda.ac.uk/collection/cci/platform/plat_noaa_13>,
        <http://vocab.ceda.ac.uk/collection/cci/platform/plat_noaa_14>,
        <http://vocab.ceda.ac.uk/collection/cci/platform/plat_noaa_15>,
        <http://vocab.ceda.ac.uk/collection/cci/platform/plat_noaa_16>,
        <http://vocab.ceda.ac.uk/collection/cci/platform/plat_noaa_17>,
        <http://vocab.ceda.ac.uk/collection/cci/platform/plat_noaa_18>,
        <http://vocab.ceda.ac.uk/collection/cci/platform/plat_noaa_19>,
        <http://vocab.ceda.ac.uk/collection/cci/platform/plat_noaa_2>,
        <http://vocab.ceda.ac.uk/collection/cci/platform/plat_noaa_3>,
        <http://vocab.ceda.ac.uk/collection/cci/platform/plat_noaa_4>,
        <http://vocab.ceda.ac.uk/collection/cci/platform/plat_noaa_5>,
        <http://vocab.ceda.ac.uk/collection/cci/platform/plat_noaa_6>,
        <http://vocab.ceda.ac.uk/collection/cci/platform/plat_noaa_7>,
        <http://vocab.ceda.ac.uk/collection/cci/platform/plat_noaa_8>,
        <http://vocab.ceda.ac.uk/collection/cci/platform/plat_noaa_9>,
        <http://vocab.ceda.ac.uk/collection/cci/platform/plat_oco2>,
        <http://vocab.ceda.ac.uk/collection/cci/platform/plat_odin>,
        <http://vocab.ceda.ac.uk/collection/cci/platform/plat_orbview2>,
        <http://vocab.ceda.ac.uk/collection/cci/platform/plat_parasol>,
        <http://vocab.ceda.ac.uk/collection/cci/platform/plat_probaV>,
        <http://vocab.ceda.ac.uk/collection/cci/platform/plat_radarsat2>,
        <http://vocab.ceda.ac.uk/collection/cci/platform/plat_sac_d>,
        <http://vocab.ceda.ac.uk/collection/cci/platform/plat_saral>,
        <http://vocab.ceda.ac.uk/collection/cci/platform/plat_scisat>,
        <http://vocab.ceda.ac.uk/collection/cci/platform/plat_sentinel1a>,
        <http://vocab.ceda.ac.uk/collection/cci/platform/plat_sentinel1b>,
        <http://vocab.ceda.ac.uk/collection/cci/platform/plat_sentinel2a>,
        <http://vocab.ceda.ac.uk/collection/cci/platform/plat_sentinel2b>,
        <http://vocab.ceda.ac.uk/collection/cci/platform/plat_sentinel3a>,
        <http://vocab.ceda.ac.uk/collection/cci/platform/plat_sentinel3b>,
        <http://vocab.ceda.ac.uk/collection/cci/platform/plat_sentinel5p>,
        <http://vocab.ceda.ac.uk/collection/cci/platform/plat_sentinel6a>,
        <http://vocab.ceda.ac.uk/collection/cci/platform/plat_sentinel6b>,
        <http://vocab.ceda.ac.uk/collection/cci/platform/plat_smap>,
        <http://vocab.ceda.ac.uk/collection/cci/platform/plat_smos>,
        <http://vocab.ceda.ac.uk/collection/cci/platform/plat_snpp>,
        <http://vocab.ceda.ac.uk/collection/cci/platform/plat_spot1>,
        <http://vocab.ceda.ac.uk/collection/cci/platform/plat_spot2>,
        <http://vocab.ceda.ac.uk/collection/cci/platform/plat_spot3>,
        <http://vocab.ceda.ac.uk/collection/cci/platform/plat_spot4>,
        <http://vocab.ceda.ac.uk/collection/cci/platform/plat_spot5>,
        <http://vocab.ceda.ac.uk/collection/cci/platform/plat_spot6>,
        <http://vocab.ceda.ac.uk/collection/cci/platform/plat_spot7>,
        <http://vocab.ceda.ac.uk/collection/cci/platform/plat_tandem_X>,
        <http://vocab.ceda.ac.uk/collection/cci/platform/plat_terra>,
        <http://vocab.ceda.ac.uk/collection/cci/platform/plat_terraSar_X>,
        <http://vocab.ceda.ac.uk/collection/cci/platform/plat_tiros_n>,
        <http://vocab.ceda.ac.uk/collection/cci/platform/plat_topexPoseidon>,
        <http://vocab.ceda.ac.uk/collection/cci/platform/plat_trmm>,
        <http://vocab.ceda.ac.uk/collection/cci/platform/plat_tsx_ng>,
        <http://vocab.ceda.ac.uk/collection/cci/platform/plat_unspecified> ;
    skos:prefLabel "Platform"@en .

cci-collection:platformGrp a skos:Collection ;
    dc:creator "Science and Technology Facilities Council" ;
    dc:date "2025-01-23" ;
    dc:description "The platform groups that have been used in the collection of data for the ESA Climate Change Initiative (CCI)." ;
    dc:publisher "STFC"@en ;
    dc:title "Platform Group" ;
    rdfs:comment "This collection represents the platform groups used by the CCI project" ;
    owl:versionInfo "0.0.1" ;
    skos:definition "The platform groups that have been used in the collection of data for the ESA Climate Change Initiative (CCI)."@en ;
    skos:member <http://vocab.ceda.ac.uk/collection/cci/platformGrp/plat_dmsp>,
        <http://vocab.ceda.ac.uk/collection/cci/platformGrp/plat_goes>,
        <http://vocab.ceda.ac.uk/collection/cci/platformGrp/plat_noaa> ;
    skos:prefLabel "Platform Group"@en .

cci-collection:platformProg a skos:Collection ;
    dc:creator "Science and Technology Facilities Council" ;
    dc:date "2025-01-23" ;
    dc:description "The platform programmes that have been used in the collection of data for the ESA Climate Change Initiative (CCI)." ;
    dc:publisher "STFC"@en ;
    dc:title "Platform Programme" ;
    rdfs:comment "This collection represents the platform programmes used by the CCI project" ;
    owl:versionInfo "0.0.1" ;
    skos:definition "The platform programmes that have been used in the collection of data for the ESA Climate Change Initiative (CCI)."@en ;
    skos:member <http://vocab.ceda.ac.uk/collection/cci/platformProg/plat_alos_prog>,
        <http://vocab.ceda.ac.uk/collection/cci/platformProg/plat_coriolis_prog>,
        <http://vocab.ceda.ac.uk/collection/cci/platformProg/plat_cryosat_prog>,
        <http://vocab.ceda.ac.uk/collection/cci/platformProg/plat_csk_prog>,
        <http://vocab.ceda.ac.uk/collection/cci/platformProg/plat_dmsp_5D1>,
        <http://vocab.ceda.ac.uk/collection/cci/platformProg/plat_dmsp_5D2>,
        <http://vocab.ceda.ac.uk/collection/cci/platformProg/plat_dmsp_5D3>,
        <http://vocab.ceda.ac.uk/collection/cci/platformProg/plat_envisat_prog>,
        <http://vocab.ceda.ac.uk/collection/cci/platformProg/plat_eos>,
        <http://vocab.ceda.ac.uk/collection/cci/platformProg/plat_ers>,
        <http://vocab.ceda.ac.uk/collection/cci/platformProg/plat_fengyun3>,
        <http://vocab.ceda.ac.uk/collection/cci/platformProg/plat_gcom>,
        <http://vocab.ceda.ac.uk/collection/cci/platformProg/plat_geodetic>,
        <http://vocab.ceda.ac.uk/collection/cci/platformProg/plat_goes_1st>,
        <http://vocab.ceda.ac.uk/collection/cci/platformProg/plat_goes_2nd>,
        <http://vocab.ceda.ac.uk/collection/cci/platformProg/plat_goes_3rd>,
        <http://vocab.ceda.ac.uk/collection/cci/platformProg/plat_gosat_prog>,
        <http://vocab.ceda.ac.uk/collection/cci/platformProg/plat_gpm_prog>,
        <http://vocab.ceda.ac.uk/collection/cci/platformProg/plat_grace_prog>,
        <http://vocab.ceda.ac.uk/collection/cci/platformProg/plat_himawari>,
        <http://vocab.ceda.ac.uk/collection/cci/platformProg/plat_icesat_prog>,
        <http://vocab.ceda.ac.uk/collection/cci/platformProg/plat_jason>,
        <http://vocab.ceda.ac.uk/collection/cci/platformProg/plat_jpss_prog>,
        <http://vocab.ceda.ac.uk/collection/cci/platformProg/plat_landsat>,
        <http://vocab.ceda.ac.uk/collection/cci/platformProg/plat_landsat_dcm>,
        <http://vocab.ceda.ac.uk/collection/cci/platformProg/plat_metop>,
        <http://vocab.ceda.ac.uk/collection/cci/platformProg/plat_mfg_prog>,
        <http://vocab.ceda.ac.uk/collection/cci/platformProg/plat_msg>,
        <http://vocab.ceda.ac.uk/collection/cci/platformProg/plat_nimbus>,
        <http://vocab.ceda.ac.uk/collection/cci/platformProg/plat_noaa_3rd>,
        <http://vocab.ceda.ac.uk/collection/cci/platformProg/plat_noaa_4th>,
        <http://vocab.ceda.ac.uk/collection/cci/platformProg/plat_noaa_5th>,
        <http://vocab.ceda.ac.uk/collection/cci/platformProg/plat_oco_prog>,
        <http://vocab.ceda.ac.uk/collection/cci/platformProg/plat_odin_prog>,
        <http://vocab.ceda.ac.uk/collection/cci/platformProg/plat_orbview2_prog>,
        <http://vocab.ceda.ac.uk/collection/cci/platformProg/plat_parasol_prog>,
        <http://vocab.ceda.ac.uk/collection/cci/platformProg/plat_proba_prog>,
        <http://vocab.ceda.ac.uk/collection/cci/platformProg/plat_radarsat_prog>,
        <http://vocab.ceda.ac.uk/collection/cci/platformProg/plat_s5p_prog>,
        <http://vocab.ceda.ac.uk/collection/cci/platformProg/plat_sac_prog>,
        <http://vocab.ceda.ac.uk/collection/cci/platformProg/plat_saral_prog>,
        <http://vocab.ceda.ac.uk/collection/cci/platformProg/plat_scisat_prog>,
        <http://vocab.ceda.ac.uk/collection/cci/platformProg/plat_sentinel1_prog>,
        <http://vocab.ceda.ac.uk/collection/cci/platformProg/plat_sentinel2_prog>,
        <http://vocab.ceda.ac.uk/collection/cci/platformProg/plat_sentinel3_prog>,
        <http://vocab.ceda.ac.uk/collection/cci/platformProg/plat_sentinel6_prog>,
        <http://vocab.ceda.ac.uk/collection/cci/platformProg/plat_smap_prog>,
        <http://vocab.ceda.ac.uk/collection/cci/platformProg/plat_smos_prog>,
        <http://vocab.ceda.ac.uk/collection/cci/platformProg/plat_spot>,
        <http://vocab.ceda.ac.uk/collection/cci/platformProg/plat_spot_prog_follow>,
        <http://vocab.ceda.ac.uk/collection/cci/platformProg/plat_terraSAR>,
        <http://vocab.ceda.ac.uk/collection/cci/platformProg/plat_topexPoseidon_prog>,
        <http://vocab.ceda.ac.uk/collection/cci/platformProg/plat_trmm_prog> ;
    skos:prefLabel "Platform Programme"@en .

cci-collection:procLev a skos:Collection ;
    dc:creator "Science and Technology Facilities Council" ;
    dc:date "2025-01-23" ;
    dc:description "The different processing levels of satellite observational data that are used within the ESA Climate Change Initiative (CCI)." ;
    dc:publisher "STFC"@en ;
    dc:title "Processing Level" ;
    rdfs:comment "This collection represents the processing levels used by the CCI project" ;
    owl:versionInfo "0.0.1" ;
    skos:definition "The different processing levels of satellite observational data that are used within the ESA Climate Change Initiative (CCI)."@en ;
    skos:member <http://vocab.ceda.ac.uk/collection/cci/procLev/proc_ind>,
        <http://vocab.ceda.ac.uk/collection/cci/procLev/proc_level0>,
        <http://vocab.ceda.ac.uk/collection/cci/procLev/proc_level1>,
        <http://vocab.ceda.ac.uk/collection/cci/procLev/proc_level1A>,
        <http://vocab.ceda.ac.uk/collection/cci/procLev/proc_level1B>,
        <http://vocab.ceda.ac.uk/collection/cci/procLev/proc_level1C>,
        <http://vocab.ceda.ac.uk/collection/cci/procLev/proc_level2>,
        <http://vocab.ceda.ac.uk/collection/cci/procLev/proc_level2P>,
        <http://vocab.ceda.ac.uk/collection/cci/procLev/proc_level3>,
        <http://vocab.ceda.ac.uk/collection/cci/procLev/proc_level3C>,
        <http://vocab.ceda.ac.uk/collection/cci/procLev/proc_level3S>,
        <http://vocab.ceda.ac.uk/collection/cci/procLev/proc_level3U>,
        <http://vocab.ceda.ac.uk/collection/cci/procLev/proc_level4>,
        <http://vocab.ceda.ac.uk/collection/cci/procLev/proc_unspecified> ;
    skos:prefLabel "Processing Level"@en .

cci-collection:product a skos:Collection ;
    dc:creator "Science and Technology Facilities Council" ;
    dc:date "2025-01-23" ;
    dc:description "The different products that are produced within the ESA Climate Change Initiative (CCI)." ;
    dc:publisher "STFC"@en ;
    dc:title "Product String" ;
    rdfs:comment "This collection represents the products used by the CCI project" ;
    owl:versionInfo "0.0.1" ;
    skos:definition "The different products that are produced within the ESA Climate Change Initiative (CCI)."@en ;
    skos:member <http://vocab.ceda.ac.uk/collection/cci/product/prod_AvhrMa>,
        <http://vocab.ceda.ac.uk/collection/cci/product/prod_AvhrrMetopA>,
        <http://vocab.ceda.ac.uk/collection/cci/product/prod_AvhrrMetopB>,
        <http://vocab.ceda.ac.uk/collection/cci/product/prod_AvhrrMetopC>,
        <http://vocab.ceda.ac.uk/collection/cci/product/prod_AvhrrNoaa10>,
        <http://vocab.ceda.ac.uk/collection/cci/product/prod_AvhrrNoaa11>,
        <http://vocab.ceda.ac.uk/collection/cci/product/prod_AvhrrNoaa12>,
        <http://vocab.ceda.ac.uk/collection/cci/product/prod_AvhrrNoaa14>,
        <http://vocab.ceda.ac.uk/collection/cci/product/prod_AvhrrNoaa16>,
        <http://vocab.ceda.ac.uk/collection/cci/product/prod_AvhrrNoaa17>,
        <http://vocab.ceda.ac.uk/collection/cci/product/prod_AvhrrNoaa18>,
        <http://vocab.ceda.ac.uk/collection/cci/product/prod_AvhrrNoaa19>,
        <http://vocab.ceda.ac.uk/collection/cci/product/prod_AvhrrNoaa6>,
        <http://vocab.ceda.ac.uk/collection/cci/product/prod_AvhrrNoaa7>,
        <http://vocab.ceda.ac.uk/collection/cci/product/prod_AvhrrNoaa8>,
        <http://vocab.ceda.ac.uk/collection/cci/product/prod_AvhrrNoaa9>,
        <http://vocab.ceda.ac.uk/collection/cci/product/prod_AvhrrTirosN>,
        <http://vocab.ceda.ac.uk/collection/cci/product/prod_CL02A01>,
        <http://vocab.ceda.ac.uk/collection/cci/product/prod_CL02A01Mos>,
        <http://vocab.ceda.ac.uk/collection/cci/product/prod_CL02A02>,
        <http://vocab.ceda.ac.uk/collection/cci/product/prod_CL02A02Mos>,
        <http://vocab.ceda.ac.uk/collection/cci/product/prod_CL02A03>,
        <http://vocab.ceda.ac.uk/collection/cci/product/prod_CL02A03Mos>,
        <http://vocab.ceda.ac.uk/collection/cci/product/prod_CryoSat2>,
        <http://vocab.ceda.ac.uk/collection/cci/product/prod_Diff>,
        <http://vocab.ceda.ac.uk/collection/cci/product/prod_GlobMerg7day>,
        <http://vocab.ceda.ac.uk/collection/cci/product/prod_GlobMergCent>,
        <http://vocab.ceda.ac.uk/collection/cci/product/prod_HRLC10A01>,
        <http://vocab.ceda.ac.uk/collection/cci/product/prod_HRLC10A02>,
        <http://vocab.ceda.ac.uk/collection/cci/product/prod_HRLC10A03>,
        <http://vocab.ceda.ac.uk/collection/cci/product/prod_HRLC30A01>,
        <http://vocab.ceda.ac.uk/collection/cci/product/prod_HRLC30A02>,
        <http://vocab.ceda.ac.uk/collection/cci/product/prod_HRLC30A03>,
        <http://vocab.ceda.ac.uk/collection/cci/product/prod_HRLCC30A01>,
        <http://vocab.ceda.ac.uk/collection/cci/product/prod_HRLCC30A02>,
        <http://vocab.ceda.ac.uk/collection/cci/product/prod_HRLCC30A03>,
        <http://vocab.ceda.ac.uk/collection/cci/product/prod_IQIXA01>,
        <http://vocab.ceda.ac.uk/collection/cci/product/prod_IQIXA01Mos>,
        <http://vocab.ceda.ac.uk/collection/cci/product/prod_IQIXA02>,
        <http://vocab.ceda.ac.uk/collection/cci/product/prod_IQIXA02Mos>,
        <http://vocab.ceda.ac.uk/collection/cci/product/prod_IQIXA03>,
        <http://vocab.ceda.ac.uk/collection/cci/product/prod_IQIXA03Mos>,
        <http://vocab.ceda.ac.uk/collection/cci/product/prod_Jason1>,
        <http://vocab.ceda.ac.uk/collection/cci/product/prod_Jason2>,
        <http://vocab.ceda.ac.uk/collection/cci/product/prod_Jason3>,
        <http://vocab.ceda.ac.uk/collection/cci/product/prod_PS01A01>,
        <http://vocab.ceda.ac.uk/collection/cci/product/prod_PS01A01Mos>,
        <http://vocab.ceda.ac.uk/collection/cci/product/prod_PS01A02>,
        <http://vocab.ceda.ac.uk/collection/cci/product/prod_PS01A02Mos>,
        <http://vocab.ceda.ac.uk/collection/cci/product/prod_PS01A03>,
        <http://vocab.ceda.ac.uk/collection/cci/product/prod_PS01A03Mos>,
        <http://vocab.ceda.ac.uk/collection/cci/product/prod_PS02A01>,
        <http://vocab.ceda.ac.uk/collection/cci/product/prod_PS02A01Mos>,
        <http://vocab.ceda.ac.uk/collection/cci/product/prod_PS02A02>,
        <http://vocab.ceda.ac.uk/collection/cci/product/prod_PS02A02Mos>,
        <http://vocab.ceda.ac.uk/collection/cci/product/prod_PS02A03>,
        <http://vocab.ceda.ac.uk/collection/cci/product/prod_PS02A03Mos>,
        <http://vocab.ceda.ac.uk/collection/cci/product/prod_PolMerg7dayNh>,
        <http://vocab.ceda.ac.uk/collection/cci/product/prod_PolMerg7daySh>,
        <http://vocab.ceda.ac.uk/collection/cci/product/prod_PolMergCentNH>,
        <http://vocab.ceda.ac.uk/collection/cci/product/prod_PolMergCentSH>,
        <http://vocab.ceda.ac.uk/collection/cci/product/prod_aFS>,
        <http://vocab.ceda.ac.uk/collection/cci/product/prod_aatsr>,
        <http://vocab.ceda.ac.uk/collection/cci/product/prod_aatsrEn>,
        <http://vocab.ceda.ac.uk/collection/cci/product/prod_aatsrEns>,
        <http://vocab.ceda.ac.uk/collection/cci/product/prod_aatsrEnsannual>,
        <http://vocab.ceda.ac.uk/collection/cci/product/prod_aatsrEnsdaily>,
        <http://vocab.ceda.ac.uk/collection/cci/product/prod_aatsrEnsmonthly>,
        <http://vocab.ceda.ac.uk/collection/cci/product/prod_active>,
        <http://vocab.ceda.ac.uk/collection/cci/product/prod_adv>,
        <http://vocab.ceda.ac.uk/collection/cci/product/prod_aergom>,
        <http://vocab.ceda.ac.uk/collection/cci/product/prod_alamo>,
        <http://vocab.ceda.ac.uk/collection/cci/product/prod_amsr>,
        <http://vocab.ceda.ac.uk/collection/cci/product/prod_amsr25E>,
        <http://vocab.ceda.ac.uk/collection/cci/product/prod_amsr50E>,
        <http://vocab.ceda.ac.uk/collection/cci/product/prod_atsr1>,
        <http://vocab.ceda.ac.uk/collection/cci/product/prod_atsr2>,
        <http://vocab.ceda.ac.uk/collection/cci/product/prod_atsr2Aatsr>,
        <http://vocab.ceda.ac.uk/collection/cci/product/prod_atsr2Er2>,
        <http://vocab.ceda.ac.uk/collection/cci/product/prod_atsr2ens>,
        <http://vocab.ceda.ac.uk/collection/cci/product/prod_atsr2ensannual>,
        <http://vocab.ceda.ac.uk/collection/cci/product/prod_atsr2ensdaily>,
        <http://vocab.ceda.ac.uk/collection/cci/product/prod_atsr2ensmonthly>,
        <http://vocab.ceda.ac.uk/collection/cci/product/prod_atsr3>,
        <http://vocab.ceda.ac.uk/collection/cci/product/prod_atsr_2>,
        <http://vocab.ceda.ac.uk/collection/cci/product/prod_avhrr07G>,
        <http://vocab.ceda.ac.uk/collection/cci/product/prod_avhrr09G>,
        <http://vocab.ceda.ac.uk/collection/cci/product/prod_avhrr11G>,
        <http://vocab.ceda.ac.uk/collection/cci/product/prod_avhrr12G>,
        <http://vocab.ceda.ac.uk/collection/cci/product/prod_avhrr14G>,
        <http://vocab.ceda.ac.uk/collection/cci/product/prod_avhrr15G>,
        <http://vocab.ceda.ac.uk/collection/cci/product/prod_avhrr16G>,
        <http://vocab.ceda.ac.uk/collection/cci/product/prod_avhrr17G>,
        <http://vocab.ceda.ac.uk/collection/cci/product/prod_avhrr18G>,
        <http://vocab.ceda.ac.uk/collection/cci/product/prod_avhrr19G>,
        <http://vocab.ceda.ac.uk/collection/cci/product/prod_avhrrAm>,
        <http://vocab.ceda.ac.uk/collection/cci/product/prod_avhrrLtdr>,
        <http://vocab.ceda.ac.uk/collection/cci/product/prod_avhrrMg>,
        <http://vocab.ceda.ac.uk/collection/cci/product/prod_avhrrNoaa>,
        <http://vocab.ceda.ac.uk/collection/cci/product/prod_avhrrPm>,
        <http://vocab.ceda.ac.uk/collection/cci/product/prod_avhrrmtag>,
        <http://vocab.ceda.ac.uk/collection/cci/product/prod_besd>,
        <http://vocab.ceda.ac.uk/collection/cci/product/prod_change>,
        <http://vocab.ceda.ac.uk/collection/cci/product/prod_cl01A01>,
        <http://vocab.ceda.ac.uk/collection/cci/product/prod_cl01A01Mos>,
        <http://vocab.ceda.ac.uk/collection/cci/product/prod_cl01A02>,
        <http://vocab.ceda.ac.uk/collection/cci/product/prod_cl01A02Mos>,
        <http://vocab.ceda.ac.uk/collection/cci/product/prod_cl01A03>,
        <http://vocab.ceda.ac.uk/collection/cci/product/prod_cl01A03Mos>,
        <http://vocab.ceda.ac.uk/collection/cci/product/prod_clim>,
        <http://vocab.ceda.ac.uk/collection/cci/product/prod_comb>,
        <http://vocab.ceda.ac.uk/collection/cci/product/prod_combAdj>,
        <http://vocab.ceda.ac.uk/collection/cci/product/prod_emma>,
        <http://vocab.ceda.ac.uk/collection/cci/product/prod_envisat>,
        <http://vocab.ceda.ac.uk/collection/cci/product/prod_eraModBias>,
        <http://vocab.ceda.ac.uk/collection/cci/product/prod_ers1>,
        <http://vocab.ceda.ac.uk/collection/cci/product/prod_ers2>,
        <http://vocab.ceda.ac.uk/collection/cci/product/prod_focal>,
        <http://vocab.ceda.ac.uk/collection/cci/product/prod_gfo>,
        <http://vocab.ceda.ac.uk/collection/cci/product/prod_gmp>,
        <http://vocab.ceda.ac.uk/collection/cci/product/prod_gmpe>,
        <http://vocab.ceda.ac.uk/collection/cci/product/prod_gomEn>,
        <http://vocab.ceda.ac.uk/collection/cci/product/prod_gosat>,
        <http://vocab.ceda.ac.uk/collection/cci/product/prod_iasDLRImars>,
        <http://vocab.ceda.ac.uk/collection/cci/product/prod_iasiLMDaero>,
        <http://vocab.ceda.ac.uk/collection/cci/product/prod_iasiMAPIR>,
        <http://vocab.ceda.ac.uk/collection/cci/product/prod_iasiULB>,
        <http://vocab.ceda.ac.uk/collection/cci/product/prod_imap>,
        <http://vocab.ceda.ac.uk/collection/cci/product/prod_ircdr>,
        <http://vocab.ceda.ac.uk/collection/cci/product/prod_irmgp>,
        <http://vocab.ceda.ac.uk/collection/cci/product/prod_map>,
        <http://vocab.ceda.ac.uk/collection/cci/product/prod_meAaEn>,
        <http://vocab.ceda.ac.uk/collection/cci/product/prod_medSea>,
        <http://vocab.ceda.ac.uk/collection/cci/product/prod_merg7dayDaily>,
        <http://vocab.ceda.ac.uk/collection/cci/product/prod_mergMon15day25km>,
        <http://vocab.ceda.ac.uk/collection/cci/product/prod_merged>,
        <http://vocab.ceda.ac.uk/collection/cci/product/prod_merris>,
        <http://vocab.ceda.ac.uk/collection/cci/product/prod_merris_envisat>,
        <http://vocab.ceda.ac.uk/collection/cci/product/prod_miEn>,
        <http://vocab.ceda.ac.uk/collection/cci/product/prod_modA>,
        <http://vocab.ceda.ac.uk/collection/cci/product/prod_modAqu>,
        <http://vocab.ceda.ac.uk/collection/cci/product/prod_modMg>,
        <http://vocab.ceda.ac.uk/collection/cci/product/prod_modT>,
        <http://vocab.ceda.ac.uk/collection/cci/product/prod_modTe>,
        <http://vocab.ceda.ac.uk/collection/cci/product/prod_modis>,
        <http://vocab.ceda.ac.uk/collection/cci/product/prod_modlstCryo>,
        <http://vocab.ceda.ac.uk/collection/cci/product/prod_msUvai>,
        <http://vocab.ceda.ac.uk/collection/cci/product/prod_msaai>,
        <http://vocab.ceda.ac.uk/collection/cci/product/prod_msi>,
        <http://vocab.ceda.ac.uk/collection/cci/product/prod_multi1d>,
        <http://vocab.ceda.ac.uk/collection/cci/product/prod_multi1m>,
        <http://vocab.ceda.ac.uk/collection/cci/product/prod_mzm>,
        <http://vocab.ceda.ac.uk/collection/cci/product/prod_nInd>,
        <http://vocab.ceda.ac.uk/collection/cci/product/prod_neAtl>,
        <http://vocab.ceda.ac.uk/collection/cci/product/prod_nh>,
        <http://vocab.ceda.ac.uk/collection/cci/product/prod_nh25kmease2>,
        <http://vocab.ceda.ac.uk/collection/cci/product/prod_nimEsmrNH>,
        <http://vocab.ceda.ac.uk/collection/cci/product/prod_nimEsmrSH>,
        <http://vocab.ceda.ac.uk/collection/cci/product/prod_ocfp>,
        <http://vocab.ceda.ac.uk/collection/cci/product/prod_ocpr>,
        <http://vocab.ceda.ac.uk/collection/cci/product/prod_opera>,
        <http://vocab.ceda.ac.uk/collection/cci/product/prod_orac>,
        <http://vocab.ceda.ac.uk/collection/cci/product/prod_osOd>,
        <http://vocab.ceda.ac.uk/collection/cci/product/prod_ostia>,
        <http://vocab.ceda.ac.uk/collection/cci/product/prod_parGrasp>,
        <http://vocab.ceda.ac.uk/collection/cci/product/prod_passive>,
        <http://vocab.ceda.ac.uk/collection/cci/product/prod_reSSMINH>,
        <http://vocab.ceda.ac.uk/collection/cci/product/prod_reSSMISH>,
        <http://vocab.ceda.ac.uk/collection/cci/product/prod_sAust>,
        <http://vocab.ceda.ac.uk/collection/cci/product/prod_saral>,
        <http://vocab.ceda.ac.uk/collection/cci/product/prod_sciam>,
        <http://vocab.ceda.ac.uk/collection/cci/product/prod_sciamEn>,
        <http://vocab.ceda.ac.uk/collection/cci/product/prod_seAsia>,
        <http://vocab.ceda.ac.uk/collection/cci/product/prod_sh>,
        <http://vocab.ceda.ac.uk/collection/cci/product/prod_sh50kmease2>,
        <http://vocab.ceda.ac.uk/collection/cci/product/prod_slstrA>,
        <http://vocab.ceda.ac.uk/collection/cci/product/prod_slstrB>,
        <http://vocab.ceda.ac.uk/collection/cci/product/prod_smm>,
        <http://vocab.ceda.ac.uk/collection/cci/product/prod_smrOd>,
        <http://vocab.ceda.ac.uk/collection/cci/product/prod_srfp>,
        <http://vocab.ceda.ac.uk/collection/cci/product/prod_srpr>,
        <http://vocab.ceda.ac.uk/collection/cci/product/prod_ssmi>,
        <http://vocab.ceda.ac.uk/collection/cci/product/prod_ssmiS>,
        <http://vocab.ceda.ac.uk/collection/cci/product/prod_su>,
        <http://vocab.ceda.ac.uk/collection/cci/product/prod_syn>,
        <http://vocab.ceda.ac.uk/collection/cci/product/prod_tcwvLand005>,
        <http://vocab.ceda.ac.uk/collection/cci/product/prod_tcwvLand05>,
        <http://vocab.ceda.ac.uk/collection/cci/product/prod_topexPos>,
        <http://vocab.ceda.ac.uk/collection/cci/product/prod_unspecified>,
        <http://vocab.ceda.ac.uk/collection/cci/product/prod_var>,
        <http://vocab.ceda.ac.uk/collection/cci/product/prod_wAfrica>,
        <http://vocab.ceda.ac.uk/collection/cci/product/prod_wfmd> ;
    skos:prefLabel "Product String"@en .

cci-collection:project a skos:Collection ;
    dc:creator "Science and Technology Facilities Council" ;
    dc:date "2025-01-23" ;
    dc:description "The different projects that are produced within the ESA Climate Change Initiative (CCI)." ;
    dc:publisher "STFC"@en ;
    dc:title "Project" ;
    rdfs:comment "This collection represents the projects used by the CCI project" ;
    owl:versionInfo "0.0.1" ;
    skos:definition "The different projects that are produced within the ESA Climate Change Initiative (CCI)."@en ;
    skos:member <http://vocab.ceda.ac.uk/collection/cci/project/cciproject_aerosol>,
        <http://vocab.ceda.ac.uk/collection/cci/project/cciproject_biomass>,
        <http://vocab.ceda.ac.uk/collection/cci/project/cciproject_cloud>,
        <http://vocab.ceda.ac.uk/collection/cci/project/cciproject_fire>,
        <http://vocab.ceda.ac.uk/collection/cci/project/cciproject_ghg>,
        <http://vocab.ceda.ac.uk/collection/cci/project/cciproject_glaciers>,
        <http://vocab.ceda.ac.uk/collection/cci/project/cciproject_iceSheet>,
        <http://vocab.ceda.ac.uk/collection/cci/project/cciproject_lakes>,
        <http://vocab.ceda.ac.uk/collection/cci/project/cciproject_landCov>,
        <http://vocab.ceda.ac.uk/collection/cci/project/cciproject_landSurfTemp>,
        <http://vocab.ceda.ac.uk/collection/cci/project/cciproject_oceanCol>,
        <http://vocab.ceda.ac.uk/collection/cci/project/cciproject_ozone>,
        <http://vocab.ceda.ac.uk/collection/cci/project/cciproject_permafrost>,
        <http://vocab.ceda.ac.uk/collection/cci/project/cciproject_riverDischarge>,
        <http://vocab.ceda.ac.uk/collection/cci/project/cciproject_salinity>,
        <http://vocab.ceda.ac.uk/collection/cci/project/cciproject_seaIce>,
        <http://vocab.ceda.ac.uk/collection/cci/project/cciproject_seaLevel>,
        <http://vocab.ceda.ac.uk/collection/cci/project/cciproject_seaState>,
        <http://vocab.ceda.ac.uk/collection/cci/project/cciproject_snow>,
        <http://vocab.ceda.ac.uk/collection/cci/project/cciproject_soilMst>,
        <http://vocab.ceda.ac.uk/collection/cci/project/cciproject_sst>,
        <http://vocab.ceda.ac.uk/collection/cci/project/cciproject_vegParam>,
        <http://vocab.ceda.ac.uk/collection/cci/project/cciproject_waterVapour> ;
    skos:prefLabel "Project"@en .

cci-collection:sensor a skos:Collection ;
    dc:creator "Science and Technology Facilities Council" ;
    dc:date "2025-01-23" ;
    dc:description "The sensors that have been used in the collection of the data for the ESA Climate Change Initiative (CCI)." ;
    dc:publisher "STFC"@en ;
    dc:title "Sensor" ;
    rdfs:comment "This collection represents the sensors used by the CCI project" ;
    owl:versionInfo "0.0.1" ;
    skos:definition "The sensors that have been used in the collection of the data for the ESA Climate Change Initiative (CCI)."@en ;
    skos:member <http://vocab.ceda.ac.uk/collection/cci/sensor/sens_aatsr>,
        <http://vocab.ceda.ac.uk/collection/cci/sensor/sens_abi>,
        <http://vocab.ceda.ac.uk/collection/cci/sensor/sens_aceFts>,
        <http://vocab.ceda.ac.uk/collection/cci/sensor/sens_airs>,
        <http://vocab.ceda.ac.uk/collection/cci/sensor/sens_altika>,
        <http://vocab.ceda.ac.uk/collection/cci/sensor/sens_amisar>,
        <http://vocab.ceda.ac.uk/collection/cci/sensor/sens_amiscat>,
        <http://vocab.ceda.ac.uk/collection/cci/sensor/sens_amsr2>,
        <http://vocab.ceda.ac.uk/collection/cci/sensor/sens_amsre>,
        <http://vocab.ceda.ac.uk/collection/cci/sensor/sens_amsua>,
        <http://vocab.ceda.ac.uk/collection/cci/sensor/sens_amsub>,
        <http://vocab.ceda.ac.uk/collection/cci/sensor/sens_aquarius>,
        <http://vocab.ceda.ac.uk/collection/cci/sensor/sens_asar>,
        <http://vocab.ceda.ac.uk/collection/cci/sensor/sens_ascat>,
        <http://vocab.ceda.ac.uk/collection/cci/sensor/sens_aster>,
        <http://vocab.ceda.ac.uk/collection/cci/sensor/sens_atsr>,
        <http://vocab.ceda.ac.uk/collection/cci/sensor/sens_atsr2>,
        <http://vocab.ceda.ac.uk/collection/cci/sensor/sens_avhrr>,
        <http://vocab.ceda.ac.uk/collection/cci/sensor/sens_avhrr2>,
        <http://vocab.ceda.ac.uk/collection/cci/sensor/sens_avhrr3>,
        <http://vocab.ceda.ac.uk/collection/cci/sensor/sens_esmrNim5>,
        <http://vocab.ceda.ac.uk/collection/cci/sensor/sens_esmrNim6>,
        <http://vocab.ceda.ac.uk/collection/cci/sensor/sens_etmplus>,
        <http://vocab.ceda.ac.uk/collection/cci/sensor/sens_gfora>,
        <http://vocab.ceda.ac.uk/collection/cci/sensor/sens_glas>,
        <http://vocab.ceda.ac.uk/collection/cci/sensor/sens_gmi>,
        <http://vocab.ceda.ac.uk/collection/cci/sensor/sens_goesImager1215>,
        <http://vocab.ceda.ac.uk/collection/cci/sensor/sens_goesImager811>,
        <http://vocab.ceda.ac.uk/collection/cci/sensor/sens_gome>,
        <http://vocab.ceda.ac.uk/collection/cci/sensor/sens_gome2>,
        <http://vocab.ceda.ac.uk/collection/cci/sensor/sens_gomos>,
        <http://vocab.ceda.ac.uk/collection/cci/sensor/sens_grace>,
        <http://vocab.ceda.ac.uk/collection/cci/sensor/sens_hirs>,
        <http://vocab.ceda.ac.uk/collection/cci/sensor/sens_hirs2>,
        <http://vocab.ceda.ac.uk/collection/cci/sensor/sens_hirs3>,
        <http://vocab.ceda.ac.uk/collection/cci/sensor/sens_hirs4>,
        <http://vocab.ceda.ac.uk/collection/cci/sensor/sens_hrs>,
        <http://vocab.ceda.ac.uk/collection/cci/sensor/sens_iasi>,
        <http://vocab.ceda.ac.uk/collection/cci/sensor/sens_imagerMtsat2>,
        <http://vocab.ceda.ac.uk/collection/cci/sensor/sens_jami>,
        <http://vocab.ceda.ac.uk/collection/cci/sensor/sens_meris>,
        <http://vocab.ceda.ac.uk/collection/cci/sensor/sens_mipas>,
        <http://vocab.ceda.ac.uk/collection/cci/sensor/sens_miras>,
        <http://vocab.ceda.ac.uk/collection/cci/sensor/sens_modis>,
        <http://vocab.ceda.ac.uk/collection/cci/sensor/sens_msi>,
        <http://vocab.ceda.ac.uk/collection/cci/sensor/sens_mss>,
        <http://vocab.ceda.ac.uk/collection/cci/sensor/sens_mviri>,
        <http://vocab.ceda.ac.uk/collection/cci/sensor/sens_mwri>,
        <http://vocab.ceda.ac.uk/collection/cci/sensor/sens_nra>,
        <http://vocab.ceda.ac.uk/collection/cci/sensor/sens_oco>,
        <http://vocab.ceda.ac.uk/collection/cci/sensor/sens_olci>,
        <http://vocab.ceda.ac.uk/collection/cci/sensor/sens_oli>,
        <http://vocab.ceda.ac.uk/collection/cci/sensor/sens_omi>,
        <http://vocab.ceda.ac.uk/collection/cci/sensor/sens_osiris>,
        <http://vocab.ceda.ac.uk/collection/cci/sensor/sens_palsar>,
        <http://vocab.ceda.ac.uk/collection/cci/sensor/sens_palsar2>,
        <http://vocab.ceda.ac.uk/collection/cci/sensor/sens_polder>,
        <http://vocab.ceda.ac.uk/collection/cci/sensor/sens_poseidon2>,
        <http://vocab.ceda.ac.uk/collection/cci/sensor/sens_poseidon3>,
        <http://vocab.ceda.ac.uk/collection/cci/sensor/sens_poseidon3b>,
        <http://vocab.ceda.ac.uk/collection/cci/sensor/sens_poseidon4>,
        <http://vocab.ceda.ac.uk/collection/cci/sensor/sens_ra>,
        <http://vocab.ceda.ac.uk/collection/cci/sensor/sens_ra2>,
        <http://vocab.ceda.ac.uk/collection/cci/sensor/sens_sar2000>,
        <http://vocab.ceda.ac.uk/collection/cci/sensor/sens_sarRadarSat2>,
        <http://vocab.ceda.ac.uk/collection/cci/sensor/sens_sarX>,
        <http://vocab.ceda.ac.uk/collection/cci/sensor/sens_sarcS1>,
        <http://vocab.ceda.ac.uk/collection/cci/sensor/sens_sciamachy>,
        <http://vocab.ceda.ac.uk/collection/cci/sensor/sens_seaWiFs>,
        <http://vocab.ceda.ac.uk/collection/cci/sensor/sens_seviri>,
        <http://vocab.ceda.ac.uk/collection/cci/sensor/sens_siral>,
        <http://vocab.ceda.ac.uk/collection/cci/sensor/sens_slstr>,
        <http://vocab.ceda.ac.uk/collection/cci/sensor/sens_smap>,
        <http://vocab.ceda.ac.uk/collection/cci/sensor/sens_smmr>,
        <http://vocab.ceda.ac.uk/collection/cci/sensor/sens_smr>,
        <http://vocab.ceda.ac.uk/collection/cci/sensor/sens_sral>,
        <http://vocab.ceda.ac.uk/collection/cci/sensor/sens_ssalt>,
        <http://vocab.ceda.ac.uk/collection/cci/sensor/sens_ssmI>,
        <http://vocab.ceda.ac.uk/collection/cci/sensor/sens_ssmiS>,
        <http://vocab.ceda.ac.uk/collection/cci/sensor/sens_tansoCai>,
        <http://vocab.ceda.ac.uk/collection/cci/sensor/sens_tansoFts>,
        <http://vocab.ceda.ac.uk/collection/cci/sensor/sens_tansoFts2>,
        <http://vocab.ceda.ac.uk/collection/cci/sensor/sens_tirs>,
        <http://vocab.ceda.ac.uk/collection/cci/sensor/sens_tm>,
        <http://vocab.ceda.ac.uk/collection/cci/sensor/sens_tmi>,
        <http://vocab.ceda.ac.uk/collection/cci/sensor/sens_toms>,
        <http://vocab.ceda.ac.uk/collection/cci/sensor/sens_tropomi>,
        <http://vocab.ceda.ac.uk/collection/cci/sensor/sens_unspecified>,
        <http://vocab.ceda.ac.uk/collection/cci/sensor/sens_vegetation>,
        <http://vocab.ceda.ac.uk/collection/cci/sensor/sens_vegetationP>,
        <http://vocab.ceda.ac.uk/collection/cci/sensor/sens_viirs>,
        <http://vocab.ceda.ac.uk/collection/cci/sensor/sens_virr>,
        <http://vocab.ceda.ac.uk/collection/cci/sensor/sens_windSat> ;
    skos:prefLabel "Sensor"@en .

<http://vocab.ceda.ac.uk/collection/cci/dataType/dtype_aai> a cci:dataType,
        skos:Concept ;
    rdfs:seeAlso <https://climate.esa.int/projects/aerosol> ;
    skos:altLabel "AAI"@en ;
    skos:definition "absorbing aerosol index"@en ;
    skos:inScheme cci-scheme:dataType ;
    skos:prefLabel "absorbing aerosol index"@en ;
    skos:scopeNote "absorbing aerosol index"@en ;
    skos:topConceptOf cci-scheme:dataType .

<http://vocab.ceda.ac.uk/collection/cci/dataType/dtype_adg> a cci:dataType,
        skos:Concept ;
    rdfs:seeAlso <https://climate.esa.int/projects/ocean-colour/> ;
    skos:altLabel "ADG"@en ;
    skos:definition "absorption by coloured dissolved organic matter"@en ;
    skos:inScheme cci-scheme:dataType ;
    skos:prefLabel "absorption by coloured dissolved organic matter"@en ;
    skos:scopeNote "absorption by coloured dissolved organic matter"@en ;
    skos:topConceptOf cci-scheme:dataType .

<http://vocab.ceda.ac.uk/collection/cci/dataType/dtype_adt> a cci:dataType,
        skos:Concept ;
    rdfs:seeAlso <https://climate.esa.int/projects/sea-level/> ;
    skos:altLabel "ADT"@en ;
    skos:definition "absolute dynamic topography"@en ;
    skos:inScheme cci-scheme:dataType ;
    skos:prefLabel "absolute dynamic topography"@en ;
    skos:scopeNote "absolute dynamic topography"@en ;
    skos:topConceptOf cci-scheme:dataType .

<http://vocab.ceda.ac.uk/collection/cci/dataType/dtype_aerProd> a cci:dataType,
        skos:Concept ;
    rdfs:seeAlso <https://climate.esa.int/projects/aerosol> ;
    skos:altLabel "AER_PRODUCTS"@en ;
    skos:definition "multiple aerosol products"@en ;
    skos:inScheme cci-scheme:dataType ;
    skos:prefLabel "multiple aerosol products"@en ;
    skos:scopeNote "multiple aerosol products"@en ;
    skos:topConceptOf cci-scheme:dataType .

<http://vocab.ceda.ac.uk/collection/cci/dataType/dtype_aex> a cci:dataType,
        skos:Concept ;
    rdfs:seeAlso <https://climate.esa.int/projects/aerosol> ;
    skos:altLabel "AEX"@en ;
    skos:definition "stratospheric aerosol extinction profile"@en ;
    skos:inScheme cci-scheme:dataType ;
    skos:prefLabel "stratospheric aerosol extinction profile"@en ;
    skos:scopeNote "stratospheric aerosol extinction profile"@en ;
    skos:topConceptOf cci-scheme:dataType .

<http://vocab.ceda.ac.uk/collection/cci/dataType/dtype_agb> a cci:dataType,
        skos:Concept ;
    rdfs:seeAlso <https://climate.esa.int/projects/biomass> ;
    skos:altLabel "AGB"@en ;
    skos:definition "above-ground biomass"@en ;
    skos:inScheme cci-scheme:dataType ;
    skos:prefLabel "above-ground biomass"@en ;
    skos:scopeNote "above-ground biomass"@en ;
    skos:topConceptOf cci-scheme:dataType .

<http://vocab.ceda.ac.uk/collection/cci/dataType/dtype_alb> a cci:dataType,
        skos:Concept ;
    rdfs:seeAlso <https://climate.esa.int/projects/land-cover/> ;
    skos:altLabel "Alb"@en ;
    skos:definition "condition albedo"@en ;
    skos:inScheme cci-scheme:dataType ;
    skos:prefLabel "condition albedo"@en ;
    skos:scopeNote "condition albedo"@en ;
    skos:topConceptOf cci-scheme:dataType .

<http://vocab.ceda.ac.uk/collection/cci/dataType/dtype_all> a cci:dataType,
        skos:Concept ;
    skos:altLabel "ALL"@en ;
    skos:definition "all"@en ;
    skos:inScheme cci-scheme:dataType ;
    skos:prefLabel "all"@en ;
    skos:scopeNote "all"@en ;
    skos:topConceptOf cci-scheme:dataType .

<http://vocab.ceda.ac.uk/collection/cci/dataType/dtype_alt> a cci:dataType,
        skos:Concept ;
    rdfs:seeAlso <https://climate.esa.int/projects/permafrost> ;
    skos:altLabel "ALT"@en ;
    skos:definition "active layer thickness"@en ;
    skos:inScheme cci-scheme:dataType ;
    skos:prefLabel "active layer thickness"@en ;
    skos:scopeNote "active layer thickness"@en ;
    skos:topConceptOf cci-scheme:dataType .

<http://vocab.ceda.ac.uk/collection/cci/dataType/dtype_aod> a cci:dataType,
        skos:Concept ;
    rdfs:seeAlso <https://climate.esa.int/projects/aerosol> ;
    skos:altLabel "AOD"@en ;
    skos:definition "aerosol optical depth"@en ;
    skos:inScheme cci-scheme:dataType ;
    skos:prefLabel "aerosol optical depth"@en ;
    skos:scopeNote "aerosol optical depth"@en ;
    skos:topConceptOf cci-scheme:dataType .

<http://vocab.ceda.ac.uk/collection/cci/dataType/dtype_aph> a cci:dataType,
        skos:Concept ;
    rdfs:seeAlso <https://climate.esa.int/projects/ocean-colour/> ;
    skos:altLabel "APH"@en ;
    skos:definition "absorption by phytoplankton"@en ;
    skos:inScheme cci-scheme:dataType ;
    skos:prefLabel "absorption by phytoplankton"@en ;
    skos:scopeNote "absorption by phytoplankton"@en ;
    skos:topConceptOf cci-scheme:dataType .

<http://vocab.ceda.ac.uk/collection/cci/dataType/dtype_atot> a cci:dataType,
        skos:Concept ;
    rdfs:seeAlso <https://climate.esa.int/projects/ocean-colour/> ;
    skos:altLabel "ATOT"@en ;
    skos:definition "total absorption"@en ;
    skos:inScheme cci-scheme:dataType ;
    skos:prefLabel "total absorption"@en ;
    skos:scopeNote "total absorption"@en ;
    skos:topConceptOf cci-scheme:dataType .

<http://vocab.ceda.ac.uk/collection/cci/dataType/dtype_aty> a cci:dataType,
        skos:Concept ;
    rdfs:seeAlso <https://climate.esa.int/projects/aerosol> ;
    skos:altLabel "ATY"@en ;
    skos:definition "aerosol type"@en ;
    skos:inScheme cci-scheme:dataType ;
    skos:prefLabel "aerosol type"@en ;
    skos:scopeNote "aerosol type"@en ;
    skos:topConceptOf cci-scheme:dataType .

<http://vocab.ceda.ac.uk/collection/cci/dataType/dtype_ba> a cci:dataType,
        skos:Concept ;
    rdfs:seeAlso <https://climate.esa.int/projects/fire>,
        <https://climate.esa.int/projects/land-cover/> ;
    skos:altLabel "BA"@en ;
    skos:definition "burned area"@en,
        "condition fire (burned area)"@en ;
    skos:inScheme cci-scheme:dataType ;
    skos:prefLabel "burned area"@en,
        "condition fire (burned area)"@en ;
    skos:scopeNote "burned area"@en,
        "condition fire (burned area)"@en ;
    skos:topConceptOf cci-scheme:dataType .

<http://vocab.ceda.ac.uk/collection/cci/dataType/dtype_bb> a cci:dataType,
        skos:Concept ;
    rdfs:seeAlso <https://climate.esa.int/projects/ocean-colour/> ;
    skos:altLabel "BB"@en ;
    skos:definition "total backscattering"@en ;
    skos:inScheme cci-scheme:dataType ;
    skos:prefLabel "total backscattering"@en ;
    skos:scopeNote "total backscattering"@en ;
    skos:topConceptOf cci-scheme:dataType .

<http://vocab.ceda.ac.uk/collection/cci/dataType/dtype_cer> a cci:dataType,
        skos:Concept ;
    rdfs:seeAlso <https://climate.esa.int/projects/cloud> ;
    skos:altLabel "CER"@en ;
    skos:definition "cloud effective radius"@en ;
    skos:inScheme cci-scheme:dataType ;
    skos:prefLabel "cloud effective radius"@en ;
    skos:scopeNote "cloud effective radius"@en ;
    skos:topConceptOf cci-scheme:dataType .

<http://vocab.ceda.ac.uk/collection/cci/dataType/dtype_cfc> a cci:dataType,
        skos:Concept ;
    rdfs:seeAlso <https://climate.esa.int/projects/cloud> ;
    skos:altLabel "CFC"@en ;
    skos:definition "cloud cover"@en ;
    skos:inScheme cci-scheme:dataType ;
    skos:prefLabel "cloud cover"@en ;
    skos:scopeNote "cloud cover"@en ;
    skos:topConceptOf cci-scheme:dataType .

<http://vocab.ceda.ac.uk/collection/cci/dataType/dtype_cfl> a cci:dataType,
        skos:Concept ;
    rdfs:seeAlso <http://www.esa-icesheets-cci.org/> ;
    skos:altLabel "CFL"@en ;
    skos:definition "glacier calving front location"@en ;
    skos:inScheme cci-scheme:dataType ;
    skos:prefLabel "glacier calving front location"@en ;
    skos:scopeNote "glacier calving front location"@en ;
    skos:topConceptOf cci-scheme:dataType .

<http://vocab.ceda.ac.uk/collection/cci/dataType/dtype_ch4> a cci:dataType,
        skos:Concept ;
    rdfs:seeAlso <https://climate.esa.int/projects/ghgs> ;
    skos:altLabel "CH4"@en ;
    skos:definition "column-averaged dry air mole fraction of CH4"@en ;
    skos:inScheme cci-scheme:dataType ;
    skos:prefLabel "column-averaged dry air mole fraction of CH4"@en ;
    skos:scopeNote "column-averaged dry air mole fraction of CH4"@en ;
    skos:topConceptOf cci-scheme:dataType .

<http://vocab.ceda.ac.uk/collection/cci/dataType/dtype_chlorA> a cci:dataType,
        skos:Concept ;
    rdfs:seeAlso <https://climate.esa.int/projects/ocean-colour/> ;
    skos:altLabel "CHLOR_A"@en ;
    skos:definition "phytoplankton chlorophyll-a concentration"@en ;
    skos:inScheme cci-scheme:dataType ;
    skos:prefLabel "phytoplankton chlorophyll-a concentration"@en ;
    skos:scopeNote "phytoplankton chlorophyll-a concentration"@en ;
    skos:topConceptOf cci-scheme:dataType .

<http://vocab.ceda.ac.uk/collection/cci/dataType/dtype_cldProd> a cci:dataType,
        skos:Concept ;
    rdfs:seeAlso <https://climate.esa.int/projects/cloud> ;
    skos:altLabel "CLD_PRODUCTS"@en ;
    skos:definition "multiple cloud products"@en ;
    skos:inScheme cci-scheme:dataType ;
    skos:prefLabel "multiple cloud products"@en ;
    skos:scopeNote "multiple cloud products"@en ;
    skos:topConceptOf cci-scheme:dataType .

<http://vocab.ceda.ac.uk/collection/cci/dataType/dtype_co2> a cci:dataType,
        skos:Concept ;
    rdfs:seeAlso <https://climate.esa.int/projects/ghgs> ;
    skos:altLabel "CO2"@en ;
    skos:definition "column-averaged dry air mole fraction of CO2"@en ;
    skos:inScheme cci-scheme:dataType ;
    skos:prefLabel "column-averaged dry air mole fraction of CO2"@en ;
    skos:scopeNote "column-averaged dry air mole fraction of CO2"@en ;
    skos:topConceptOf cci-scheme:dataType .

<http://vocab.ceda.ac.uk/collection/cci/dataType/dtype_cot> a cci:dataType,
        skos:Concept ;
    rdfs:seeAlso <https://climate.esa.int/projects/cloud> ;
    skos:altLabel "COT"@en ;
    skos:definition "cloud optical thickness"@en ;
    skos:inScheme cci-scheme:dataType ;
    skos:prefLabel "cloud optical thickness"@en ;
    skos:scopeNote "cloud optical thickness"@en ;
    skos:topConceptOf cci-scheme:dataType .

<http://vocab.ceda.ac.uk/collection/cci/dataType/dtype_cth> a cci:dataType,
        skos:Concept ;
    rdfs:seeAlso <https://climate.esa.int/projects/cloud> ;
    skos:altLabel "CTH"@en ;
    skos:definition "cloud top height"@en ;
    skos:inScheme cci-scheme:dataType ;
    skos:prefLabel "cloud top height"@en ;
    skos:scopeNote "cloud top height"@en ;
    skos:topConceptOf cci-scheme:dataType .

<http://vocab.ceda.ac.uk/collection/cci/dataType/dtype_ctp> a cci:dataType,
        skos:Concept ;
    rdfs:seeAlso <https://climate.esa.int/projects/cloud> ;
    skos:altLabel "CTP"@en ;
    skos:definition "cloud top pressure"@en ;
    skos:inScheme cci-scheme:dataType ;
    skos:prefLabel "cloud top pressure"@en ;
    skos:scopeNote "cloud top pressure"@en ;
    skos:topConceptOf cci-scheme:dataType .

<http://vocab.ceda.ac.uk/collection/cci/dataType/dtype_ctt> a cci:dataType,
        skos:Concept ;
    rdfs:seeAlso <https://climate.esa.int/projects/cloud> ;
    skos:altLabel "CTT"@en ;
    skos:definition "cloud top temperature"@en ;
    skos:inScheme cci-scheme:dataType ;
    skos:prefLabel "cloud top temperature"@en ;
    skos:scopeNote "cloud top temperature"@en ;
    skos:topConceptOf cci-scheme:dataType .

<http://vocab.ceda.ac.uk/collection/cci/dataType/dtype_ga> a cci:dataType,
        skos:Concept ;
    rdfs:seeAlso <https://climate.esa.int/projects/glaciers> ;
    skos:altLabel "GA"@en ;
    skos:definition "glacier area"@en ;
    skos:inScheme cci-scheme:dataType ;
    skos:prefLabel "glacier area"@en ;
    skos:scopeNote "glacier area"@en ;
    skos:topConceptOf cci-scheme:dataType .

<http://vocab.ceda.ac.uk/collection/cci/dataType/dtype_gll> a cci:dataType,
        skos:Concept ;
    rdfs:seeAlso <http://www.esa-icesheets-cci.org/> ;
    skos:altLabel "GLL"@en ;
    skos:definition "glacier grounding line location"@en ;
    skos:inScheme cci-scheme:dataType ;
    skos:prefLabel "glacier grounding line location"@en ;
    skos:scopeNote "glacier grounding line location"@en ;
    skos:topConceptOf cci-scheme:dataType .

<http://vocab.ceda.ac.uk/collection/cci/dataType/dtype_gmb> a cci:dataType,
        skos:Concept ;
    rdfs:seeAlso <http://www.esa-icesheets-cci.org/> ;
    skos:altLabel "GMB"@en ;
    skos:definition "gravimetric mass balance"@en ;
    skos:inScheme cci-scheme:dataType ;
    skos:prefLabel "gravimetric mass balance"@en ;
    skos:scopeNote "gravimetric mass balance"@en ;
    skos:topConceptOf cci-scheme:dataType .

<http://vocab.ceda.ac.uk/collection/cci/dataType/dtype_gtd> a cci:dataType,
        skos:Concept ;
    rdfs:seeAlso <https://climate.esa.int/projects/permafrost> ;
    skos:altLabel "GTD"@en ;
    skos:definition "ground temperature at a certain depth"@en ;
    skos:inScheme cci-scheme:dataType ;
    skos:prefLabel "ground temperature"@en ;
    skos:scopeNote "ground temperature at a certain depth"@en ;
    skos:topConceptOf cci-scheme:dataType .

<http://vocab.ceda.ac.uk/collection/cci/dataType/dtype_iop> a cci:dataType,
        skos:Concept ;
    rdfs:seeAlso <https://climate.esa.int/projects/ocean-colour/> ;
    skos:altLabel "IOP"@en ;
    skos:definition "inherent optical properties"@en ;
    skos:inScheme cci-scheme:dataType ;
    skos:prefLabel "inherent optical properties"@en ;
    skos:scopeNote "inherent optical properties"@en ;
    skos:topConceptOf cci-scheme:dataType .

<http://vocab.ceda.ac.uk/collection/cci/dataType/dtype_iv> a cci:dataType,
        skos:Concept ;
    rdfs:seeAlso <http://www.esa-icesheets-cci.org/> ;
    skos:altLabel "IV"@en ;
    skos:definition "ice sheet velocity"@en ;
    skos:inScheme cci-scheme:dataType ;
    skos:prefLabel "ice sheet velocity"@en ;
    skos:scopeNote "ice sheet velocity"@en ;
    skos:topConceptOf cci-scheme:dataType .

<http://vocab.ceda.ac.uk/collection/cci/dataType/dtype_iwp> a cci:dataType,
        skos:Concept ;
    rdfs:seeAlso <https://climate.esa.int/projects/cloud> ;
    skos:altLabel "IWP"@en ;
    skos:definition "cloud ice water path"@en ;
    skos:inScheme cci-scheme:dataType ;
    skos:prefLabel "cloud ice water path"@en ;
    skos:scopeNote "cloud ice water path"@en ;
    skos:topConceptOf cci-scheme:dataType .

<http://vocab.ceda.ac.uk/collection/cci/dataType/dtype_jch> a cci:dataType,
        skos:Concept ;
    rdfs:seeAlso <https://climate.esa.int/projects/cloud> ;
    skos:altLabel "JCH"@en ;
    skos:definition "joint cloud physical properties"@en ;
    skos:inScheme cci-scheme:dataType ;
    skos:prefLabel "joint cloud physical properties"@en ;
    skos:scopeNote "joint cloud physical properties"@en ;
    skos:topConceptOf cci-scheme:dataType .

<http://vocab.ceda.ac.uk/collection/cci/dataType/dtype_k_490> a cci:dataType,
        skos:Concept ;
    rdfs:seeAlso <https://climate.esa.int/projects/ocean-colour/> ;
    skos:altLabel "K_490"@en ;
    skos:definition "spectral attenuation coefficient for downwelling irradiance"@en ;
    skos:inScheme cci-scheme:dataType ;
    skos:prefLabel "spectral attenuation coefficient for downwelling irradiance"@en ;
    skos:scopeNote "spectral attenuation coefficient for downwelling irradiance"@en ;
    skos:topConceptOf cci-scheme:dataType .

<http://vocab.ceda.ac.uk/collection/cci/dataType/dtype_lai> a cci:dataType,
        skos:Concept ;
    rdfs:seeAlso <https://climate.esa.int/projects/land-cover/> ;
    skos:altLabel "LAI"@en ;
    skos:definition "leaf area Index"@en ;
    skos:inScheme cci-scheme:dataType ;
    skos:prefLabel "leaf area Index"@en ;
    skos:scopeNote "leaf area Index"@en ;
    skos:topConceptOf cci-scheme:dataType .

<http://vocab.ceda.ac.uk/collection/cci/dataType/dtype_lcchange> a cci:dataType,
        skos:Concept ;
    rdfs:seeAlso <https://climate.esa.int/projects/high-resolution-land-cover> ;
    skos:altLabel "CHANGE"@en ;
    skos:definition "land cover change uncertainty maps"@en ;
    skos:inScheme cci-scheme:dataType ;
    skos:prefLabel "land cover change"@en ;
    skos:scopeNote "land cover change uncertainty maps"@en ;
    skos:topConceptOf cci-scheme:dataType .

<http://vocab.ceda.ac.uk/collection/cci/dataType/dtype_lccs> a cci:dataType,
        skos:Concept ;
    rdfs:seeAlso <https://climate.esa.int/projects/land-cover/> ;
    skos:altLabel "LCCS"@en ;
    skos:definition "land cover classification system"@en ;
    skos:inScheme cci-scheme:dataType ;
    skos:prefLabel "land cover classification system"@en ;
    skos:scopeNote "land cover classification system"@en ;
    skos:topConceptOf cci-scheme:dataType .

<http://vocab.ceda.ac.uk/collection/cci/dataType/dtype_lkProds> a cci:dataType,
        skos:Concept ;
    rdfs:seeAlso <https://climate.esa.int/projects/lakes> ;
    skos:altLabel "LK_PRODUCTS"@en ;
    skos:definition "multiple lake products"@en ;
    skos:inScheme cci-scheme:dataType ;
    skos:prefLabel "multiple lake products"@en ;
    skos:scopeNote "multiple lake products"@en ;
    skos:topConceptOf cci-scheme:dataType .

<http://vocab.ceda.ac.uk/collection/cci/dataType/dtype_lp> a cci:dataType,
        skos:Concept ;
    rdfs:seeAlso <https://climate.esa.int/projects/ozone> ;
    skos:altLabel "LP"@en ;
    skos:definition "ozone limb profile"@en ;
    skos:inScheme cci-scheme:dataType ;
    skos:prefLabel "ozone limb profile"@en ;
    skos:scopeNote "ozone limb profile"@en ;
    skos:topConceptOf cci-scheme:dataType .

<http://vocab.ceda.ac.uk/collection/cci/dataType/dtype_lst> a cci:dataType,
        skos:Concept ;
    rdfs:seeAlso <https://climate.esa.int/projects/land-surface-temperature> ;
    skos:altLabel "LST"@en ;
    skos:definition "land surface temperature"@en ;
    skos:inScheme cci-scheme:dataType ;
    skos:prefLabel "land surface temperature"@en ;
    skos:scopeNote "land surface temperature"@en ;
    skos:topConceptOf cci-scheme:dataType .

<http://vocab.ceda.ac.uk/collection/cci/dataType/dtype_lwp> a cci:dataType,
        skos:Concept ;
    rdfs:seeAlso <https://climate.esa.int/projects/cloud> ;
    skos:altLabel "LWP"@en ;
    skos:definition "cloud liquid water path"@en ;
    skos:inScheme cci-scheme:dataType ;
    skos:prefLabel "cloud liquid water path"@en ;
    skos:scopeNote "cloud liquid water path"@en ;
    skos:topConceptOf cci-scheme:dataType .

<http://vocab.ceda.ac.uk/collection/cci/dataType/dtype_map> a cci:dataType,
        skos:Concept ;
    rdfs:seeAlso <https://climate.esa.int/projects/land-cover/> ;
    skos:altLabel "Map"@en ;
    skos:definition "land cover map"@en ;
    skos:inScheme cci-scheme:dataType ;
    skos:prefLabel "land cover map"@en ;
    skos:scopeNote "land cover map"@en ;
    skos:topConceptOf cci-scheme:dataType .

<http://vocab.ceda.ac.uk/collection/cci/dataType/dtype_msl> a cci:dataType,
        skos:Concept ;
    rdfs:seeAlso <https://climate.esa.int/projects/sea-level/> ;
    skos:altLabel "MSL"@en ;
    skos:definition "mean sea level"@en ;
    skos:inScheme cci-scheme:dataType ;
    skos:prefLabel "mean sea level"@en ;
    skos:scopeNote "mean sea level"@en ;
    skos:topConceptOf cci-scheme:dataType .

<http://vocab.ceda.ac.uk/collection/cci/dataType/dtype_msla> a cci:dataType,
        skos:Concept ;
    rdfs:seeAlso <https://climate.esa.int/projects/sea-level/> ;
    skos:altLabel "MSLA"@en ;
    skos:definition "maps of sea level anomalies"@en ;
    skos:inScheme cci-scheme:dataType ;
    skos:prefLabel "maps of sea level anomalies"@en ;
    skos:scopeNote "maps of sea level anomalies"@en ;
    skos:topConceptOf cci-scheme:dataType .

<http://vocab.ceda.ac.uk/collection/cci/dataType/dtype_mslamph> a cci:dataType,
        skos:Concept ;
    rdfs:seeAlso <https://climate.esa.int/projects/sea-level/> ;
    skos:altLabel "MSLAMPH"@en ;
    skos:definition "mean sea level amplitude and phase"@en ;
    skos:inScheme cci-scheme:dataType ;
    skos:prefLabel "mean sea level amplitude and phase"@en ;
    skos:scopeNote "mean sea level amplitude and phase"@en ;
    skos:topConceptOf cci-scheme:dataType .

<http://vocab.ceda.ac.uk/collection/cci/dataType/dtype_msltr> a cci:dataType,
        skos:Concept ;
    rdfs:seeAlso <https://climate.esa.int/projects/sea-level/> ;
    skos:altLabel "MSLTR"@en ;
    skos:definition "mean sea level trends"@en ;
    skos:inScheme cci-scheme:dataType ;
    skos:prefLabel "mean sea level trends"@en ;
    skos:scopeNote "mean sea level trends"@en ;
    skos:topConceptOf cci-scheme:dataType .

<http://vocab.ceda.ac.uk/collection/cci/dataType/dtype_ndvi> a cci:dataType,
        skos:Concept ;
    rdfs:seeAlso <https://climate.esa.int/projects/land-cover/> ;
    skos:altLabel "NDVI"@en ;
    skos:definition "condition normalised difference vegetation index"@en ;
    skos:inScheme cci-scheme:dataType ;
    skos:prefLabel "condition normalised difference vegetation index"@en ;
    skos:scopeNote "condition normalised difference vegetation index"@en ;
    skos:topConceptOf cci-scheme:dataType .

<http://vocab.ceda.ac.uk/collection/cci/dataType/dtype_nlw> a cci:dataType,
        skos:Concept ;
    rdfs:seeAlso <https://climate.esa.int/projects/ocean-colour/> ;
    skos:altLabel "NLW"@en ;
    skos:definition "normalised water leaving radiance"@en ;
    skos:inScheme cci-scheme:dataType ;
    skos:prefLabel "normalised water leaving radiance"@en ;
    skos:scopeNote "normalised water leaving radiance"@en ;
    skos:topConceptOf cci-scheme:dataType .

<http://vocab.ceda.ac.uk/collection/cci/dataType/dtype_np> a cci:dataType,
        skos:Concept ;
    rdfs:seeAlso <https://climate.esa.int/projects/ozone> ;
    skos:altLabel "NP"@en ;
    skos:definition "ozone nadir profile"@en ;
    skos:inScheme cci-scheme:dataType ;
    skos:prefLabel "ozone nadir profile"@en ;
    skos:scopeNote "ozone nadir profile"@en ;
    skos:topConceptOf cci-scheme:dataType .

<http://vocab.ceda.ac.uk/collection/cci/dataType/dtype_ocProd> a cci:dataType,
        skos:Concept ;
    rdfs:seeAlso <https://climate.esa.int/projects/ocean-colour/> ;
    skos:altLabel "OC_PRODUCTS"@en ;
    skos:definition "multiple products (chla, nlw, IOPs, etc)"@en ;
    skos:inScheme cci-scheme:dataType ;
    skos:prefLabel "multiple products (chla, nlw, IOPs, etc)"@en ;
    skos:scopeNote "multiple products (chla, nlw, IOPs, etc)"@en ;
    skos:topConceptOf cci-scheme:dataType .

<http://vocab.ceda.ac.uk/collection/cci/dataType/dtype_pfr> a cci:dataType,
        skos:Concept ;
    rdfs:seeAlso <https://climate.esa.int/projects/permafrost> ;
    skos:altLabel "PFR"@en ;
    skos:definition "permafrost extent (fraction)"@en ;
    skos:inScheme cci-scheme:dataType ;
    skos:prefLabel "permafrost extent"@en ;
    skos:scopeNote "permafrost extent (fraction)"@en ;
    skos:topConceptOf cci-scheme:dataType .

<http://vocab.ceda.ac.uk/collection/cci/dataType/dtype_pft> a cci:dataType,
        skos:Concept ;
    rdfs:seeAlso <https://climate.esa.int/projects/land-cover> ;
    skos:altLabel "PFT"@en ;
    skos:definition "plant functional types"@en ;
    skos:inScheme cci-scheme:dataType ;
    skos:prefLabel "plant functional types"@en ;
    skos:scopeNote "plant functional types"@en ;
    skos:topConceptOf cci-scheme:dataType .

<http://vocab.ceda.ac.uk/collection/cci/dataType/dtype_rrs> a cci:dataType,
        skos:Concept ;
    rdfs:seeAlso <https://climate.esa.int/projects/ocean-colour/> ;
    skos:altLabel "RRS"@en ;
    skos:definition "remote sensing reflectance"@en ;
    skos:inScheme cci-scheme:dataType ;
    skos:prefLabel "remote sensing reflectance"@en ;
    skos:scopeNote "remote sensing reflectance"@en ;
    skos:topConceptOf cci-scheme:dataType .

<http://vocab.ceda.ac.uk/collection/cci/dataType/dtype_scfg> a cci:dataType,
        skos:Concept ;
    rdfs:seeAlso <https://climate.esa.int/projects/snow> ;
    skos:altLabel "SCFG"@en ;
    skos:definition "snow cover fraction - snow on ground"@en ;
    skos:inScheme cci-scheme:dataType ;
    skos:prefLabel "snow cover fraction - snow on ground"@en ;
    skos:scopeNote "snow cover fraction - snow on ground"@en ;
    skos:topConceptOf cci-scheme:dataType .

<http://vocab.ceda.ac.uk/collection/cci/dataType/dtype_scfv> a cci:dataType,
        skos:Concept ;
    rdfs:seeAlso <https://climate.esa.int/projects/snow> ;
    skos:altLabel "SCFV"@en ;
    skos:definition "snow cover fraction  - viewable"@en ;
    skos:inScheme cci-scheme:dataType ;
    skos:prefLabel "snow cover fraction - viewable"@en ;
    skos:scopeNote "snow cover fraction  - viewable"@en ;
    skos:topConceptOf cci-scheme:dataType .

<http://vocab.ceda.ac.uk/collection/cci/dataType/dtype_sec> a cci:dataType,
        skos:Concept ;
    rdfs:seeAlso <http://www.esa-icesheets-cci.org/> ;
    skos:altLabel "SEC"@en ;
    skos:definition "ice sheet surface elevation change"@en ;
    skos:inScheme cci-scheme:dataType ;
    skos:prefLabel "ice sheet surface elevation change"@en ;
    skos:scopeNote "ice sheet surface elevation change"@en ;
    skos:topConceptOf cci-scheme:dataType .

<http://vocab.ceda.ac.uk/collection/cci/dataType/dtype_sic> a cci:dataType,
        skos:Concept ;
    rdfs:seeAlso <https://climate.esa.int/projects/sea-ice/> ;
    skos:altLabel "SICONC"@en ;
    skos:definition "sea ice concentration"@en ;
    skos:inScheme cci-scheme:dataType ;
    skos:prefLabel "sea ice concentration"@en ;
    skos:scopeNote "sea ice concentration"@en ;
    skos:topConceptOf cci-scheme:dataType .

<http://vocab.ceda.ac.uk/collection/cci/dataType/dtype_sie> a cci:dataType,
        skos:Concept ;
    rdfs:seeAlso <https://climate.esa.int/projects/sea-ice/> ;
    skos:altLabel "SIEXTENT"@en ;
    skos:definition "sea ice extent"@en ;
    skos:inScheme cci-scheme:dataType ;
    skos:prefLabel "sea ice extent"@en ;
    skos:scopeNote "sea ice extent"@en ;
    skos:topConceptOf cci-scheme:dataType .

<http://vocab.ceda.ac.uk/collection/cci/dataType/dtype_sit> a cci:dataType,
        skos:Concept ;
    rdfs:seeAlso <https://climate.esa.int/projects/sea-ice/> ;
    skos:altLabel "SITHICK"@en ;
    skos:definition "sea ice thickness"@en ;
    skos:inScheme cci-scheme:dataType ;
    skos:prefLabel "sea ice thickness"@en ;
    skos:scopeNote "sea ice thickness"@en ;
    skos:topConceptOf cci-scheme:dataType .

<http://vocab.ceda.ac.uk/collection/cci/dataType/dtype_sla> a cci:dataType,
        skos:Concept ;
    rdfs:seeAlso <https://climate.esa.int/projects/sea-level/> ;
    skos:altLabel "SLA"@en ;
    skos:definition "sea level anomaly"@en ;
    skos:inScheme cci-scheme:dataType ;
    skos:prefLabel "sea level anomaly"@en ;
    skos:scopeNote "sea level anomaly"@en ;
    skos:topConceptOf cci-scheme:dataType .

<http://vocab.ceda.ac.uk/collection/cci/dataType/dtype_snow> a cci:dataType,
        skos:Concept ;
    rdfs:seeAlso <https://climate.esa.int/projects/land-cover/> ;
    skos:altLabel "Snow"@en ;
    skos:definition "condition snow"@en ;
    skos:inScheme cci-scheme:dataType ;
    skos:prefLabel "condition snow"@en ;
    skos:scopeNote "condition snow"@en ;
    skos:topConceptOf cci-scheme:dataType .

<http://vocab.ceda.ac.uk/collection/cci/dataType/dtype_sr> a cci:dataType,
        skos:Concept ;
    rdfs:seeAlso <https://climate.esa.int/projects/land-cover/> ;
    skos:altLabel "SR"@en ;
    skos:definition "surface reflectance"@en ;
    skos:inScheme cci-scheme:dataType ;
    skos:prefLabel "surface reflectance"@en ;
    skos:scopeNote "surface reflectance"@en ;
    skos:topConceptOf cci-scheme:dataType .

<http://vocab.ceda.ac.uk/collection/cci/dataType/dtype_ssh> a cci:dataType,
        skos:Concept ;
    rdfs:seeAlso <https://climate.esa.int/projects/sea-level/> ;
    skos:altLabel "SSH"@en ;
    skos:definition "corrected sea surface height"@en ;
    skos:inScheme cci-scheme:dataType ;
    skos:prefLabel "corrected sea surface height"@en ;
    skos:scopeNote "corrected sea surface height"@en ;
    skos:topConceptOf cci-scheme:dataType .

<http://vocab.ceda.ac.uk/collection/cci/dataType/dtype_ssms> a cci:dataType,
        skos:Concept ;
    rdfs:seeAlso <https://climate.esa.int/projects/soil-moisture/> ;
    skos:altLabel "SSMS"@en ;
    skos:definition "surface soil moisture degree of saturation absolute"@en ;
    skos:inScheme cci-scheme:dataType ;
    skos:prefLabel "surface soil moisture degree of saturation absolute"@en ;
    skos:scopeNote "surface soil moisture degree of saturation absolute"@en ;
    skos:topConceptOf cci-scheme:dataType .

<http://vocab.ceda.ac.uk/collection/cci/dataType/dtype_ssmsa> a cci:dataType,
        skos:Concept ;
    rdfs:seeAlso <https://climate.esa.int/projects/soil-moisture/> ;
    skos:altLabel "SSMSA"@en ;
    skos:definition "surface soil moisture degree of saturation anomalies"@en ;
    skos:inScheme cci-scheme:dataType ;
    skos:prefLabel "surface soil moisture degree of saturation anomalies"@en ;
    skos:scopeNote "surface soil moisture degree of saturation anomalies"@en ;
    skos:topConceptOf cci-scheme:dataType .

<http://vocab.ceda.ac.uk/collection/cci/dataType/dtype_ssmv> a cci:dataType,
        skos:Concept ;
    rdfs:seeAlso <https://climate.esa.int/projects/soil-moisture/> ;
    skos:altLabel "SSMV"@en ;
    skos:definition "surface soil moisture volumetric absolutes"@en ;
    skos:inScheme cci-scheme:dataType ;
    skos:prefLabel "surface soil moisture volumetric absolutes"@en ;
    skos:scopeNote "surface soil moisture volumetric absolutes"@en ;
    skos:topConceptOf cci-scheme:dataType .

<http://vocab.ceda.ac.uk/collection/cci/dataType/dtype_ssmva> a cci:dataType,
        skos:Concept ;
    rdfs:seeAlso <https://climate.esa.int/projects/soil-moisture/> ;
    skos:altLabel "SSMVA"@en ;
    skos:definition "surface soil moisture volumetric anomalies"@en ;
    skos:inScheme cci-scheme:dataType ;
    skos:prefLabel "surface soil moisture volumetric anomalies"@en ;
    skos:scopeNote "surface soil moisture volumetric anomalies"@en ;
    skos:topConceptOf cci-scheme:dataType .

<http://vocab.ceda.ac.uk/collection/cci/dataType/dtype_sss> a cci:dataType,
        skos:Concept ;
    rdfs:seeAlso <https://climate.esa.int/projects/sea-surface-salinity> ;
    skos:altLabel "SSS"@en ;
    skos:definition "sea surface salinity"@en ;
    skos:inScheme cci-scheme:dataType ;
    skos:prefLabel "sea surface salinity"@en ;
    skos:scopeNote "sea surface salinity"@en ;
    skos:topConceptOf cci-scheme:dataType .

<http://vocab.ceda.ac.uk/collection/cci/dataType/dtype_sstDepth> a cci:dataType,
        skos:Concept ;
    rdfs:seeAlso <https://climate.esa.int/projects/sea-surface-temperature/> ;
    skos:altLabel "SSTdepth"@en ;
    skos:definition "sea water temperature"@en ;
    skos:inScheme cci-scheme:dataType ;
    skos:prefLabel "sea water temperature"@en ;
    skos:scopeNote "sea water temperature"@en ;
    skos:topConceptOf cci-scheme:dataType .

<http://vocab.ceda.ac.uk/collection/cci/dataType/dtype_sstFnd> a cci:dataType,
        skos:Concept ;
    rdfs:seeAlso <https://climate.esa.int/projects/sea-surface-temperature/> ;
    skos:altLabel "SSTfnd"@en ;
    skos:definition "sea surface foundation temperature"@en ;
    skos:inScheme cci-scheme:dataType ;
    skos:prefLabel "sea surface foundation temperature"@en ;
    skos:scopeNote "sea surface foundation temperature"@en ;
    skos:topConceptOf cci-scheme:dataType .

<http://vocab.ceda.ac.uk/collection/cci/dataType/dtype_sstInt> a cci:dataType,
        skos:Concept ;
    rdfs:seeAlso <https://climate.esa.int/projects/sea-surface-temperature/> ;
    skos:altLabel "SSTint"@en ;
    skos:definition "sea surface temperature"@en ;
    skos:inScheme cci-scheme:dataType ;
    skos:prefLabel "sea surface temperature"@en ;
    skos:scopeNote "sea surface temperature"@en ;
    skos:topConceptOf cci-scheme:dataType .

<http://vocab.ceda.ac.uk/collection/cci/dataType/dtype_sstSkin> a cci:dataType,
        skos:Concept ;
    rdfs:seeAlso <https://climate.esa.int/projects/sea-surface-temperature/> ;
    skos:altLabel "SSTskin"@en ;
    skos:definition "sea surface skin temperature"@en ;
    skos:inScheme cci-scheme:dataType ;
    skos:prefLabel "sea surface skin temperature"@en ;
    skos:scopeNote "sea surface skin temperature"@en ;
    skos:topConceptOf cci-scheme:dataType .

<http://vocab.ceda.ac.uk/collection/cci/dataType/dtype_sstSubsk> a cci:dataType,
        skos:Concept ;
    rdfs:seeAlso <https://climate.esa.int/projects/sea-surface-temperature/> ;
    skos:altLabel "SSTsubskin"@en ;
    skos:definition "sea surface subskin temperature"@en ;
    skos:inScheme cci-scheme:dataType ;
    skos:prefLabel "sea surface subskin temperature"@en ;
    skos:scopeNote "sea surface subskin temperature"@en ;
    skos:topConceptOf cci-scheme:dataType .

<http://vocab.ceda.ac.uk/collection/cci/dataType/dtype_swe> a cci:dataType,
        skos:Concept ;
    rdfs:seeAlso <https://climate.esa.int/projects/snow> ;
    skos:altLabel "SWE"@en ;
    skos:definition "snow water equivalent"@en ;
    skos:inScheme cci-scheme:dataType ;
    skos:prefLabel "snow water equivalent"@en ;
    skos:scopeNote "snow water equivalent"@en ;
    skos:topConceptOf cci-scheme:dataType .

<http://vocab.ceda.ac.uk/collection/cci/dataType/dtype_swh> a cci:dataType,
        skos:Concept ;
    rdfs:seeAlso <https://climate.esa.int/projects/sea-state/> ;
    skos:altLabel "SWH"@en ;
    skos:definition "significant wave height"@en ;
    skos:inScheme cci-scheme:dataType ;
    skos:prefLabel "significant wave height"@en ;
    skos:scopeNote "significant wave height"@en ;
    skos:topConceptOf cci-scheme:dataType .

<http://vocab.ceda.ac.uk/collection/cci/dataType/dtype_swis> a cci:dataType,
        skos:Concept ;
    rdfs:seeAlso <https://climate.esa.int/projects/soil-moisture/> ;
    skos:altLabel "SWIS"@en ;
    skos:definition "soil water index degree of saturation absolute"@en ;
    skos:inScheme cci-scheme:dataType ;
    skos:prefLabel "soil water index degree of saturation absolute"@en ;
    skos:scopeNote "soil water index degree of saturation absolute"@en ;
    skos:topConceptOf cci-scheme:dataType .

<http://vocab.ceda.ac.uk/collection/cci/dataType/dtype_swisa> a cci:dataType,
        skos:Concept ;
    rdfs:seeAlso <https://climate.esa.int/projects/soil-moisture/> ;
    skos:altLabel "SWISA"@en ;
    skos:definition "soil water index degree of saturation anomalie"@en ;
    skos:inScheme cci-scheme:dataType ;
    skos:prefLabel "soil water index degree of saturation anomalie"@en ;
    skos:scopeNote "soil water index degree of saturation anomalie"@en ;
    skos:topConceptOf cci-scheme:dataType .

<http://vocab.ceda.ac.uk/collection/cci/dataType/dtype_swiv> a cci:dataType,
        skos:Concept ;
    rdfs:seeAlso <https://climate.esa.int/projects/soil-moisture/> ;
    skos:altLabel "SWIV"@en ;
    skos:definition "soil water index volumetric absolute"@en ;
    skos:inScheme cci-scheme:dataType ;
    skos:prefLabel "soil water index volumetric absolute"@en ;
    skos:scopeNote "soil water index volumetric absolute"@en ;
    skos:topConceptOf cci-scheme:dataType .

<http://vocab.ceda.ac.uk/collection/cci/dataType/dtype_swiva> a cci:dataType,
        skos:Concept ;
    rdfs:seeAlso <https://climate.esa.int/projects/soil-moisture/> ;
    skos:altLabel "SWIVA"@en ;
    skos:definition "soil water index volumetric anomalies"@en ;
    skos:inScheme cci-scheme:dataType ;
    skos:prefLabel "soil water index volumetric anomalies"@en ;
    skos:scopeNote "soil water index volumetric anomalies"@en ;
    skos:topConceptOf cci-scheme:dataType .

<http://vocab.ceda.ac.uk/collection/cci/dataType/dtype_tc> a cci:dataType,
        skos:Concept ;
    rdfs:seeAlso <https://climate.esa.int/projects/ozone> ;
    skos:altLabel "TC"@en ;
    skos:definition "ozone total column"@en ;
    skos:inScheme cci-scheme:dataType ;
    skos:prefLabel "ozone total column"@en ;
    skos:scopeNote "ozone total column"@en ;
    skos:topConceptOf cci-scheme:dataType .

<http://vocab.ceda.ac.uk/collection/cci/dataType/dtype_tcwv> a cci:dataType,
        skos:Concept ;
    rdfs:seeAlso <https://climate.esa.int/projects/water-vapour> ;
    skos:altLabel "TCWV"@en ;
    skos:definition "total column water vapour"@en ;
    skos:inScheme cci-scheme:dataType ;
    skos:prefLabel "total column water vapour"@en ;
    skos:scopeNote "total column water vapour"@en ;
    skos:topConceptOf cci-scheme:dataType .

<http://vocab.ceda.ac.uk/collection/cci/dataType/dtype_uncert> a cci:dataType,
        skos:Concept ;
    rdfs:seeAlso <https://climate.esa.int/projects/high-resolution-land-cover> ;
    skos:altLabel "UNCERT"@en ;
    skos:definition "land cover uncertainty maps"@en ;
    skos:inScheme cci-scheme:dataType ;
    skos:prefLabel "uncertainty"@en ;
    skos:scopeNote "land cover uncertainty maps"@en ;
    skos:topConceptOf cci-scheme:dataType .

<http://vocab.ceda.ac.uk/collection/cci/dataType/dtype_unspecified> a cci:dataType,
        skos:Concept ;
    skos:altLabel "UNSPECIFIED"@en ;
    skos:definition "unspecified"@en ;
    skos:inScheme cci-scheme:dataType ;
    skos:prefLabel "unspecified"@en ;
    skos:scopeNote "unspecified"@en ;
    skos:topConceptOf cci-scheme:dataType .

<http://vocab.ceda.ac.uk/collection/cci/dataType/dtype_v> a cci:dataType,
        skos:Concept ;
    rdfs:seeAlso <https://climate.esa.int/projects/ocean-colour/> ;
    skos:altLabel "v"@en ;
    skos:definition "backscattering by particulate matter"@en ;
    skos:inScheme cci-scheme:dataType ;
    skos:prefLabel "backscattering by particulate matter"@en ;
    skos:scopeNote "backscattering by particulate matter"@en ;
    skos:topConceptOf cci-scheme:dataType .

<http://vocab.ceda.ac.uk/collection/cci/dataType/dtype_vp> a cci:dataType,
        skos:Concept ;
    rdfs:seeAlso <https://climate.esa.int/en/projects/vegetation-parameters/> ;
    skos:altLabel "VP_PRODUCTS"@en ;
    skos:definition "vegetation parameters"@en ;
    skos:inScheme cci-scheme:dataType ;
    skos:prefLabel "vegetation parameters"@en ;
    skos:scopeNote "vegetation parameters"@en ;
    skos:topConceptOf cci-scheme:dataType .

<http://vocab.ceda.ac.uk/collection/cci/dataType/dtype_wb> a cci:dataType,
        skos:Concept ;
    rdfs:seeAlso <https://climate.esa.int/projects/land-cover/> ;
    skos:altLabel "WB"@en ;
    skos:definition "condition water (water bodies)"@en ;
    skos:inScheme cci-scheme:dataType ;
    skos:prefLabel "condition water (water bodies)"@en ;
    skos:scopeNote "condition water (water bodies)"@en ;
    skos:topConceptOf cci-scheme:dataType .

<http://vocab.ceda.ac.uk/collection/cci/dataType/dtype_wl> a cci:dataType,
        skos:Concept ;
    rdfs:seeAlso <https://climate.esa.int/en/projects/river-discharge/> ;
    skos:altLabel "WL"@en ;
    skos:definition "water level"@en ;
    skos:inScheme cci-scheme:dataType ;
    skos:prefLabel "water level"@en ;
    skos:scopeNote "water level"@en ;
    skos:topConceptOf cci-scheme:dataType .

<http://vocab.ceda.ac.uk/collection/cci/ecv/cciecv_aerosol> a cci:ecv,
        skos:Concept ;
    skos:altLabel "AEROSOL"@en ;
    skos:definition "Aerosol properties climate data record produced from satellite data as part of the European Space Agency (ESA) Climate Change Initiative (CCI)"@en ;
    skos:inScheme cci-scheme:ecv ;
    skos:narrowMatch <http://vocab.ceda.ac.uk/collection/gcos/ecv/atmosphericCompositionOzoneAndAerosol>,
        <http://vocab.nerc.ac.uk/collection/P07/current/CFSN0763/> ;
    skos:prefLabel "aerosol"@en ;
    skos:scopeNote "Aerosol properties climate data record produced from satellite data as part of the European Space Agency (ESA) Climate Change Initiative (CCI)"@en ;
    skos:topConceptOf cci-scheme:ecv .

<http://vocab.ceda.ac.uk/collection/cci/ecv/cciecv_biomass> a cci:ecv,
        skos:Concept ;
    skos:altLabel "BIOMASS"@en ;
    skos:definition "Above-ground biomass climate data record produced from satellite data as part of the European Space Agency (ESA) Climate Change Initiative (CCI)"@en ;
    skos:inScheme cci-scheme:ecv ;
    skos:prefLabel "above-ground biomass"@en ;
    skos:scopeNote "Above-ground biomass climate data record produced from satellite data as part of the European Space Agency (ESA) Climate Change Initiative (CCI)"@en ;
    skos:topConceptOf cci-scheme:ecv .

<http://vocab.ceda.ac.uk/collection/cci/ecv/cciecv_cloud> a cci:ecv,
        skos:Concept ;
    skos:altLabel "CLOUD"@en ;
    skos:definition "Cloud properties climate data record produced from satellite data as part of the European Space Agency (ESA) Climate Change Initiative (CCI)"@en ;
    skos:inScheme cci-scheme:ecv ;
    skos:narrowMatch <http://vocab.ceda.ac.uk/collection/gcos/ecv/atmosphericUpperairCloudProperties>,
        <http://vocab.nerc.ac.uk/collection/P07/current/72YUKQJR/>,
        <http://vocab.nerc.ac.uk/collection/P07/current/BBAD2149/>,
        <http://vocab.nerc.ac.uk/collection/P07/current/BBAD2158/>,
        <http://vocab.nerc.ac.uk/collection/P07/current/BBAD2159/>,
        <http://vocab.nerc.ac.uk/collection/P07/current/CF12N184/>,
        <http://vocab.nerc.ac.uk/collection/P07/current/CFSN0018/>,
        <http://vocab.nerc.ac.uk/collection/P07/current/CFSN0025/>,
        <http://vocab.nerc.ac.uk/collection/P07/current/CFSN0704/>,
        <http://vocab.nerc.ac.uk/collection/P07/current/CFSN0745/>,
        <http://vocab.nerc.ac.uk/collection/P07/current/CFSN0746/> ;
    skos:prefLabel "cloud"@en ;
    skos:scopeNote "Cloud properties climate data record produced from satellite data as part of the European Space Agency (ESA) Climate Change Initiative (CCI)"@en ;
    skos:topConceptOf cci-scheme:ecv .

<http://vocab.ceda.ac.uk/collection/cci/ecv/cciecv_fire> a cci:ecv,
        skos:Concept ;
    skos:altLabel "FIRE"@en ;
    skos:closeMatch <http://vocab.ceda.ac.uk/collection/gcos/ecv/terrestrialFireDisturbance> ;
    skos:definition "Fire disturbance (burned area) climate data record produced from satellite data as part of the European Space Agency (ESA) Climate Change Initiative (CCI)"@en ;
    skos:inScheme cci-scheme:ecv ;
    skos:narrowMatch <http://vocab.nerc.ac.uk/collection/P07/current/CEDABECC/>,
        <http://vocab.nerc.ac.uk/collection/P07/current/GACJJFFJ/> ;
    skos:prefLabel "fire"@en ;
    skos:scopeNote "Fire disturbance (burned area) climate data record produced from satellite data as part of the European Space Agency (ESA) Climate Change Initiative (CCI)"@en ;
    skos:topConceptOf cci-scheme:ecv .

<http://vocab.ceda.ac.uk/collection/cci/ecv/cciecv_ghg> a cci:ecv,
        skos:Concept ;
    skos:altLabel "GHG"@en ;
    skos:definition "Greenhouse gasses (carbon dioxide and methane) climate data record produced from satellite data as part of the European Space Agency (ESA) Climate Change Initiative (CCI)"@en ;
    skos:inScheme cci-scheme:ecv ;
    skos:narrowMatch <http://vocab.ceda.ac.uk/collection/gcos/ecv/atmosphericCompositionCarbonDioxide>,
        <http://vocab.ceda.ac.uk/collection/gcos/ecv/atmosphericCompositionMethane>,
        <http://vocab.ceda.ac.uk/collection/gcos/ecv/atmosphericCompositionOtherLonglivedGreenhouseGases>,
        <http://vocab.ceda.ac.uk/collection/gcos/ecv/atmosphericUpperairWaterVapour> ;
    skos:prefLabel "greenhouse gases"@en ;
    skos:scopeNote "Greenhouse gasses (carbon dioxide and methane) climate data record produced from satellite data as part of the European Space Agency (ESA) Climate Change Initiative (CCI)"@en ;
    skos:topConceptOf cci-scheme:ecv .

<http://vocab.ceda.ac.uk/collection/cci/ecv/cciecv_glaciers> a cci:ecv,
        skos:Concept ;
    skos:altLabel "GLACIERS"@en ;
    skos:broadMatch <http://vocab.ceda.ac.uk/collection/gcos/ecv/terrestrialGlaciersAndIceCaps> ;
    skos:definition "Glacier inventory climate data record produced from satellite data as part of the European Space Agency (ESA) Climate Change Initiative (CCI)"@en ;
    skos:inScheme cci-scheme:ecv ;
    skos:narrowMatch <http://vocab.nerc.ac.uk/collection/P07/current/CFSN0576/> ;
    skos:prefLabel "glaciers"@en ;
    skos:scopeNote "Glacier inventory climate data record produced from satellite data as part of the European Space Agency (ESA) Climate Change Initiative (CCI)"@en ;
    skos:topConceptOf cci-scheme:ecv .

<http://vocab.ceda.ac.uk/collection/cci/ecv/cciecv_iceSheet> a cci:ecv,
        skos:Concept ;
    skos:altLabel "ICESHEETS"@en ;
    skos:closeMatch <http://vocab.ceda.ac.uk/collection/gcos/ecv/terrestrialIceSheets> ;
    skos:definition "Ice sheets climate data record produced from satellite data as part of the European Space Agency (ESA) Climate Change Initiative (CCI)"@en ;
    skos:inScheme cci-scheme:ecv ;
    skos:prefLabel "ice sheets"@en ;
    skos:scopeNote "Ice sheets climate data record produced from satellite data as part of the European Space Agency (ESA) Climate Change Initiative (CCI)"@en ;
    skos:topConceptOf cci-scheme:ecv .

<http://vocab.ceda.ac.uk/collection/cci/ecv/cciecv_lakes> a cci:ecv,
        skos:Concept ;
    skos:altLabel "LAKES"@en ;
    skos:definition "Lakes climate data record produced from satellite data as part of the European Space Agency (ESA) Climate Change Initiative (CCI)"@en ;
    skos:inScheme cci-scheme:ecv ;
    skos:prefLabel "lakes"@en ;
    skos:scopeNote "Lakes climate data record produced from satellite data as part of the European Space Agency (ESA) Climate Change Initiative (CCI)"@en ;
    skos:topConceptOf cci-scheme:ecv .

<http://vocab.ceda.ac.uk/collection/cci/ecv/cciecv_landCov> a cci:ecv,
        skos:Concept ;
    skos:altLabel "LC"@en ;
    skos:closeMatch <http://vocab.ceda.ac.uk/collection/gcos/ecv/terrestrialLandCover> ;
    skos:definition "Land cover climate data record produced from satellite data as part of the European Space Agency (ESA) Climate Change Initiative (CCI)"@en ;
    skos:inScheme cci-scheme:ecv ;
    skos:prefLabel "land cover"@en ;
    skos:scopeNote "Land cover climate data record produced from satellite data as part of the European Space Agency (ESA) Climate Change Initiative (CCI)"@en ;
    skos:topConceptOf cci-scheme:ecv .

<http://vocab.ceda.ac.uk/collection/cci/ecv/cciecv_landSurfTemp> a cci:ecv,
        skos:Concept ;
    skos:altLabel "LST"@en ;
    skos:definition "Land Surface Temperature climate data record produced from satellite data as part of the European Space Agency (ESA) Climate Change Initiative (CCI)"@en ;
    skos:inScheme cci-scheme:ecv ;
    skos:prefLabel "land surface temperature"@en ;
    skos:scopeNote "Land Surface Temperature climate data record produced from satellite data as part of the European Space Agency (ESA) Climate Change Initiative (CCI)"@en ;
    skos:topConceptOf cci-scheme:ecv .

<http://vocab.ceda.ac.uk/collection/cci/ecv/cciecv_oceanCol> a cci:ecv,
        skos:Concept ;
    skos:altLabel "OC"@en ;
    skos:closeMatch <http://vocab.ceda.ac.uk/collection/gcos/ecv/oceanicSurfaceOceanColour> ;
    skos:definition "Ocean colour climate data record produced from satellite data as part of the European Space Agency (ESA) Climate Change Initiative (CCI)"@en ;
    skos:inScheme cci-scheme:ecv ;
    skos:narrowMatch <http://vocab.nerc.ac.uk/collection/P07/current/CF14N7/>,
        <http://vocab.nerc.ac.uk/collection/P07/current/CFSN0062/>,
        <http://vocab.nerc.ac.uk/collection/P07/current/CFSN0064/>,
        <http://vocab.nerc.ac.uk/collection/P07/current/CFSN0065/>,
        <http://vocab.nerc.ac.uk/collection/P07/current/CFV13N26/> ;
    skos:prefLabel "ocean colour"@en ;
    skos:scopeNote "Ocean colour climate data record produced from satellite data as part of the European Space Agency (ESA) Climate Change Initiative (CCI)"@en ;
    skos:topConceptOf cci-scheme:ecv .

<http://vocab.ceda.ac.uk/collection/cci/ecv/cciecv_ozone> a cci:ecv,
        skos:Concept ;
    skos:altLabel "OZONE"@en ;
    skos:definition "Ozone climate data record produced from satellite data as part of the European Space Agency (ESA) Climate Change Initiative (CCI)"@en ;
    skos:inScheme cci-scheme:ecv ;
    skos:narrowMatch <http://vocab.ceda.ac.uk/collection/gcos/ecv/atmosphericCompositionOzoneAndAerosol>,
        <http://vocab.nerc.ac.uk/collection/P07/current/CF12N499/>,
        <http://vocab.nerc.ac.uk/collection/P07/current/CFSN0513/>,
        <http://vocab.nerc.ac.uk/collection/P07/current/IDDFFADF/>,
        <http://vocab.nerc.ac.uk/collection/P07/current/IFDIAFIF/> ;
    skos:prefLabel "ozone"@en ;
    skos:scopeNote "Ozone climate data record produced from satellite data as part of the European Space Agency (ESA) Climate Change Initiative (CCI)"@en ;
    skos:topConceptOf cci-scheme:ecv .

<http://vocab.ceda.ac.uk/collection/cci/ecv/cciecv_permafrost> a cci:ecv,
        skos:Concept ;
    skos:altLabel "PERMAFROST"@en ;
    skos:definition "Permafrost climate data record produced from satellite data as part of the European Space Agency (ESA) Climate Change Initiative (CCI)"@en ;
    skos:inScheme cci-scheme:ecv ;
    skos:prefLabel "permafrost"@en ;
    skos:scopeNote "Permafrost climate data record produced from satellite data as part of the European Space Agency (ESA) Climate Change Initiative (CCI)"@en ;
    skos:topConceptOf cci-scheme:ecv .

<http://vocab.ceda.ac.uk/collection/cci/ecv/cciecv_riverDischarge> a cci:ecv,
        skos:Concept ;
    skos:altLabel "RD"@en ;
    skos:definition "River discharge climate data record produced from satellite data as part of the European Space Agency (ESA) Climate Change Initiative (CCI)"@en ;
    skos:inScheme cci-scheme:ecv ;
    skos:prefLabel "river discharge"@en ;
    skos:scopeNote "River discharge climate data record produced from satellite data as part of the European Space Agency (ESA) Climate Change Initiative (CCI)"@en ;
    skos:topConceptOf cci-scheme:ecv .

<http://vocab.ceda.ac.uk/collection/cci/ecv/cciecv_salinity> a cci:ecv,
        skos:Concept ;
    skos:altLabel "SEASURFACESALINITY"@en ;
    skos:definition "Sea Surface Salinity climate data record produced from satellite data as part of the European Space Agency (ESA) Climate Change Initiative (CCI)"@en ;
    skos:inScheme cci-scheme:ecv ;
    skos:prefLabel "sea surface salinity"@en ;
    skos:scopeNote "Sea Surface Salinity climate data record produced from satellite data as part of the European Space Agency (ESA) Climate Change Initiative (CCI)"@en ;
    skos:topConceptOf cci-scheme:ecv .

<http://vocab.ceda.ac.uk/collection/cci/ecv/cciecv_seaIce> a cci:ecv,
        skos:Concept ;
    skos:altLabel "SEAICE"@en ;
    skos:closeMatch <http://vocab.ceda.ac.uk/collection/gcos/ecv/oceanicSurfaceSeaIce> ;
    skos:definition "Sea ice climate data record produced from satellite data as part of the European Space Agency (ESA) Climate Change Initiative (CCI)"@en ;
    skos:inScheme cci-scheme:ecv ;
    skos:narrowMatch <http://vocab.nerc.ac.uk/collection/P07/current/CFSN0424/> ;
    skos:prefLabel "sea ice"@en ;
    skos:scopeNote "Sea ice climate data record produced from satellite data as part of the European Space Agency (ESA) Climate Change Initiative (CCI)"@en ;
    skos:topConceptOf cci-scheme:ecv .

<http://vocab.ceda.ac.uk/collection/cci/ecv/cciecv_seaLevel> a cci:ecv,
        skos:Concept ;
    skos:altLabel "SEALEVEL"@en ;
    skos:closeMatch <http://vocab.ceda.ac.uk/collection/gcos/ecv/oceanicSurfaceSeaLevel> ;
    skos:definition "Sea level climate data record produced from satellite data as part of the European Space Agency (ESA) Climate Change Initiative (CCI)"@en ;
    skos:inScheme cci-scheme:ecv ;
    skos:narrowMatch <http://vocab.nerc.ac.uk/collection/P07/current/CFSN0375/>,
        <http://vocab.nerc.ac.uk/collection/P07/current/CFSN0632/>,
        <http://vocab.nerc.ac.uk/collection/P07/current/EJ5JLPG7/>,
        <http://vocab.nerc.ac.uk/collection/P07/current/RQ2Q233Z/>,
        <http://vocab.nerc.ac.uk/collection/P07/current/SHGEIZRR/>,
        <http://vocab.nerc.ac.uk/collection/P07/current/XRCBF7SB/>,
        <http://vocab.nerc.ac.uk/collection/P07/current/ZSDAR2KM/> ;
    skos:prefLabel "sea level"@en ;
    skos:scopeNote "Sea level climate data record produced from satellite data as part of the European Space Agency (ESA) Climate Change Initiative (CCI)"@en ;
    skos:topConceptOf cci-scheme:ecv .

<http://vocab.ceda.ac.uk/collection/cci/ecv/cciecv_seaState> a cci:ecv,
        skos:Concept ;
    skos:altLabel "SEASTATE"@en ;
    skos:definition "Sea state climate data record produced from satellite data as part of the European Space Agency (ESA) Climate Change Initiative (CCI)"@en ;
    skos:inScheme cci-scheme:ecv ;
    skos:prefLabel "sea state"@en ;
    skos:scopeNote "Sea state climate data record produced from satellite data as part of the European Space Agency (ESA) Climate Change Initiative (CCI)"@en ;
    skos:topConceptOf cci-scheme:ecv .

<http://vocab.ceda.ac.uk/collection/cci/ecv/cciecv_snow> a cci:ecv,
        skos:Concept ;
    skos:altLabel "SNOW"@en ;
    skos:definition "Snow climate data record produced from satellite data as part of the European Space Agency (ESA) Climate Change Initiative (CCI)"@en ;
    skos:inScheme cci-scheme:ecv ;
    skos:prefLabel "snow"@en ;
    skos:scopeNote "Snow climate data record produced from satellite data as part of the European Space Agency (ESA) Climate Change Initiative (CCI)"@en ;
    skos:topConceptOf cci-scheme:ecv .

<http://vocab.ceda.ac.uk/collection/cci/ecv/cciecv_soilMst> a cci:ecv,
        skos:Concept ;
    skos:altLabel "SOILMOISTURE"@en ;
    skos:closeMatch <http://vocab.ceda.ac.uk/collection/gcos/ecv/terrestrialSoilMoisture> ;
    skos:definition "Soil moisture climate data record produced from satellite data as part of the European Space Agency (ESA) Climate Change Initiative (CCI)"@en ;
    skos:inScheme cci-scheme:ecv ;
    skos:prefLabel "soil moisture"@en ;
    skos:scopeNote "Soil moisture climate data record produced from satellite data as part of the European Space Agency (ESA) Climate Change Initiative (CCI)"@en ;
    skos:topConceptOf cci-scheme:ecv .

<http://vocab.ceda.ac.uk/collection/cci/ecv/cciecv_sst> a cci:ecv,
        skos:Concept ;
    skos:altLabel "SST"@en ;
    skos:closeMatch <http://vocab.ceda.ac.uk/collection/gcos/ecv/oceanicSurfaceSeaSurfaceTemperature> ;
    skos:definition "Sea surface temperature climate data record produced from satellite data as part of the European Space Agency (ESA) Climate Change Initiative (CCI)"@en ;
    skos:inScheme cci-scheme:ecv ;
    skos:narrowMatch <http://vocab.nerc.ac.uk/collection/P07/current/CFSN0335/>,
        <http://vocab.nerc.ac.uk/collection/P07/current/CFV9N2/> ;
    skos:prefLabel "sea surface temperature"@en ;
    skos:scopeNote "Sea surface temperature climate data record produced from satellite data as part of the European Space Agency (ESA) Climate Change Initiative (CCI)"@en ;
    skos:topConceptOf cci-scheme:ecv .

<http://vocab.ceda.ac.uk/collection/cci/ecv/cciecv_vegParam> a cci:ecv,
        skos:Concept ;
    skos:altLabel "VEGETATION"@en ;
    skos:definition "Vegetation Parameters climate data record produced from satellite data as part of the European Space Agency (ESA) Climate Change Initiative (CCI)"@en ;
    skos:inScheme cci-scheme:ecv ;
    skos:prefLabel "vegetation parameters"@en ;
    skos:scopeNote "Vegetation Parameters climate data record produced from satellite data as part of the European Space Agency (ESA) Climate Change Initiative (CCI)"@en ;
    skos:topConceptOf cci-scheme:ecv .

<http://vocab.ceda.ac.uk/collection/cci/ecv/cciecv_waterVapour> a cci:ecv,
        skos:Concept ;
    skos:altLabel "WATERVAPOUR"@en ;
    skos:definition "Water vapour climate data record produced from satellite data as part of the European Space Agency (ESA) Climate Change Initiative (CCI)"@en ;
    skos:inScheme cci-scheme:ecv ;
    skos:prefLabel "water vapour"@en ;
    skos:scopeNote "Water vapour climate data record produced from satellite data as part of the European Space Agency (ESA) Climate Change Initiative (CCI)"@en ;
    skos:topConceptOf cci-scheme:ecv .

<http://vocab.ceda.ac.uk/collection/cci/freq/feq_min> a cci:freq,
        skos:Concept ;
    skos:altLabel "P0DT0H1M"@en ;
    skos:inScheme cci-scheme:freq ;
    skos:prefLabel "minute"@en ;
    skos:topConceptOf cci-scheme:freq .

<http://vocab.ceda.ac.uk/collection/cci/freq/freq_10day> a cci:freq,
        skos:Concept ;
    skos:altLabel "P10D"@en ;
    skos:inScheme cci-scheme:freq ;
    skos:prefLabel "10 days"@en ;
    skos:topConceptOf cci-scheme:freq .

<http://vocab.ceda.ac.uk/collection/cci/freq/freq_13yr> a cci:freq,
        skos:Concept ;
    skos:altLabel "P13Y"@en ;
    skos:inScheme cci-scheme:freq ;
    skos:prefLabel "13 years"@en ;
    skos:topConceptOf cci-scheme:freq .

<http://vocab.ceda.ac.uk/collection/cci/freq/freq_15day> a cci:freq,
        skos:Concept ;
    skos:altLabel "P15D"@en ;
    skos:inScheme cci-scheme:freq ;
    skos:prefLabel "15 days"@en ;
    skos:topConceptOf cci-scheme:freq .

<http://vocab.ceda.ac.uk/collection/cci/freq/freq_3hr> a cci:freq,
        skos:Concept ;
    skos:altLabel "P0DT3H"@en ;
    skos:inScheme cci-scheme:freq ;
    skos:prefLabel "3 hours"@en ;
    skos:topConceptOf cci-scheme:freq .

<http://vocab.ceda.ac.uk/collection/cci/freq/freq_5day> a cci:freq,
        skos:Concept ;
    skos:altLabel "P5D"@en ;
    skos:inScheme cci-scheme:freq ;
    skos:prefLabel "5 days"@en ;
    skos:topConceptOf cci-scheme:freq .

<http://vocab.ceda.ac.uk/collection/cci/freq/freq_5yr> a cci:freq,
        skos:Concept ;
    skos:altLabel "P5Y"@en ;
    skos:inScheme cci-scheme:freq ;
    skos:prefLabel "5 years"@en ;
    skos:topConceptOf cci-scheme:freq .

<http://vocab.ceda.ac.uk/collection/cci/freq/freq_8day> a cci:freq,
        skos:Concept ;
    skos:altLabel "P8D"@en ;
    skos:inScheme cci-scheme:freq ;
    skos:prefLabel "8 days"@en ;
    skos:topConceptOf cci-scheme:freq .

<http://vocab.ceda.ac.uk/collection/cci/freq/freq_clim> a cci:freq,
        skos:Concept ;
    skos:altLabel "CLIM"@en ;
    skos:inScheme cci-scheme:freq ;
    skos:prefLabel "climatology"@en ;
    skos:topConceptOf cci-scheme:freq .

<http://vocab.ceda.ac.uk/collection/cci/freq/freq_day> a cci:freq,
        skos:Concept ;
    skos:altLabel "P1D"@en ;
    skos:inScheme cci-scheme:freq ;
    skos:prefLabel "day"@en ;
    skos:topConceptOf cci-scheme:freq .

<http://vocab.ceda.ac.uk/collection/cci/freq/freq_hr> a cci:freq,
        skos:Concept ;
    skos:altLabel "P0DT1H"@en ;
    skos:inScheme cci-scheme:freq ;
    skos:prefLabel "hour"@en ;
    skos:topConceptOf cci-scheme:freq .

<http://vocab.ceda.ac.uk/collection/cci/freq/freq_mon> a cci:freq,
        skos:Concept ;
    skos:altLabel "P1M"@en ;
    skos:inScheme cci-scheme:freq ;
    skos:prefLabel "month"@en ;
    skos:topConceptOf cci-scheme:freq .

<http://vocab.ceda.ac.uk/collection/cci/freq/freq_sat_orb> a cci:freq,
        skos:Concept ;
    skos:inScheme cci-scheme:freq ;
    skos:prefLabel "satellite orbit frequency"@en ;
    skos:topConceptOf cci-scheme:freq .

<http://vocab.ceda.ac.uk/collection/cci/freq/freq_sec> a cci:freq,
        skos:Concept ;
    skos:altLabel "P0DT0H0M1S"@en ;
    skos:inScheme cci-scheme:freq ;
    skos:prefLabel "second"@en ;
    skos:topConceptOf cci-scheme:freq .

<http://vocab.ceda.ac.uk/collection/cci/freq/freq_unspecified> a cci:freq,
        skos:Concept ;
    skos:inScheme cci-scheme:freq ;
    skos:prefLabel "unspecified"@en ;
    skos:topConceptOf cci-scheme:freq .

<http://vocab.ceda.ac.uk/collection/cci/freq/freq_week> a cci:freq,
        skos:Concept ;
    skos:altLabel "P7D"@en ;
    skos:inScheme cci-scheme:freq ;
    skos:prefLabel "week"@en ;
    skos:topConceptOf cci-scheme:freq .

<http://vocab.ceda.ac.uk/collection/cci/freq/freq_yr> a cci:freq,
        skos:Concept ;
    skos:altLabel "P1Y"@en ;
    skos:inScheme cci-scheme:freq ;
    skos:prefLabel "year"@en ;
    skos:topConceptOf cci-scheme:freq .

<http://vocab.ceda.ac.uk/collection/cci/org/org01> a cci:org,
        skos:Concept ;
    rdfs:seeAlso <http://isni.org/isni/121525373> ;
    skos:altLabel "AUTH"@en ;
    skos:inScheme cci-scheme:org ;
    skos:prefLabel "Aristotle University of Thessalonikii"@en ;
    skos:topConceptOf cci-scheme:org .

<http://vocab.ceda.ac.uk/collection/cci/org/org02> a cci:org,
        skos:Concept ;
    rdfs:seeAlso <http://isni.org/isni/419368948> ;
    skos:altLabel "AOPP"@en ;
    skos:inScheme cci-scheme:org ;
    skos:prefLabel "Atmospheric, Oceanic and Planetary Physics, University of Oxford"@en ;
    skos:topConceptOf cci-scheme:org .

<http://vocab.ceda.ac.uk/collection/cci/org/org03> a cci:org,
        skos:Concept ;
    rdfs:seeAlso <http://isni.org/isni/122893389> ;
    skos:altLabel "BIRA"@en ;
    skos:inScheme cci-scheme:org ;
    skos:prefLabel "Belgian Institute for Space Aeronomy"@en ;
    skos:topConceptOf cci-scheme:org .

<http://vocab.ceda.ac.uk/collection/cci/org/org04> a cci:org,
        skos:Concept ;
    skos:altLabel "BC"@en ;
    skos:inScheme cci-scheme:org ;
    skos:prefLabel "Brockmann Consult GmbH"@en ;
    skos:topConceptOf cci-scheme:org .

<http://vocab.ceda.ac.uk/collection/cci/org/org05> a cci:org,
        skos:Concept ;
    rdfs:seeAlso <http://isni.org/isni/121129282> ;
    skos:altLabel "CNRS"@en ;
    skos:inScheme cci-scheme:org ;
    skos:prefLabel "Centre National de la Recherche Scientific"@en ;
    skos:topConceptOf cci-scheme:org .

<http://vocab.ceda.ac.uk/collection/cci/org/org06> a cci:org,
        skos:Concept ;
    rdfs:seeAlso <http://isni.org/isni/121584330> ;
    skos:altLabel "CNES"@en ;
    skos:inScheme cci-scheme:org ;
    skos:prefLabel "Centre National d'Etudes Spatiales"@en ;
    skos:topConceptOf cci-scheme:org .

<http://vocab.ceda.ac.uk/collection/cci/org/org07> a cci:org,
        skos:Concept ;
    rdfs:seeAlso <http://isni.org/isni/122425235> ;
    skos:altLabel "CHA"@en ;
    skos:inScheme cci-scheme:org ;
    skos:prefLabel "Chalmers University of Technology, Göteberg, Sweden"@en ;
    skos:topConceptOf cci-scheme:org .

<http://vocab.ceda.ac.uk/collection/cci/org/org08> a cci:org,
        skos:Concept ;
    rdfs:seeAlso <http://isni.org/isni/106573633> ;
    skos:altLabel "CLS"@en ;
    skos:inScheme cci-scheme:org ;
    skos:prefLabel "Collecte Localisation Satellites"@en ;
    skos:topConceptOf cci-scheme:org .

<http://vocab.ceda.ac.uk/collection/cci/org/org09> a cci:org,
        skos:Concept ;
    rdfs:seeAlso <http://isni.org/isni/419370650> ;
    skos:altLabel "GIUZ"@en ;
    skos:inScheme cci-scheme:org ;
    skos:prefLabel "Department of Geography, University of Zurich"@en ;
    skos:topConceptOf cci-scheme:org .

<http://vocab.ceda.ac.uk/collection/cci/org/org10> a cci:org,
        skos:Concept ;
    rdfs:seeAlso <http://isni.org/isni/406109007> ;
    skos:altLabel "GUIO"@en ;
    skos:inScheme cci-scheme:org ;
    skos:prefLabel "Department of Geosciences, University of Oslo"@en ;
    skos:topConceptOf cci-scheme:org .

<http://vocab.ceda.ac.uk/collection/cci/org/org100> a cci:org,
        skos:Concept ;
    rdfs:seeAlso <http://isni.org/isni/107301058> ;
    skos:altLabel "NCC"@en ;
    skos:inScheme cci-scheme:org ;
    skos:prefLabel "Norwegian Computing Center"@en ;
    skos:topConceptOf cci-scheme:org .

<http://vocab.ceda.ac.uk/collection/cci/org/org101> a cci:org,
        skos:Concept ;
    rdfs:seeAlso <http://isni.org/isni/493345234> ;
    skos:inScheme cci-scheme:org ;
    skos:prefLabel "Planet Labs"@en ;
    skos:topConceptOf cci-scheme:org .

<http://vocab.ceda.ac.uk/collection/cci/org/org102> a cci:org,
        skos:Concept ;
    rdfs:seeAlso <http://isni.org/isni/403828364> ;
    skos:altLabel "CESBIO"@en ;
    skos:inScheme cci-scheme:org ;
    skos:prefLabel "Centre d'Etudes Spatiales de la Biosphère"@en ;
    skos:topConceptOf cci-scheme:org .

<http://vocab.ceda.ac.uk/collection/cci/org/org103> a cci:org,
        skos:Concept ;
    skos:altLabel "EODC"@en ;
    skos:inScheme cci-scheme:org ;
    skos:prefLabel "EODC Gmbh"@en ;
    skos:topConceptOf cci-scheme:org .

<http://vocab.ceda.ac.uk/collection/cci/org/org104> a cci:org,
        skos:Concept ;
    skos:inScheme cci-scheme:org ;
    skos:prefLabel "VITO"@en ;
    skos:topConceptOf cci-scheme:org .

<http://vocab.ceda.ac.uk/collection/cci/org/org105> a cci:org,
        skos:Concept ;
    skos:inScheme cci-scheme:org ;
    skos:prefLabel "Hydro Matters"@en ;
    skos:topConceptOf cci-scheme:org .

<http://vocab.ceda.ac.uk/collection/cci/org/org106> a cci:org,
        skos:Concept ;
    skos:inScheme cci-scheme:org ;
    skos:prefLabel "EOLA"@en ;
    skos:topConceptOf cci-scheme:org .

<http://vocab.ceda.ac.uk/collection/cci/org/org107> a cci:org,
        skos:Concept ;
    skos:inScheme cci-scheme:org ;
    skos:prefLabel "University of Trento"@en ;
    skos:topConceptOf cci-scheme:org .

<http://vocab.ceda.ac.uk/collection/cci/org/org11> a cci:org,
        skos:Concept ;
    rdfs:seeAlso <http://isni.org/isni/123217956> ;
    skos:altLabel "DWD"@en ;
    skos:inScheme cci-scheme:org ;
    skos:prefLabel "Deutscher Wetterdienst"@en ;
    skos:topConceptOf cci-scheme:org .

<http://vocab.ceda.ac.uk/collection/cci/org/org12> a cci:org,
        skos:Concept ;
    rdfs:seeAlso <http://isni.org/isni/89837915> ;
    skos:altLabel "DLR"@en ;
    skos:inScheme cci-scheme:org ;
    skos:prefLabel "Deutsches Zentrum fuer Luft- und Raumfahrt"@en ;
    skos:topConceptOf cci-scheme:org .

<http://vocab.ceda.ac.uk/collection/cci/org/org13> a cci:org,
        skos:Concept ;
    rdfs:seeAlso <http://isni.org/isni/000000040618578X> ;
    skos:altLabel "DTU-S"@en ;
    skos:inScheme cci-scheme:org ;
    skos:prefLabel "DTU Space"@en ;
    skos:topConceptOf cci-scheme:org .

<http://vocab.ceda.ac.uk/collection/cci/org/org14> a cci:org,
        skos:Concept ;
    skos:altLabel "ENVEO"@en ;
    skos:inScheme cci-scheme:org ;
    skos:prefLabel "ENVironmental Earth Observation IT GmbH"@en ;
    skos:topConceptOf cci-scheme:org .

<http://vocab.ceda.ac.uk/collection/cci/org/org15> a cci:org,
        skos:Concept ;
    rdfs:seeAlso <http://isni.org/isni/406236946> ;
    skos:altLabel "ESA"@en ;
    skos:inScheme cci-scheme:org ;
    skos:prefLabel "European Space Agency"@en ;
    skos:topConceptOf cci-scheme:org .

<http://vocab.ceda.ac.uk/collection/cci/org/org16> a cci:org,
        skos:Concept ;
    rdfs:seeAlso <http://isni.org/isni/122538678> ;
    skos:altLabel "FMI"@en ;
    skos:inScheme cci-scheme:org ;
    skos:prefLabel "Finnish Meteorological Institute"@en ;
    skos:topConceptOf cci-scheme:org .

<http://vocab.ceda.ac.uk/collection/cci/org/org17> a cci:org,
        skos:Concept ;
    rdfs:seeAlso <http://isni.org/isni/91164836> ;
    skos:altLabel "FUB"@en ;
    skos:inScheme cci-scheme:org ;
    skos:prefLabel "Freie Universitaet Berlin"@en ;
    skos:topConceptOf cci-scheme:org .

<http://vocab.ceda.ac.uk/collection/cci/org/org18> a cci:org,
        skos:Concept ;
    skos:altLabel "Gamma"@en ;
    skos:inScheme cci-scheme:org ;
    skos:prefLabel "Gamma Remote Sensing"@en ;
    skos:topConceptOf cci-scheme:org .

<http://vocab.ceda.ac.uk/collection/cci/org/org19> a cci:org,
        skos:Concept ;
    skos:altLabel "GEUS"@en ;
    skos:inScheme cci-scheme:org ;
    skos:prefLabel "The Geological Survey of Denmark and Greenland"@en ;
    skos:topConceptOf cci-scheme:org .

<http://vocab.ceda.ac.uk/collection/cci/org/org20> a cci:org,
        skos:Concept ;
    rdfs:seeAlso <http://isni.org/isni/106814708> ;
    skos:altLabel "GMV"@en ;
    skos:inScheme cci-scheme:org ;
    skos:prefLabel "GMV"@en ;
    skos:topConceptOf cci-scheme:org .

<http://vocab.ceda.ac.uk/collection/cci/org/org21> a cci:org,
        skos:Concept ;
    rdfs:seeAlso <http://isni.org/isni/446732899> ;
    skos:altLabel "HZG"@en ;
    skos:inScheme cci-scheme:org ;
    skos:prefLabel "Helmholtz-Zentrum Geesthacht"@en ;
    skos:topConceptOf cci-scheme:org .

<http://vocab.ceda.ac.uk/collection/cci/org/org22> a cci:org,
        skos:Concept ;
    skos:inScheme cci-scheme:org ;
    skos:prefLabel "HYGEOS"@en ;
    skos:topConceptOf cci-scheme:org .

<http://vocab.ceda.ac.uk/collection/cci/org/org23> a cci:org,
        skos:Concept ;
    rdfs:seeAlso <http://isni.org/isni/404050603> ;
    skos:inScheme cci-scheme:org ;
    skos:prefLabel "ICARE"@en ;
    skos:topConceptOf cci-scheme:org .

<http://vocab.ceda.ac.uk/collection/cci/org/org24> a cci:org,
        skos:Concept ;
    skos:altLabel "IMKIAA"@en ;
    skos:inScheme cci-scheme:org ;
    skos:prefLabel "Institut für Meterologie und Klimaforschung, KIT and Instituto de Astrofisca de Andalucia, Granada"@en ;
    skos:topConceptOf cci-scheme:org .

<http://vocab.ceda.ac.uk/collection/cci/org/org25> a cci:org,
        skos:Concept ;
    skos:altLabel "IMK"@en ;
    skos:inScheme cci-scheme:org ;
    skos:prefLabel "Institut für Meterologie und Klimaforschung, KIT, Karlsruhe"@en ;
    skos:topConceptOf cci-scheme:org .

<http://vocab.ceda.ac.uk/collection/cci/org/org26> a cci:org,
        skos:Concept ;
    skos:altLabel "IAC"@en ;
    skos:inScheme cci-scheme:org ;
    skos:prefLabel "Institute for Atmospheric and Climate Science"@en ;
    skos:topConceptOf cci-scheme:org .

<http://vocab.ceda.ac.uk/collection/cci/org/org27> a cci:org,
        skos:Concept ;
    skos:altLabel "IES-JRC"@en ;
    skos:inScheme cci-scheme:org ;
    skos:prefLabel "Institute for Environment and Sustainability"@en ;
    skos:topConceptOf cci-scheme:org .

<http://vocab.ceda.ac.uk/collection/cci/org/org28> a cci:org,
        skos:Concept ;
    skos:altLabel "IUP"@en ;
    skos:inScheme cci-scheme:org ;
    skos:prefLabel "Institute of Environmental Physics"@en ;
    skos:topConceptOf cci-scheme:org .

<http://vocab.ceda.ac.uk/collection/cci/org/org29> a cci:org,
        skos:Concept ;
    rdfs:seeAlso <http://isni.org/isni/417937043> ;
    skos:altLabel "IAA"@en ;
    skos:inScheme cci-scheme:org ;
    skos:prefLabel "Instituto de Astrofisca de Andalucia, Granada"@en ;
    skos:topConceptOf cci-scheme:org .

<http://vocab.ceda.ac.uk/collection/cci/org/org30> a cci:org,
        skos:Concept ;
    rdfs:seeAlso <http://isni.org/isni/000000012300669X> ;
    skos:altLabel "INIA"@en ;
    skos:inScheme cci-scheme:org ;
    skos:prefLabel "Instituto Nacional de Investigacion y Tecnologia Agraria y Alimentaria"@en ;
    skos:topConceptOf cci-scheme:org .

<http://vocab.ceda.ac.uk/collection/cci/org/org31> a cci:org,
        skos:Concept ;
    rdfs:seeAlso <http://isni.org/isni/122154586> ;
    skos:altLabel "ISA"@en ;
    skos:inScheme cci-scheme:org ;
    skos:prefLabel "Instituto Superior de Agronomia"@en ;
    skos:topConceptOf cci-scheme:org .

<http://vocab.ceda.ac.uk/collection/cci/org/org32> a cci:org,
        skos:Concept ;
    rdfs:seeAlso <http://isni.org/isni/403820442> ;
    skos:altLabel "ICIMOD"@en ;
    skos:inScheme cci-scheme:org ;
    skos:prefLabel "International Centre for Integrated Mountain Development"@en ;
    skos:topConceptOf cci-scheme:org .

<http://vocab.ceda.ac.uk/collection/cci/org/org33> a cci:org,
        skos:Concept ;
    skos:inScheme cci-scheme:org ;
    skos:prefLabel "Juelich Forschungszentrum"@en ;
    skos:topConceptOf cci-scheme:org .

<http://vocab.ceda.ac.uk/collection/cci/org/org34> a cci:org,
        skos:Concept ;
    skos:altLabel "KEG"@en ;
    skos:inScheme cci-scheme:org ;
    skos:prefLabel "Kommission fuer Erdmessung und Glaziologie"@en ;
    skos:topConceptOf cci-scheme:org .

<http://vocab.ceda.ac.uk/collection/cci/org/org35> a cci:org,
        skos:Concept ;
    rdfs:seeAlso <http://isni.org/isni/104563087> ;
    skos:altLabel "LATMOS"@en ;
    skos:inScheme cci-scheme:org ;
    skos:prefLabel "Laboratoire Atmospheres, Milieux, Observations Spatiales"@en ;
    skos:topConceptOf cci-scheme:org .

<http://vocab.ceda.ac.uk/collection/cci/org/org36> a cci:org,
        skos:Concept ;
    skos:altLabel "LEGOS"@en ;
    skos:inScheme cci-scheme:org ;
    skos:prefLabel "Laboratoire d'Etudes en Géophysique et  Océanographie Spatiales"@en ;
    skos:topConceptOf cci-scheme:org .

<http://vocab.ceda.ac.uk/collection/cci/org/org37> a cci:org,
        skos:Concept ;
    rdfs:seeAlso <http://isni.org/isni/403683740> ;
    skos:altLabel "LOA"@en ;
    skos:inScheme cci-scheme:org ;
    skos:prefLabel "Laboratoire d'Optique Atmosphérique"@en ;
    skos:topConceptOf cci-scheme:org .

<http://vocab.ceda.ac.uk/collection/cci/org/org38> a cci:org,
        skos:Concept ;
    rdfs:seeAlso <http://isni.org/isni/105849722> ;
    skos:altLabel "LSCE"@en ;
    skos:inScheme cci-scheme:org ;
    skos:prefLabel "Laboratoire des Sciences du Climat et L'Environement"@en ;
    skos:topConceptOf cci-scheme:org .

<http://vocab.ceda.ac.uk/collection/cci/org/org39> a cci:org,
        skos:Concept ;
    skos:altLabel "MPI-M"@en ;
    skos:inScheme cci-scheme:org ;
    skos:prefLabel "Max-Planck Institute for Meteorology"@en ;
    skos:topConceptOf cci-scheme:org .

<http://vocab.ceda.ac.uk/collection/cci/org/org40> a cci:org,
        skos:Concept ;
    rdfs:seeAlso <http://isni.org/isni/405133830> ;
    skos:altLabel "MOHC"@en ;
    skos:definition "UKMO"@en ;
    skos:inScheme cci-scheme:org ;
    skos:prefLabel "Met Office Hadley Centre"@en ;
    skos:scopeNote "UKMO"@en ;
    skos:topConceptOf cci-scheme:org .

<http://vocab.ceda.ac.uk/collection/cci/org/org41> a cci:org,
        skos:Concept ;
    rdfs:seeAlso <http://isni.org/isni/120343615> ;
    skos:inScheme cci-scheme:org ;
    skos:prefLabel "Meteo Swiss"@en ;
    skos:topConceptOf cci-scheme:org .

<http://vocab.ceda.ac.uk/collection/cci/org/org42> a cci:org,
        skos:Concept ;
    rdfs:seeAlso <http://isni.org/isni/122289878> ;
    skos:altLabel "NERSC"@en ;
    skos:inScheme cci-scheme:org ;
    skos:prefLabel "Nansen Environmental and Remote Sensing Center"@en ;
    skos:topConceptOf cci-scheme:org .

<http://vocab.ceda.ac.uk/collection/cci/org/org43> a cci:org,
        skos:Concept ;
    rdfs:seeAlso <http://isni.org/isni/000000012204386X> ;
    skos:altLabel "NSIDC"@en ;
    skos:inScheme cci-scheme:org ;
    skos:prefLabel "National Snow and Ice Data Center"@en ;
    skos:topConceptOf cci-scheme:org .

<http://vocab.ceda.ac.uk/collection/cci/org/org44> a cci:org,
        skos:Concept ;
    skos:altLabel "SRON"@en ;
    skos:inScheme cci-scheme:org ;
    skos:prefLabel "Netherlands Institute for Space Research"@en ;
    skos:topConceptOf cci-scheme:org .

<http://vocab.ceda.ac.uk/collection/cci/org/org45> a cci:org,
        skos:Concept ;
    rdfs:seeAlso <http://isni.org/isni/98886866> ;
    skos:altLabel "NILU"@en ;
    skos:inScheme cci-scheme:org ;
    skos:prefLabel "Norwegian Institute for Air Research"@en ;
    skos:topConceptOf cci-scheme:org .

<http://vocab.ceda.ac.uk/collection/cci/org/org46> a cci:org,
        skos:Concept ;
    rdfs:seeAlso <http://isni.org/isni/102261499> ;
    skos:altLabel "MetNo"@en ;
    skos:inScheme cci-scheme:org ;
    skos:prefLabel "Norwegian Meteorological Institute"@en ;
    skos:topConceptOf cci-scheme:org .

<http://vocab.ceda.ac.uk/collection/cci/org/org47> a cci:org,
        skos:Concept ;
    rdfs:seeAlso <http://isni.org/isni/122367549> ;
    skos:altLabel "NVE"@en ;
    skos:inScheme cci-scheme:org ;
    skos:prefLabel "Norwegian Water Resources and Energy Directorate"@en ;
    skos:topConceptOf cci-scheme:org .

<http://vocab.ceda.ac.uk/collection/cci/org/org48> a cci:org,
        skos:Concept ;
    rdfs:seeAlso <http://isni.org/isni/110907501> ;
    skos:altLabel "PSI"@en ;
    skos:inScheme cci-scheme:org ;
    skos:prefLabel "Paul-Scherrer-Institut"@en ;
    skos:topConceptOf cci-scheme:org .

<http://vocab.ceda.ac.uk/collection/cci/org/org49> a cci:org,
        skos:Concept ;
    rdfs:seeAlso <http://isni.org/isni/121062153> ;
    skos:altLabel "PML"@en ;
    skos:inScheme cci-scheme:org ;
    skos:prefLabel "Plymouth Marine Laboratory"@en ;
    skos:topConceptOf cci-scheme:org .

<http://vocab.ceda.ac.uk/collection/cci/org/org50> a cci:org,
        skos:Concept ;
    rdfs:seeAlso <http://isni.org/isni/110892733> ;
    skos:altLabel "RMIB"@en ;
    skos:inScheme cci-scheme:org ;
    skos:prefLabel "Royal Meteorological Institute of Belgium"@en ;
    skos:topConceptOf cci-scheme:org .

<http://vocab.ceda.ac.uk/collection/cci/org/org51> a cci:org,
        skos:Concept ;
    rdfs:seeAlso <http://isni.org/isni/417979868> ;
    skos:altLabel "KNMI"@en ;
    skos:inScheme cci-scheme:org ;
    skos:prefLabel "Royal Netherlands Meteorological Institute"@en ;
    skos:topConceptOf cci-scheme:org .

<http://vocab.ceda.ac.uk/collection/cci/org/org52> a cci:org,
        skos:Concept ;
    rdfs:seeAlso <http://isni.org/isni/122375485> ;
    skos:altLabel "RAL"@en ;
    skos:inScheme cci-scheme:org ;
    skos:prefLabel "Rutherford Appleton Laboratory"@en ;
    skos:topConceptOf cci-scheme:org .

<http://vocab.ceda.ac.uk/collection/cci/org/org53> a cci:org,
        skos:Concept ;
    rdfs:seeAlso <http://isni.org/isni/446804119> ;
    skos:altLabel "SEEL"@en ;
    skos:inScheme cci-scheme:org ;
    skos:prefLabel "School of Earth and Environment, University of Leeds"@en ;
    skos:topConceptOf cci-scheme:org .

<http://vocab.ceda.ac.uk/collection/cci/org/org54> a cci:org,
        skos:Concept ;
    rdfs:seeAlso <http://isni.org/isni/403720564> ;
    skos:altLabel "SGS"@en ;
    skos:inScheme cci-scheme:org ;
    skos:prefLabel "School of Geographical Sciences, University of Bristol"@en ;
    skos:topConceptOf cci-scheme:org .

<http://vocab.ceda.ac.uk/collection/cci/org/org55> a cci:org,
        skos:Concept ;
    skos:altLabel "S[&]T"@en ;
    skos:inScheme cci-scheme:org ;
    skos:prefLabel "Science [&] Technology AS"@en ;
    skos:topConceptOf cci-scheme:org .

<http://vocab.ceda.ac.uk/collection/cci/org/org56> a cci:org,
        skos:Concept ;
    rdfs:seeAlso <http://isni.org/isni/106588800> ;
    skos:inScheme cci-scheme:org ;
    skos:prefLabel "Swansea University"@en ;
    skos:topConceptOf cci-scheme:org .

<http://vocab.ceda.ac.uk/collection/cci/org/org57> a cci:org,
        skos:Concept ;
    rdfs:seeAlso <http://isni.org/isni/123313059> ;
    skos:altLabel "EMPA"@en ;
    skos:inScheme cci-scheme:org ;
    skos:prefLabel "Swiss Federal Laboratories for Material Testing and Research"@en ;
    skos:topConceptOf cci-scheme:org .

<http://vocab.ceda.ac.uk/collection/cci/org/org58> a cci:org,
        skos:Concept ;
    rdfs:seeAlso <http://isni.org/isni/123232283> ;
    skos:altLabel "UCL"@en ;
    skos:inScheme cci-scheme:org ;
    skos:prefLabel "Universite Catholique de Louvain"@en ;
    skos:topConceptOf cci-scheme:org .

<http://vocab.ceda.ac.uk/collection/cci/org/org59> a cci:org,
        skos:Concept ;
    rdfs:seeAlso <http://isni.org/isni/419370239> ;
    skos:altLabel "UAH"@en ;
    skos:inScheme cci-scheme:org ;
    skos:prefLabel "University of Alcala"@en ;
    skos:topConceptOf cci-scheme:org .

<http://vocab.ceda.ac.uk/collection/cci/org/org60> a cci:org,
        skos:Concept ;
    rdfs:seeAlso <http://isni.org/isni/121663573> ;
    skos:altLabel "NKUA"@en ;
    skos:inScheme cci-scheme:org ;
    skos:prefLabel "University of Athens"@en ;
    skos:topConceptOf cci-scheme:org .

<http://vocab.ceda.ac.uk/collection/cci/org/org61> a cci:org,
        skos:Concept ;
    rdfs:seeAlso <http://isni.org/isni/122974381> ;
    skos:inScheme cci-scheme:org ;
    skos:prefLabel "University of Bremen"@en ;
    skos:topConceptOf cci-scheme:org .

<http://vocab.ceda.ac.uk/collection/cci/org/org62> a cci:org,
        skos:Concept ;
    rdfs:seeAlso <http://isni.org/isni/121885934> ;
    skos:inScheme cci-scheme:org ;
    skos:prefLabel "University of Cambridge"@en ;
    skos:topConceptOf cci-scheme:org .

<http://vocab.ceda.ac.uk/collection/cci/org/org63> a cci:org,
        skos:Concept ;
    skos:inScheme cci-scheme:org ;
    skos:prefLabel "University of Edinburgh"@en ;
    skos:topConceptOf cci-scheme:org .

<http://vocab.ceda.ac.uk/collection/cci/org/org64> a cci:org,
        skos:Concept ;
    rdfs:seeAlso <http://isni.org/isni/119424776> ;
    skos:altLabel "UJENA"@en ;
    skos:inScheme cci-scheme:org ;
    skos:prefLabel "University of Jena"@en ;
    skos:topConceptOf cci-scheme:org .

<http://vocab.ceda.ac.uk/collection/cci/org/org65> a cci:org,
        skos:Concept ;
    rdfs:seeAlso <http://isni.org/isni/419368411> ;
    skos:inScheme cci-scheme:org ;
    skos:prefLabel "University of Leicester"@en ;
    skos:topConceptOf cci-scheme:org .

<http://vocab.ceda.ac.uk/collection/cci/org/org66> a cci:org,
        skos:Concept ;
    rdfs:seeAlso <http://isni.org/isni/419368403> ;
    skos:altLabel "UL"@en ;
    skos:inScheme cci-scheme:org ;
    skos:prefLabel "University of Leeds"@en ;
    skos:topConceptOf cci-scheme:org .

<http://vocab.ceda.ac.uk/collection/cci/org/org67> a cci:org,
        skos:Concept ;
    rdfs:seeAlso <http://isni.org/isni/419369246> ;
    skos:altLabel "SASK"@en ;
    skos:inScheme cci-scheme:org ;
    skos:prefLabel "University of Saskatchewan, Canada"@en ;
    skos:topConceptOf cci-scheme:org .

<http://vocab.ceda.ac.uk/collection/cci/org/org68> a cci:org,
        skos:Concept ;
    rdfs:seeAlso <http://isni.org/isni/419369668> ;
    skos:altLabel "UoY"@en ;
    skos:inScheme cci-scheme:org ;
    skos:prefLabel "University of York"@en ;
    skos:topConceptOf cci-scheme:org .

<http://vocab.ceda.ac.uk/collection/cci/org/org69> a cci:org,
        skos:Concept ;
    rdfs:seeAlso <http://isni.org/isni/419370650> ;
    skos:altLabel "UZH"@en ;
    skos:inScheme cci-scheme:org ;
    skos:prefLabel "University of Zurich"@en ;
    skos:topConceptOf cci-scheme:org .

<http://vocab.ceda.ac.uk/collection/cci/org/org70> a cci:org,
        skos:Concept ;
    rdfs:seeAlso <http://isni.org/isni/419370669> ;
    skos:altLabel "TU Wien"@en ;
    skos:inScheme cci-scheme:org ;
    skos:prefLabel "Vienna University of Technology"@en ;
    skos:topConceptOf cci-scheme:org .

<http://vocab.ceda.ac.uk/collection/cci/org/org71> a cci:org,
        skos:Concept ;
    rdfs:seeAlso <http://isni.org/isni/417549227> ;
    skos:altLabel "VUA"@en ;
    skos:inScheme cci-scheme:org ;
    skos:prefLabel "VU University Amsterdam"@en ;
    skos:topConceptOf cci-scheme:org .

<http://vocab.ceda.ac.uk/collection/cci/org/org72> a cci:org,
        skos:Concept ;
    rdfs:seeAlso <http://isni.org/isni/122848633> ;
    skos:inScheme cci-scheme:org ;
    skos:prefLabel "Wageningen University"@en ;
    skos:topConceptOf cci-scheme:org .

<http://vocab.ceda.ac.uk/collection/cci/org/org73> a cci:org,
        skos:Concept ;
    rdfs:seeAlso <http://isni.org/isni/109421088> ;
    skos:altLabel "WGMS"@en ;
    skos:inScheme cci-scheme:org ;
    skos:prefLabel "World Glacier Monitoring Service"@en ;
    skos:topConceptOf cci-scheme:org .

<http://vocab.ceda.ac.uk/collection/cci/org/org74> a cci:org,
        skos:Concept ;
    skos:inScheme cci-scheme:org ;
    skos:prefLabel "ESACCI_SST"@en ;
    skos:topConceptOf cci-scheme:org .

<http://vocab.ceda.ac.uk/collection/cci/org/org75> a cci:org,
        skos:Concept ;
    rdfs:seeAlso <http://isni.org/isni/405983800> ;
    skos:altLabel "BAS"@en ;
    skos:inScheme cci-scheme:org ;
    skos:prefLabel "British Antarctic Survey"@en ;
    skos:topConceptOf cci-scheme:org .

<http://vocab.ceda.ac.uk/collection/cci/org/org76> a cci:org,
        skos:Concept ;
    skos:altLabel "DLR-IMF"@en ;
    skos:inScheme cci-scheme:org ;
    skos:prefLabel "Deutschen Zentrums für Luft- und Raumfahrt, Institut für Methodik der Fernerkundung"@en ;
    skos:topConceptOf cci-scheme:org .

<http://vocab.ceda.ac.uk/collection/cci/org/org77> a cci:org,
        skos:Concept ;
    skos:altLabel "DMI"@en ;
    skos:inScheme cci-scheme:org ;
    skos:prefLabel "Danish Meteorological Institute"@en ;
    skos:topConceptOf cci-scheme:org .

<http://vocab.ceda.ac.uk/collection/cci/org/org78> a cci:org,
        skos:Concept ;
    skos:altLabel "DTU-GDK"@en ;
    skos:inScheme cci-scheme:org ;
    skos:prefLabel "DTU-Space, Department of Geodynamics"@en ;
    skos:topConceptOf cci-scheme:org .

<http://vocab.ceda.ac.uk/collection/cci/org/org79> a cci:org,
        skos:Concept ;
    skos:altLabel "DTU-MRS"@en ;
    skos:inScheme cci-scheme:org ;
    skos:prefLabel "DTU-Space, Department of Microwaves and Remote Sensing"@en ;
    skos:topConceptOf cci-scheme:org .

<http://vocab.ceda.ac.uk/collection/cci/org/org80> a cci:org,
        skos:Concept ;
    skos:altLabel "NBI"@en ;
    skos:inScheme cci-scheme:org ;
    skos:prefLabel "Niels Bohr Institute"@en ;
    skos:topConceptOf cci-scheme:org .

<http://vocab.ceda.ac.uk/collection/cci/org/org81> a cci:org,
        skos:Concept ;
    skos:altLabel "TUDr"@en ;
    skos:inScheme cci-scheme:org ;
    skos:prefLabel "Technische Universität Dresden"@en ;
    skos:topConceptOf cci-scheme:org .

<http://vocab.ceda.ac.uk/collection/cci/org/org82> a cci:org,
        skos:Concept ;
    skos:altLabel "TUM"@en ;
    skos:inScheme cci-scheme:org ;
    skos:prefLabel "Technische Universität München"@en ;
    skos:topConceptOf cci-scheme:org .

<http://vocab.ceda.ac.uk/collection/cci/org/org83> a cci:org,
        skos:Concept ;
    rdfs:seeAlso <http://isni.org/isni/121901201> ;
    skos:altLabel "UCLON"@en ;
    skos:inScheme cci-scheme:org ;
    skos:prefLabel "University College London"@en ;
    skos:topConceptOf cci-scheme:org .

<http://vocab.ceda.ac.uk/collection/cci/org/org84> a cci:org,
        skos:Concept ;
    skos:altLabel "UL-CPOM"@en ;
    skos:inScheme cci-scheme:org ;
    skos:prefLabel "University of Leeds, Centre for Polar Observation and Modelling"@en ;
    skos:topConceptOf cci-scheme:org .

<http://vocab.ceda.ac.uk/collection/cci/org/org85> a cci:org,
        skos:Concept ;
    skos:altLabel "UL-SEE"@en ;
    skos:inScheme cci-scheme:org ;
    skos:prefLabel "University of Leeds, School of Earth and Environment"@en ;
    skos:topConceptOf cci-scheme:org .

<http://vocab.ceda.ac.uk/collection/cci/org/org86> a cci:org,
        skos:Concept ;
    skos:altLabel "AWI"@en ;
    skos:inScheme cci-scheme:org ;
    skos:prefLabel "Alfred-Wegener-Institut Helmholtz-Zentrum für Polar- und Meeresforschung"@en ;
    skos:topConceptOf cci-scheme:org .

<http://vocab.ceda.ac.uk/collection/cci/org/org87> a cci:org,
        skos:Concept ;
    skos:altLabel "ACRI-ST"@en ;
    skos:inScheme cci-scheme:org ;
    skos:prefLabel "ACRI-ST"@en ;
    skos:topConceptOf cci-scheme:org .

<http://vocab.ceda.ac.uk/collection/cci/org/org88> a cci:org,
        skos:Concept ;
    rdfs:seeAlso <http://isni.org/isni/107285406> ;
    skos:altLabel "LOCEAN"@en ;
    skos:inScheme cci-scheme:org ;
    skos:prefLabel "LOCEAN"@en ;
    skos:topConceptOf cci-scheme:org .

<http://vocab.ceda.ac.uk/collection/cci/org/org89> a cci:org,
        skos:Concept ;
    skos:altLabel "IFREMER/CERSAT"@en ;
    skos:inScheme cci-scheme:org ;
    skos:prefLabel "Institut Francais de Recherche pour l'Exploitation de la mer / CERSAT"@en ;
    skos:topConceptOf cci-scheme:org .

<http://vocab.ceda.ac.uk/collection/cci/org/org90> a cci:org,
        skos:Concept ;
    skos:inScheme cci-scheme:org ;
    skos:prefLabel "Transmissivity B.V. / VanderSat B.V."@en ;
    skos:topConceptOf cci-scheme:org .

<http://vocab.ceda.ac.uk/collection/cci/org/org91> a cci:org,
        skos:Concept ;
    skos:inScheme cci-scheme:org ;
    skos:prefLabel "University of Reading"@en ;
    skos:topConceptOf cci-scheme:org .

<http://vocab.ceda.ac.uk/collection/cci/org/org92> a cci:org,
        skos:Concept ;
    skos:inScheme cci-scheme:org ;
    skos:prefLabel "H2O Geomatics"@en ;
    skos:topConceptOf cci-scheme:org .

<http://vocab.ceda.ac.uk/collection/cci/org/org93> a cci:org,
        skos:Concept ;
    rdfs:seeAlso <http://isni.org/isni/405502827> ;
    skos:altLabel "DFD"@en ;
    skos:inScheme cci-scheme:org ;
    skos:prefLabel "Deutsches Fernerkundungsdatenzentrum"@en ;
    skos:topConceptOf cci-scheme:org .

<http://vocab.ceda.ac.uk/collection/cci/org/org94> a cci:org,
        skos:Concept ;
    rdfs:seeAlso <http://isni.org/isni/403850473> ;
    skos:altLabel "LMD"@en ;
    skos:inScheme cci-scheme:org ;
    skos:prefLabel "Laboratoire de Meteorologie Dynamique"@en ;
    skos:topConceptOf cci-scheme:org .

<http://vocab.ceda.ac.uk/collection/cci/org/org95> a cci:org,
        skos:Concept ;
    rdfs:seeAlso <http://isni.org/isni/123486355> ;
    skos:altLabel "ULB"@en ;
    skos:inScheme cci-scheme:org ;
    skos:prefLabel "Universite Libre de Bruxelles"@en ;
    skos:topConceptOf cci-scheme:org .

<http://vocab.ceda.ac.uk/collection/cci/org/org96> a cci:org,
        skos:Concept ;
    rdfs:seeAlso <http://isni.org/isni/123531689> ;
    skos:inScheme cci-scheme:org ;
    skos:prefLabel "Université de Toulouse"@en ;
    skos:topConceptOf cci-scheme:org .

<http://vocab.ceda.ac.uk/collection/cci/org/org97> a cci:org,
        skos:Concept ;
    rdfs:seeAlso <http://isni.org/isni/122879528> ;
    skos:altLabel "IRD"@en ;
    skos:inScheme cci-scheme:org ;
    skos:prefLabel "Institut de Recherche pour le Développement"@en ;
    skos:topConceptOf cci-scheme:org .

<http://vocab.ceda.ac.uk/collection/cci/org/org98> a cci:org,
        skos:Concept ;
    rdfs:seeAlso <http://isni.org/isni/404779832> ;
    skos:inScheme cci-scheme:org ;
    skos:prefLabel "University of Bern"@en ;
    skos:topConceptOf cci-scheme:org .

<http://vocab.ceda.ac.uk/collection/cci/org/org99> a cci:org,
        skos:Concept ;
    skos:inScheme cci-scheme:org ;
    skos:prefLabel "Estellus"@en ;
    skos:topConceptOf cci-scheme:org .

<http://vocab.ceda.ac.uk/collection/cci/platform/plat_unspecified> a cci:platform,
        skos:Concept ;
    skos:definition "Unspecified platform"@en ;
    skos:inScheme cci-scheme:platform ;
    skos:prefLabel "Unspecified"@en ;
    skos:scopeNote "Unspecified platform"@en ;
    skos:topConceptOf cci-scheme:platform .

<http://vocab.ceda.ac.uk/collection/cci/procLev/proc_ind> a cci:procLev,
        skos:Concept ;
    skos:altLabel "IND"@en ;
    skos:definition "Indicators derived from satellite data."@en ;
    skos:inScheme cci-scheme:procLev ;
    skos:prefLabel "Indicator"@en ;
    skos:scopeNote "Indicators derived from satellite data."@en ;
    skos:topConceptOf cci-scheme:procLev .

<http://vocab.ceda.ac.uk/collection/cci/procLev/proc_level0> a cci:procLev,
        skos:Concept ;
    rdfs:seeAlso <https://www.ghrsst.org/> ;
    skos:altLabel "L0"@en ;
    skos:definition "Unprocessed instrument and payload data at full resolution. CCI does not make recommendations regarding formats or content for data at this processing level."@en ;
    skos:inScheme cci-scheme:procLev ;
    skos:prefLabel "Level 0"@en ;
    skos:scopeNote "Unprocessed instrument and payload data at full resolution. CCI does not make recommendations regarding formats or content for data at this processing level."@en ;
    skos:topConceptOf cci-scheme:procLev .

<http://vocab.ceda.ac.uk/collection/cci/procLev/proc_level4> a cci:procLev,
        skos:Concept ;
    rdfs:seeAlso <https://www.ghrsst.org/> ;
    skos:altLabel "L4"@en ;
    skos:definition "Data sets created from the analysis of lower level data that result in gridded, gap-free products."@en ;
    skos:inScheme cci-scheme:procLev ;
    skos:prefLabel "Level 4"@en ;
    skos:scopeNote "Data sets created from the analysis of lower level data that result in gridded, gap-free products."@en ;
    skos:topConceptOf cci-scheme:procLev .

<http://vocab.ceda.ac.uk/collection/cci/procLev/proc_unspecified> a cci:procLev,
        skos:Concept ;
    skos:altLabel "Unspecified"@en ;
    skos:definition "Unspecified"@en ;
    skos:inScheme cci-scheme:procLev ;
    skos:prefLabel "Unspecified"@en ;
    skos:scopeNote "Unspecified"@en ;
    skos:topConceptOf cci-scheme:procLev .

<http://vocab.ceda.ac.uk/collection/cci/product/prod_AvhrMa> a cci:product,
        skos:Concept ;
    skos:inScheme cci-scheme:product ;
    skos:prefLabel "AVHRMA"@en ;
    skos:topConceptOf cci-scheme:product .

<http://vocab.ceda.ac.uk/collection/cci/product/prod_AvhrrMetopA> a cci:product,
        skos:Concept ;
    skos:inScheme cci-scheme:product ;
    skos:prefLabel "AVHRR_METOPA"@en ;
    skos:topConceptOf cci-scheme:product .

<http://vocab.ceda.ac.uk/collection/cci/product/prod_AvhrrMetopB> a cci:product,
        skos:Concept ;
    skos:inScheme cci-scheme:product ;
    skos:prefLabel "AVHRR_METOPB"@en ;
    skos:topConceptOf cci-scheme:product .

<http://vocab.ceda.ac.uk/collection/cci/product/prod_AvhrrMetopC> a cci:product,
        skos:Concept ;
    skos:inScheme cci-scheme:product ;
    skos:prefLabel "AVHRR_METOPC"@en ;
    skos:topConceptOf cci-scheme:product .

<http://vocab.ceda.ac.uk/collection/cci/product/prod_AvhrrNoaa10> a cci:product,
        skos:Concept ;
    skos:inScheme cci-scheme:product ;
    skos:prefLabel "AVHRR_NOAA10"@en ;
    skos:topConceptOf cci-scheme:product .

<http://vocab.ceda.ac.uk/collection/cci/product/prod_AvhrrNoaa11> a cci:product,
        skos:Concept ;
    skos:inScheme cci-scheme:product ;
    skos:prefLabel "AVHRR_NOAA11"@en ;
    skos:topConceptOf cci-scheme:product .

<http://vocab.ceda.ac.uk/collection/cci/product/prod_AvhrrNoaa12> a cci:product,
        skos:Concept ;
    skos:inScheme cci-scheme:product ;
    skos:prefLabel "AVHRR_NOAA12"@en ;
    skos:topConceptOf cci-scheme:product .

<http://vocab.ceda.ac.uk/collection/cci/product/prod_AvhrrNoaa14> a cci:product,
        skos:Concept ;
    skos:inScheme cci-scheme:product ;
    skos:prefLabel "AVHRR_NOAA14"@en ;
    skos:topConceptOf cci-scheme:product .

<http://vocab.ceda.ac.uk/collection/cci/product/prod_AvhrrNoaa16> a cci:product,
        skos:Concept ;
    skos:inScheme cci-scheme:product ;
    skos:prefLabel "AVHRR_NOAA16"@en ;
    skos:topConceptOf cci-scheme:product .

<http://vocab.ceda.ac.uk/collection/cci/product/prod_AvhrrNoaa17> a cci:product,
        skos:Concept ;
    skos:inScheme cci-scheme:product ;
    skos:prefLabel "AVHRR_NOAA17"@en ;
    skos:topConceptOf cci-scheme:product .

<http://vocab.ceda.ac.uk/collection/cci/product/prod_AvhrrNoaa18> a cci:product,
        skos:Concept ;
    skos:inScheme cci-scheme:product ;
    skos:prefLabel "AVHRR_NOAA18"@en ;
    skos:topConceptOf cci-scheme:product .

<http://vocab.ceda.ac.uk/collection/cci/product/prod_AvhrrNoaa19> a cci:product,
        skos:Concept ;
    skos:inScheme cci-scheme:product ;
    skos:prefLabel "AVHRR_NOAA19"@en ;
    skos:topConceptOf cci-scheme:product .

<http://vocab.ceda.ac.uk/collection/cci/product/prod_AvhrrNoaa6> a cci:product,
        skos:Concept ;
    skos:inScheme cci-scheme:product ;
    skos:prefLabel "AVHRR_NOAA6"@en ;
    skos:topConceptOf cci-scheme:product .

<http://vocab.ceda.ac.uk/collection/cci/product/prod_AvhrrNoaa7> a cci:product,
        skos:Concept ;
    skos:inScheme cci-scheme:product ;
    skos:prefLabel "AVHRR_NOAA7"@en ;
    skos:topConceptOf cci-scheme:product .

<http://vocab.ceda.ac.uk/collection/cci/product/prod_AvhrrNoaa8> a cci:product,
        skos:Concept ;
    skos:inScheme cci-scheme:product ;
    skos:prefLabel "AVHRR_NOAA8"@en ;
    skos:topConceptOf cci-scheme:product .

<http://vocab.ceda.ac.uk/collection/cci/product/prod_AvhrrNoaa9> a cci:product,
        skos:Concept ;
    skos:inScheme cci-scheme:product ;
    skos:prefLabel "AVHRR_NOAA9"@en ;
    skos:topConceptOf cci-scheme:product .

<http://vocab.ceda.ac.uk/collection/cci/product/prod_AvhrrTirosN> a cci:product,
        skos:Concept ;
    skos:inScheme cci-scheme:product ;
    skos:prefLabel "AVHRR_TIROSN"@en ;
    skos:topConceptOf cci-scheme:product .

<http://vocab.ceda.ac.uk/collection/cci/product/prod_CL02A01> a cci:product,
        skos:Concept ;
    skos:definition "CL02 layer from high resolution land cover for region A01 - Tiles"@en ;
    skos:inScheme cci-scheme:product ;
    skos:prefLabel "CL02-A01"@en ;
    skos:scopeNote "CL02 layer from high resolution land cover for region A01 - Tiles"@en ;
    skos:topConceptOf cci-scheme:product .

<http://vocab.ceda.ac.uk/collection/cci/product/prod_CL02A01Mos> a cci:product,
        skos:Concept ;
    skos:definition "CL02 layer from high resolution land cover for region A01 - Mosaics"@en ;
    skos:inScheme cci-scheme:product ;
    skos:prefLabel "CL02-A01MOSAIC"@en ;
    skos:scopeNote "CL02 layer from high resolution land cover for region A01 - Mosaics"@en ;
    skos:topConceptOf cci-scheme:product .

<http://vocab.ceda.ac.uk/collection/cci/product/prod_CL02A02> a cci:product,
        skos:Concept ;
    skos:definition "CL02 layer from high resolution land cover for region A02 - Tiles"@en ;
    skos:inScheme cci-scheme:product ;
    skos:prefLabel "CL02-A02"@en ;
    skos:scopeNote "CL02 layer from high resolution land cover for region A02 - Tiles"@en ;
    skos:topConceptOf cci-scheme:product .

<http://vocab.ceda.ac.uk/collection/cci/product/prod_CL02A02Mos> a cci:product,
        skos:Concept ;
    skos:definition "CL02 layer from high resolution land cover for region A02 - Mosaics"@en ;
    skos:inScheme cci-scheme:product ;
    skos:prefLabel "CL02-A02MOSAIC"@en ;
    skos:scopeNote "CL02 layer from high resolution land cover for region A02 - Mosaics"@en ;
    skos:topConceptOf cci-scheme:product .

<http://vocab.ceda.ac.uk/collection/cci/product/prod_CL02A03> a cci:product,
        skos:Concept ;
    skos:definition "CL02 layer from high resolution land cover for region A03 - Tiles"@en ;
    skos:inScheme cci-scheme:product ;
    skos:prefLabel "CL02-A03"@en ;
    skos:scopeNote "CL02 layer from high resolution land cover for region A03 - Tiles"@en ;
    skos:topConceptOf cci-scheme:product .

<http://vocab.ceda.ac.uk/collection/cci/product/prod_CL02A03Mos> a cci:product,
        skos:Concept ;
    skos:definition "CL02 layer from high resolution land cover for region A03 - Mosaics"@en ;
    skos:inScheme cci-scheme:product ;
    skos:prefLabel "CL02-A03MOSAIC"@en ;
    skos:scopeNote "CL02 layer from high resolution land cover for region A03 - Mosaics"@en ;
    skos:topConceptOf cci-scheme:product .

<http://vocab.ceda.ac.uk/collection/cci/product/prod_CryoSat2> a cci:product,
        skos:Concept ;
    skos:inScheme cci-scheme:product ;
    skos:prefLabel "CryoSat-2"@en ;
    skos:topConceptOf cci-scheme:product .

<http://vocab.ceda.ac.uk/collection/cci/product/prod_Diff> a cci:product,
        skos:Concept ;
    skos:inScheme cci-scheme:product ;
    skos:prefLabel "DIFF"@en ;
    skos:topConceptOf cci-scheme:product .

<http://vocab.ceda.ac.uk/collection/cci/product/prod_GlobMerg7day> a cci:product,
        skos:Concept ;
    skos:definition "Daily 7 day running mean on a globl 0.25 degree grid for the SH (salinity product)"@en ;
    skos:inScheme cci-scheme:product ;
    skos:prefLabel "GLOBAL-MERGED_OI_7DAY_RUNNINGMEAN_DAILY_0.25deg"@en ;
    skos:scopeNote "Daily 7 day running mean on a globl 0.25 degree grid for the SH (salinity product)"@en ;
    skos:topConceptOf cci-scheme:product .

<http://vocab.ceda.ac.uk/collection/cci/product/prod_GlobMergCent> a cci:product,
        skos:Concept ;
    skos:definition "Monthly running mean on a global 0.25degree grid"@en ;
    skos:inScheme cci-scheme:product ;
    skos:prefLabel "GLOBAL-MERGED_OI_Monthly_CENTRED_15Day_0.25deg"@en ;
    skos:scopeNote "Monthly running mean on a global 0.25degree grid"@en ;
    skos:topConceptOf cci-scheme:product .

<http://vocab.ceda.ac.uk/collection/cci/product/prod_HRLC10A01> a cci:product,
        skos:Concept ;
    skos:definition "high resolution land cover static product for region A01"@en ;
    skos:inScheme cci-scheme:product ;
    skos:prefLabel "HRLC10-A01"@en ;
    skos:scopeNote "high resolution land cover static product for region A01"@en ;
    skos:topConceptOf cci-scheme:product .

<http://vocab.ceda.ac.uk/collection/cci/product/prod_HRLC10A02> a cci:product,
        skos:Concept ;
    skos:definition "high resolution land cover static product for region A02"@en ;
    skos:inScheme cci-scheme:product ;
    skos:prefLabel "HRLC10-A02"@en ;
    skos:scopeNote "high resolution land cover static product for region A02"@en ;
    skos:topConceptOf cci-scheme:product .

<http://vocab.ceda.ac.uk/collection/cci/product/prod_HRLC10A03> a cci:product,
        skos:Concept ;
    skos:definition "high resolution land cover static product for region A03"@en ;
    skos:inScheme cci-scheme:product ;
    skos:prefLabel "HRLC10-A03"@en ;
    skos:scopeNote "high resolution land cover static product for region A03"@en ;
    skos:topConceptOf cci-scheme:product .

<http://vocab.ceda.ac.uk/collection/cci/product/prod_HRLC30A01> a cci:product,
        skos:Concept ;
    skos:definition "high resolution land cover historical map product for region A01"@en ;
    skos:inScheme cci-scheme:product ;
    skos:prefLabel "HRLC30-A01"@en ;
    skos:scopeNote "high resolution land cover historical map product for region A01"@en ;
    skos:topConceptOf cci-scheme:product .

<http://vocab.ceda.ac.uk/collection/cci/product/prod_HRLC30A02> a cci:product,
        skos:Concept ;
    skos:definition "high resolution land cover historical map product for region A02"@en ;
    skos:inScheme cci-scheme:product ;
    skos:prefLabel "HRLC30-A02"@en ;
    skos:scopeNote "high resolution land cover historical map product for region A02"@en ;
    skos:topConceptOf cci-scheme:product .

<http://vocab.ceda.ac.uk/collection/cci/product/prod_HRLC30A03> a cci:product,
        skos:Concept ;
    skos:definition "high resolution land cover historical map product for region A03"@en ;
    skos:inScheme cci-scheme:product ;
    skos:prefLabel "HRLC30-A03"@en ;
    skos:scopeNote "high resolution land cover historical map product for region A03"@en ;
    skos:topConceptOf cci-scheme:product .

<http://vocab.ceda.ac.uk/collection/cci/product/prod_HRLCC30A01> a cci:product,
        skos:Concept ;
    skos:definition "high resolution land cover historical change product for region A01"@en ;
    skos:inScheme cci-scheme:product ;
    skos:prefLabel "HRLCC30-A01"@en ;
    skos:scopeNote "high resolution land cover historical change product for region A01"@en ;
    skos:topConceptOf cci-scheme:product .

<http://vocab.ceda.ac.uk/collection/cci/product/prod_HRLCC30A02> a cci:product,
        skos:Concept ;
    skos:definition "high resolution land cover historical change product for region A02"@en ;
    skos:inScheme cci-scheme:product ;
    skos:prefLabel "HRLCC30-A02"@en ;
    skos:scopeNote "high resolution land cover historical change product for region A02"@en ;
    skos:topConceptOf cci-scheme:product .

<http://vocab.ceda.ac.uk/collection/cci/product/prod_HRLCC30A03> a cci:product,
        skos:Concept ;
    skos:definition "high resolution land cover historical change product for region A03"@en ;
    skos:inScheme cci-scheme:product ;
    skos:prefLabel "HRLCC30-A03"@en ;
    skos:scopeNote "high resolution land cover historical change product for region A03"@en ;
    skos:topConceptOf cci-scheme:product .

<http://vocab.ceda.ac.uk/collection/cci/product/prod_IQIXA01> a cci:product,
        skos:Concept ;
    skos:definition "IQIX layer from high resolution land cover for region A01 - Tiles"@en ;
    skos:inScheme cci-scheme:product ;
    skos:prefLabel "IQIX-A01"@en ;
    skos:scopeNote "IQIX layer from high resolution land cover for region A01 - Tiles"@en ;
    skos:topConceptOf cci-scheme:product .

<http://vocab.ceda.ac.uk/collection/cci/product/prod_IQIXA01Mos> a cci:product,
        skos:Concept ;
    skos:definition "IQIX layer from high resolution land cover for region A01 - Mosaics"@en ;
    skos:inScheme cci-scheme:product ;
    skos:prefLabel "IQIX-A01MOSAIC"@en ;
    skos:scopeNote "IQIX layer from high resolution land cover for region A01 - Mosaics"@en ;
    skos:topConceptOf cci-scheme:product .

<http://vocab.ceda.ac.uk/collection/cci/product/prod_IQIXA02> a cci:product,
        skos:Concept ;
    skos:definition "IQIX layer from high resolution land cover for region A02 - Tiles"@en ;
    skos:inScheme cci-scheme:product ;
    skos:prefLabel "IQIX-A02"@en ;
    skos:scopeNote "IQIX layer from high resolution land cover for region A02 - Tiles"@en ;
    skos:topConceptOf cci-scheme:product .

<http://vocab.ceda.ac.uk/collection/cci/product/prod_IQIXA02Mos> a cci:product,
        skos:Concept ;
    skos:definition "IQIX layer from high resolution land cover for region A02 - Mosaics"@en ;
    skos:inScheme cci-scheme:product ;
    skos:prefLabel "IQIX-A02MOSAIC"@en ;
    skos:scopeNote "IQIX layer from high resolution land cover for region A02 - Mosaics"@en ;
    skos:topConceptOf cci-scheme:product .

<http://vocab.ceda.ac.uk/collection/cci/product/prod_IQIXA03> a cci:product,
        skos:Concept ;
    skos:definition "IQIX layer from high resolution land cover for region A03 - Tiles"@en ;
    skos:inScheme cci-scheme:product ;
    skos:prefLabel "IQIX-A03"@en ;
    skos:scopeNote "IQIX layer from high resolution land cover for region A03 - Tiles"@en ;
    skos:topConceptOf cci-scheme:product .

<http://vocab.ceda.ac.uk/collection/cci/product/prod_IQIXA03Mos> a cci:product,
        skos:Concept ;
    skos:definition "IQIX layer from high resolution land cover for region A03 - Mosaics"@en ;
    skos:inScheme cci-scheme:product ;
    skos:prefLabel "IQIX-A03MOSAIC"@en ;
    skos:scopeNote "IQIX layer from high resolution land cover for region A03 - Mosaics"@en ;
    skos:topConceptOf cci-scheme:product .

<http://vocab.ceda.ac.uk/collection/cci/product/prod_Jason1> a cci:product,
        skos:Concept ;
    skos:inScheme cci-scheme:product ;
    skos:prefLabel "Jason-1"@en ;
    skos:topConceptOf cci-scheme:product .

<http://vocab.ceda.ac.uk/collection/cci/product/prod_Jason2> a cci:product,
        skos:Concept ;
    skos:inScheme cci-scheme:product ;
    skos:prefLabel "Jason-2"@en ;
    skos:topConceptOf cci-scheme:product .

<http://vocab.ceda.ac.uk/collection/cci/product/prod_Jason3> a cci:product,
        skos:Concept ;
    skos:inScheme cci-scheme:product ;
    skos:prefLabel "Jason-3"@en ;
    skos:topConceptOf cci-scheme:product .

<http://vocab.ceda.ac.uk/collection/cci/product/prod_PS01A01> a cci:product,
        skos:Concept ;
    skos:definition "PS01 layer from high resolution land cover for region A01 - Tiles"@en ;
    skos:inScheme cci-scheme:product ;
    skos:prefLabel "PS01-A01"@en ;
    skos:scopeNote "PS01 layer from high resolution land cover for region A01 - Tiles"@en ;
    skos:topConceptOf cci-scheme:product .

<http://vocab.ceda.ac.uk/collection/cci/product/prod_PS01A01Mos> a cci:product,
        skos:Concept ;
    skos:definition "PS01 layer from high resolution land cover for region A01 - Mosaics"@en ;
    skos:inScheme cci-scheme:product ;
    skos:prefLabel "PS01-A01MOSAIC"@en ;
    skos:scopeNote "PS01 layer from high resolution land cover for region A01 - Mosaics"@en ;
    skos:topConceptOf cci-scheme:product .

<http://vocab.ceda.ac.uk/collection/cci/product/prod_PS01A02> a cci:product,
        skos:Concept ;
    skos:definition "PS01 layer from high resolution land cover for region A02 - Tiles"@en ;
    skos:inScheme cci-scheme:product ;
    skos:prefLabel "PS01-A02"@en ;
    skos:scopeNote "PS01 layer from high resolution land cover for region A02 - Tiles"@en ;
    skos:topConceptOf cci-scheme:product .

<http://vocab.ceda.ac.uk/collection/cci/product/prod_PS01A02Mos> a cci:product,
        skos:Concept ;
    skos:definition "PS01 layer from high resolution land cover for region A02 - Mosaics"@en ;
    skos:inScheme cci-scheme:product ;
    skos:prefLabel "PS01-A02MOSAIC"@en ;
    skos:scopeNote "PS01 layer from high resolution land cover for region A02 - Mosaics"@en ;
    skos:topConceptOf cci-scheme:product .

<http://vocab.ceda.ac.uk/collection/cci/product/prod_PS01A03> a cci:product,
        skos:Concept ;
    skos:definition "PS01 layer from high resolution land cover for region A03 - Tiles"@en ;
    skos:inScheme cci-scheme:product ;
    skos:prefLabel "PS01-A03"@en ;
    skos:scopeNote "PS01 layer from high resolution land cover for region A03 - Tiles"@en ;
    skos:topConceptOf cci-scheme:product .

<http://vocab.ceda.ac.uk/collection/cci/product/prod_PS01A03Mos> a cci:product,
        skos:Concept ;
    skos:definition "PS01 layer from high resolution land cover for region A03 - Mosaics"@en ;
    skos:inScheme cci-scheme:product ;
    skos:prefLabel "PS01-A03MOSAIC"@en ;
    skos:scopeNote "PS01 layer from high resolution land cover for region A03 - Mosaics"@en ;
    skos:topConceptOf cci-scheme:product .

<http://vocab.ceda.ac.uk/collection/cci/product/prod_PS02A01> a cci:product,
        skos:Concept ;
    skos:definition "PS02 layer from high resolution land cover for region A01 - Tiles"@en ;
    skos:inScheme cci-scheme:product ;
    skos:prefLabel "PS02-A01"@en ;
    skos:scopeNote "PS02 layer from high resolution land cover for region A01 - Tiles"@en ;
    skos:topConceptOf cci-scheme:product .

<http://vocab.ceda.ac.uk/collection/cci/product/prod_PS02A01Mos> a cci:product,
        skos:Concept ;
    skos:definition "PS02 layer from high resolution land cover for region A01 - Mosaics"@en ;
    skos:inScheme cci-scheme:product ;
    skos:prefLabel "PS02-A01MOSAIC"@en ;
    skos:scopeNote "PS02 layer from high resolution land cover for region A01 - Mosaics"@en ;
    skos:topConceptOf cci-scheme:product .

<http://vocab.ceda.ac.uk/collection/cci/product/prod_PS02A02> a cci:product,
        skos:Concept ;
    skos:definition "PS02 layer from high resolution land cover for region A02 - Tiles"@en ;
    skos:inScheme cci-scheme:product ;
    skos:prefLabel "PS02-A02"@en ;
    skos:scopeNote "PS02 layer from high resolution land cover for region A02 - Tiles"@en ;
    skos:topConceptOf cci-scheme:product .

<http://vocab.ceda.ac.uk/collection/cci/product/prod_PS02A02Mos> a cci:product,
        skos:Concept ;
    skos:definition "PS02 layer from high resolution land cover for region A02 - Mosaics"@en ;
    skos:inScheme cci-scheme:product ;
    skos:prefLabel "PS02-A02MOSAIC"@en ;
    skos:scopeNote "PS02 layer from high resolution land cover for region A02 - Mosaics"@en ;
    skos:topConceptOf cci-scheme:product .

<http://vocab.ceda.ac.uk/collection/cci/product/prod_PS02A03> a cci:product,
        skos:Concept ;
    skos:definition "PS02 layer from high resolution land cover for region A03 - Tiles"@en ;
    skos:inScheme cci-scheme:product ;
    skos:prefLabel "PS02-A03"@en ;
    skos:scopeNote "PS02 layer from high resolution land cover for region A03 - Tiles"@en ;
    skos:topConceptOf cci-scheme:product .

<http://vocab.ceda.ac.uk/collection/cci/product/prod_PS02A03Mos> a cci:product,
        skos:Concept ;
    skos:definition "PS02 layer from high resolution land cover for region A03 - Mosaics"@en ;
    skos:inScheme cci-scheme:product ;
    skos:prefLabel "PS02-A03MOSAIC"@en ;
    skos:scopeNote "PS02 layer from high resolution land cover for region A03 - Mosaics"@en ;
    skos:topConceptOf cci-scheme:product .

<http://vocab.ceda.ac.uk/collection/cci/product/prod_PolMerg7dayNh> a cci:product,
        skos:Concept ;
    skos:definition "Daily 7 day running mean on a 25km EASE2 grid for the NH (salinity product)"@en ;
    skos:inScheme cci-scheme:product ;
    skos:prefLabel "POLAR-MERGED_OI_7DAY_RUNNINGMEAN_DAILY_25kmEASE2-NH"@en ;
    skos:scopeNote "Daily 7 day running mean on a 25km EASE2 grid for the NH (salinity product)"@en ;
    skos:topConceptOf cci-scheme:product .

<http://vocab.ceda.ac.uk/collection/cci/product/prod_PolMerg7daySh> a cci:product,
        skos:Concept ;
    skos:definition "Daily 7 day running mean on a 25km EASE2 grid for the SH (salinity product)"@en ;
    skos:inScheme cci-scheme:product ;
    skos:prefLabel "POLAR-MERGED_OI_7DAY_RUNNINGMEAN_DAILY_25kmEASE2-SH"@en ;
    skos:scopeNote "Daily 7 day running mean on a 25km EASE2 grid for the SH (salinity product)"@en ;
    skos:topConceptOf cci-scheme:product .

<http://vocab.ceda.ac.uk/collection/cci/product/prod_PolMergCentNH> a cci:product,
        skos:Concept ;
    skos:definition "Monthly running mean on a global 0.25degree grid"@en ;
    skos:inScheme cci-scheme:product ;
    skos:prefLabel "POLAR-MERGED_OI_Monthly_CENTRED_15Day_25kmEASE2-NH"@en ;
    skos:scopeNote "Monthly running mean on a global 0.25degree grid"@en ;
    skos:topConceptOf cci-scheme:product .

<http://vocab.ceda.ac.uk/collection/cci/product/prod_PolMergCentSH> a cci:product,
        skos:Concept ;
    skos:definition "Monthly running mean on a global 0.25degree grid"@en ;
    skos:inScheme cci-scheme:product ;
    skos:prefLabel "POLAR-MERGED_OI_Monthly_CENTRED_15Day_25kmEASE2-SH"@en ;
    skos:scopeNote "Monthly running mean on a global 0.25degree grid"@en ;
    skos:topConceptOf cci-scheme:product .

<http://vocab.ceda.ac.uk/collection/cci/product/prod_aFS> a cci:product,
        skos:Concept ;
    skos:inScheme cci-scheme:product ;
    skos:prefLabel "ACE_FTS_SCISAT"@en ;
    skos:topConceptOf cci-scheme:product .

<http://vocab.ceda.ac.uk/collection/cci/product/prod_aatsr> a cci:product,
        skos:Concept ;
    skos:inScheme cci-scheme:product ;
    skos:prefLabel "AATSR"@en ;
    skos:topConceptOf cci-scheme:product .

<http://vocab.ceda.ac.uk/collection/cci/product/prod_aatsrEn> a cci:product,
        skos:Concept ;
    skos:definition "Data from AATSR on Envisat"@en ;
    skos:inScheme cci-scheme:product ;
    skos:prefLabel "AATSR_ENVISAT"@en ;
    skos:scopeNote "Data from AATSR on Envisat"@en ;
    skos:topConceptOf cci-scheme:product .

<http://vocab.ceda.ac.uk/collection/cci/product/prod_aatsrEns> a cci:product,
        skos:Concept ;
    skos:inScheme cci-scheme:product ;
    skos:prefLabel "AATSR-ENVISAT-ENS"@en ;
    skos:topConceptOf cci-scheme:product .

<http://vocab.ceda.ac.uk/collection/cci/product/prod_aatsrEnsannual> a cci:product,
        skos:Concept ;
    skos:inScheme cci-scheme:product ;
    skos:prefLabel "AATSR-ENVISAT-ENS_ANNUAL"@en ;
    skos:topConceptOf cci-scheme:product .

<http://vocab.ceda.ac.uk/collection/cci/product/prod_aatsrEnsdaily> a cci:product,
        skos:Concept ;
    skos:inScheme cci-scheme:product ;
    skos:prefLabel "AATSR-ENVISAT-ENS_DAILY"@en ;
    skos:topConceptOf cci-scheme:product .

<http://vocab.ceda.ac.uk/collection/cci/product/prod_aatsrEnsmonthly> a cci:product,
        skos:Concept ;
    skos:inScheme cci-scheme:product ;
    skos:prefLabel "AATSR-ENVISAT-ENS_MONTHLY"@en ;
    skos:topConceptOf cci-scheme:product .

<http://vocab.ceda.ac.uk/collection/cci/product/prod_active> a cci:product,
        skos:Concept ;
    skos:inScheme cci-scheme:product ;
    skos:prefLabel "ACTIVE"@en ;
    skos:topConceptOf cci-scheme:product .

<http://vocab.ceda.ac.uk/collection/cci/product/prod_adv> a cci:product,
        skos:Concept ;
    skos:inScheme cci-scheme:product ;
    skos:prefLabel "ADV"@en ;
    skos:topConceptOf cci-scheme:product .

<http://vocab.ceda.ac.uk/collection/cci/product/prod_aergom> a cci:product,
        skos:Concept ;
    skos:inScheme cci-scheme:product ;
    skos:prefLabel "AERGOM"@en ;
    skos:topConceptOf cci-scheme:product .

<http://vocab.ceda.ac.uk/collection/cci/product/prod_alamo> a cci:product,
        skos:Concept ;
    skos:inScheme cci-scheme:product ;
    skos:prefLabel "ALAMO"@en ;
    skos:topConceptOf cci-scheme:product .

<http://vocab.ceda.ac.uk/collection/cci/product/prod_amsr> a cci:product,
        skos:Concept ;
    skos:inScheme cci-scheme:product ;
    skos:prefLabel "AMSR"@en ;
    skos:topConceptOf cci-scheme:product .

<http://vocab.ceda.ac.uk/collection/cci/product/prod_amsr25E> a cci:product,
        skos:Concept ;
    skos:inScheme cci-scheme:product ;
    skos:prefLabel "AMSR_25kmEASE2"@en ;
    skos:topConceptOf cci-scheme:product .

<http://vocab.ceda.ac.uk/collection/cci/product/prod_amsr50E> a cci:product,
        skos:Concept ;
    skos:inScheme cci-scheme:product ;
    skos:prefLabel "AMSR_50kmEASE2"@en ;
    skos:topConceptOf cci-scheme:product .

<http://vocab.ceda.ac.uk/collection/cci/product/prod_atsr1> a cci:product,
        skos:Concept ;
    skos:inScheme cci-scheme:product ;
    skos:prefLabel "ATSR1"@en ;
    skos:topConceptOf cci-scheme:product .

<http://vocab.ceda.ac.uk/collection/cci/product/prod_atsr2> a cci:product,
        skos:Concept ;
    skos:altLabel "ATSR-2"@en ;
    skos:inScheme cci-scheme:product ;
    skos:prefLabel "ATSR2"@en ;
    skos:topConceptOf cci-scheme:product .

<http://vocab.ceda.ac.uk/collection/cci/product/prod_atsr2Aatsr> a cci:product,
        skos:Concept ;
    skos:inScheme cci-scheme:product ;
    skos:prefLabel "ATSR2-AATSR"@en ;
    skos:topConceptOf cci-scheme:product .

<http://vocab.ceda.ac.uk/collection/cci/product/prod_atsr2Er2> a cci:product,
        skos:Concept ;
    skos:inScheme cci-scheme:product ;
    skos:prefLabel "ATSR2_ERS2"@en ;
    skos:topConceptOf cci-scheme:product .

<http://vocab.ceda.ac.uk/collection/cci/product/prod_atsr2ens> a cci:product,
        skos:Concept ;
    skos:inScheme cci-scheme:product ;
    skos:prefLabel "ATSR2-ENVISAT-ENS"@en ;
    skos:topConceptOf cci-scheme:product .

<http://vocab.ceda.ac.uk/collection/cci/product/prod_atsr2ensannual> a cci:product,
        skos:Concept ;
    skos:inScheme cci-scheme:product ;
    skos:prefLabel "ATSR2-ENVISAT-ENS_ANNUAL"@en ;
    skos:topConceptOf cci-scheme:product .

<http://vocab.ceda.ac.uk/collection/cci/product/prod_atsr2ensdaily> a cci:product,
        skos:Concept ;
    skos:inScheme cci-scheme:product ;
    skos:prefLabel "ATSR2-ENVISAT-ENS_DAILY"@en ;
    skos:topConceptOf cci-scheme:product .

<http://vocab.ceda.ac.uk/collection/cci/product/prod_atsr2ensmonthly> a cci:product,
        skos:Concept ;
    skos:inScheme cci-scheme:product ;
    skos:prefLabel "ATSR2-ENVISAT-ENS_MONTHLY"@en ;
    skos:topConceptOf cci-scheme:product .

<http://vocab.ceda.ac.uk/collection/cci/product/prod_atsr3> a cci:product,
        skos:Concept ;
    skos:definition "derived from AATSR on ENVISAT"@en ;
    skos:inScheme cci-scheme:product ;
    skos:prefLabel "ATSR_3"@en ;
    skos:scopeNote "derived from AATSR on ENVISAT"@en ;
    skos:topConceptOf cci-scheme:product .

<http://vocab.ceda.ac.uk/collection/cci/product/prod_atsr_2> a cci:product,
        skos:Concept ;
    skos:definition "derived from ATSR-2 on ERS_2"@en ;
    skos:inScheme cci-scheme:product ;
    skos:prefLabel "ATSR_2"@en ;
    skos:scopeNote "derived from ATSR-2 on ERS_2"@en ;
    skos:topConceptOf cci-scheme:product .

<http://vocab.ceda.ac.uk/collection/cci/product/prod_avhrr07G> a cci:product,
        skos:Concept ;
    skos:inScheme cci-scheme:product ;
    skos:prefLabel "AVHRR07_G"@en ;
    skos:topConceptOf cci-scheme:product .

<http://vocab.ceda.ac.uk/collection/cci/product/prod_avhrr09G> a cci:product,
        skos:Concept ;
    skos:inScheme cci-scheme:product ;
    skos:prefLabel "AVHRR09_G"@en ;
    skos:topConceptOf cci-scheme:product .

<http://vocab.ceda.ac.uk/collection/cci/product/prod_avhrr11G> a cci:product,
        skos:Concept ;
    skos:inScheme cci-scheme:product ;
    skos:prefLabel "AVHRR11_G"@en ;
    skos:topConceptOf cci-scheme:product .

<http://vocab.ceda.ac.uk/collection/cci/product/prod_avhrr12G> a cci:product,
        skos:Concept ;
    skos:inScheme cci-scheme:product ;
    skos:prefLabel "AVHRR12_G"@en ;
    skos:topConceptOf cci-scheme:product .

<http://vocab.ceda.ac.uk/collection/cci/product/prod_avhrr14G> a cci:product,
        skos:Concept ;
    skos:inScheme cci-scheme:product ;
    skos:prefLabel "AVHRR14_G"@en ;
    skos:topConceptOf cci-scheme:product .

<http://vocab.ceda.ac.uk/collection/cci/product/prod_avhrr15G> a cci:product,
        skos:Concept ;
    skos:inScheme cci-scheme:product ;
    skos:prefLabel "AVHRR15_G"@en ;
    skos:topConceptOf cci-scheme:product .

<http://vocab.ceda.ac.uk/collection/cci/product/prod_avhrr16G> a cci:product,
        skos:Concept ;
    skos:inScheme cci-scheme:product ;
    skos:prefLabel "AVHRR16_G"@en ;
    skos:topConceptOf cci-scheme:product .

<http://vocab.ceda.ac.uk/collection/cci/product/prod_avhrr17G> a cci:product,
        skos:Concept ;
    skos:inScheme cci-scheme:product ;
    skos:prefLabel "AVHRR17_G"@en ;
    skos:topConceptOf cci-scheme:product .

<http://vocab.ceda.ac.uk/collection/cci/product/prod_avhrr18G> a cci:product,
        skos:Concept ;
    skos:inScheme cci-scheme:product ;
    skos:prefLabel "AVHRR18_G"@en ;
    skos:topConceptOf cci-scheme:product .

<http://vocab.ceda.ac.uk/collection/cci/product/prod_avhrr19G> a cci:product,
        skos:Concept ;
    skos:inScheme cci-scheme:product ;
    skos:prefLabel "AVHRR19_G"@en ;
    skos:topConceptOf cci-scheme:product .

<http://vocab.ceda.ac.uk/collection/cci/product/prod_avhrrAm> a cci:product,
        skos:Concept ;
    skos:inScheme cci-scheme:product ;
    skos:prefLabel "AVHRR-AM"@en ;
    skos:topConceptOf cci-scheme:product .

<http://vocab.ceda.ac.uk/collection/cci/product/prod_avhrrLtdr> a cci:product,
        skos:Concept ;
    skos:inScheme cci-scheme:product ;
    skos:prefLabel "AVHRR-LTDR"@en ;
    skos:topConceptOf cci-scheme:product .

<http://vocab.ceda.ac.uk/collection/cci/product/prod_avhrrMg> a cci:product,
        skos:Concept ;
    skos:definition "Data from AVHRR, more than one platform"@en ;
    skos:inScheme cci-scheme:product ;
    skos:prefLabel "AVHRR_MERGED"@en ;
    skos:scopeNote "Data from AVHRR, more than one platform"@en ;
    skos:topConceptOf cci-scheme:product .

<http://vocab.ceda.ac.uk/collection/cci/product/prod_avhrrNoaa> a cci:product,
        skos:Concept ;
    skos:inScheme cci-scheme:product ;
    skos:prefLabel "AVHRR_NOAA"@en ;
    skos:topConceptOf cci-scheme:product .

<http://vocab.ceda.ac.uk/collection/cci/product/prod_avhrrPm> a cci:product,
        skos:Concept ;
    skos:inScheme cci-scheme:product ;
    skos:prefLabel "AVHRR-PM"@en ;
    skos:topConceptOf cci-scheme:product .

<http://vocab.ceda.ac.uk/collection/cci/product/prod_avhrrmtag> a cci:product,
        skos:Concept ;
    skos:inScheme cci-scheme:product ;
    skos:prefLabel "AVHRRMTA_G"@en ;
    skos:topConceptOf cci-scheme:product .

<http://vocab.ceda.ac.uk/collection/cci/product/prod_besd> a cci:product,
        skos:Concept ;
    skos:definition "Data from the GHG BESD algorithm"@en ;
    skos:inScheme cci-scheme:product ;
    skos:prefLabel "BESD"@en ;
    skos:scopeNote "Data from the GHG BESD algorithm"@en ;
    skos:topConceptOf cci-scheme:product .

<http://vocab.ceda.ac.uk/collection/cci/product/prod_change> a cci:product,
        skos:Concept ;
    skos:inScheme cci-scheme:product ;
    skos:prefLabel "CHANGE"@en ;
    skos:topConceptOf cci-scheme:product .

<http://vocab.ceda.ac.uk/collection/cci/product/prod_cl01A01> a cci:product,
        skos:Concept ;
    skos:definition "CL01 layer from high resolution land cover for region A01 - Tiles"@en ;
    skos:inScheme cci-scheme:product ;
    skos:prefLabel "CL01-A01"@en ;
    skos:scopeNote "CL01 layer from high resolution land cover for region A01 - Tiles"@en ;
    skos:topConceptOf cci-scheme:product .

<http://vocab.ceda.ac.uk/collection/cci/product/prod_cl01A01Mos> a cci:product,
        skos:Concept ;
    skos:definition "CL01 layer from high resolution land cover for region A01 - Mosaics"@en ;
    skos:inScheme cci-scheme:product ;
    skos:prefLabel "CL01-A01MOSAIC"@en ;
    skos:scopeNote "CL01 layer from high resolution land cover for region A01 - Mosaics"@en ;
    skos:topConceptOf cci-scheme:product .

<http://vocab.ceda.ac.uk/collection/cci/product/prod_cl01A02> a cci:product,
        skos:Concept ;
    skos:definition "CL01 layer from high resolution land cover for region A02 - Tiles"@en ;
    skos:inScheme cci-scheme:product ;
    skos:prefLabel "CL01-A02"@en ;
    skos:scopeNote "CL01 layer from high resolution land cover for region A02 - Tiles"@en ;
    skos:topConceptOf cci-scheme:product .

<http://vocab.ceda.ac.uk/collection/cci/product/prod_cl01A02Mos> a cci:product,
        skos:Concept ;
    skos:definition "CL01 layer from high resolution land cover for region A02 - Mosaics"@en ;
    skos:inScheme cci-scheme:product ;
    skos:prefLabel "CL01-A02MOSAIC"@en ;
    skos:scopeNote "CL01 layer from high resolution land cover for region A02 - Mosaics"@en ;
    skos:topConceptOf cci-scheme:product .

<http://vocab.ceda.ac.uk/collection/cci/product/prod_cl01A03> a cci:product,
        skos:Concept ;
    skos:definition "CL01 layer from high resolution land cover for region A03 - Tiles"@en ;
    skos:inScheme cci-scheme:product ;
    skos:prefLabel "CL01-A03"@en ;
    skos:scopeNote "CL01 layer from high resolution land cover for region A03 - Tiles"@en ;
    skos:topConceptOf cci-scheme:product .

<http://vocab.ceda.ac.uk/collection/cci/product/prod_cl01A03Mos> a cci:product,
        skos:Concept ;
    skos:definition "CL01 layer from high resolution land cover for region A03 - Mosaics"@en ;
    skos:inScheme cci-scheme:product ;
    skos:prefLabel "CL01-A03MOSAIC"@en ;
    skos:scopeNote "CL01 layer from high resolution land cover for region A03 - Mosaics"@en ;
    skos:topConceptOf cci-scheme:product .

<http://vocab.ceda.ac.uk/collection/cci/product/prod_clim> a cci:product,
        skos:Concept ;
    skos:inScheme cci-scheme:product ;
    skos:prefLabel "Climatology"@en ;
    skos:topConceptOf cci-scheme:product .

<http://vocab.ceda.ac.uk/collection/cci/product/prod_comb> a cci:product,
        skos:Concept ;
    skos:inScheme cci-scheme:product ;
    skos:prefLabel "COMBINED"@en ;
    skos:topConceptOf cci-scheme:product .

<http://vocab.ceda.ac.uk/collection/cci/product/prod_combAdj> a cci:product,
        skos:Concept ;
    skos:inScheme cci-scheme:product ;
    skos:prefLabel "COMBINED_ADJUSTED"@en ;
    skos:topConceptOf cci-scheme:product .

<http://vocab.ceda.ac.uk/collection/cci/product/prod_emma> a cci:product,
        skos:Concept ;
    skos:definition "Data from the GHG EMMA algorithm"@en ;
    skos:inScheme cci-scheme:product ;
    skos:prefLabel "EMMA"@en ;
    skos:scopeNote "Data from the GHG EMMA algorithm"@en ;
    skos:topConceptOf cci-scheme:product .

<http://vocab.ceda.ac.uk/collection/cci/product/prod_envisat> a cci:product,
        skos:Concept ;
    skos:inScheme cci-scheme:product ;
    skos:prefLabel "Envisat"@en ;
    skos:topConceptOf cci-scheme:product .

<http://vocab.ceda.ac.uk/collection/cci/product/prod_eraModBias> a cci:product,
        skos:Concept ;
    skos:definition "Permafrost dataset"@en ;
    skos:inScheme cci-scheme:product ;
    skos:prefLabel "ERA5_MODISLST_BIASCORRECTED"@en ;
    skos:scopeNote "Permafrost dataset"@en ;
    skos:topConceptOf cci-scheme:product .

<http://vocab.ceda.ac.uk/collection/cci/product/prod_ers1> a cci:product,
        skos:Concept ;
    skos:inScheme cci-scheme:product ;
    skos:prefLabel "ERS-1"@en ;
    skos:topConceptOf cci-scheme:product .

<http://vocab.ceda.ac.uk/collection/cci/product/prod_ers2> a cci:product,
        skos:Concept ;
    skos:inScheme cci-scheme:product ;
    skos:prefLabel "ERS-2"@en ;
    skos:topConceptOf cci-scheme:product .

<http://vocab.ceda.ac.uk/collection/cci/product/prod_focal> a cci:product,
        skos:Concept ;
    skos:definition "Data from the GHG FOCAL algorithm"@en ;
    skos:inScheme cci-scheme:product ;
    skos:prefLabel "FOCAL"@en ;
    skos:scopeNote "Data from the GHG FOCAL algorithm"@en ;
    skos:topConceptOf cci-scheme:product .

<http://vocab.ceda.ac.uk/collection/cci/product/prod_gfo> a cci:product,
        skos:Concept ;
    skos:inScheme cci-scheme:product ;
    skos:prefLabel "GFO"@en ;
    skos:topConceptOf cci-scheme:product .

<http://vocab.ceda.ac.uk/collection/cci/product/prod_gmp> a cci:product,
        skos:Concept ;
    skos:inScheme cci-scheme:product ;
    skos:prefLabel "GMPEREAN"@en ;
    skos:topConceptOf cci-scheme:product .

<http://vocab.ceda.ac.uk/collection/cci/product/prod_gmpe> a cci:product,
        skos:Concept ;
    skos:inScheme cci-scheme:product ;
    skos:prefLabel "GMPE"@en ;
    skos:topConceptOf cci-scheme:product .

<http://vocab.ceda.ac.uk/collection/cci/product/prod_gomEn> a cci:product,
        skos:Concept ;
    skos:inScheme cci-scheme:product ;
    skos:prefLabel "GOMOS_ENVISAT"@en ;
    skos:topConceptOf cci-scheme:product .

<http://vocab.ceda.ac.uk/collection/cci/product/prod_gosat> a cci:product,
        skos:Concept ;
    skos:inScheme cci-scheme:product ;
    skos:prefLabel "GOSAT"@en ;
    skos:topConceptOf cci-scheme:product .

<http://vocab.ceda.ac.uk/collection/cci/product/prod_iasDLRImars> a cci:product,
        skos:Concept ;
    skos:definition "Aerosol data from IASI Metop-A using the DLR IMARS algorithm"@en ;
    skos:inScheme cci-scheme:product ;
    skos:prefLabel "IASI_METOPA-DLR-IMARS"@en ;
    skos:scopeNote "Aerosol data from IASI Metop-A using the DLR IMARS algorithm"@en ;
    skos:topConceptOf cci-scheme:product .

<http://vocab.ceda.ac.uk/collection/cci/product/prod_iasiLMDaero> a cci:product,
        skos:Concept ;
    skos:definition "Aerosol data from IASI Metop-A produced by LMD"@en ;
    skos:inScheme cci-scheme:product ;
    skos:prefLabel "IASI-METOPA-LMDAERO"@en ;
    skos:scopeNote "Aerosol data from IASI Metop-A produced by LMD"@en ;
    skos:topConceptOf cci-scheme:product .

<http://vocab.ceda.ac.uk/collection/cci/product/prod_iasiMAPIR> a cci:product,
        skos:Concept ;
    skos:definition "Aerosol data from IASI Metop-A using the MAPIR algorithm"@en ;
    skos:inScheme cci-scheme:product ;
    skos:prefLabel "IASI-METOPA-MAPIR"@en ;
    skos:scopeNote "Aerosol data from IASI Metop-A using the MAPIR algorithm"@en ;
    skos:topConceptOf cci-scheme:product .

<http://vocab.ceda.ac.uk/collection/cci/product/prod_iasiULB> a cci:product,
        skos:Concept ;
    skos:definition "Aersols data from IASI Metop-A produced by ULB"@en ;
    skos:inScheme cci-scheme:product ;
    skos:prefLabel "IASI-METOPA-ULB"@en ;
    skos:scopeNote "Aersols data from IASI Metop-A produced by ULB"@en ;
    skos:topConceptOf cci-scheme:product .

<http://vocab.ceda.ac.uk/collection/cci/product/prod_imap> a cci:product,
        skos:Concept ;
    skos:definition "Data from the GHG IMAP algorithm"@en ;
    skos:inScheme cci-scheme:product ;
    skos:prefLabel "IMAP"@en ;
    skos:scopeNote "Data from the GHG IMAP algorithm"@en ;
    skos:topConceptOf cci-scheme:product .

<http://vocab.ceda.ac.uk/collection/cci/product/prod_ircdr> a cci:product,
        skos:Concept ;
    skos:inScheme cci-scheme:product ;
    skos:prefLabel "IRCDR"@en ;
    skos:topConceptOf cci-scheme:product .

<http://vocab.ceda.ac.uk/collection/cci/product/prod_irmgp> a cci:product,
        skos:Concept ;
    skos:inScheme cci-scheme:product ;
    skos:prefLabel "IRMGP"@en ;
    skos:topConceptOf cci-scheme:product .

<http://vocab.ceda.ac.uk/collection/cci/product/prod_map> a cci:product,
        skos:Concept ;
    skos:inScheme cci-scheme:product ;
    skos:prefLabel "Map"@en ;
    skos:topConceptOf cci-scheme:product .

<http://vocab.ceda.ac.uk/collection/cci/product/prod_meAaEn> a cci:product,
        skos:Concept ;
    skos:inScheme cci-scheme:product ;
    skos:prefLabel "MERISAATSR_ENVISAT"@en ;
    skos:topConceptOf cci-scheme:product .

<http://vocab.ceda.ac.uk/collection/cci/product/prod_medSea> a cci:product,
        skos:Concept ;
    skos:definition "Mediterranean sea"@en ;
    skos:inScheme cci-scheme:product ;
    skos:prefLabel "MED_SEA"@en ;
    skos:scopeNote "Mediterranean sea"@en ;
    skos:topConceptOf cci-scheme:product .

<http://vocab.ceda.ac.uk/collection/cci/product/prod_merg7dayDaily> a cci:product,
        skos:Concept ;
    skos:definition "Daily 7 day running mean from merged satellite data (salinity product)"@en ;
    skos:inScheme cci-scheme:product ;
    skos:prefLabel "MERGED_OI_7DAY_RUNNINGMEAN_DAILY_25km"@en ;
    skos:scopeNote "Daily 7 day running mean from merged satellite data (salinity product)"@en ;
    skos:topConceptOf cci-scheme:product .

<http://vocab.ceda.ac.uk/collection/cci/product/prod_mergMon15day25km> a cci:product,
        skos:Concept ;
    skos:definition "15 day rolling monthly average from merged satellite data (salinity product)"@en ;
    skos:inScheme cci-scheme:product ;
    skos:prefLabel "MERGED_OI_Monthly_CENTRED_15Day_25km"@en ;
    skos:scopeNote "15 day rolling monthly average from merged satellite data (salinity product)"@en ;
    skos:topConceptOf cci-scheme:product .

<http://vocab.ceda.ac.uk/collection/cci/product/prod_merged> a cci:product,
        skos:Concept ;
    skos:definition "Data from more than one platform and/or sensor"@en ;
    skos:inScheme cci-scheme:product ;
    skos:prefLabel "MERGED"@en ;
    skos:scopeNote "Data from more than one platform and/or sensor"@en ;
    skos:topConceptOf cci-scheme:product .

<http://vocab.ceda.ac.uk/collection/cci/product/prod_merris> a cci:product,
        skos:Concept ;
    skos:inScheme cci-scheme:product ;
    skos:prefLabel "MERIS"@en ;
    skos:topConceptOf cci-scheme:product .

<http://vocab.ceda.ac.uk/collection/cci/product/prod_merris_envisat> a cci:product,
        skos:Concept ;
    skos:inScheme cci-scheme:product ;
    skos:prefLabel "MERIS_ENVISAT"@en ;
    skos:topConceptOf cci-scheme:product .

<http://vocab.ceda.ac.uk/collection/cci/product/prod_miEn> a cci:product,
        skos:Concept ;
    skos:inScheme cci-scheme:product ;
    skos:prefLabel "MIPAS_ENVISAT"@en ;
    skos:topConceptOf cci-scheme:product .

<http://vocab.ceda.ac.uk/collection/cci/product/prod_modA> a cci:product,
        skos:Concept ;
    skos:definition "derived from MODIS aqua"@en ;
    skos:inScheme cci-scheme:product ;
    skos:prefLabel "MODISA"@en ;
    skos:scopeNote "derived from MODIS aqua"@en ;
    skos:topConceptOf cci-scheme:product .

<http://vocab.ceda.ac.uk/collection/cci/product/prod_modAqu> a cci:product,
        skos:Concept ;
    skos:inScheme cci-scheme:product ;
    skos:prefLabel "MODIS_AQUA"@en ;
    skos:topConceptOf cci-scheme:product .

<http://vocab.ceda.ac.uk/collection/cci/product/prod_modMg> a cci:product,
        skos:Concept ;
    skos:inScheme cci-scheme:product ;
    skos:prefLabel "MODIS_MERGED"@en ;
    skos:topConceptOf cci-scheme:product .

<http://vocab.ceda.ac.uk/collection/cci/product/prod_modT> a cci:product,
        skos:Concept ;
    skos:definition "derived from MODIS terra"@en ;
    skos:inScheme cci-scheme:product ;
    skos:prefLabel "MODIST"@en ;
    skos:scopeNote "derived from MODIS terra"@en ;
    skos:topConceptOf cci-scheme:product .

<http://vocab.ceda.ac.uk/collection/cci/product/prod_modTe> a cci:product,
        skos:Concept ;
    skos:inScheme cci-scheme:product ;
    skos:prefLabel "MODIS_TERRA"@en ;
    skos:topConceptOf cci-scheme:product .

<http://vocab.ceda.ac.uk/collection/cci/product/prod_modis> a cci:product,
        skos:Concept ;
    skos:inScheme cci-scheme:product ;
    skos:prefLabel "MODIS"@en ;
    skos:topConceptOf cci-scheme:product .

<http://vocab.ceda.ac.uk/collection/cci/product/prod_modlstCryo> a cci:product,
        skos:Concept ;
    skos:definition "Permafrost dataset"@en ;
    skos:inScheme cci-scheme:product ;
    skos:prefLabel "MODISLST_CRYOGRID"@en ;
    skos:scopeNote "Permafrost dataset"@en ;
    skos:topConceptOf cci-scheme:product .

<http://vocab.ceda.ac.uk/collection/cci/product/prod_msUvai> a cci:product,
        skos:Concept ;
    skos:inScheme cci-scheme:product ;
    skos:prefLabel "MS_UVAI"@en ;
    skos:topConceptOf cci-scheme:product .

<http://vocab.ceda.ac.uk/collection/cci/product/prod_msaai> a cci:product,
        skos:Concept ;
    skos:inScheme cci-scheme:product ;
    skos:prefLabel "MSAAI"@en ;
    skos:topConceptOf cci-scheme:product .

<http://vocab.ceda.ac.uk/collection/cci/product/prod_msi> a cci:product,
        skos:Concept ;
    skos:inScheme cci-scheme:product ;
    skos:prefLabel "MSI"@en ;
    skos:topConceptOf cci-scheme:product .

<http://vocab.ceda.ac.uk/collection/cci/product/prod_multi1d> a cci:product,
        skos:Concept ;
    skos:inScheme cci-scheme:product ;
    skos:prefLabel "MULTI_1D"@en ;
    skos:topConceptOf cci-scheme:product .

<http://vocab.ceda.ac.uk/collection/cci/product/prod_multi1m> a cci:product,
        skos:Concept ;
    skos:inScheme cci-scheme:product ;
    skos:prefLabel "MULTI_1M"@en ;
    skos:topConceptOf cci-scheme:product .

<http://vocab.ceda.ac.uk/collection/cci/product/prod_mzm> a cci:product,
        skos:Concept ;
    skos:inScheme cci-scheme:product ;
    skos:prefLabel "MZM"@en ;
    skos:topConceptOf cci-scheme:product .

<http://vocab.ceda.ac.uk/collection/cci/product/prod_nInd> a cci:product,
        skos:Concept ;
    skos:definition "Northern Indian Oceean"@en ;
    skos:inScheme cci-scheme:product ;
    skos:prefLabel "N_INDIAN"@en ;
    skos:scopeNote "Northern Indian Oceean"@en ;
    skos:topConceptOf cci-scheme:product .

<http://vocab.ceda.ac.uk/collection/cci/product/prod_neAtl> a cci:product,
        skos:Concept ;
    skos:definition "NE Atlantic"@en ;
    skos:inScheme cci-scheme:product ;
    skos:prefLabel "NE_ATL"@en ;
    skos:scopeNote "NE Atlantic"@en ;
    skos:topConceptOf cci-scheme:product .

<http://vocab.ceda.ac.uk/collection/cci/product/prod_nh> a cci:product,
        skos:Concept ;
    skos:inScheme cci-scheme:product ;
    skos:prefLabel "NH"@en ;
    skos:topConceptOf cci-scheme:product .

<http://vocab.ceda.ac.uk/collection/cci/product/prod_nh25kmease2> a cci:product,
        skos:Concept ;
    skos:inScheme cci-scheme:product ;
    skos:prefLabel "NH25KMEASE2"@en ;
    skos:topConceptOf cci-scheme:product .

<http://vocab.ceda.ac.uk/collection/cci/product/prod_nimEsmrNH> a cci:product,
        skos:Concept ;
    skos:inScheme cci-scheme:product ;
    skos:prefLabel "NIMBUS5_ESMR-EASE2_NH"@en ;
    skos:topConceptOf cci-scheme:product .

<http://vocab.ceda.ac.uk/collection/cci/product/prod_nimEsmrSH> a cci:product,
        skos:Concept ;
    skos:inScheme cci-scheme:product ;
    skos:prefLabel "NIMBUS5_ESMR-EASE2_SH"@en ;
    skos:topConceptOf cci-scheme:product .

<http://vocab.ceda.ac.uk/collection/cci/product/prod_ocfp> a cci:product,
        skos:Concept ;
    skos:definition "Data from the GHG OCFP algorithm"@en ;
    skos:inScheme cci-scheme:product ;
    skos:prefLabel "OCFP"@en ;
    skos:scopeNote "Data from the GHG OCFP algorithm"@en ;
    skos:topConceptOf cci-scheme:product .

<http://vocab.ceda.ac.uk/collection/cci/product/prod_ocpr> a cci:product,
        skos:Concept ;
    skos:definition "Data from the GHG OCPR algorithm"@en ;
    skos:inScheme cci-scheme:product ;
    skos:prefLabel "OCPR"@en ;
    skos:scopeNote "Data from the GHG OCPR algorithm"@en ;
    skos:topConceptOf cci-scheme:product .

<http://vocab.ceda.ac.uk/collection/cci/product/prod_opera> a cci:product,
        skos:Concept ;
    skos:definition "Data from OPERA analysis"@en ;
    skos:inScheme cci-scheme:product ;
    skos:prefLabel "OPERA"@en ;
    skos:scopeNote "Data from OPERA analysis"@en ;
    skos:topConceptOf cci-scheme:product .

<http://vocab.ceda.ac.uk/collection/cci/product/prod_orac> a cci:product,
        skos:Concept ;
    skos:definition "Data from Oxford RAL Aerosol and Cloud algorithm"@en ;
    skos:inScheme cci-scheme:product ;
    skos:prefLabel "ORAC"@en ;
    skos:scopeNote "Data from Oxford RAL Aerosol and Cloud algorithm"@en ;
    skos:topConceptOf cci-scheme:product .

<http://vocab.ceda.ac.uk/collection/cci/product/prod_osOd> a cci:product,
        skos:Concept ;
    skos:inScheme cci-scheme:product ;
    skos:prefLabel "OSIRIS_ODIN"@en ;
    skos:topConceptOf cci-scheme:product .

<http://vocab.ceda.ac.uk/collection/cci/product/prod_ostia> a cci:product,
        skos:Concept ;
    skos:inScheme cci-scheme:product ;
    skos:prefLabel "OSTIA"@en ;
    skos:topConceptOf cci-scheme:product .

<http://vocab.ceda.ac.uk/collection/cci/product/prod_parGrasp> a cci:product,
        skos:Concept ;
    skos:inScheme cci-scheme:product ;
    skos:prefLabel "PARASOL-GRASP"@en ;
    skos:topConceptOf cci-scheme:product .

<http://vocab.ceda.ac.uk/collection/cci/product/prod_passive> a cci:product,
        skos:Concept ;
    skos:inScheme cci-scheme:product ;
    skos:prefLabel "PASSIVE"@en ;
    skos:topConceptOf cci-scheme:product .

<http://vocab.ceda.ac.uk/collection/cci/product/prod_reSSMINH> a cci:product,
        skos:Concept ;
    skos:inScheme cci-scheme:product ;
    skos:prefLabel "RE_SSMI_12.5kmEASE2-NH"@en ;
    skos:topConceptOf cci-scheme:product .

<http://vocab.ceda.ac.uk/collection/cci/product/prod_reSSMISH> a cci:product,
        skos:Concept ;
    skos:inScheme cci-scheme:product ;
    skos:prefLabel "RE_SSMI_12.5kmEASE2-SH"@en ;
    skos:topConceptOf cci-scheme:product .

<http://vocab.ceda.ac.uk/collection/cci/product/prod_sAust> a cci:product,
        skos:Concept ;
    skos:definition "South Australia"@en ;
    skos:inScheme cci-scheme:product ;
    skos:prefLabel "S_AUSTRALIA"@en ;
    skos:scopeNote "South Australia"@en ;
    skos:topConceptOf cci-scheme:product .

<http://vocab.ceda.ac.uk/collection/cci/product/prod_saral> a cci:product,
        skos:Concept ;
    skos:inScheme cci-scheme:product ;
    skos:prefLabel "Saral"@en ;
    skos:topConceptOf cci-scheme:product .

<http://vocab.ceda.ac.uk/collection/cci/product/prod_sciam> a cci:product,
        skos:Concept ;
    skos:inScheme cci-scheme:product ;
    skos:prefLabel "SCIAMACHY"@en ;
    skos:topConceptOf cci-scheme:product .

<http://vocab.ceda.ac.uk/collection/cci/product/prod_sciamEn> a cci:product,
        skos:Concept ;
    skos:inScheme cci-scheme:product ;
    skos:prefLabel "SCIAMACHY_ENVISAT"@en ;
    skos:topConceptOf cci-scheme:product .

<http://vocab.ceda.ac.uk/collection/cci/product/prod_seAsia> a cci:product,
        skos:Concept ;
    skos:definition "South-east Asia"@en ;
    skos:inScheme cci-scheme:product ;
    skos:prefLabel "SE_ASIA"@en ;
    skos:scopeNote "South-east Asia"@en ;
    skos:topConceptOf cci-scheme:product .

<http://vocab.ceda.ac.uk/collection/cci/product/prod_sh> a cci:product,
        skos:Concept ;
    skos:inScheme cci-scheme:product ;
    skos:prefLabel "SH"@en ;
    skos:topConceptOf cci-scheme:product .

<http://vocab.ceda.ac.uk/collection/cci/product/prod_sh50kmease2> a cci:product,
        skos:Concept ;
    skos:inScheme cci-scheme:product ;
    skos:prefLabel "SH50KMEASE2"@en ;
    skos:topConceptOf cci-scheme:product .

<http://vocab.ceda.ac.uk/collection/cci/product/prod_slstrA> a cci:product,
        skos:Concept ;
    skos:definition "derived from SLSTR on Sentinel3A"@en ;
    skos:inScheme cci-scheme:product ;
    skos:prefLabel "SLSTRA"@en ;
    skos:scopeNote "derived from SLSTR on Sentinel3A"@en ;
    skos:topConceptOf cci-scheme:product .

<http://vocab.ceda.ac.uk/collection/cci/product/prod_slstrB> a cci:product,
        skos:Concept ;
    skos:definition "derived from SLSTR on Sentinel3B"@en ;
    skos:inScheme cci-scheme:product ;
    skos:prefLabel "SLSTRB"@en ;
    skos:scopeNote "derived from SLSTR on Sentinel3B"@en ;
    skos:topConceptOf cci-scheme:product .

<http://vocab.ceda.ac.uk/collection/cci/product/prod_smm> a cci:product,
        skos:Concept ;
    skos:inScheme cci-scheme:product ;
    skos:prefLabel "SMM"@en ;
    skos:topConceptOf cci-scheme:product .

<http://vocab.ceda.ac.uk/collection/cci/product/prod_smrOd> a cci:product,
        skos:Concept ;
    skos:inScheme cci-scheme:product ;
    skos:prefLabel "SMR_ODIN"@en ;
    skos:topConceptOf cci-scheme:product .

<http://vocab.ceda.ac.uk/collection/cci/product/prod_srfp> a cci:product,
        skos:Concept ;
    skos:definition "Data from the GHG SRFP algorithm"@en ;
    skos:inScheme cci-scheme:product ;
    skos:prefLabel "SRFP"@en ;
    skos:scopeNote "Data from the GHG SRFP algorithm"@en ;
    skos:topConceptOf cci-scheme:product .

<http://vocab.ceda.ac.uk/collection/cci/product/prod_srpr> a cci:product,
        skos:Concept ;
    skos:definition "Data from the GHG SRPR algorithm"@en ;
    skos:inScheme cci-scheme:product ;
    skos:prefLabel "SRPR"@en ;
    skos:scopeNote "Data from the GHG SRPR algorithm"@en ;
    skos:topConceptOf cci-scheme:product .

<http://vocab.ceda.ac.uk/collection/cci/product/prod_ssmi> a cci:product,
        skos:Concept ;
    skos:inScheme cci-scheme:product ;
    skos:prefLabel "SSMI"@en ;
    skos:topConceptOf cci-scheme:product .

<http://vocab.ceda.ac.uk/collection/cci/product/prod_ssmiS> a cci:product,
        skos:Concept ;
    skos:definition "data derived from SSMI on DSMP-F13 and SSMI/S on DSMP-F17"@en ;
    skos:inScheme cci-scheme:product ;
    skos:prefLabel "SSMI_SSMIS"@en ;
    skos:scopeNote "data derived from SSMI on DSMP-F13 and SSMI/S on DSMP-F17"@en ;
    skos:topConceptOf cci-scheme:product .

<http://vocab.ceda.ac.uk/collection/cci/product/prod_su> a cci:product,
        skos:Concept ;
    skos:inScheme cci-scheme:product ;
    skos:prefLabel "SU"@en ;
    skos:topConceptOf cci-scheme:product .

<http://vocab.ceda.ac.uk/collection/cci/product/prod_syn> a cci:product,
        skos:Concept ;
    skos:inScheme cci-scheme:product ;
    skos:prefLabel "SYN"@en ;
    skos:topConceptOf cci-scheme:product .

<http://vocab.ceda.ac.uk/collection/cci/product/prod_tcwvLand005> a cci:product,
        skos:Concept ;
    skos:definition "0.05deg total column water vapour over land"@en ;
    skos:inScheme cci-scheme:product ;
    skos:prefLabel "TCWV_land_005deg"@en ;
    skos:scopeNote "0.05deg total column water vapour over land"@en ;
    skos:topConceptOf cci-scheme:product .

<http://vocab.ceda.ac.uk/collection/cci/product/prod_tcwvLand05> a cci:product,
        skos:Concept ;
    skos:definition "0.5 degree total column water vapour over land"@en ;
    skos:inScheme cci-scheme:product ;
    skos:prefLabel "TCWV_land_05deg"@en ;
    skos:scopeNote "0.5 degree total column water vapour over land"@en ;
    skos:topConceptOf cci-scheme:product .

<http://vocab.ceda.ac.uk/collection/cci/product/prod_topexPos> a cci:product,
        skos:Concept ;
    skos:inScheme cci-scheme:product ;
    skos:prefLabel "Topex-Poseidon"@en ;
    skos:topConceptOf cci-scheme:product .

<http://vocab.ceda.ac.uk/collection/cci/product/prod_unspecified> a cci:product,
        skos:Concept ;
    skos:definition "unspecified product name"@en ;
    skos:inScheme cci-scheme:product ;
    skos:prefLabel "UNSPECIFIED"@en ;
    skos:scopeNote "unspecified product name"@en ;
    skos:topConceptOf cci-scheme:product .

<http://vocab.ceda.ac.uk/collection/cci/product/prod_var> a cci:product,
        skos:Concept ;
    skos:inScheme cci-scheme:product ;
    skos:prefLabel "VARIOUS"@en ;
    skos:topConceptOf cci-scheme:product .

<http://vocab.ceda.ac.uk/collection/cci/product/prod_wAfrica> a cci:product,
        skos:Concept ;
    skos:definition "West Africa"@en ;
    skos:inScheme cci-scheme:product ;
    skos:prefLabel "WAFRICA"@en ;
    skos:scopeNote "West Africa"@en ;
    skos:topConceptOf cci-scheme:product .

<http://vocab.ceda.ac.uk/collection/cci/product/prod_wfmd> a cci:product,
        skos:Concept ;
    skos:definition "Data from the GHG WFMD algorithm"@en ;
    skos:inScheme cci-scheme:product ;
    skos:prefLabel "WFMD"@en ;
    skos:scopeNote "Data from the GHG WFMD algorithm"@en ;
    skos:topConceptOf cci-scheme:product .

<http://vocab.ceda.ac.uk/collection/cci/project/cciproject_aerosol> a cci:project,
        skos:Concept ;
    skos:altLabel "AEROSOL"@en ;
    skos:definition "Aerosol properties climate data record produced from satellite data as part of the European Space Agency (ESA) Climate Change Initiative (CCI)"@en ;
    skos:inScheme cci-scheme:project ;
    skos:prefLabel "aerosol"@en ;
    skos:scopeNote "Aerosol properties climate data record produced from satellite data as part of the European Space Agency (ESA) Climate Change Initiative (CCI)"@en ;
    skos:topConceptOf cci-scheme:project .

<http://vocab.ceda.ac.uk/collection/cci/project/cciproject_biomass> a cci:project,
        skos:Concept ;
    skos:altLabel "BIOMASS"@en ;
    skos:definition "Above-ground biomass climate data record produced from satellite data as part of the European Space Agency (ESA) Climate Change Initiative (CCI)"@en ;
    skos:inScheme cci-scheme:project ;
    skos:prefLabel "above-ground biomass"@en ;
    skos:scopeNote "Above-ground biomass climate data record produced from satellite data as part of the European Space Agency (ESA) Climate Change Initiative (CCI)"@en ;
    skos:topConceptOf cci-scheme:project .

<http://vocab.ceda.ac.uk/collection/cci/project/cciproject_cloud> a cci:project,
        skos:Concept ;
    skos:altLabel "CLOUD"@en ;
    skos:definition "Cloud properties climate data record produced from satellite data as part of the European Space Agency (ESA) Climate Change Initiative (CCI)"@en ;
    skos:inScheme cci-scheme:project ;
    skos:prefLabel "cloud"@en ;
    skos:scopeNote "Cloud properties climate data record produced from satellite data as part of the European Space Agency (ESA) Climate Change Initiative (CCI)"@en ;
    skos:topConceptOf cci-scheme:project .

<http://vocab.ceda.ac.uk/collection/cci/project/cciproject_fire> a cci:project,
        skos:Concept ;
    skos:altLabel "FIRE"@en ;
    skos:definition "Fire disturbance (burned area) climate data record produced from satellite data as part of the European Space Agency (ESA) Climate Change Initiative (CCI)"@en ;
    skos:inScheme cci-scheme:project ;
    skos:prefLabel "fire"@en ;
    skos:scopeNote "Fire disturbance (burned area) climate data record produced from satellite data as part of the European Space Agency (ESA) Climate Change Initiative (CCI)"@en ;
    skos:topConceptOf cci-scheme:project .

<http://vocab.ceda.ac.uk/collection/cci/project/cciproject_ghg> a cci:project,
        skos:Concept ;
    skos:altLabel "GHG"@en ;
    skos:definition "Greenhouse gasses (carbon dioxide and methane) climate data record produced from satellite data as part of the European Space Agency (ESA) Climate Change Initiative (CCI)"@en ;
    skos:inScheme cci-scheme:project ;
    skos:prefLabel "greenhouse gases"@en ;
    skos:scopeNote "Greenhouse gasses (carbon dioxide and methane) climate data record produced from satellite data as part of the European Space Agency (ESA) Climate Change Initiative (CCI)"@en ;
    skos:topConceptOf cci-scheme:project .

<http://vocab.ceda.ac.uk/collection/cci/project/cciproject_glaciers> a cci:project,
        skos:Concept ;
    skos:altLabel "GLACIERS"@en ;
    skos:definition "Glacier inventory climate data record produced from satellite data as part of the European Space Agency (ESA) Climate Change Initiative (CCI)"@en ;
    skos:inScheme cci-scheme:project ;
    skos:prefLabel "glaciers"@en ;
    skos:scopeNote "Glacier inventory climate data record produced from satellite data as part of the European Space Agency (ESA) Climate Change Initiative (CCI)"@en ;
    skos:topConceptOf cci-scheme:project .

<http://vocab.ceda.ac.uk/collection/cci/project/cciproject_iceSheet> a cci:project,
        skos:Concept ;
    skos:altLabel "ICESHEETS"@en ;
    skos:definition "Ice sheets climate data record produced from satellite data as part of the European Space Agency (ESA) Climate Change Initiative (CCI)"@en ;
    skos:inScheme cci-scheme:project ;
    skos:prefLabel "ice sheets"@en ;
    skos:scopeNote "Ice sheets climate data record produced from satellite data as part of the European Space Agency (ESA) Climate Change Initiative (CCI)"@en ;
    skos:topConceptOf cci-scheme:project .

<http://vocab.ceda.ac.uk/collection/cci/project/cciproject_lakes> a cci:project,
        skos:Concept ;
    skos:altLabel "LAKES"@en ;
    skos:definition "Lakes climate data record produced from satellite data as part of the European Space Agency (ESA) Climate Change Initiative (CCI)"@en ;
    skos:inScheme cci-scheme:project ;
    skos:prefLabel "lakes"@en ;
    skos:scopeNote "Lakes climate data record produced from satellite data as part of the European Space Agency (ESA) Climate Change Initiative (CCI)"@en ;
    skos:topConceptOf cci-scheme:project .

<http://vocab.ceda.ac.uk/collection/cci/project/cciproject_landCov> a cci:project,
        skos:Concept ;
    skos:altLabel "LC"@en ;
    skos:definition "Land cover climate data record produced from satellite data as part of the European Space Agency (ESA) Climate Change Initiative (CCI)"@en ;
    skos:inScheme cci-scheme:project ;
    skos:prefLabel "land cover"@en ;
    skos:scopeNote "Land cover climate data record produced from satellite data as part of the European Space Agency (ESA) Climate Change Initiative (CCI)"@en ;
    skos:topConceptOf cci-scheme:project .

<http://vocab.ceda.ac.uk/collection/cci/project/cciproject_landSurfTemp> a cci:project,
        skos:Concept ;
    skos:altLabel "LST"@en ;
    skos:definition "Land Surface Temperature climate data record produced from satellite data as part of the European Space Agency (ESA) Climate Change Initiative (CCI)"@en ;
    skos:inScheme cci-scheme:project ;
    skos:prefLabel "land surface temperature"@en ;
    skos:scopeNote "Land Surface Temperature climate data record produced from satellite data as part of the European Space Agency (ESA) Climate Change Initiative (CCI)"@en ;
    skos:topConceptOf cci-scheme:project .

<http://vocab.ceda.ac.uk/collection/cci/project/cciproject_oceanCol> a cci:project,
        skos:Concept ;
    skos:altLabel "OC"@en ;
    skos:definition "Ocean colour climate data record produced from satellite data as part of the European Space Agency (ESA) Climate Change Initiative (CCI)"@en ;
    skos:inScheme cci-scheme:project ;
    skos:prefLabel "ocean colour"@en ;
    skos:scopeNote "Ocean colour climate data record produced from satellite data as part of the European Space Agency (ESA) Climate Change Initiative (CCI)"@en ;
    skos:topConceptOf cci-scheme:project .

<http://vocab.ceda.ac.uk/collection/cci/project/cciproject_ozone> a cci:project,
        skos:Concept ;
    skos:altLabel "OZONE"@en ;
    skos:definition "Ozone climate data record produced from satellite data as part of the European Space Agency (ESA) Climate Change Initiative (CCI)"@en ;
    skos:inScheme cci-scheme:project ;
    skos:prefLabel "ozone"@en ;
    skos:scopeNote "Ozone climate data record produced from satellite data as part of the European Space Agency (ESA) Climate Change Initiative (CCI)"@en ;
    skos:topConceptOf cci-scheme:project .

<http://vocab.ceda.ac.uk/collection/cci/project/cciproject_permafrost> a cci:project,
        skos:Concept ;
    skos:altLabel "PERMAFROST"@en ;
    skos:definition "Permafrost climate data record produced from satellite data as part of the European Space Agency (ESA) Climate Change Initiative (CCI)"@en ;
    skos:inScheme cci-scheme:project ;
    skos:prefLabel "permafrost"@en ;
    skos:scopeNote "Permafrost climate data record produced from satellite data as part of the European Space Agency (ESA) Climate Change Initiative (CCI)"@en ;
    skos:topConceptOf cci-scheme:project .

<http://vocab.ceda.ac.uk/collection/cci/project/cciproject_riverDischarge> a cci:project,
        skos:Concept ;
    skos:altLabel "RD"@en ;
    skos:definition "River discharge climate data record produced from satellite data as part of the European Space Agency (ESA) Climate Change Initiative (CCI)"@en ;
    skos:inScheme cci-scheme:project ;
    skos:prefLabel "river discharge"@en ;
    skos:scopeNote "River discharge climate data record produced from satellite data as part of the European Space Agency (ESA) Climate Change Initiative (CCI)"@en ;
    skos:topConceptOf cci-scheme:project .

<http://vocab.ceda.ac.uk/collection/cci/project/cciproject_salinity> a cci:project,
        skos:Concept ;
    skos:altLabel "SEASURFACESALINITY"@en ;
    skos:definition "Sea Surface Salinity climate data record produced from satellite data as part of the European Space Agency (ESA) Climate Change Initiative (CCI)"@en ;
    skos:inScheme cci-scheme:project ;
    skos:prefLabel "sea surface salinity"@en ;
    skos:scopeNote "Sea Surface Salinity climate data record produced from satellite data as part of the European Space Agency (ESA) Climate Change Initiative (CCI)"@en ;
    skos:topConceptOf cci-scheme:project .

<http://vocab.ceda.ac.uk/collection/cci/project/cciproject_seaIce> a cci:project,
        skos:Concept ;
    skos:altLabel "SEAICE"@en ;
    skos:definition "Sea ice climate data record produced from satellite data as part of the European Space Agency (ESA) Climate Change Initiative (CCI)"@en ;
    skos:inScheme cci-scheme:project ;
    skos:prefLabel "sea ice"@en ;
    skos:scopeNote "Sea ice climate data record produced from satellite data as part of the European Space Agency (ESA) Climate Change Initiative (CCI)"@en ;
    skos:topConceptOf cci-scheme:project .

<http://vocab.ceda.ac.uk/collection/cci/project/cciproject_seaLevel> a cci:project,
        skos:Concept ;
    skos:altLabel "SEALEVEL"@en ;
    skos:definition "Sea level climate data record produced from satellite data as part of the European Space Agency (ESA) Climate Change Initiative (CCI)"@en ;
    skos:inScheme cci-scheme:project ;
    skos:prefLabel "sea level"@en ;
    skos:scopeNote "Sea level climate data record produced from satellite data as part of the European Space Agency (ESA) Climate Change Initiative (CCI)"@en ;
    skos:topConceptOf cci-scheme:project .

<http://vocab.ceda.ac.uk/collection/cci/project/cciproject_seaState> a cci:project,
        skos:Concept ;
    skos:altLabel "SEASTATE"@en ;
    skos:definition "Sea state climate data record produced from satellite data as part of the European Space Agency (ESA) Climate Change Initiative (CCI)"@en ;
    skos:inScheme cci-scheme:project ;
    skos:prefLabel "sea state"@en ;
    skos:scopeNote "Sea state climate data record produced from satellite data as part of the European Space Agency (ESA) Climate Change Initiative (CCI)"@en ;
    skos:topConceptOf cci-scheme:project .

<http://vocab.ceda.ac.uk/collection/cci/project/cciproject_snow> a cci:project,
        skos:Concept ;
    skos:altLabel "SNOW"@en ;
    skos:definition "Snow climate data record produced from satellite data as part of the European Space Agency (ESA) Climate Change Initiative (CCI)"@en ;
    skos:inScheme cci-scheme:project ;
    skos:prefLabel "snow"@en ;
    skos:scopeNote "Snow climate data record produced from satellite data as part of the European Space Agency (ESA) Climate Change Initiative (CCI)"@en ;
    skos:topConceptOf cci-scheme:project .

<http://vocab.ceda.ac.uk/collection/cci/project/cciproject_soilMst> a cci:project,
        skos:Concept ;
    skos:altLabel "SOILMOISTURE"@en ;
    skos:definition "Soil moisture climate data record produced from satellite data as part of the European Space Agency (ESA) Climate Change Initiative (CCI)"@en ;
    skos:inScheme cci-scheme:project ;
    skos:prefLabel "soil moisture"@en ;
    skos:scopeNote "Soil moisture climate data record produced from satellite data as part of the European Space Agency (ESA) Climate Change Initiative (CCI)"@en ;
    skos:topConceptOf cci-scheme:project .

<http://vocab.ceda.ac.uk/collection/cci/project/cciproject_sst> a cci:project,
        skos:Concept ;
    skos:altLabel "SST"@en ;
    skos:definition "Sea surface temperature climate data record produced from satellite data as part of the European Space Agency (ESA) Climate Change Initiative (CCI)"@en ;
    skos:inScheme cci-scheme:project ;
    skos:prefLabel "sea surface temperature"@en ;
    skos:scopeNote "Sea surface temperature climate data record produced from satellite data as part of the European Space Agency (ESA) Climate Change Initiative (CCI)"@en ;
    skos:topConceptOf cci-scheme:project .

<http://vocab.ceda.ac.uk/collection/cci/project/cciproject_vegParam> a cci:project,
        skos:Concept ;
    skos:altLabel "VEGETATION"@en ;
    skos:definition "Vegetation Parameters climate data record produced from satellite data as part of the European Space Agency (ESA) Climate Change Initiative (CCI)"@en ;
    skos:inScheme cci-scheme:project ;
    skos:prefLabel "vegetation parameters"@en ;
    skos:scopeNote "Vegetation Parameters climate data record produced from satellite data as part of the European Space Agency (ESA) Climate Change Initiative (CCI)"@en ;
    skos:topConceptOf cci-scheme:project .

<http://vocab.ceda.ac.uk/collection/cci/project/cciproject_waterVapour> a cci:project,
        skos:Concept ;
    skos:altLabel "WATERVAPOUR"@en ;
    skos:definition "Water vapour climate data record produced from satellite data as part of the European Space Agency (ESA) Climate Change Initiative (CCI)"@en ;
    skos:inScheme cci-scheme:project ;
    skos:prefLabel "water vapour"@en ;
    skos:scopeNote "Water vapour climate data record produced from satellite data as part of the European Space Agency (ESA) Climate Change Initiative (CCI)"@en ;
    skos:topConceptOf cci-scheme:project .

<http://vocab.ceda.ac.uk/collection/cci/sensor/sens_etmplus> a cci:sensor,
        skos:Concept ;
    rdfs:seeAlso <http://www.wmo-sat.info/oscar/instruments/view/136> ;
    skos:definition "Enhanced Thematic Mapper Plus"@en ;
    skos:inScheme cci-scheme:sensor ;
    skos:prefLabel "ETM+"@en ;
    skos:scopeNote "Enhanced Thematic Mapper Plus"@en ;
    skos:topConceptOf cci-scheme:sensor .

<http://vocab.ceda.ac.uk/collection/cci/sensor/sens_sarRadarSat2> a cci:sensor,
        skos:Concept ;
    rdfs:seeAlso <http://www.wmo-sat.info/oscar/instruments/view/445> ;
    skos:definition "Synthetic Aperture Radar (C-band)"@en ;
    skos:inScheme cci-scheme:sensor ;
    skos:prefLabel "SAR (RadarSat-2)"@en ;
    skos:scopeNote "Synthetic Aperture Radar (C-band)"@en ;
    skos:topConceptOf cci-scheme:sensor .

<http://vocab.ceda.ac.uk/collection/cci/sensor/sens_ssmiS> a cci:sensor,
        skos:Concept ;
    rdfs:seeAlso <http://www.wmo-sat.info/oscar/instruments/view/536> ;
    skos:altLabel "SSMIS"@en ;
    skos:definition "Special Sensor Microwave Imager Sounder"@en ;
    skos:inScheme cci-scheme:sensor ;
    skos:prefLabel "SSMI/S"@en ;
    skos:scopeNote "Special Sensor Microwave Imager Sounder"@en ;
    skos:topConceptOf cci-scheme:sensor .

<http://vocab.ceda.ac.uk/collection/cci/sensor/sens_unspecified> a cci:sensor,
        skos:Concept ;
    skos:definition "Unspecified sensor"@en ;
    skos:inScheme cci-scheme:sensor ;
    skos:prefLabel "Unspecified"@en ;
    skos:scopeNote "Unspecified sensor"@en ;
    skos:topConceptOf cci-scheme:sensor .

<http://vocab.ceda.ac.uk/collection/cci/platform/plat_FY-3E> a cci:platform,
        skos:Concept ;
    rdfs:seeAlso <http://www.wmo-sat.info/oscar/satellites/view/117> ;
    skos:altLabel "Feng-Yun - 3E"@en ;
    skos:broader <http://vocab.ceda.ac.uk/collection/cci/platformProg/plat_fengyun3> ;
    skos:definition "CMA Feng-Yun – 3E"@en ;
    skos:inScheme cci-scheme:platform ;
    skos:prefLabel "FY-3E"@en ;
    skos:scopeNote "CMA Feng-Yun – 3E"@en ;
    skos:topConceptOf cci-scheme:platform .

<http://vocab.ceda.ac.uk/collection/cci/platform/plat_FY-3G> a cci:platform,
        skos:Concept ;
    rdfs:seeAlso <http://www.wmo-sat.info/oscar/satellites/view/119> ;
    skos:altLabel "Feng-Yun - 3G"@en ;
    skos:broader <http://vocab.ceda.ac.uk/collection/cci/platformProg/plat_fengyun3> ;
    skos:definition "CMA Feng-Yun – 3G"@en ;
    skos:inScheme cci-scheme:platform ;
    skos:prefLabel "FY-3G"@en ;
    skos:scopeNote "CMA Feng-Yun – 3G"@en ;
    skos:topConceptOf cci-scheme:platform .

<http://vocab.ceda.ac.uk/collection/cci/platform/plat_alos-3> a cci:platform,
        skos:Concept ;
    rdfs:seeAlso <http://www.wmo-sat.info/oscar/satellites/view/7> ;
    skos:broader <http://vocab.ceda.ac.uk/collection/cci/platformProg/plat_alos_prog> ;
    skos:definition "JAXA Advanced Land Observation Satellite 3"@en ;
    skos:inScheme cci-scheme:platform ;
    skos:prefLabel "ALOS-3"@en ;
    skos:scopeNote "JAXA Advanced Land Observation Satellite 3"@en ;
    skos:topConceptOf cci-scheme:platform .

<http://vocab.ceda.ac.uk/collection/cci/platform/plat_dmsp_F01> a cci:platform,
        skos:Concept ;
    rdfs:seeAlso <http://www.wmo-sat.info/oscar/satellites/view/48> ;
    skos:broader <http://vocab.ceda.ac.uk/collection/cci/platformProg/plat_dmsp_5D1> ;
    skos:definition "US Defense Meteorological Satellite Program – F01"@en ;
    skos:inScheme cci-scheme:platform ;
    skos:prefLabel "DMSP-F01"@en ;
    skos:scopeNote "US Defense Meteorological Satellite Program – F01"@en ;
    skos:topConceptOf cci-scheme:platform .

<http://vocab.ceda.ac.uk/collection/cci/platform/plat_dmsp_F02> a cci:platform,
        skos:Concept ;
    rdfs:seeAlso <http://www.wmo-sat.info/oscar/satellites/view/49> ;
    skos:broader <http://vocab.ceda.ac.uk/collection/cci/platformProg/plat_dmsp_5D1> ;
    skos:definition "US Defense Meteorological Satellite Program – F02"@en ;
    skos:inScheme cci-scheme:platform ;
    skos:prefLabel "DMSP-F02"@en ;
    skos:scopeNote "US Defense Meteorological Satellite Program – F02"@en ;
    skos:topConceptOf cci-scheme:platform .

<http://vocab.ceda.ac.uk/collection/cci/platform/plat_dmsp_F03> a cci:platform,
        skos:Concept ;
    rdfs:seeAlso <http://www.wmo-sat.info/oscar/satellites/view/50> ;
    skos:broader <http://vocab.ceda.ac.uk/collection/cci/platformProg/plat_dmsp_5D1> ;
    skos:definition "US Defense Meteorological Satellite Program – F03"@en ;
    skos:inScheme cci-scheme:platform ;
    skos:prefLabel "DMSP-F03"@en ;
    skos:scopeNote "US Defense Meteorological Satellite Program – F03"@en ;
    skos:topConceptOf cci-scheme:platform .

<http://vocab.ceda.ac.uk/collection/cci/platform/plat_dmsp_F04> a cci:platform,
        skos:Concept ;
    rdfs:seeAlso <http://www.wmo-sat.info/oscar/satellites/view/51> ;
    skos:broader <http://vocab.ceda.ac.uk/collection/cci/platformProg/plat_dmsp_5D1> ;
    skos:definition "US Defense Meteorological Satellite Program – F04"@en ;
    skos:inScheme cci-scheme:platform ;
    skos:prefLabel "DMSP-F04"@en ;
    skos:scopeNote "US Defense Meteorological Satellite Program – F04"@en ;
    skos:topConceptOf cci-scheme:platform .

<http://vocab.ceda.ac.uk/collection/cci/platform/plat_dmsp_F05> a cci:platform,
        skos:Concept ;
    rdfs:seeAlso <http://www.wmo-sat.info/oscar/satellites/view/52> ;
    skos:broader <http://vocab.ceda.ac.uk/collection/cci/platformProg/plat_dmsp_5D1> ;
    skos:definition "US Defense Meteorological Satellite Program – F05"@en ;
    skos:inScheme cci-scheme:platform ;
    skos:prefLabel "DMSP-F05"@en ;
    skos:scopeNote "US Defense Meteorological Satellite Program – F05"@en ;
    skos:topConceptOf cci-scheme:platform .

<http://vocab.ceda.ac.uk/collection/cci/platform/plat_dmsp_F06> a cci:platform,
        skos:Concept ;
    rdfs:seeAlso <http://www.wmo-sat.info/oscar/satellites/view/53> ;
    skos:broader <http://vocab.ceda.ac.uk/collection/cci/platformProg/plat_dmsp_5D2> ;
    skos:definition "US Defense Meteorological Satellite Program – F06"@en ;
    skos:inScheme cci-scheme:platform ;
    skos:prefLabel "DMSP-F06"@en ;
    skos:scopeNote "US Defense Meteorological Satellite Program – F06"@en ;
    skos:topConceptOf cci-scheme:platform .

<http://vocab.ceda.ac.uk/collection/cci/platform/plat_dmsp_F07> a cci:platform,
        skos:Concept ;
    rdfs:seeAlso <http://www.wmo-sat.info/oscar/satellites/view/54> ;
    skos:broader <http://vocab.ceda.ac.uk/collection/cci/platformProg/plat_dmsp_5D2> ;
    skos:definition "US Defense Meteorological Satellite Program – F07"@en ;
    skos:inScheme cci-scheme:platform ;
    skos:prefLabel "DMSP-F07"@en ;
    skos:scopeNote "US Defense Meteorological Satellite Program – F07"@en ;
    skos:topConceptOf cci-scheme:platform .

<http://vocab.ceda.ac.uk/collection/cci/platform/plat_dmsp_F09> a cci:platform,
        skos:Concept ;
    rdfs:seeAlso <http://www.wmo-sat.info/oscar/satellites/view/56> ;
    skos:broader <http://vocab.ceda.ac.uk/collection/cci/platformProg/plat_dmsp_5D2> ;
    skos:definition "US Defense Meteorological Satellite Program – F09"@en ;
    skos:inScheme cci-scheme:platform ;
    skos:prefLabel "DMSP-F09"@en ;
    skos:scopeNote "US Defense Meteorological Satellite Program – F09"@en ;
    skos:topConceptOf cci-scheme:platform .

<http://vocab.ceda.ac.uk/collection/cci/platform/plat_dmsp_F16> a cci:platform,
        skos:Concept ;
    rdfs:seeAlso <http://www.wmo-sat.info/oscar/satellites/view/63> ;
    skos:broader <http://vocab.ceda.ac.uk/collection/cci/platformProg/plat_dmsp_5D3> ;
    skos:definition "US Defense Meteorological Satellite Program – F16"@en ;
    skos:inScheme cci-scheme:platform ;
    skos:prefLabel "DMSP-F16"@en ;
    skos:scopeNote "US Defense Meteorological Satellite Program – F16"@en ;
    skos:topConceptOf cci-scheme:platform .

<http://vocab.ceda.ac.uk/collection/cci/platform/plat_dmsp_F17> a cci:platform,
        skos:Concept ;
    rdfs:seeAlso <http://www.wmo-sat.info/oscar/satellites/view/64> ;
    skos:broader <http://vocab.ceda.ac.uk/collection/cci/platformProg/plat_dmsp_5D3> ;
    skos:definition "US Defense Meteorological Satellite Program – F17"@en ;
    skos:inScheme cci-scheme:platform ;
    skos:prefLabel "DMSP-F17"@en ;
    skos:scopeNote "US Defense Meteorological Satellite Program – F17"@en ;
    skos:topConceptOf cci-scheme:platform .

<http://vocab.ceda.ac.uk/collection/cci/platform/plat_dmsp_F18> a cci:platform,
        skos:Concept ;
    rdfs:seeAlso <http://www.wmo-sat.info/oscar/satellites/view/65> ;
    skos:broader <http://vocab.ceda.ac.uk/collection/cci/platformProg/plat_dmsp_5D3> ;
    skos:definition "US Defense Meteorological Satellite Program – F18"@en ;
    skos:inScheme cci-scheme:platform ;
    skos:prefLabel "DMSP-F18"@en ;
    skos:scopeNote "US Defense Meteorological Satellite Program – F18"@en ;
    skos:topConceptOf cci-scheme:platform .

<http://vocab.ceda.ac.uk/collection/cci/platform/plat_dmsp_F19> a cci:platform,
        skos:Concept ;
    rdfs:seeAlso <http://www.wmo-sat.info/oscar/satellites/view/66> ;
    skos:broader <http://vocab.ceda.ac.uk/collection/cci/platformProg/plat_dmsp_5D3> ;
    skos:definition "US Defense Meteorological Satellite Program – F19"@en ;
    skos:inScheme cci-scheme:platform ;
    skos:prefLabel "DMSP-F19"@en ;
    skos:scopeNote "US Defense Meteorological Satellite Program – F19"@en ;
    skos:topConceptOf cci-scheme:platform .

<http://vocab.ceda.ac.uk/collection/cci/platform/plat_dmsp_S20> a cci:platform,
        skos:Concept ;
    rdfs:seeAlso <http://www.wmo-sat.info/oscar/satellites/view/67> ;
    skos:broader <http://vocab.ceda.ac.uk/collection/cci/platformProg/plat_dmsp_5D3> ;
    skos:definition "US Defense Meteorological Satellite Program – S20"@en ;
    skos:inScheme cci-scheme:platform ;
    skos:prefLabel "DMSP-S20"@en ;
    skos:scopeNote "US Defense Meteorological Satellite Program – S20"@en ;
    skos:topConceptOf cci-scheme:platform .

<http://vocab.ceda.ac.uk/collection/cci/platform/plat_geosat> a cci:platform,
        skos:Concept ;
    rdfs:seeAlso <http://www.wmo-sat.info/oscar/satellites/view/133> ;
    skos:broader <http://vocab.ceda.ac.uk/collection/cci/platformProg/plat_geodetic> ;
    skos:definition "NASA GEOSat"@en ;
    skos:inScheme cci-scheme:platform ;
    skos:prefLabel "GEOSat"@en ;
    skos:scopeNote "NASA GEOSat"@en ;
    skos:topConceptOf cci-scheme:platform .

<http://vocab.ceda.ac.uk/collection/cci/platform/plat_goes_01> a cci:platform,
        skos:Concept ;
    rdfs:seeAlso <http://www.wmo-sat.info/oscar/satellites/view/137> ;
    skos:broader <http://vocab.ceda.ac.uk/collection/cci/platformProg/plat_goes_1st> ;
    skos:definition "NASA Geostationary Operational Environmental Satellite – 01"@en ;
    skos:inScheme cci-scheme:platform ;
    skos:prefLabel "GOES-1"@en ;
    skos:scopeNote "NASA Geostationary Operational Environmental Satellite – 01"@en ;
    skos:topConceptOf cci-scheme:platform .

<http://vocab.ceda.ac.uk/collection/cci/platform/plat_goes_02> a cci:platform,
        skos:Concept ;
    rdfs:seeAlso <http://www.wmo-sat.info/oscar/satellites/view/138> ;
    skos:broader <http://vocab.ceda.ac.uk/collection/cci/platformProg/plat_goes_1st> ;
    skos:definition "NASA Geostationary Operational Environmental Satellite – 02"@en ;
    skos:inScheme cci-scheme:platform ;
    skos:prefLabel "GOES-2"@en ;
    skos:scopeNote "NASA Geostationary Operational Environmental Satellite – 02"@en ;
    skos:topConceptOf cci-scheme:platform .

<http://vocab.ceda.ac.uk/collection/cci/platform/plat_goes_03> a cci:platform,
        skos:Concept ;
    rdfs:seeAlso <http://www.wmo-sat.info/oscar/satellites/view/139> ;
    skos:broader <http://vocab.ceda.ac.uk/collection/cci/platformProg/plat_goes_1st> ;
    skos:definition "NASA Geostationary Operational Environmental Satellite – 03"@en ;
    skos:inScheme cci-scheme:platform ;
    skos:prefLabel "GOES-3"@en ;
    skos:scopeNote "NASA Geostationary Operational Environmental Satellite – 03"@en ;
    skos:topConceptOf cci-scheme:platform .

<http://vocab.ceda.ac.uk/collection/cci/platform/plat_goes_04> a cci:platform,
        skos:Concept ;
    rdfs:seeAlso <http://www.wmo-sat.info/oscar/satellites/view/140> ;
    skos:broader <http://vocab.ceda.ac.uk/collection/cci/platformProg/plat_goes_1st> ;
    skos:definition "NASA Geostationary Operational Environmental Satellite – 04"@en ;
    skos:inScheme cci-scheme:platform ;
    skos:prefLabel "GOES-4"@en ;
    skos:scopeNote "NASA Geostationary Operational Environmental Satellite – 04"@en ;
    skos:topConceptOf cci-scheme:platform .

<http://vocab.ceda.ac.uk/collection/cci/platform/plat_goes_05> a cci:platform,
        skos:Concept ;
    rdfs:seeAlso <http://www.wmo-sat.info/oscar/satellites/view/141> ;
    skos:broader <http://vocab.ceda.ac.uk/collection/cci/platformProg/plat_goes_1st> ;
    skos:definition "NASA Geostationary Operational Environmental Satellite – 05"@en ;
    skos:inScheme cci-scheme:platform ;
    skos:prefLabel "GOES-5"@en ;
    skos:scopeNote "NASA Geostationary Operational Environmental Satellite – 05"@en ;
    skos:topConceptOf cci-scheme:platform .

<http://vocab.ceda.ac.uk/collection/cci/platform/plat_goes_06> a cci:platform,
        skos:Concept ;
    rdfs:seeAlso <http://www.wmo-sat.info/oscar/satellites/view/142> ;
    skos:broader <http://vocab.ceda.ac.uk/collection/cci/platformProg/plat_goes_1st> ;
    skos:definition "NASA Geostationary Operational Environmental Satellite – 06"@en ;
    skos:inScheme cci-scheme:platform ;
    skos:prefLabel "GOES-6"@en ;
    skos:scopeNote "NASA Geostationary Operational Environmental Satellite – 06"@en ;
    skos:topConceptOf cci-scheme:platform .

<http://vocab.ceda.ac.uk/collection/cci/platform/plat_goes_07> a cci:platform,
        skos:Concept ;
    rdfs:seeAlso <http://www.wmo-sat.info/oscar/satellites/view/143> ;
    skos:broader <http://vocab.ceda.ac.uk/collection/cci/platformProg/plat_goes_1st> ;
    skos:definition "NASA Geostationary Operational Environmental Satellite – 07"@en ;
    skos:inScheme cci-scheme:platform ;
    skos:prefLabel "GOES-7"@en ;
    skos:scopeNote "NASA Geostationary Operational Environmental Satellite – 07"@en ;
    skos:topConceptOf cci-scheme:platform .

<http://vocab.ceda.ac.uk/collection/cci/platform/plat_goes_T> a cci:platform,
        skos:Concept ;
    rdfs:seeAlso <http://www.wmo-sat.info/oscar/satellites/view/665> ;
    skos:broader <http://vocab.ceda.ac.uk/collection/cci/platformProg/plat_goes_3rd> ;
    skos:definition "NASA Geostationary Operational Environmental Satellite – T"@en ;
    skos:inScheme cci-scheme:platform ;
    skos:prefLabel "GOES-T"@en ;
    skos:scopeNote "NASA Geostationary Operational Environmental Satellite – T"@en ;
    skos:topConceptOf cci-scheme:platform .

<http://vocab.ceda.ac.uk/collection/cci/platform/plat_goes_U> a cci:platform,
        skos:Concept ;
    rdfs:seeAlso <http://www.wmo-sat.info/oscar/satellites/view/666> ;
    skos:broader <http://vocab.ceda.ac.uk/collection/cci/platformProg/plat_goes_3rd> ;
    skos:definition "NASA Geostationary Operational Environmental Satellite – U"@en ;
    skos:inScheme cci-scheme:platform ;
    skos:prefLabel "GOES-U"@en ;
    skos:scopeNote "NASA Geostationary Operational Environmental Satellite – U"@en ;
    skos:topConceptOf cci-scheme:platform .

<http://vocab.ceda.ac.uk/collection/cci/platform/plat_hrws_sar> a cci:platform,
        skos:Concept ;
    rdfs:seeAlso <http://www.wmo-sat.info/oscar/satellites/view/638> ;
    skos:broader <http://vocab.ceda.ac.uk/collection/cci/platformProg/plat_terraSAR> ;
    skos:definition "DLR HRWS-SAR"@en ;
    skos:inScheme cci-scheme:platform ;
    skos:prefLabel "HRWS-SAR"@en ;
    skos:scopeNote "DLR HRWS-SAR"@en ;
    skos:topConceptOf cci-scheme:platform .

<http://vocab.ceda.ac.uk/collection/cci/platform/plat_icesat-2> a cci:platform,
        skos:Concept ;
    rdfs:seeAlso <http://www.wmo-sat.info/oscar/satellites/view/178> ;
    skos:broader <http://vocab.ceda.ac.uk/collection/cci/platformProg/plat_icesat_prog> ;
    skos:definition "NASA Ice, Cloud and land Elevation Satellite"@en ;
    skos:inScheme cci-scheme:platform ;
    skos:prefLabel "ICESat-2"@en ;
    skos:scopeNote "NASA Ice, Cloud and land Elevation Satellite"@en ;
    skos:topConceptOf cci-scheme:platform .

<http://vocab.ceda.ac.uk/collection/cci/platform/plat_landsat_6> a cci:platform,
        skos:Concept ;
    rdfs:seeAlso <http://www.wmo-sat.info/oscar/satellites/view/224> ;
    skos:broader <http://vocab.ceda.ac.uk/collection/cci/platformProg/plat_landsat> ;
    skos:definition "NASA Landsat"@en ;
    skos:inScheme cci-scheme:platform ;
    skos:prefLabel "Landsat-6"@en ;
    skos:scopeNote "NASA Landsat"@en ;
    skos:topConceptOf cci-scheme:platform .

<http://vocab.ceda.ac.uk/collection/cci/platform/plat_nimbus1> a cci:platform,
        skos:Concept ;
    rdfs:seeAlso <http://www.wmo-sat.info/oscar/satellites/view/315> ;
    skos:broader <http://vocab.ceda.ac.uk/collection/cci/platformProg/plat_nimbus> ;
    skos:definition "NASA Research-and-development satellite 1"@en ;
    skos:inScheme cci-scheme:platform ;
    skos:prefLabel "Nimbus-1"@en ;
    skos:scopeNote "NASA Research-and-development satellite 1"@en ;
    skos:topConceptOf cci-scheme:platform .

<http://vocab.ceda.ac.uk/collection/cci/platform/plat_nimbus2> a cci:platform,
        skos:Concept ;
    rdfs:seeAlso <http://www.wmo-sat.info/oscar/satellites/view/316> ;
    skos:broader <http://vocab.ceda.ac.uk/collection/cci/platformProg/plat_nimbus> ;
    skos:definition "NASA Research-and-development satellite 2"@en ;
    skos:inScheme cci-scheme:platform ;
    skos:prefLabel "Nimbus-2"@en ;
    skos:scopeNote "NASA Research-and-development satellite 2"@en ;
    skos:topConceptOf cci-scheme:platform .

<http://vocab.ceda.ac.uk/collection/cci/platform/plat_nimbus3> a cci:platform,
        skos:Concept ;
    rdfs:seeAlso <http://www.wmo-sat.info/oscar/satellites/view/317> ;
    skos:broader <http://vocab.ceda.ac.uk/collection/cci/platformProg/plat_nimbus> ;
    skos:definition "NASA Research-and-development satellite 3"@en ;
    skos:inScheme cci-scheme:platform ;
    skos:prefLabel "Nimbus-3"@en ;
    skos:scopeNote "NASA Research-and-development satellite 3"@en ;
    skos:topConceptOf cci-scheme:platform .

<http://vocab.ceda.ac.uk/collection/cci/platform/plat_nimbus4> a cci:platform,
        skos:Concept ;
    rdfs:seeAlso <http://www.wmo-sat.info/oscar/satellites/view/318> ;
    skos:broader <http://vocab.ceda.ac.uk/collection/cci/platformProg/plat_nimbus> ;
    skos:definition "NASA Research-and-development satellite 4"@en ;
    skos:inScheme cci-scheme:platform ;
    skos:prefLabel "Nimbus-4"@en ;
    skos:scopeNote "NASA Research-and-development satellite 4"@en ;
    skos:topConceptOf cci-scheme:platform .

<http://vocab.ceda.ac.uk/collection/cci/platform/plat_noaa_1> a cci:platform,
        skos:Concept ;
    rdfs:seeAlso <http://www.wmo-sat.info/oscar/satellites/view/323> ;
    skos:broader <http://vocab.ceda.ac.uk/collection/cci/platformProg/plat_noaa_3rd> ;
    skos:definition "NASA NOAA Environmental satellite 1"@en ;
    skos:inScheme cci-scheme:platform ;
    skos:prefLabel "NOAA-1"@en ;
    skos:scopeNote "NASA NOAA Environmental satellite 1"@en ;
    skos:topConceptOf cci-scheme:platform .

<http://vocab.ceda.ac.uk/collection/cci/platform/plat_noaa_2> a cci:platform,
        skos:Concept ;
    rdfs:seeAlso <http://www.wmo-sat.info/oscar/satellites/view/324> ;
    skos:broader <http://vocab.ceda.ac.uk/collection/cci/platformProg/plat_noaa_3rd> ;
    skos:definition "NASA NOAA Environmental satellite 2"@en ;
    skos:inScheme cci-scheme:platform ;
    skos:prefLabel "NOAA-2"@en ;
    skos:scopeNote "NASA NOAA Environmental satellite 2"@en ;
    skos:topConceptOf cci-scheme:platform .

<http://vocab.ceda.ac.uk/collection/cci/platform/plat_noaa_3> a cci:platform,
        skos:Concept ;
    rdfs:seeAlso <http://www.wmo-sat.info/oscar/satellites/view/325> ;
    skos:broader <http://vocab.ceda.ac.uk/collection/cci/platformProg/plat_noaa_3rd> ;
    skos:definition "NASA NOAA Environmental satellite 3"@en ;
    skos:inScheme cci-scheme:platform ;
    skos:prefLabel "NOAA-3"@en ;
    skos:scopeNote "NASA NOAA Environmental satellite 3"@en ;
    skos:topConceptOf cci-scheme:platform .

<http://vocab.ceda.ac.uk/collection/cci/platform/plat_noaa_4> a cci:platform,
        skos:Concept ;
    rdfs:seeAlso <http://www.wmo-sat.info/oscar/satellites/view/326> ;
    skos:broader <http://vocab.ceda.ac.uk/collection/cci/platformProg/plat_noaa_3rd> ;
    skos:definition "NASA NOAA Environmental satellite 4"@en ;
    skos:inScheme cci-scheme:platform ;
    skos:prefLabel "NOAA-4"@en ;
    skos:scopeNote "NASA NOAA Environmental satellite 4"@en ;
    skos:topConceptOf cci-scheme:platform .

<http://vocab.ceda.ac.uk/collection/cci/platform/plat_noaa_5> a cci:platform,
        skos:Concept ;
    rdfs:seeAlso <http://www.wmo-sat.info/oscar/satellites/view/327> ;
    skos:broader <http://vocab.ceda.ac.uk/collection/cci/platformProg/plat_noaa_3rd> ;
    skos:definition "NASA NOAA Environmental satellite 5"@en ;
    skos:inScheme cci-scheme:platform ;
    skos:prefLabel "NOAA-5"@en ;
    skos:scopeNote "NASA NOAA Environmental satellite 5"@en ;
    skos:topConceptOf cci-scheme:platform .

<http://vocab.ceda.ac.uk/collection/cci/platform/plat_radarsat2> a cci:platform,
        skos:Concept ;
    rdfs:seeAlso <https://www.wmo-sat.info/oscar/satellites/view/367> ;
    skos:altLabel "RADARSAT-2"@en ;
    skos:broader <http://vocab.ceda.ac.uk/collection/cci/platformProg/plat_radarsat_prog> ;
    skos:definition "RadarSat-2"@en ;
    skos:inScheme cci-scheme:platform ;
    skos:prefLabel "RadarSat-2"@en ;
    skos:scopeNote "RadarSat-2"@en ;
    skos:topConceptOf cci-scheme:platform .

<http://vocab.ceda.ac.uk/collection/cci/platform/plat_spot1> a cci:platform,
        skos:Concept ;
    rdfs:seeAlso <http://www.wmo-sat.info/oscar/satellites/view/412> ;
    skos:broader <http://vocab.ceda.ac.uk/collection/cci/platformProg/plat_spot> ;
    skos:definition "CNES Satellite Pour l'Observation de la Terre 1"@en ;
    skos:inScheme cci-scheme:platform ;
    skos:prefLabel "SPOT-1"@en ;
    skos:scopeNote "CNES Satellite Pour l'Observation de la Terre 1"@en ;
    skos:topConceptOf cci-scheme:platform .

<http://vocab.ceda.ac.uk/collection/cci/platform/plat_spot2> a cci:platform,
        skos:Concept ;
    rdfs:seeAlso <http://www.wmo-sat.info/oscar/satellites/view/413> ;
    skos:broader <http://vocab.ceda.ac.uk/collection/cci/platformProg/plat_spot> ;
    skos:definition "CNES Satellite Pour l'Observation de la Terre 2"@en ;
    skos:inScheme cci-scheme:platform ;
    skos:prefLabel "SPOT-2"@en ;
    skos:scopeNote "CNES Satellite Pour l'Observation de la Terre 2"@en ;
    skos:topConceptOf cci-scheme:platform .

<http://vocab.ceda.ac.uk/collection/cci/platform/plat_spot3> a cci:platform,
        skos:Concept ;
    rdfs:seeAlso <http://www.wmo-sat.info/oscar/satellites/view/414> ;
    skos:broader <http://vocab.ceda.ac.uk/collection/cci/platformProg/plat_spot> ;
    skos:definition "CNES Satellite Pour l'Observation de la Terre 3"@en ;
    skos:inScheme cci-scheme:platform ;
    skos:prefLabel "SPOT-3"@en ;
    skos:scopeNote "CNES Satellite Pour l'Observation de la Terre 3"@en ;
    skos:topConceptOf cci-scheme:platform .

<http://vocab.ceda.ac.uk/collection/cci/platform/plat_spot6> a cci:platform,
        skos:Concept ;
    rdfs:seeAlso <https://www.wmo-sat.info/oscar/satellites/view/417> ;
    skos:broader <http://vocab.ceda.ac.uk/collection/cci/platformProg/plat_spot_prog_follow> ;
    skos:definition "CNES Satellite Pour l'Observation de la Terre 6"@en ;
    skos:inScheme cci-scheme:platform ;
    skos:prefLabel "SPOT-6"@en ;
    skos:scopeNote "CNES Satellite Pour l'Observation de la Terre 6"@en ;
    skos:topConceptOf cci-scheme:platform .

<http://vocab.ceda.ac.uk/collection/cci/platform/plat_spot7> a cci:platform,
        skos:Concept ;
    rdfs:seeAlso <https://www.wmo-sat.info/oscar/satellites/view/418> ;
    skos:broader <http://vocab.ceda.ac.uk/collection/cci/platformProg/plat_spot_prog_follow> ;
    skos:definition "CNES Satellite Pour l'Observation de la Terre 7"@en ;
    skos:inScheme cci-scheme:platform ;
    skos:prefLabel "SPOT-7"@en ;
    skos:scopeNote "CNES Satellite Pour l'Observation de la Terre 7"@en ;
    skos:topConceptOf cci-scheme:platform .

<http://vocab.ceda.ac.uk/collection/cci/platformProg/plat_coriolis_prog> a cci:platformProg,
        skos:Concept ;
    rdfs:seeAlso <http://www.wmo-sat.info/oscar/satelliteprogrammes/view/25> ;
    skos:definition "DoD NASA"@en ;
    skos:inScheme cci-scheme:platformProg ;
    skos:narrower <http://vocab.ceda.ac.uk/collection/cci/platform/plat_coriolis> ;
    skos:prefLabel "Coriolis"@en ;
    skos:scopeNote "DoD NASA"@en ;
    skos:topConceptOf cci-scheme:platformProg .

<http://vocab.ceda.ac.uk/collection/cci/platformProg/plat_cryosat_prog> a cci:platformProg,
        skos:Concept ;
    rdfs:seeAlso <https://www.wmo-sat.info/oscar/satelliteprogrammes/view/29> ;
    skos:definition "ESA CryoSat Programme"@en ;
    skos:inScheme cci-scheme:platformProg ;
    skos:narrower <http://vocab.ceda.ac.uk/collection/cci/platform/plat_cryosat2> ;
    skos:prefLabel "CryoSat Programme"@en ;
    skos:scopeNote "ESA CryoSat Programme"@en ;
    skos:topConceptOf cci-scheme:platformProg .

<http://vocab.ceda.ac.uk/collection/cci/platformProg/plat_envisat_prog> a cci:platformProg,
        skos:Concept ;
    rdfs:seeAlso <http://www.wmo-sat.info/oscar/satelliteprogrammes/view/42> ;
    skos:definition "ESA"@en ;
    skos:inScheme cci-scheme:platformProg ;
    skos:narrower <http://vocab.ceda.ac.uk/collection/cci/platform/plat_envisat> ;
    skos:prefLabel "Environmental Satellite"@en ;
    skos:scopeNote "ESA"@en ;
    skos:topConceptOf cci-scheme:platformProg .

<http://vocab.ceda.ac.uk/collection/cci/platformProg/plat_gpm_prog> a cci:platformProg,
        skos:Concept ;
    rdfs:seeAlso <https://www.wmo-sat.info/oscar/satelliteprogrammes/view/gpm> ;
    skos:definition "Global Precipitation Measurement mission Programme"@en ;
    skos:inScheme cci-scheme:platformProg ;
    skos:narrower <http://vocab.ceda.ac.uk/collection/cci/platform/plat_gpm> ;
    skos:prefLabel "Global Precipitation Measurement mission"@en ;
    skos:scopeNote "Global Precipitation Measurement mission Programme"@en ;
    skos:topConceptOf cci-scheme:platformProg .

<http://vocab.ceda.ac.uk/collection/cci/platformProg/plat_grace_prog> a cci:platformProg,
        skos:Concept ;
    rdfs:seeAlso <https://www.wmo-sat.info/oscar/satelliteprogrammes/view/68> ;
    skos:definition "NASA Gravity Recovery and Climate Experiment Programme"@en ;
    skos:inScheme cci-scheme:platformProg ;
    skos:narrower <http://vocab.ceda.ac.uk/collection/cci/platform/plat_grace> ;
    skos:prefLabel "GRACE Programme"@en ;
    skos:scopeNote "NASA Gravity Recovery and Climate Experiment Programme"@en ;
    skos:topConceptOf cci-scheme:platformProg .

<http://vocab.ceda.ac.uk/collection/cci/platformProg/plat_jpss_prog> a cci:platformProg,
        skos:Concept ;
    rdfs:seeAlso <https://www.wmo-sat.info/oscar/satelliteprogrammes/view/87> ;
    skos:altLabel "JPSS"@en ;
    skos:definition "NASA/NOAA Joint Polar Satellite System"@en ;
    skos:inScheme cci-scheme:platformProg ;
    skos:narrower <http://vocab.ceda.ac.uk/collection/cci/platform/plat_snpp> ;
    skos:prefLabel "Joint Polar Satellite System"@en ;
    skos:scopeNote "NASA/NOAA Joint Polar Satellite System"@en ;
    skos:topConceptOf cci-scheme:platformProg .

<http://vocab.ceda.ac.uk/collection/cci/platformProg/plat_landsat_dcm> a cci:platformProg,
        skos:Concept ;
    rdfs:seeAlso <http://www.wmo-sat.info/oscar/satelliteprogrammes/view/94> ;
    skos:definition "NASA/USGS Satellite imagery of Earth"@en ;
    skos:inScheme cci-scheme:platformProg ;
    skos:narrower <http://vocab.ceda.ac.uk/collection/cci/platform/plat_landsat_8> ;
    skos:prefLabel "Landsat Data Continuity Mission"@en ;
    skos:scopeNote "NASA/USGS Satellite imagery of Earth"@en ;
    skos:topConceptOf cci-scheme:platformProg .

<http://vocab.ceda.ac.uk/collection/cci/platformProg/plat_oco_prog> a cci:platformProg,
        skos:Concept ;
    rdfs:seeAlso <https://www.wmo-sat.info/oscar/satelliteprogrammes/view/115> ;
    skos:definition "NASA Orbiting Carbon Observatory programme"@en ;
    skos:inScheme cci-scheme:platformProg ;
    skos:narrower <http://vocab.ceda.ac.uk/collection/cci/platform/plat_oco2> ;
    skos:prefLabel "Orbiting Carbon Observatory"@en ;
    skos:scopeNote "NASA Orbiting Carbon Observatory programme"@en ;
    skos:topConceptOf cci-scheme:platformProg .

<http://vocab.ceda.ac.uk/collection/cci/platformProg/plat_odin_prog> a cci:platformProg,
        skos:Concept ;
    rdfs:seeAlso <http://www.wmo-sat.info/oscar/satelliteprogrammes/view/117> ;
    skos:inScheme cci-scheme:platformProg ;
    skos:narrower <http://vocab.ceda.ac.uk/collection/cci/platform/plat_odin> ;
    skos:prefLabel "Odin"@en ;
    skos:topConceptOf cci-scheme:platformProg .

<http://vocab.ceda.ac.uk/collection/cci/platformProg/plat_orbview2_prog> a cci:platformProg,
        skos:Concept ;
    rdfs:seeAlso <http://www.wmo-sat.info/oscar/satelliteprogrammes/view/144> ;
    skos:altLabel "SeaStar"@en ;
    skos:definition "GeoEye OrbView-2 (former: SeaStar)"@en ;
    skos:inScheme cci-scheme:platformProg ;
    skos:narrower <http://vocab.ceda.ac.uk/collection/cci/platform/plat_orbview2> ;
    skos:prefLabel "Orbview-2"@en ;
    skos:scopeNote "GeoEye OrbView-2 (former: SeaStar)"@en ;
    skos:topConceptOf cci-scheme:platformProg .

<http://vocab.ceda.ac.uk/collection/cci/platformProg/plat_parasol_prog> a cci:platformProg,
        skos:Concept ;
    rdfs:seeAlso <http://www.wmo-sat.info/oscar/satelliteprogrammes/view/121> ;
    skos:definition "CNES Polarisation et Anisotropie des Réflectances au sommet de l'Atmosphère couplées avec un Satellite d'Observation emportant un Lidar"@en ;
    skos:inScheme cci-scheme:platformProg ;
    skos:narrower <http://vocab.ceda.ac.uk/collection/cci/platform/plat_parasol> ;
    skos:prefLabel "PARASOL"@en ;
    skos:scopeNote "CNES Polarisation et Anisotropie des Réflectances au sommet de l'Atmosphère couplées avec un Satellite d'Observation emportant un Lidar"@en ;
    skos:topConceptOf cci-scheme:platformProg .

<http://vocab.ceda.ac.uk/collection/cci/platformProg/plat_proba_prog> a cci:platformProg,
        skos:Concept ;
    rdfs:seeAlso <https://www.wmo-sat.info/oscar/satelliteprogrammes/view/127> ;
    skos:altLabel "PROBA"@en ;
    skos:definition "Project for On-Board Autonomy (PROBA) programme"@en ;
    skos:inScheme cci-scheme:platformProg ;
    skos:narrower <http://vocab.ceda.ac.uk/collection/cci/platform/plat_probaV> ;
    skos:prefLabel "Project for On-Board Autonomy"@en ;
    skos:scopeNote "Project for On-Board Autonomy (PROBA) programme"@en ;
    skos:topConceptOf cci-scheme:platformProg .

<http://vocab.ceda.ac.uk/collection/cci/platformProg/plat_radarsat_prog> a cci:platformProg,
        skos:Concept ;
    rdfs:seeAlso <https://www.wmo-sat.info/oscar/satelliteprogrammes/view/129> ;
    skos:definition "RadarSat Programme"@en ;
    skos:inScheme cci-scheme:platformProg ;
    skos:narrower <http://vocab.ceda.ac.uk/collection/cci/platform/plat_radarsat2> ;
    skos:prefLabel "RadarSat"@en ;
    skos:scopeNote "RadarSat Programme"@en ;
    skos:topConceptOf cci-scheme:platformProg .

<http://vocab.ceda.ac.uk/collection/cci/platformProg/plat_s5p_prog> a cci:platformProg,
        skos:Concept ;
    rdfs:seeAlso <https://www.wmo-sat.info/oscar/satelliteprogrammes/view/148> ;
    skos:definition "ESA Sentinel-5 precursor programme"@en ;
    skos:inScheme cci-scheme:platformProg ;
    skos:narrower <http://vocab.ceda.ac.uk/collection/cci/platform/plat_sentinel5p> ;
    skos:prefLabel "Sentinel-5 precursor"@en ;
    skos:scopeNote "ESA Sentinel-5 precursor programme"@en ;
    skos:topConceptOf cci-scheme:platformProg .

<http://vocab.ceda.ac.uk/collection/cci/platformProg/plat_sac_prog> a cci:platformProg,
        skos:Concept ;
    rdfs:seeAlso <https://www.wmo-sat.info/oscar/satelliteprogrammes/view/137> ;
    skos:altLabel "SAC"@en ;
    skos:definition "Satélite de Aplicaciones Cientificas"@en ;
    skos:inScheme cci-scheme:platformProg ;
    skos:narrower <http://vocab.ceda.ac.uk/collection/cci/platform/plat_sac_d> ;
    skos:prefLabel "Satélite de Aplicaciones Cientificas"@en ;
    skos:scopeNote "Satélite de Aplicaciones Cientificas"@en ;
    skos:topConceptOf cci-scheme:platformProg .

<http://vocab.ceda.ac.uk/collection/cci/platformProg/plat_saral_prog> a cci:platformProg,
        skos:Concept ;
    rdfs:seeAlso <https://www.wmo-sat.info/oscar/satelliteprogrammes/view/139> ;
    skos:definition "CNES Satellite with ARgos and AltiKa"@en ;
    skos:inScheme cci-scheme:platformProg ;
    skos:narrower <http://vocab.ceda.ac.uk/collection/cci/platform/plat_saral> ;
    skos:prefLabel "SARAL Programme"@en ;
    skos:scopeNote "CNES Satellite with ARgos and AltiKa"@en ;
    skos:topConceptOf cci-scheme:platformProg .

<http://vocab.ceda.ac.uk/collection/cci/platformProg/plat_scisat_prog> a cci:platformProg,
        skos:Concept ;
    rdfs:seeAlso <http://www.wmo-sat.info/oscar/satelliteprogrammes/view/141> ;
    skos:definition "CSA NASA Science Satellite / Atmospheric Chemistry Experiment"@en ;
    skos:inScheme cci-scheme:platformProg ;
    skos:narrower <http://vocab.ceda.ac.uk/collection/cci/platform/plat_scisat> ;
    skos:prefLabel "SCISAT"@en ;
    skos:scopeNote "CSA NASA Science Satellite / Atmospheric Chemistry Experiment"@en ;
    skos:topConceptOf cci-scheme:platformProg .

<http://vocab.ceda.ac.uk/collection/cci/platformProg/plat_smap_prog> a cci:platformProg,
        skos:Concept ;
    rdfs:seeAlso <https://www.wmo-sat.info/oscar/satelliteprogrammes/view/151> ;
    skos:definition "Soil Moisture Active – Passive"@en ;
    skos:inScheme cci-scheme:platformProg ;
    skos:narrower <http://vocab.ceda.ac.uk/collection/cci/platform/plat_smap> ;
    skos:prefLabel "SMAP"@en ;
    skos:scopeNote "Soil Moisture Active – Passive"@en ;
    skos:topConceptOf cci-scheme:platformProg .

<http://vocab.ceda.ac.uk/collection/cci/platformProg/plat_smos_prog> a cci:platformProg,
        skos:Concept ;
    rdfs:seeAlso <https://www.wmo-sat.info/oscar/satelliteprogrammes/view/153> ;
    skos:definition "ESA Soil Moisture and Ocean Salinity"@en ;
    skos:inScheme cci-scheme:platformProg ;
    skos:narrower <http://vocab.ceda.ac.uk/collection/cci/platform/plat_smos> ;
    skos:prefLabel "Soil Moisture and Ocean Salinity"@en ;
    skos:scopeNote "ESA Soil Moisture and Ocean Salinity"@en ;
    skos:topConceptOf cci-scheme:platformProg .

<http://vocab.ceda.ac.uk/collection/cci/platformProg/plat_topexPoseidon_prog> a cci:platformProg,
        skos:Concept ;
    rdfs:seeAlso <http://www.wmo-sat.info/oscar/satelliteprogrammes/view/169> ;
    skos:definition "NASA CNES Topography Experiment + Poseidon"@en ;
    skos:inScheme cci-scheme:platformProg ;
    skos:narrower <http://vocab.ceda.ac.uk/collection/cci/platform/plat_topexPoseidon> ;
    skos:prefLabel "Topex/Poseidon"@en ;
    skos:scopeNote "NASA CNES Topography Experiment + Poseidon"@en ;
    skos:topConceptOf cci-scheme:platformProg .

<http://vocab.ceda.ac.uk/collection/cci/platformProg/plat_trmm_prog> a cci:platformProg,
        skos:Concept ;
    rdfs:seeAlso <http://www.wmo-sat.info/oscar/satelliteprogrammes/view/171> ;
    skos:definition "NASA JAXA Tropical Rainfall Measuring Mission"@en ;
    skos:inScheme cci-scheme:platformProg ;
    skos:narrower <http://vocab.ceda.ac.uk/collection/cci/platform/plat_trmm> ;
    skos:prefLabel "TRMM"@en ;
    skos:scopeNote "NASA JAXA Tropical Rainfall Measuring Mission"@en ;
    skos:topConceptOf cci-scheme:platformProg .

<http://vocab.ceda.ac.uk/collection/cci/procLev/proc_level1A> a cci:procLev,
        skos:Concept ;
    rdfs:seeAlso <https://www.ghrsst.org/> ;
    skos:altLabel "L1A"@en ;
    skos:broader <http://vocab.ceda.ac.uk/collection/cci/procLev/proc_level1> ;
    skos:definition "Reconstructed unprocessed instrument data at full resolution, time referenced, and annotated with ancillary information, including radiometric and geometric calibration coefficients and georeferencing parameters, computed and appended, but not applied, to L0 data."@en ;
    skos:inScheme cci-scheme:procLev ;
    skos:prefLabel "Level 1A"@en ;
    skos:scopeNote "Reconstructed unprocessed instrument data at full resolution, time referenced, and annotated with ancillary information, including radiometric and geometric calibration coefficients and georeferencing parameters, computed and appended, but not applied, to L0 data."@en ;
    skos:topConceptOf cci-scheme:procLev .

<http://vocab.ceda.ac.uk/collection/cci/procLev/proc_level1B> a cci:procLev,
        skos:Concept ;
    rdfs:seeAlso <https://www.ghrsst.org/> ;
    skos:altLabel "L1B"@en ;
    skos:broader <http://vocab.ceda.ac.uk/collection/cci/procLev/proc_level1> ;
    skos:definition "Level 1A data that have been processed to sensor units."@en ;
    skos:inScheme cci-scheme:procLev ;
    skos:prefLabel "Level 1B"@en ;
    skos:scopeNote "Level 1A data that have been processed to sensor units."@en ;
    skos:topConceptOf cci-scheme:procLev .

<http://vocab.ceda.ac.uk/collection/cci/procLev/proc_level1C> a cci:procLev,
        skos:Concept ;
    skos:altLabel "L1C"@en ;
    skos:broader <http://vocab.ceda.ac.uk/collection/cci/procLev/proc_level1> ;
    skos:definition "Level 1b data that have been further processed, e.g. by correcting radiances or by mapping onto a spatial grid, prior to deriving geophysical variables from the data."@en ;
    skos:inScheme cci-scheme:procLev ;
    skos:prefLabel "Level 1C"@en ;
    skos:scopeNote "Level 1b data that have been further processed, e.g. by correcting radiances or by mapping onto a spatial grid, prior to deriving geophysical variables from the data."@en ;
    skos:topConceptOf cci-scheme:procLev .

<http://vocab.ceda.ac.uk/collection/cci/procLev/proc_level2> a cci:procLev,
        skos:Concept ;
    rdfs:seeAlso <http://wiki.ieee-earth.org/@api/deki/files/7/=Handbook_0802.pdf> ;
    skos:altLabel "L2"@en ;
    skos:definition "Retrieved environmental variables at the same resolution and location as the level 1 source"@en ;
    skos:inScheme cci-scheme:procLev ;
    skos:narrower <http://vocab.ceda.ac.uk/collection/cci/procLev/proc_level2P> ;
    skos:prefLabel "Level 2"@en ;
    skos:scopeNote "Retrieved environmental variables at the same resolution and location as the level 1 source"@en ;
    skos:topConceptOf cci-scheme:procLev .

<http://vocab.ceda.ac.uk/collection/cci/procLev/proc_level2P> a cci:procLev,
        skos:Concept ;
    rdfs:seeAlso <https://www.ghrsst.org/> ;
    skos:altLabel "L2P"@en ;
    skos:broader <http://vocab.ceda.ac.uk/collection/cci/procLev/proc_level2> ;
    skos:definition "Geophysical variables derived from Level 1 source data at the same resolution and location as the level 1 data, typically in a satellite projection with geographic information. These data form the fundamental basis for higher level CCI products."@en ;
    skos:inScheme cci-scheme:procLev ;
    skos:prefLabel "Level 2 Pre-processing"@en ;
    skos:scopeNote "Geophysical variables derived from Level 1 source data at the same resolution and location as the level 1 data, typically in a satellite projection with geographic information. These data form the fundamental basis for higher level CCI products."@en ;
    skos:topConceptOf cci-scheme:procLev .

<http://vocab.ceda.ac.uk/collection/cci/procLev/proc_level3C> a cci:procLev,
        skos:Concept ;
    skos:altLabel "L3C"@en ;
    skos:broader <http://vocab.ceda.ac.uk/collection/cci/procLev/proc_level3> ;
    skos:definition "Collated (L3C): Observations combined from a single instrument into a space-time grid."@en ;
    skos:inScheme cci-scheme:procLev ;
    skos:prefLabel "Level 3C"@en ;
    skos:scopeNote "Collated (L3C): Observations combined from a single instrument into a space-time grid."@en ;
    skos:topConceptOf cci-scheme:procLev .

<http://vocab.ceda.ac.uk/collection/cci/procLev/proc_level3S> a cci:procLev,
        skos:Concept ;
    skos:altLabel "L3S"@en ;
    skos:broader <http://vocab.ceda.ac.uk/collection/cci/procLev/proc_level3> ;
    skos:definition "Super-collated (L3S): observations combined from multiple instruments into a space-time grid."@en ;
    skos:inScheme cci-scheme:procLev ;
    skos:prefLabel "Level 3S"@en ;
    skos:scopeNote "Super-collated (L3S): observations combined from multiple instruments into a space-time grid."@en ;
    skos:topConceptOf cci-scheme:procLev .

<http://vocab.ceda.ac.uk/collection/cci/procLev/proc_level3U> a cci:procLev,
        skos:Concept ;
    skos:altLabel "L3U"@en ;
    skos:broader <http://vocab.ceda.ac.uk/collection/cci/procLev/proc_level3> ;
    skos:definition "Uncollated (L3U): L2 data granules remapped to a space grid without combining any observations from overlapping orbits."@en ;
    skos:inScheme cci-scheme:procLev ;
    skos:prefLabel "Level 3U"@en ;
    skos:scopeNote "Uncollated (L3U): L2 data granules remapped to a space grid without combining any observations from overlapping orbits."@en ;
    skos:topConceptOf cci-scheme:procLev .

<http://vocab.ceda.ac.uk/collection/cci/sensor/sens_aatsr> a cci:sensor,
        skos:Concept ;
    cci:hasPlatform <http://vocab.ceda.ac.uk/collection/cci/platform/plat_envisat> ;
    rdfs:seeAlso <http://www.wmo-sat.info/oscar/instruments/view/2> ;
    skos:definition "Advanced Along-Track Scanning Radiometer"@en ;
    skos:inScheme cci-scheme:sensor ;
    skos:prefLabel "AATSR"@en ;
    skos:scopeNote "Advanced Along-Track Scanning Radiometer"@en ;
    skos:topConceptOf cci-scheme:sensor .

<http://vocab.ceda.ac.uk/collection/cci/sensor/sens_aceFts> a cci:sensor,
        skos:Concept ;
    cci:hasPlatform <http://vocab.ceda.ac.uk/collection/cci/platform/plat_scisat> ;
    rdfs:seeAlso <http://www.wmo-sat.info/oscar/instruments/view/6> ;
    skos:definition "Advanced Composition Explorer Fourier Transform Spectrometer"@en ;
    skos:inScheme cci-scheme:sensor ;
    skos:prefLabel "ACE-FTS"@en ;
    skos:scopeNote "Advanced Composition Explorer Fourier Transform Spectrometer"@en ;
    skos:topConceptOf cci-scheme:sensor .

<http://vocab.ceda.ac.uk/collection/cci/sensor/sens_airs> a cci:sensor,
        skos:Concept ;
    cci:hasPlatform <http://vocab.ceda.ac.uk/collection/cci/platform/plat_aqua> ;
    rdfs:seeAlso <http://www.wmo-sat.info/oscar/instruments/view/16> ;
    skos:definition "Atmospheric Infra-Red Sounder"@en ;
    skos:inScheme cci-scheme:sensor ;
    skos:prefLabel "AIRS"@en ;
    skos:scopeNote "Atmospheric Infra-Red Sounder"@en ;
    skos:topConceptOf cci-scheme:sensor .

<http://vocab.ceda.ac.uk/collection/cci/sensor/sens_altika> a cci:sensor,
        skos:Concept ;
    cci:hasPlatform <http://vocab.ceda.ac.uk/collection/cci/platform/plat_saral> ;
    rdfs:seeAlso <https://www.wmo-sat.info/oscar/instruments/view/21> ;
    skos:definition "CNES Ka-band Altimeter"@en ;
    skos:inScheme cci-scheme:sensor ;
    skos:prefLabel "AltiKa"@en ;
    skos:scopeNote "CNES Ka-band Altimeter"@en ;
    skos:topConceptOf cci-scheme:sensor .

<http://vocab.ceda.ac.uk/collection/cci/sensor/sens_amsre> a cci:sensor,
        skos:Concept ;
    cci:hasPlatform <http://vocab.ceda.ac.uk/collection/cci/platform/plat_aqua> ;
    rdfs:seeAlso <http://www.wmo-sat.info/oscar/instruments/view/29> ;
    skos:definition "Advanced Microwave Scanning Radiometer for Earth Observation from Space"@en ;
    skos:inScheme cci-scheme:sensor ;
    skos:prefLabel "AMSRE"@en ;
    skos:scopeNote "Advanced Microwave Scanning Radiometer for Earth Observation from Space"@en ;
    skos:topConceptOf cci-scheme:sensor .

<http://vocab.ceda.ac.uk/collection/cci/sensor/sens_aquarius> a cci:sensor,
        skos:Concept ;
    cci:hasPlatform <http://vocab.ceda.ac.uk/collection/cci/platform/plat_sac_d> ;
    rdfs:seeAlso <https://www.wmo-sat.info/oscar/instruments/view/41> ;
    skos:definition "Aquarius"@en ;
    skos:inScheme cci-scheme:sensor ;
    skos:prefLabel "Aquarius"@en ;
    skos:scopeNote "Aquarius"@en ;
    skos:topConceptOf cci-scheme:sensor .

<http://vocab.ceda.ac.uk/collection/cci/sensor/sens_asar> a cci:sensor,
        skos:Concept ;
    cci:hasPlatform <http://vocab.ceda.ac.uk/collection/cci/platform/plat_envisat> ;
    rdfs:seeAlso <http://www.wmo-sat.info/oscar/instruments/view/44> ;
    skos:definition "Advanced Synthetic Aperture Radar"@en ;
    skos:inScheme cci-scheme:sensor ;
    skos:prefLabel "ASAR"@en ;
    skos:scopeNote "Advanced Synthetic Aperture Radar"@en ;
    skos:topConceptOf cci-scheme:sensor .

<http://vocab.ceda.ac.uk/collection/cci/sensor/sens_aster> a cci:sensor,
        skos:Concept ;
    cci:hasPlatform <http://vocab.ceda.ac.uk/collection/cci/platform/plat_terra> ;
    rdfs:seeAlso <http://www.wmo-sat.info/oscar/instruments/view/50> ;
    skos:definition "Advanced Spaceborne Thermal Emission and Reflection Radiometer"@en ;
    skos:inScheme cci-scheme:sensor ;
    skos:prefLabel "ASTER"@en ;
    skos:scopeNote "Advanced Spaceborne Thermal Emission and Reflection Radiometer"@en ;
    skos:topConceptOf cci-scheme:sensor .

<http://vocab.ceda.ac.uk/collection/cci/sensor/sens_atsr> a cci:sensor,
        skos:Concept ;
    cci:hasPlatform <http://vocab.ceda.ac.uk/collection/cci/platform/plat_ers1> ;
    rdfs:seeAlso <http://www.wmo-sat.info/oscar/instruments/view/55> ;
    skos:definition "Along Track Scanning Radiometer"@en ;
    skos:inScheme cci-scheme:sensor ;
    skos:prefLabel "ATSR"@en ;
    skos:scopeNote "Along Track Scanning Radiometer"@en ;
    skos:topConceptOf cci-scheme:sensor .

<http://vocab.ceda.ac.uk/collection/cci/sensor/sens_atsr2> a cci:sensor,
        skos:Concept ;
    cci:hasPlatform <http://vocab.ceda.ac.uk/collection/cci/platform/plat_ers2> ;
    rdfs:seeAlso <http://www.wmo-sat.info/oscar/instruments/view/56> ;
    skos:definition "Along Track Scanning Radiometer – 2"@en ;
    skos:inScheme cci-scheme:sensor ;
    skos:prefLabel "ATSR-2"@en ;
    skos:scopeNote "Along Track Scanning Radiometer – 2"@en ;
    skos:topConceptOf cci-scheme:sensor .

<http://vocab.ceda.ac.uk/collection/cci/sensor/sens_esmrNim5> a cci:sensor,
        skos:Concept ;
    cci:hasPlatform <http://vocab.ceda.ac.uk/collection/cci/platform/plat_nimbus5> ;
    rdfs:seeAlso <https://space.oscar.wmo.int/instruments/view/esmr_nimbus_5> ;
    skos:definition "Electrically Scanning Microwave Radiometer (Nimbus-6)"@en ;
    skos:inScheme cci-scheme:sensor ;
    skos:prefLabel "ESMR (Nimbus-5)"@en ;
    skos:scopeNote "Electrically Scanning Microwave Radiometer (Nimbus-6)"@en ;
    skos:topConceptOf cci-scheme:sensor .

<http://vocab.ceda.ac.uk/collection/cci/sensor/sens_esmrNim6> a cci:sensor,
        skos:Concept ;
    cci:hasPlatform <http://vocab.ceda.ac.uk/collection/cci/platform/plat_nimbus6> ;
    rdfs:seeAlso <https://space.oscar.wmo.int/instruments/view/esmr_nimbus_6> ;
    skos:definition "Electrically Scanning Microwave Radiometer (Nimbus-5)"@en ;
    skos:inScheme cci-scheme:sensor ;
    skos:prefLabel "ESMR (Nimbus-6)"@en ;
    skos:scopeNote "Electrically Scanning Microwave Radiometer (Nimbus-5)"@en ;
    skos:topConceptOf cci-scheme:sensor .

<http://vocab.ceda.ac.uk/collection/cci/sensor/sens_gfora> a cci:sensor,
        skos:Concept ;
    cci:hasPlatform <http://vocab.ceda.ac.uk/collection/cci/platform/plat_gfo> ;
    rdfs:seeAlso <http://www.wmo-sat.info/oscar/instruments/view/154> ;
    skos:definition "Geosat Follow-On"@en ;
    skos:inScheme cci-scheme:sensor ;
    skos:prefLabel "GFO-RA"@en ;
    skos:scopeNote "Geosat Follow-On"@en ;
    skos:topConceptOf cci-scheme:sensor .

<http://vocab.ceda.ac.uk/collection/cci/sensor/sens_glas> a cci:sensor,
        skos:Concept ;
    cci:hasPlatform <http://vocab.ceda.ac.uk/collection/cci/platform/plat_icesat> ;
    rdfs:seeAlso <http://www.wmo-sat.info/oscar/instruments/view/155> ;
    skos:definition "Geoscience Laser Altimeter System"@en ;
    skos:inScheme cci-scheme:sensor ;
    skos:prefLabel "GLAS"@en ;
    skos:scopeNote "Geoscience Laser Altimeter System"@en ;
    skos:topConceptOf cci-scheme:sensor .

<http://vocab.ceda.ac.uk/collection/cci/sensor/sens_gmi> a cci:sensor,
        skos:Concept ;
    cci:hasPlatform <http://vocab.ceda.ac.uk/collection/cci/platform/plat_gpm> ;
    rdfs:seeAlso <https://www.wmo-sat.info/oscar/instruments/view/gmi_core> ;
    skos:altLabel "GMI (core)"@en ;
    skos:definition "GPM Microwave Imager"@en ;
    skos:inScheme cci-scheme:sensor ;
    skos:prefLabel "GMI"@en ;
    skos:scopeNote "GPM Microwave Imager"@en ;
    skos:topConceptOf cci-scheme:sensor .

<http://vocab.ceda.ac.uk/collection/cci/sensor/sens_gome> a cci:sensor,
        skos:Concept ;
    cci:hasPlatform <http://vocab.ceda.ac.uk/collection/cci/platform/plat_ers2> ;
    rdfs:seeAlso <http://www.wmo-sat.info/oscar/instruments/view/166> ;
    skos:definition "Global Monitoring of Atmospheric Ozone"@en ;
    skos:inScheme cci-scheme:sensor ;
    skos:prefLabel "GOME"@en ;
    skos:scopeNote "Global Monitoring of Atmospheric Ozone"@en ;
    skos:topConceptOf cci-scheme:sensor .

<http://vocab.ceda.ac.uk/collection/cci/sensor/sens_gomos> a cci:sensor,
        skos:Concept ;
    cci:hasPlatform <http://vocab.ceda.ac.uk/collection/cci/platform/plat_envisat> ;
    rdfs:seeAlso <http://www.wmo-sat.info/oscar/instruments/view/168> ;
    skos:definition "Global Ozone Monitoring by Occultation of Stars"@en ;
    skos:inScheme cci-scheme:sensor ;
    skos:prefLabel "GOMOS"@en ;
    skos:scopeNote "Global Ozone Monitoring by Occultation of Stars"@en ;
    skos:topConceptOf cci-scheme:sensor .

<http://vocab.ceda.ac.uk/collection/cci/sensor/sens_grace> a cci:sensor,
        skos:Concept ;
    cci:hasPlatform <http://vocab.ceda.ac.uk/collection/cci/platform/plat_grace> ;
    rdfs:seeAlso <https://www.wmo-sat.info/oscar/instruments/view/269>,
        <https://www.wmo-sat.info/oscar/instruments/view/469> ;
    skos:altLabel "GRACE"@en ;
    skos:definition "GRACE instrument"@en ;
    skos:inScheme cci-scheme:sensor ;
    skos:prefLabel "GRACE instrument"@en ;
    skos:scopeNote "GRACE instrument"@en ;
    skos:topConceptOf cci-scheme:sensor .

<http://vocab.ceda.ac.uk/collection/cci/sensor/sens_hirs> a cci:sensor,
        skos:Concept ;
    cci:hasPlatform <http://vocab.ceda.ac.uk/collection/cci/platform/plat_nimbus6> ;
    rdfs:seeAlso <https://www.wmo-sat.info/oscar/instruments/view/181> ;
    skos:definition "High-Resolution Infra-Red Sounder"@en ;
    skos:inScheme cci-scheme:sensor ;
    skos:prefLabel "HIRS"@en ;
    skos:scopeNote "High-Resolution Infra-Red Sounder"@en ;
    skos:topConceptOf cci-scheme:sensor .

<http://vocab.ceda.ac.uk/collection/cci/sensor/sens_hrs> a cci:sensor,
        skos:Concept ;
    cci:hasPlatform <http://vocab.ceda.ac.uk/collection/cci/platform/plat_spot5> ;
    rdfs:seeAlso <http://www.wmo-sat.info/oscar/instruments/view/193> ;
    skos:definition "High-Resolution Stereoscope"@en ;
    skos:inScheme cci-scheme:sensor ;
    skos:prefLabel "HRS"@en ;
    skos:scopeNote "High-Resolution Stereoscope"@en ;
    skos:topConceptOf cci-scheme:sensor .

<http://vocab.ceda.ac.uk/collection/cci/sensor/sens_imagerMtsat2> a cci:sensor,
        skos:Concept ;
    cci:hasPlatform <http://vocab.ceda.ac.uk/collection/cci/platform/plat_himawari-7> ;
    rdfs:seeAlso <https://space.oscar.wmo.int/instruments/view/imager_mtsat_2> ;
    skos:definition "MTSAT-2 Imager"@en ;
    skos:inScheme cci-scheme:sensor ;
    skos:prefLabel "IMAGER (MTSAT-2)"@en ;
    skos:scopeNote "MTSAT-2 Imager"@en ;
    skos:topConceptOf cci-scheme:sensor .

<http://vocab.ceda.ac.uk/collection/cci/sensor/sens_jami> a cci:sensor,
        skos:Concept ;
    cci:hasPlatform <http://vocab.ceda.ac.uk/collection/cci/platform/plat_himawari-6> ;
    rdfs:seeAlso <http://www.wmo-sat.info/oscar/instruments/view/236> ;
    skos:definition "Japanese Advanced Meteorological Imager"@en ;
    skos:inScheme cci-scheme:sensor ;
    skos:prefLabel "JAMI"@en ;
    skos:scopeNote "Japanese Advanced Meteorological Imager"@en ;
    skos:topConceptOf cci-scheme:sensor .

<http://vocab.ceda.ac.uk/collection/cci/sensor/sens_meris> a cci:sensor,
        skos:Concept ;
    cci:hasPlatform <http://vocab.ceda.ac.uk/collection/cci/platform/plat_envisat> ;
    rdfs:seeAlso <http://www.wmo-sat.info/oscar/instruments/view/277> ;
    skos:definition "Medium-Spectral Resolution, Imaging Spectrometer"@en ;
    skos:inScheme cci-scheme:sensor ;
    skos:prefLabel "MERIS"@en ;
    skos:scopeNote "Medium-Spectral Resolution, Imaging Spectrometer"@en ;
    skos:topConceptOf cci-scheme:sensor .

<http://vocab.ceda.ac.uk/collection/cci/sensor/sens_mipas> a cci:sensor,
        skos:Concept ;
    cci:hasPlatform <http://vocab.ceda.ac.uk/collection/cci/platform/plat_envisat> ;
    rdfs:seeAlso <http://www.wmo-sat.info/oscar/instruments/view/286> ;
    skos:definition "Michelson Interferometer for Passive Atmospheric Sounding"@en ;
    skos:inScheme cci-scheme:sensor ;
    skos:prefLabel "MIPAS"@en ;
    skos:scopeNote "Michelson Interferometer for Passive Atmospheric Sounding"@en ;
    skos:topConceptOf cci-scheme:sensor .

<http://vocab.ceda.ac.uk/collection/cci/sensor/sens_miras> a cci:sensor,
        skos:Concept ;
    cci:hasPlatform <http://vocab.ceda.ac.uk/collection/cci/platform/plat_smos> ;
    rdfs:seeAlso <https://www.wmo-sat.info/oscar/instruments/view/287> ;
    skos:definition "Microwave Imaging Radiometer using Aperture Synthesis"@en ;
    skos:inScheme cci-scheme:sensor ;
    skos:prefLabel "MIRAS"@en ;
    skos:scopeNote "Microwave Imaging Radiometer using Aperture Synthesis"@en ;
    skos:topConceptOf cci-scheme:sensor .

<http://vocab.ceda.ac.uk/collection/cci/sensor/sens_nra> a cci:sensor,
        skos:Concept ;
    cci:hasPlatform <http://vocab.ceda.ac.uk/collection/cci/platform/plat_topexPoseidon> ;
    rdfs:seeAlso <https://www.wmo-sat.info/oscar/instruments/view/1016> ;
    skos:altLabel "TOPEX"@en ;
    skos:definition "NASA Radar Altimeter"@en ;
    skos:inScheme cci-scheme:sensor ;
    skos:prefLabel "NRA"@en ;
    skos:scopeNote "NASA Radar Altimeter"@en ;
    skos:topConceptOf cci-scheme:sensor .

<http://vocab.ceda.ac.uk/collection/cci/sensor/sens_oco> a cci:sensor,
        skos:Concept ;
    cci:hasPlatform <http://vocab.ceda.ac.uk/collection/cci/platform/plat_oco2> ;
    rdfs:seeAlso <https://www.wmo-sat.info/oscar/instruments/view/368> ;
    skos:definition "Orbiting Carbon Observatory"@en ;
    skos:inScheme cci-scheme:sensor ;
    skos:prefLabel "OCO"@en ;
    skos:scopeNote "Orbiting Carbon Observatory"@en ;
    skos:topConceptOf cci-scheme:sensor .

<http://vocab.ceda.ac.uk/collection/cci/sensor/sens_oli> a cci:sensor,
        skos:Concept ;
    cci:hasPlatform <http://vocab.ceda.ac.uk/collection/cci/platform/plat_landsat_8> ;
    rdfs:seeAlso <http://www.wmo-sat.info/oscar/instruments/view/375> ;
    skos:definition "Operational Land Image"@en ;
    skos:inScheme cci-scheme:sensor ;
    skos:prefLabel "OLI"@en ;
    skos:scopeNote "Operational Land Image"@en ;
    skos:topConceptOf cci-scheme:sensor .

<http://vocab.ceda.ac.uk/collection/cci/sensor/sens_omi> a cci:sensor,
        skos:Concept ;
    cci:hasPlatform <http://vocab.ceda.ac.uk/collection/cci/platform/plat_aura> ;
    rdfs:seeAlso <http://www.wmo-sat.info/oscar/instruments/view/377> ;
    skos:definition "Ozone Monitoring Instrument"@en ;
    skos:inScheme cci-scheme:sensor ;
    skos:prefLabel "OMI"@en ;
    skos:scopeNote "Ozone Monitoring Instrument"@en ;
    skos:topConceptOf cci-scheme:sensor .

<http://vocab.ceda.ac.uk/collection/cci/sensor/sens_osiris> a cci:sensor,
        skos:Concept ;
    cci:hasPlatform <http://vocab.ceda.ac.uk/collection/cci/platform/plat_odin> ;
    rdfs:seeAlso <http://www.wmo-sat.info/oscar/instruments/view/383> ;
    skos:definition "Optical Spectrograph and Infra-Red Imager System"@en ;
    skos:inScheme cci-scheme:sensor ;
    skos:prefLabel "OSIRIS"@en ;
    skos:scopeNote "Optical Spectrograph and Infra-Red Imager System"@en ;
    skos:topConceptOf cci-scheme:sensor .

<http://vocab.ceda.ac.uk/collection/cci/sensor/sens_palsar> a cci:sensor,
        skos:Concept ;
    cci:hasPlatform <http://vocab.ceda.ac.uk/collection/cci/platform/plat_alos> ;
    rdfs:seeAlso <http://www.wmo-sat.info/oscar/instruments/view/387> ;
    skos:definition "Phased Array type L-band Synthetic Aperture Radar"@en ;
    skos:inScheme cci-scheme:sensor ;
    skos:prefLabel "PALSAR"@en ;
    skos:scopeNote "Phased Array type L-band Synthetic Aperture Radar"@en ;
    skos:topConceptOf cci-scheme:sensor .

<http://vocab.ceda.ac.uk/collection/cci/sensor/sens_palsar2> a cci:sensor,
        skos:Concept ;
    cci:hasPlatform <http://vocab.ceda.ac.uk/collection/cci/platform/plat_alos-2> ;
    rdfs:seeAlso <https://www.wmo-sat.info/oscar/instruments/view/388> ;
    skos:definition "Phased Array type L-band Synthetic Aperture Radar – 2"@en ;
    skos:inScheme cci-scheme:sensor ;
    skos:prefLabel "PALSAR-2"@en ;
    skos:scopeNote "Phased Array type L-band Synthetic Aperture Radar – 2"@en ;
    skos:topConceptOf cci-scheme:sensor .

<http://vocab.ceda.ac.uk/collection/cci/sensor/sens_polder> a cci:sensor,
        skos:Concept ;
    cci:hasPlatform <http://vocab.ceda.ac.uk/collection/cci/platform/plat_parasol> ;
    rdfs:seeAlso <http://www.wmo-sat.info/oscar/instruments/view/405> ;
    skos:definition "POLarization and Directionality of the Earth's Reflectances"@en ;
    skos:inScheme cci-scheme:sensor ;
    skos:prefLabel "POLDER"@en ;
    skos:scopeNote "POLarization and Directionality of the Earth's Reflectances"@en ;
    skos:topConceptOf cci-scheme:sensor .

<http://vocab.ceda.ac.uk/collection/cci/sensor/sens_poseidon2> a cci:sensor,
        skos:Concept ;
    cci:hasPlatform <http://vocab.ceda.ac.uk/collection/cci/platform/plat_jason1> ;
    rdfs:seeAlso <http://www.wmo-sat.info/oscar/instruments/view/406> ;
    skos:definition "Poseidon 2"@en ;
    skos:inScheme cci-scheme:sensor ;
    skos:prefLabel "Poseidon-2"@en ;
    skos:scopeNote "Poseidon 2"@en ;
    skos:topConceptOf cci-scheme:sensor .

<http://vocab.ceda.ac.uk/collection/cci/sensor/sens_poseidon3> a cci:sensor,
        skos:Concept ;
    cci:hasPlatform <http://vocab.ceda.ac.uk/collection/cci/platform/plat_jason2> ;
    rdfs:seeAlso <http://www.wmo-sat.info/oscar/instruments/view/407> ;
    skos:definition "Poseidon 3"@en ;
    skos:inScheme cci-scheme:sensor ;
    skos:prefLabel "Poseidon-3"@en ;
    skos:scopeNote "Poseidon 3"@en ;
    skos:topConceptOf cci-scheme:sensor .

<http://vocab.ceda.ac.uk/collection/cci/sensor/sens_poseidon3b> a cci:sensor,
        skos:Concept ;
    cci:hasPlatform <http://vocab.ceda.ac.uk/collection/cci/platform/plat_jason3> ;
    rdfs:seeAlso <https://www.wmo-sat.info/oscar/instruments/view/408> ;
    skos:definition "Poseidon 3b"@en ;
    skos:inScheme cci-scheme:sensor ;
    skos:prefLabel "Poseidon-3B"@en ;
    skos:scopeNote "Poseidon 3b"@en ;
    skos:topConceptOf cci-scheme:sensor .

<http://vocab.ceda.ac.uk/collection/cci/sensor/sens_ra2> a cci:sensor,
        skos:Concept ;
    cci:hasPlatform <http://vocab.ceda.ac.uk/collection/cci/platform/plat_envisat> ;
    rdfs:seeAlso <http://www.wmo-sat.info/oscar/instruments/view/416> ;
    skos:definition "Radar Altimeter"@en ;
    skos:inScheme cci-scheme:sensor ;
    skos:prefLabel "RA-2"@en ;
    skos:scopeNote "Radar Altimeter"@en ;
    skos:topConceptOf cci-scheme:sensor .

<http://vocab.ceda.ac.uk/collection/cci/sensor/sens_sciamachy> a cci:sensor,
        skos:Concept ;
    cci:hasPlatform <http://vocab.ceda.ac.uk/collection/cci/platform/plat_envisat> ;
    rdfs:seeAlso <http://www.wmo-sat.info/oscar/instruments/view/477>,
        <http://www.wmo-sat.info/oscar/instruments/view/478> ;
    skos:definition "SCanning Imaging Absorption spectroMeter for AtmosphericCHartographY"@en ;
    skos:inScheme cci-scheme:sensor ;
    skos:prefLabel "SCIAMACHY"@en ;
    skos:scopeNote "SCanning Imaging Absorption spectroMeter for AtmosphericCHartographY"@en ;
    skos:topConceptOf cci-scheme:sensor .

<http://vocab.ceda.ac.uk/collection/cci/sensor/sens_seaWiFs> a cci:sensor,
        skos:Concept ;
    cci:hasPlatform <http://vocab.ceda.ac.uk/collection/cci/platform/plat_orbview2> ;
    rdfs:seeAlso <http://www.wmo-sat.info/oscar/instruments/view/481> ;
    skos:definition "Sea-viewing Wide Field-of-view Sensor"@en ;
    skos:inScheme cci-scheme:sensor ;
    skos:prefLabel "SeaWiFS"@en ;
    skos:scopeNote "Sea-viewing Wide Field-of-view Sensor"@en ;
    skos:topConceptOf cci-scheme:sensor .

<http://vocab.ceda.ac.uk/collection/cci/sensor/sens_siral> a cci:sensor,
        skos:Concept ;
    cci:hasPlatform <http://vocab.ceda.ac.uk/collection/cci/platform/plat_cryosat2> ;
    rdfs:seeAlso <https://www.wmo-sat.info/oscar/instruments/view/509> ;
    skos:definition "SAR Interferometer Radar Altimeter"@en ;
    skos:inScheme cci-scheme:sensor ;
    skos:prefLabel "SIRAL"@en ;
    skos:scopeNote "SAR Interferometer Radar Altimeter"@en ;
    skos:topConceptOf cci-scheme:sensor .

<http://vocab.ceda.ac.uk/collection/cci/sensor/sens_smap> a cci:sensor,
        skos:Concept ;
    cci:hasPlatform <http://vocab.ceda.ac.uk/collection/cci/platform/plat_smap> ;
    rdfs:seeAlso <https://www.wmo-sat.info/oscar/instruments/view/521> ;
    skos:definition "Soil Moisture Active-Passive (intended as payload)"@en ;
    skos:inScheme cci-scheme:sensor ;
    skos:prefLabel "SMAP"@en ;
    skos:scopeNote "Soil Moisture Active-Passive (intended as payload)"@en ;
    skos:topConceptOf cci-scheme:sensor .

<http://vocab.ceda.ac.uk/collection/cci/sensor/sens_smmr> a cci:sensor,
        skos:Concept ;
    cci:hasPlatform <http://vocab.ceda.ac.uk/collection/cci/platform/plat_nimbus7> ;
    rdfs:seeAlso <http://www.wmo-sat.info/oscar/instruments/view/522> ;
    skos:definition "Scanning Multichannel Microwave Radiometer"@en ;
    skos:inScheme cci-scheme:sensor ;
    skos:prefLabel "SMMR"@en ;
    skos:scopeNote "Scanning Multichannel Microwave Radiometer"@en ;
    skos:topConceptOf cci-scheme:sensor .

<http://vocab.ceda.ac.uk/collection/cci/sensor/sens_smr> a cci:sensor,
        skos:Concept ;
    cci:hasPlatform <http://vocab.ceda.ac.uk/collection/cci/platform/plat_odin> ;
    rdfs:seeAlso <http://www.wmo-sat.info/oscar/instruments/view/524> ;
    skos:definition "Sub-Millimetre Radiometer"@en ;
    skos:inScheme cci-scheme:sensor ;
    skos:prefLabel "SMR"@en ;
    skos:scopeNote "Sub-Millimetre Radiometer"@en ;
    skos:topConceptOf cci-scheme:sensor .

<http://vocab.ceda.ac.uk/collection/cci/sensor/sens_ssalt> a cci:sensor,
        skos:Concept ;
    cci:hasPlatform <http://vocab.ceda.ac.uk/collection/cci/platform/plat_topexPoseidon> ;
    rdfs:seeAlso <http://www.wmo-sat.info/oscar/instruments/view/531> ;
    skos:altLabel "Poseidon-1"@en ;
    skos:definition "Single-frequency Solid-state Altimeter"@en ;
    skos:inScheme cci-scheme:sensor ;
    skos:prefLabel "SSALT"@en ;
    skos:scopeNote "Single-frequency Solid-state Altimeter"@en ;
    skos:topConceptOf cci-scheme:sensor .

<http://vocab.ceda.ac.uk/collection/cci/sensor/sens_tansoCai> a cci:sensor,
        skos:Concept ;
    cci:hasPlatform <http://vocab.ceda.ac.uk/collection/cci/platform/plat_gosat> ;
    rdfs:seeAlso <http://www.wmo-sat.info/oscar/instruments/view/553> ;
    skos:definition "Thermal And Near-infrared Sensor for carbon Observation Cloud and Aerosol Imager"@en ;
    skos:inScheme cci-scheme:sensor ;
    skos:prefLabel "TANSO-CAI"@en ;
    skos:scopeNote "Thermal And Near-infrared Sensor for carbon Observation Cloud and Aerosol Imager"@en ;
    skos:topConceptOf cci-scheme:sensor .

<http://vocab.ceda.ac.uk/collection/cci/sensor/sens_tansoFts> a cci:sensor,
        skos:Concept ;
    cci:hasPlatform <http://vocab.ceda.ac.uk/collection/cci/platform/plat_gosat> ;
    rdfs:seeAlso <http://www.wmo-sat.info/oscar/instruments/view/554> ;
    skos:definition "Thermal And Near-infrared Sensor for carbon Observation Fourier Transform Spectrometer"@en ;
    skos:inScheme cci-scheme:sensor ;
    skos:prefLabel "TANSO-FTS"@en ;
    skos:scopeNote "Thermal And Near-infrared Sensor for carbon Observation Fourier Transform Spectrometer"@en ;
    skos:topConceptOf cci-scheme:sensor .

<http://vocab.ceda.ac.uk/collection/cci/sensor/sens_tansoFts2> a cci:sensor,
        skos:Concept ;
    cci:hasPlatform <http://vocab.ceda.ac.uk/collection/cci/platform/plat_gosat-2> ;
    rdfs:seeAlso <https://space.oscar.wmo.int/instruments/view/tanso_fts_2> ;
    skos:definition "Thermal And Near infrared Sensor for carbon Observations - Fourier Transform Spectrometer / 2"@en ;
    skos:inScheme cci-scheme:sensor ;
    skos:prefLabel "TANSO-FTS-2"@en ;
    skos:scopeNote "Thermal And Near infrared Sensor for carbon Observations - Fourier Transform Spectrometer / 2"@en ;
    skos:topConceptOf cci-scheme:sensor .

<http://vocab.ceda.ac.uk/collection/cci/sensor/sens_tirs> a cci:sensor,
        skos:Concept ;
    cci:hasPlatform <http://vocab.ceda.ac.uk/collection/cci/platform/plat_landsat_8> ;
    rdfs:seeAlso <http://www.wmo-sat.info/oscar/instruments/view/567> ;
    skos:definition "Thermal Infrared Sensor"@en ;
    skos:inScheme cci-scheme:sensor ;
    skos:prefLabel "TIRS"@en ;
    skos:scopeNote "Thermal Infrared Sensor"@en ;
    skos:topConceptOf cci-scheme:sensor .

<http://vocab.ceda.ac.uk/collection/cci/sensor/sens_tmi> a cci:sensor,
        skos:Concept ;
    cci:hasPlatform <http://vocab.ceda.ac.uk/collection/cci/platform/plat_trmm> ;
    rdfs:seeAlso <http://www.wmo-sat.info/oscar/instruments/view/569> ;
    skos:definition "TRMM Microwave Imager"@en ;
    skos:inScheme cci-scheme:sensor ;
    skos:prefLabel "TMI"@en ;
    skos:scopeNote "TRMM Microwave Imager"@en ;
    skos:topConceptOf cci-scheme:sensor .

<http://vocab.ceda.ac.uk/collection/cci/sensor/sens_toms> a cci:sensor,
        skos:Concept ;
    rdfs:seeAlso <https://www.wmo-sat.info/oscar/instruments/view/571> ;
    skos:definition "Total Ozone Mapping Spectrometer"@en ;
    skos:inScheme cci-scheme:sensor ;
    skos:prefLabel "TOMS"@en ;
    skos:scopeNote "Total Ozone Mapping Spectrometer"@en ;
    skos:topConceptOf cci-scheme:sensor .

<http://vocab.ceda.ac.uk/collection/cci/sensor/sens_tropomi> a cci:sensor,
        skos:Concept ;
    cci:hasPlatform <http://vocab.ceda.ac.uk/collection/cci/platform/plat_sentinel5p> ;
    rdfs:seeAlso <https://www.wmo-sat.info/oscar/instruments/view/586> ;
    skos:definition "Tropospheric Monitoring Instrument"@en ;
    skos:inScheme cci-scheme:sensor ;
    skos:prefLabel "TROPOMI"@en ;
    skos:scopeNote "Tropospheric Monitoring Instrument"@en ;
    skos:topConceptOf cci-scheme:sensor .

<http://vocab.ceda.ac.uk/collection/cci/sensor/sens_vegetationP> a cci:sensor,
        skos:Concept ;
    cci:hasPlatform <http://vocab.ceda.ac.uk/collection/cci/platform/plat_probaV> ;
    rdfs:seeAlso <https://www.wmo-sat.info/oscar/instruments/view/961> ;
    skos:altLabel "Vegetation-P"@en ;
    skos:definition "Végétation for PROBA"@en ;
    skos:inScheme cci-scheme:sensor ;
    skos:prefLabel "Végétation-P"@en ;
    skos:scopeNote "Végétation for PROBA"@en ;
    skos:topConceptOf cci-scheme:sensor .

<http://vocab.ceda.ac.uk/collection/cci/sensor/sens_viirs> a cci:sensor,
        skos:Concept ;
    cci:hasPlatform <http://vocab.ceda.ac.uk/collection/cci/platform/plat_snpp> ;
    rdfs:seeAlso <https://www.wmo-sat.info/oscar/instruments/view/604> ;
    skos:definition "Visible/Infrared Imager Radiometer Suite"@en ;
    skos:inScheme cci-scheme:sensor ;
    skos:prefLabel "VIIRS"@en ;
    skos:scopeNote "Visible/Infrared Imager Radiometer Suite"@en ;
    skos:topConceptOf cci-scheme:sensor .

<http://vocab.ceda.ac.uk/collection/cci/sensor/sens_windSat> a cci:sensor,
        skos:Concept ;
    cci:hasPlatform <http://vocab.ceda.ac.uk/collection/cci/platform/plat_coriolis> ;
    rdfs:seeAlso <http://www.wmo-sat.info/oscar/instruments/view/623> ;
    skos:definition "Polarimetric microwave radiometer"@en ;
    skos:inScheme cci-scheme:sensor ;
    skos:prefLabel "WindSat"@en ;
    skos:scopeNote "Polarimetric microwave radiometer"@en ;
    skos:topConceptOf cci-scheme:sensor .

cci:platformGrp a owl:Class ;
    rdfs:label "Platform Group" ;
    dc:description "The platform groups that have been used in the collection of data for the ESA Climate Change Initiative (CCI). A group consists of a number of <a href=#platformPrg>programmes</a>" ;
    rdfs:isDefinedBy <http://vocab.ceda.ac.uk/ontology/cci#> .

<http://vocab.ceda.ac.uk/collection/cci/platform/plat_FY-3D> a cci:platform,
        skos:Concept ;
    cci:hasSensor <http://vocab.ceda.ac.uk/collection/cci/sensor/sens_mwri> ;
    rdfs:seeAlso <http://www.wmo-sat.info/oscar/satellites/view/116> ;
    skos:altLabel "Feng-Yun - 3D"@en ;
    skos:broader <http://vocab.ceda.ac.uk/collection/cci/platformProg/plat_fengyun3> ;
    skos:definition "CMA Feng-Yun – 3D"@en ;
    skos:inScheme cci-scheme:platform ;
    skos:prefLabel "FY-3D"@en ;
    skos:scopeNote "CMA Feng-Yun – 3D"@en ;
    skos:topConceptOf cci-scheme:platform .

<http://vocab.ceda.ac.uk/collection/cci/platform/plat_FY-3F> a cci:platform,
        skos:Concept ;
    cci:hasSensor <http://vocab.ceda.ac.uk/collection/cci/sensor/sens_mwri> ;
    rdfs:seeAlso <http://www.wmo-sat.info/oscar/satellites/view/118> ;
    skos:altLabel "Feng-Yun - 3F"@en ;
    skos:broader <http://vocab.ceda.ac.uk/collection/cci/platformProg/plat_fengyun3> ;
    skos:definition "CMA Feng-Yun – 3F"@en ;
    skos:inScheme cci-scheme:platform ;
    skos:prefLabel "FY-3F"@en ;
    skos:scopeNote "CMA Feng-Yun – 3F"@en ;
    skos:topConceptOf cci-scheme:platform .

<http://vocab.ceda.ac.uk/collection/cci/platform/plat_alos> a cci:platform,
        skos:Concept ;
    cci:hasSensor <http://vocab.ceda.ac.uk/collection/cci/sensor/sens_palsar> ;
    rdfs:seeAlso <http://www.wmo-sat.info/oscar/satellites/view/5> ;
    skos:broader <http://vocab.ceda.ac.uk/collection/cci/platformProg/plat_alos_prog> ;
    skos:definition "JAXA Advanced Land Observation Satellite"@en ;
    skos:inScheme cci-scheme:platform ;
    skos:prefLabel "ALOS"@en ;
    skos:scopeNote "JAXA Advanced Land Observation Satellite"@en ;
    skos:topConceptOf cci-scheme:platform .

<http://vocab.ceda.ac.uk/collection/cci/platform/plat_alos-2> a cci:platform,
        skos:Concept ;
    cci:hasSensor <http://vocab.ceda.ac.uk/collection/cci/sensor/sens_palsar2> ;
    rdfs:seeAlso <http://www.wmo-sat.info/oscar/satellites/view/6> ;
    skos:broader <http://vocab.ceda.ac.uk/collection/cci/platformProg/plat_alos_prog> ;
    skos:definition "JAXA Advanced Land Observation Satellite 2"@en ;
    skos:inScheme cci-scheme:platform ;
    skos:prefLabel "ALOS-2"@en ;
    skos:scopeNote "JAXA Advanced Land Observation Satellite 2"@en ;
    skos:topConceptOf cci-scheme:platform .

<http://vocab.ceda.ac.uk/collection/cci/platform/plat_aura> a cci:platform,
        skos:Concept ;
    cci:hasSensor <http://vocab.ceda.ac.uk/collection/cci/sensor/sens_omi> ;
    rdfs:seeAlso <http://www.wmo-sat.info/oscar/satellites/view/80> ;
    skos:broader <http://vocab.ceda.ac.uk/collection/cci/platformProg/plat_eos> ;
    skos:definition "NASA  Earth Observing System Satellite"@en ;
    skos:inScheme cci-scheme:platform ;
    skos:prefLabel "Aura"@en ;
    skos:scopeNote "NASA  Earth Observing System Satellite"@en ;
    skos:topConceptOf cci-scheme:platform .

<http://vocab.ceda.ac.uk/collection/cci/platform/plat_coriolis> a cci:platform,
        skos:Concept ;
    cci:hasSensor <http://vocab.ceda.ac.uk/collection/cci/sensor/sens_windSat> ;
    rdfs:seeAlso <http://www.wmo-sat.info/oscar/satellites/view/36> ;
    skos:broader <http://vocab.ceda.ac.uk/collection/cci/platformProg/plat_coriolis_prog> ;
    skos:definition "US Naval Research Laboratory Satellite"@en ;
    skos:inScheme cci-scheme:platform ;
    skos:prefLabel "Coriolis"@en ;
    skos:scopeNote "US Naval Research Laboratory Satellite"@en ;
    skos:topConceptOf cci-scheme:platform .

<http://vocab.ceda.ac.uk/collection/cci/platform/plat_cryosat2> a cci:platform,
        skos:Concept ;
    cci:hasSensor <http://vocab.ceda.ac.uk/collection/cci/sensor/sens_siral> ;
    rdfs:seeAlso <https://www.wmo-sat.info/oscar/satellites/view/39> ;
    skos:broader <http://vocab.ceda.ac.uk/collection/cci/platformProg/plat_cryosat_prog> ;
    skos:definition "ESA Operational satellite CryoSat-2"@en ;
    skos:inScheme cci-scheme:platform ;
    skos:prefLabel "CryoSat-2"@en ;
    skos:scopeNote "ESA Operational satellite CryoSat-2"@en ;
    skos:topConceptOf cci-scheme:platform .

<http://vocab.ceda.ac.uk/collection/cci/platform/plat_csk1> a cci:platform,
        skos:Concept ;
    cci:hasSensor <http://vocab.ceda.ac.uk/collection/cci/sensor/sens_sar2000> ;
    rdfs:seeAlso <https://www.wmo-sat.info/oscar/satellites/view/42> ;
    skos:broader <http://vocab.ceda.ac.uk/collection/cci/platformProg/plat_csk_prog> ;
    skos:definition "COSMO-SkyMed-1"@en ;
    skos:inScheme cci-scheme:platform ;
    skos:prefLabel "CSK-1"@en ;
    skos:scopeNote "COSMO-SkyMed-1"@en ;
    skos:topConceptOf cci-scheme:platform .

<http://vocab.ceda.ac.uk/collection/cci/platform/plat_csk2> a cci:platform,
        skos:Concept ;
    cci:hasSensor <http://vocab.ceda.ac.uk/collection/cci/sensor/sens_sar2000> ;
    rdfs:seeAlso <https://www.wmo-sat.info/oscar/satellites/view/43> ;
    skos:broader <http://vocab.ceda.ac.uk/collection/cci/platformProg/plat_csk_prog> ;
    skos:definition "COSMO-SkyMed-2"@en ;
    skos:inScheme cci-scheme:platform ;
    skos:prefLabel "CSK-2"@en ;
    skos:scopeNote "COSMO-SkyMed-2"@en ;
    skos:topConceptOf cci-scheme:platform .

<http://vocab.ceda.ac.uk/collection/cci/platform/plat_csk3> a cci:platform,
        skos:Concept ;
    cci:hasSensor <http://vocab.ceda.ac.uk/collection/cci/sensor/sens_sar2000> ;
    rdfs:seeAlso <https://www.wmo-sat.info/oscar/satellites/view/44> ;
    skos:broader <http://vocab.ceda.ac.uk/collection/cci/platformProg/plat_csk_prog> ;
    skos:definition "COSMO-SkyMed-3"@en ;
    skos:inScheme cci-scheme:platform ;
    skos:prefLabel "CSK-3"@en ;
    skos:scopeNote "COSMO-SkyMed-3"@en ;
    skos:topConceptOf cci-scheme:platform .

<http://vocab.ceda.ac.uk/collection/cci/platform/plat_csk4> a cci:platform,
        skos:Concept ;
    cci:hasSensor <http://vocab.ceda.ac.uk/collection/cci/sensor/sens_sar2000> ;
    rdfs:seeAlso <https://www.wmo-sat.info/oscar/satellites/view/45> ;
    skos:broader <http://vocab.ceda.ac.uk/collection/cci/platformProg/plat_csk_prog> ;
    skos:definition "COSMO-SkyMed-4"@en ;
    skos:inScheme cci-scheme:platform ;
    skos:prefLabel "CSK-4"@en ;
    skos:scopeNote "COSMO-SkyMed-4"@en ;
    skos:topConceptOf cci-scheme:platform .

<http://vocab.ceda.ac.uk/collection/cci/platform/plat_dmsp_F08> a cci:platform,
        skos:Concept ;
    cci:hasSensor <http://vocab.ceda.ac.uk/collection/cci/sensor/sens_ssmI> ;
    rdfs:seeAlso <http://www.wmo-sat.info/oscar/satellites/view/55> ;
    skos:broader <http://vocab.ceda.ac.uk/collection/cci/platformProg/plat_dmsp_5D2> ;
    skos:definition "US Defense Meteorological Satellite Program – F08"@en ;
    skos:inScheme cci-scheme:platform ;
    skos:prefLabel "DMSP-F08"@en ;
    skos:scopeNote "US Defense Meteorological Satellite Program – F08"@en ;
    skos:topConceptOf cci-scheme:platform .

<http://vocab.ceda.ac.uk/collection/cci/platform/plat_dmsp_F10> a cci:platform,
        skos:Concept ;
    cci:hasSensor <http://vocab.ceda.ac.uk/collection/cci/sensor/sens_ssmI> ;
    rdfs:seeAlso <http://www.wmo-sat.info/oscar/satellites/view/57> ;
    skos:broader <http://vocab.ceda.ac.uk/collection/cci/platformProg/plat_dmsp_5D2> ;
    skos:definition "US Defense Meteorological Satellite Program – F10"@en ;
    skos:inScheme cci-scheme:platform ;
    skos:prefLabel "DMSP-F10"@en ;
    skos:scopeNote "US Defense Meteorological Satellite Program – F10"@en ;
    skos:topConceptOf cci-scheme:platform .

<http://vocab.ceda.ac.uk/collection/cci/platform/plat_dmsp_F11> a cci:platform,
        skos:Concept ;
    cci:hasSensor <http://vocab.ceda.ac.uk/collection/cci/sensor/sens_ssmI> ;
    rdfs:seeAlso <http://www.wmo-sat.info/oscar/satellites/view/58> ;
    skos:broader <http://vocab.ceda.ac.uk/collection/cci/platformProg/plat_dmsp_5D2> ;
    skos:definition "US Defense Meteorological Satellite Program – F11"@en ;
    skos:inScheme cci-scheme:platform ;
    skos:prefLabel "DMSP-F11"@en ;
    skos:scopeNote "US Defense Meteorological Satellite Program – F11"@en ;
    skos:topConceptOf cci-scheme:platform .

<http://vocab.ceda.ac.uk/collection/cci/platform/plat_dmsp_F12> a cci:platform,
        skos:Concept ;
    cci:hasSensor <http://vocab.ceda.ac.uk/collection/cci/sensor/sens_ssmI> ;
    rdfs:seeAlso <http://www.wmo-sat.info/oscar/satellites/view/59> ;
    skos:broader <http://vocab.ceda.ac.uk/collection/cci/platformProg/plat_dmsp_5D2> ;
    skos:definition "US Defense Meteorological Satellite Program – F12"@en ;
    skos:inScheme cci-scheme:platform ;
    skos:prefLabel "DMSP-F12"@en ;
    skos:scopeNote "US Defense Meteorological Satellite Program – F12"@en ;
    skos:topConceptOf cci-scheme:platform .

<http://vocab.ceda.ac.uk/collection/cci/platform/plat_dmsp_F13> a cci:platform,
        skos:Concept ;
    cci:hasSensor <http://vocab.ceda.ac.uk/collection/cci/sensor/sens_ssmI> ;
    rdfs:seeAlso <http://www.wmo-sat.info/oscar/satellites/view/60> ;
    skos:broader <http://vocab.ceda.ac.uk/collection/cci/platformProg/plat_dmsp_5D2> ;
    skos:definition "US Defense Meteorological Satellite Program – F13"@en ;
    skos:inScheme cci-scheme:platform ;
    skos:prefLabel "DMSP-F13"@en ;
    skos:scopeNote "US Defense Meteorological Satellite Program – F13"@en ;
    skos:topConceptOf cci-scheme:platform .

<http://vocab.ceda.ac.uk/collection/cci/platform/plat_dmsp_F14> a cci:platform,
        skos:Concept ;
    cci:hasSensor <http://vocab.ceda.ac.uk/collection/cci/sensor/sens_ssmI> ;
    rdfs:seeAlso <http://www.wmo-sat.info/oscar/satellites/view/61> ;
    skos:broader <http://vocab.ceda.ac.uk/collection/cci/platformProg/plat_dmsp_5D2> ;
    skos:definition "US Defense Meteorological Satellite Program – F14"@en ;
    skos:inScheme cci-scheme:platform ;
    skos:prefLabel "DMSP-F14"@en ;
    skos:scopeNote "US Defense Meteorological Satellite Program – F14"@en ;
    skos:topConceptOf cci-scheme:platform .

<http://vocab.ceda.ac.uk/collection/cci/platform/plat_dmsp_F15> a cci:platform,
        skos:Concept ;
    cci:hasSensor <http://vocab.ceda.ac.uk/collection/cci/sensor/sens_ssmI> ;
    rdfs:seeAlso <http://www.wmo-sat.info/oscar/satellites/view/62> ;
    skos:broader <http://vocab.ceda.ac.uk/collection/cci/platformProg/plat_dmsp_5D3> ;
    skos:definition "US Defense Meteorological Satellite Program – F15"@en ;
    skos:inScheme cci-scheme:platform ;
    skos:prefLabel "DMSP-F15"@en ;
    skos:scopeNote "US Defense Meteorological Satellite Program – F15"@en ;
    skos:topConceptOf cci-scheme:platform .

<http://vocab.ceda.ac.uk/collection/cci/platform/plat_gcomW1> a cci:platform,
        skos:Concept ;
    cci:hasSensor <http://vocab.ceda.ac.uk/collection/cci/sensor/sens_amsr2> ;
    rdfs:seeAlso <http://www.wmo-sat.info/oscar/satellites/view/130> ;
    skos:broader <http://vocab.ceda.ac.uk/collection/cci/platformProg/plat_gcom> ;
    skos:definition "NASA Global Change Observation Mission for Water – 1"@en ;
    skos:inScheme cci-scheme:platform ;
    skos:prefLabel "GCOM-W1"@en ;
    skos:scopeNote "NASA Global Change Observation Mission for Water – 1"@en ;
    skos:topConceptOf cci-scheme:platform .

<http://vocab.ceda.ac.uk/collection/cci/platform/plat_gcomW2> a cci:platform,
        skos:Concept ;
    cci:hasSensor <http://vocab.ceda.ac.uk/collection/cci/sensor/sens_amsr2> ;
    rdfs:seeAlso <http://www.wmo-sat.info/oscar/satellites/view/131> ;
    skos:broader <http://vocab.ceda.ac.uk/collection/cci/platformProg/plat_gcom> ;
    skos:definition "NASA Global Change Observation Mission for Water – 2"@en ;
    skos:inScheme cci-scheme:platform ;
    skos:prefLabel "GCOM-W2"@en ;
    skos:scopeNote "NASA Global Change Observation Mission for Water – 2"@en ;
    skos:topConceptOf cci-scheme:platform .

<http://vocab.ceda.ac.uk/collection/cci/platform/plat_gcomW3> a cci:platform,
        skos:Concept ;
    cci:hasSensor <http://vocab.ceda.ac.uk/collection/cci/sensor/sens_amsr2> ;
    rdfs:seeAlso <http://www.wmo-sat.info/oscar/satellites/view/132> ;
    skos:broader <http://vocab.ceda.ac.uk/collection/cci/platformProg/plat_gcom> ;
    skos:definition "NASA Global Change Observation Mission for Water – 3"@en ;
    skos:inScheme cci-scheme:platform ;
    skos:prefLabel "GCOM-W3"@en ;
    skos:scopeNote "NASA Global Change Observation Mission for Water – 3"@en ;
    skos:topConceptOf cci-scheme:platform .

<http://vocab.ceda.ac.uk/collection/cci/platform/plat_gfo> a cci:platform,
        skos:Concept ;
    cci:hasSensor <http://vocab.ceda.ac.uk/collection/cci/sensor/sens_gfora> ;
    rdfs:seeAlso <http://www.wmo-sat.info/oscar/satellites/view/134> ;
    skos:broader <http://vocab.ceda.ac.uk/collection/cci/platformProg/plat_geodetic> ;
    skos:definition "US Geosat Follow-On Satellite"@en ;
    skos:inScheme cci-scheme:platform ;
    skos:prefLabel "GFO"@en ;
    skos:scopeNote "US Geosat Follow-On Satellite"@en ;
    skos:topConceptOf cci-scheme:platform .

<http://vocab.ceda.ac.uk/collection/cci/platform/plat_goes_08> a cci:platform,
        skos:Concept ;
    cci:hasSensor <http://vocab.ceda.ac.uk/collection/cci/sensor/sens_goesImager811> ;
    rdfs:seeAlso <http://www.wmo-sat.info/oscar/satellites/view/144> ;
    skos:broader <http://vocab.ceda.ac.uk/collection/cci/platformProg/plat_goes_2nd> ;
    skos:definition "NASA Geostationary Operational Environmental Satellite – 08"@en ;
    skos:inScheme cci-scheme:platform ;
    skos:prefLabel "GOES-8"@en ;
    skos:scopeNote "NASA Geostationary Operational Environmental Satellite – 08"@en ;
    skos:topConceptOf cci-scheme:platform .

<http://vocab.ceda.ac.uk/collection/cci/platform/plat_goes_09> a cci:platform,
        skos:Concept ;
    cci:hasSensor <http://vocab.ceda.ac.uk/collection/cci/sensor/sens_goesImager811> ;
    rdfs:seeAlso <http://www.wmo-sat.info/oscar/satellites/view/145> ;
    skos:broader <http://vocab.ceda.ac.uk/collection/cci/platformProg/plat_goes_2nd> ;
    skos:definition "NASA Geostationary Operational Environmental Satellite – 09"@en ;
    skos:inScheme cci-scheme:platform ;
    skos:prefLabel "GOES-9"@en ;
    skos:scopeNote "NASA Geostationary Operational Environmental Satellite – 09"@en ;
    skos:topConceptOf cci-scheme:platform .

<http://vocab.ceda.ac.uk/collection/cci/platform/plat_goes_09_bk> a cci:platform,
        skos:Concept ;
    cci:hasSensor <http://vocab.ceda.ac.uk/collection/cci/sensor/sens_goesImager811> ;
    rdfs:seeAlso <http://www.wmo-sat.info/oscar/satellites/view/536> ;
    skos:altLabel "GOES 09 Backup"@en ;
    skos:broader <http://vocab.ceda.ac.uk/collection/cci/platformProg/plat_goes_2nd> ;
    skos:definition "NASA Geostationary Operational Environmental Satellite – 09  GMS Backup"@en ;
    skos:inScheme cci-scheme:platform ;
    skos:prefLabel "GOES-9 Backup"@en ;
    skos:scopeNote "NASA Geostationary Operational Environmental Satellite – 09  GMS Backup"@en ;
    skos:topConceptOf cci-scheme:platform .

<http://vocab.ceda.ac.uk/collection/cci/platform/plat_goes_10> a cci:platform,
        skos:Concept ;
    cci:hasSensor <http://vocab.ceda.ac.uk/collection/cci/sensor/sens_goesImager811> ;
    rdfs:seeAlso <http://www.wmo-sat.info/oscar/satellites/view/146> ;
    skos:broader <http://vocab.ceda.ac.uk/collection/cci/platformProg/plat_goes_2nd> ;
    skos:definition "NASA Geostationary Operational Environmental Satellite – 10"@en ;
    skos:inScheme cci-scheme:platform ;
    skos:prefLabel "GOES-10"@en ;
    skos:scopeNote "NASA Geostationary Operational Environmental Satellite – 10"@en ;
    skos:topConceptOf cci-scheme:platform .

<http://vocab.ceda.ac.uk/collection/cci/platform/plat_goes_10_SA> a cci:platform,
        skos:Concept ;
    cci:hasSensor <http://vocab.ceda.ac.uk/collection/cci/sensor/sens_goesImager811> ;
    rdfs:seeAlso <http://www.wmo-sat.info/oscar/satellites/view/537> ;
    skos:altLabel "GOES 10 South America"@en ;
    skos:broader <http://vocab.ceda.ac.uk/collection/cci/platformProg/plat_goes_2nd> ;
    skos:definition "NASA Geostationary Operational Environmental Satellite – 10 South America"@en ;
    skos:inScheme cci-scheme:platform ;
    skos:prefLabel "GOES-10 S. America"@en ;
    skos:scopeNote "NASA Geostationary Operational Environmental Satellite – 10 South America"@en ;
    skos:topConceptOf cci-scheme:platform .

<http://vocab.ceda.ac.uk/collection/cci/platform/plat_goes_11> a cci:platform,
        skos:Concept ;
    cci:hasSensor <http://vocab.ceda.ac.uk/collection/cci/sensor/sens_goesImager811> ;
    rdfs:seeAlso <http://www.wmo-sat.info/oscar/satellites/view/147> ;
    skos:broader <http://vocab.ceda.ac.uk/collection/cci/platformProg/plat_goes_2nd> ;
    skos:definition "NASA Geostationary Operational Environmental Satellite – 11"@en ;
    skos:inScheme cci-scheme:platform ;
    skos:prefLabel "GOES-11"@en ;
    skos:scopeNote "NASA Geostationary Operational Environmental Satellite – 11"@en ;
    skos:topConceptOf cci-scheme:platform .

<http://vocab.ceda.ac.uk/collection/cci/platform/plat_goes_12> a cci:platform,
        skos:Concept ;
    cci:hasSensor <http://vocab.ceda.ac.uk/collection/cci/sensor/sens_goesImager1215> ;
    rdfs:seeAlso <http://www.wmo-sat.info/oscar/satellites/view/148> ;
    skos:broader <http://vocab.ceda.ac.uk/collection/cci/platformProg/plat_goes_2nd> ;
    skos:definition "NASA Geostationary Operational Environmental Satellite – 12"@en ;
    skos:inScheme cci-scheme:platform ;
    skos:prefLabel "GOES-12"@en ;
    skos:scopeNote "NASA Geostationary Operational Environmental Satellite – 12"@en ;
    skos:topConceptOf cci-scheme:platform .

<http://vocab.ceda.ac.uk/collection/cci/platform/plat_goes_12_SA> a cci:platform,
        skos:Concept ;
    cci:hasSensor <http://vocab.ceda.ac.uk/collection/cci/sensor/sens_goesImager1215> ;
    rdfs:seeAlso <http://www.wmo-sat.info/oscar/satellites/view/538> ;
    skos:altLabel "GOES 12 South America"@en ;
    skos:broader <http://vocab.ceda.ac.uk/collection/cci/platformProg/plat_goes_2nd> ;
    skos:definition "NASA Geostationary Operational Environmental Satellite – 12 South America"@en ;
    skos:inScheme cci-scheme:platform ;
    skos:prefLabel "GOES 12 S. America"@en ;
    skos:scopeNote "NASA Geostationary Operational Environmental Satellite – 12 South America"@en ;
    skos:topConceptOf cci-scheme:platform .

<http://vocab.ceda.ac.uk/collection/cci/platform/plat_goes_13> a cci:platform,
        skos:Concept ;
    cci:hasSensor <http://vocab.ceda.ac.uk/collection/cci/sensor/sens_goesImager1215> ;
    rdfs:seeAlso <http://www.wmo-sat.info/oscar/satellites/view/149> ;
    skos:broader <http://vocab.ceda.ac.uk/collection/cci/platformProg/plat_goes_2nd> ;
    skos:definition "NASA Geostationary Operational Environmental Satellite – 13"@en ;
    skos:inScheme cci-scheme:platform ;
    skos:prefLabel "GOES-13"@en ;
    skos:scopeNote "NASA Geostationary Operational Environmental Satellite – 13"@en ;
    skos:topConceptOf cci-scheme:platform .

<http://vocab.ceda.ac.uk/collection/cci/platform/plat_goes_14> a cci:platform,
        skos:Concept ;
    cci:hasSensor <http://vocab.ceda.ac.uk/collection/cci/sensor/sens_goesImager1215> ;
    rdfs:seeAlso <http://www.wmo-sat.info/oscar/satellites/view/150> ;
    skos:broader <http://vocab.ceda.ac.uk/collection/cci/platformProg/plat_goes_2nd> ;
    skos:definition "NASA Geostationary Operational Environmental Satellite – 14"@en ;
    skos:inScheme cci-scheme:platform ;
    skos:prefLabel "GOES-14"@en ;
    skos:scopeNote "NASA Geostationary Operational Environmental Satellite – 14"@en ;
    skos:topConceptOf cci-scheme:platform .

<http://vocab.ceda.ac.uk/collection/cci/platform/plat_goes_15> a cci:platform,
        skos:Concept ;
    cci:hasSensor <http://vocab.ceda.ac.uk/collection/cci/sensor/sens_goesImager1215> ;
    rdfs:seeAlso <http://www.wmo-sat.info/oscar/satellites/view/151> ;
    skos:broader <http://vocab.ceda.ac.uk/collection/cci/platformProg/plat_goes_2nd> ;
    skos:definition "NASA Geostationary Operational Environmental Satellite – 15"@en ;
    skos:inScheme cci-scheme:platform ;
    skos:prefLabel "GOES-15"@en ;
    skos:scopeNote "NASA Geostationary Operational Environmental Satellite – 15"@en ;
    skos:topConceptOf cci-scheme:platform .

<http://vocab.ceda.ac.uk/collection/cci/platform/plat_goes_16> a cci:platform,
        skos:Concept ;
    cci:hasSensor <http://vocab.ceda.ac.uk/collection/cci/sensor/sens_abi> ;
    rdfs:seeAlso <https://space.oscar.wmo.int/satellites/view/goes_16> ;
    skos:altLabel "GOES-R"@en ;
    skos:broader <http://vocab.ceda.ac.uk/collection/cci/platformProg/plat_goes_3rd> ;
    skos:definition "NASA Geostationary Operational Environmental Satellite – 16"@en ;
    skos:inScheme cci-scheme:platform ;
    skos:prefLabel "GOES-16"@en ;
    skos:scopeNote "NASA Geostationary Operational Environmental Satellite – 16"@en ;
    skos:topConceptOf cci-scheme:platform .

<http://vocab.ceda.ac.uk/collection/cci/platform/plat_goes_17> a cci:platform,
        skos:Concept ;
    cci:hasSensor <http://vocab.ceda.ac.uk/collection/cci/sensor/sens_abi> ;
    rdfs:seeAlso <https://space.oscar.wmo.int/satellites/view/goes_17> ;
    skos:altLabel "GOES-S"@en ;
    skos:broader <http://vocab.ceda.ac.uk/collection/cci/platformProg/plat_goes_3rd> ;
    skos:definition "NASA Geostationary Operational Environmental Satellite – 17"@en ;
    skos:inScheme cci-scheme:platform ;
    skos:prefLabel "GOES-17"@en ;
    skos:scopeNote "NASA Geostationary Operational Environmental Satellite – 17"@en ;
    skos:topConceptOf cci-scheme:platform .

<http://vocab.ceda.ac.uk/collection/cci/platform/plat_gosat-2> a cci:platform,
        skos:Concept ;
    cci:hasSensor <http://vocab.ceda.ac.uk/collection/cci/sensor/sens_tansoFts2> ;
    rdfs:seeAlso <http://www.wmo-sat.info/oscar/satellites/view/155> ;
    skos:altLabel "GOSAT"@en ;
    skos:broader <http://vocab.ceda.ac.uk/collection/cci/platformProg/plat_gosat_prog> ;
    skos:definition "JAXA Greenhouse gas Observing Satellite – 2"@en ;
    skos:inScheme cci-scheme:platform ;
    skos:prefLabel "GOSAT-2"@en ;
    skos:scopeNote "JAXA Greenhouse gas Observing Satellite – 2"@en ;
    skos:topConceptOf cci-scheme:platform .

<http://vocab.ceda.ac.uk/collection/cci/platform/plat_gpm> a cci:platform,
        skos:Concept ;
    cci:hasSensor <http://vocab.ceda.ac.uk/collection/cci/sensor/sens_gmi> ;
    rdfs:seeAlso <https://www.wmo-sat.info/oscar/satellites/view/gpm_core_observatory> ;
    skos:altLabel "GPM Core Observatory"@en ;
    skos:broader <http://vocab.ceda.ac.uk/collection/cci/platformProg/plat_gpm_prog> ;
    skos:definition "Global Precipitation Mission -  Core Observatory"@en ;
    skos:inScheme cci-scheme:platform ;
    skos:prefLabel "GPM Core"@en ;
    skos:scopeNote "Global Precipitation Mission -  Core Observatory"@en ;
    skos:topConceptOf cci-scheme:platform .

<http://vocab.ceda.ac.uk/collection/cci/platform/plat_grace> a cci:platform,
        skos:Concept ;
    cci:hasSensor <http://vocab.ceda.ac.uk/collection/cci/sensor/sens_grace> ;
    rdfs:seeAlso <https://www.wmo-sat.info/oscar/satellites/view/158> ;
    skos:broader <http://vocab.ceda.ac.uk/collection/cci/platformProg/plat_grace_prog> ;
    skos:definition "NASA Gravity Recovery and Climate Experiment"@en ;
    skos:inScheme cci-scheme:platform ;
    skos:prefLabel "GRACE"@en ;
    skos:scopeNote "NASA Gravity Recovery and Climate Experiment"@en ;
    skos:topConceptOf cci-scheme:platform .

<http://vocab.ceda.ac.uk/collection/cci/platform/plat_himawari-6> a cci:platform,
        skos:Concept ;
    cci:hasSensor <http://vocab.ceda.ac.uk/collection/cci/sensor/sens_jami> ;
    rdfs:seeAlso <http://www.wmo-sat.info/oscar/satellites/view/165> ;
    skos:altLabel "MTSAT1R"@en ;
    skos:broader <http://vocab.ceda.ac.uk/collection/cci/platformProg/plat_himawari> ;
    skos:definition "JMA Meteorological Satellite"@en ;
    skos:inScheme cci-scheme:platform ;
    skos:prefLabel "Himawari-6"@en ;
    skos:scopeNote "JMA Meteorological Satellite"@en ;
    skos:topConceptOf cci-scheme:platform .

<http://vocab.ceda.ac.uk/collection/cci/platform/plat_himawari-7> a cci:platform,
        skos:Concept ;
    cci:hasSensor <http://vocab.ceda.ac.uk/collection/cci/sensor/sens_imagerMtsat2> ;
    rdfs:seeAlso <http://www.wmo-sat.info/oscar/satellites/view/166> ;
    skos:altLabel "MTSAT2"@en ;
    skos:broader <http://vocab.ceda.ac.uk/collection/cci/platformProg/plat_himawari> ;
    skos:definition "JMA Meteorological Satellite"@en ;
    skos:inScheme cci-scheme:platform ;
    skos:prefLabel "Himawari-7"@en ;
    skos:scopeNote "JMA Meteorological Satellite"@en ;
    skos:topConceptOf cci-scheme:platform .

<http://vocab.ceda.ac.uk/collection/cci/platform/plat_icesat> a cci:platform,
        skos:Concept ;
    cci:hasSensor <http://vocab.ceda.ac.uk/collection/cci/sensor/sens_glas> ;
    rdfs:seeAlso <http://www.wmo-sat.info/oscar/satellites/view/177> ;
    skos:broader <http://vocab.ceda.ac.uk/collection/cci/platformProg/plat_icesat_prog> ;
    skos:definition "NASA Ice, Cloud and land Elevation Satellite"@en ;
    skos:inScheme cci-scheme:platform ;
    skos:prefLabel "ICESat"@en ;
    skos:scopeNote "NASA Ice, Cloud and land Elevation Satellite"@en ;
    skos:topConceptOf cci-scheme:platform .

<http://vocab.ceda.ac.uk/collection/cci/platform/plat_jason1> a cci:platform,
        skos:Concept ;
    cci:hasSensor <http://vocab.ceda.ac.uk/collection/cci/sensor/sens_poseidon2> ;
    rdfs:seeAlso <http://www.wmo-sat.info/oscar/satellites/view/204> ;
    skos:broader <http://vocab.ceda.ac.uk/collection/cci/platformProg/plat_jason> ;
    skos:definition "NASA Joint Altimetry Satellite Oceanography Network – 1"@en ;
    skos:inScheme cci-scheme:platform ;
    skos:prefLabel "Jason-1"@en ;
    skos:scopeNote "NASA Joint Altimetry Satellite Oceanography Network – 1"@en ;
    skos:topConceptOf cci-scheme:platform .

<http://vocab.ceda.ac.uk/collection/cci/platform/plat_jason2> a cci:platform,
        skos:Concept ;
    cci:hasSensor <http://vocab.ceda.ac.uk/collection/cci/sensor/sens_poseidon3> ;
    rdfs:seeAlso <http://www.wmo-sat.info/oscar/satellites/view/205> ;
    skos:broader <http://vocab.ceda.ac.uk/collection/cci/platformProg/plat_jason> ;
    skos:definition "NASA Joint Altimetry Satellite Oceanography Network – 2"@en ;
    skos:inScheme cci-scheme:platform ;
    skos:prefLabel "Jason-2"@en ;
    skos:scopeNote "NASA Joint Altimetry Satellite Oceanography Network – 2"@en ;
    skos:topConceptOf cci-scheme:platform .

<http://vocab.ceda.ac.uk/collection/cci/platform/plat_jason3> a cci:platform,
        skos:Concept ;
    cci:hasSensor <http://vocab.ceda.ac.uk/collection/cci/sensor/sens_poseidon3b> ;
    rdfs:seeAlso <http://www.wmo-sat.info/oscar/satellites/view/206> ;
    skos:broader <http://vocab.ceda.ac.uk/collection/cci/platformProg/plat_jason> ;
    skos:definition "NASA Joint Altimetry Satellite Oceanography Network – 3"@en ;
    skos:inScheme cci-scheme:platform ;
    skos:prefLabel "Jason-3"@en ;
    skos:scopeNote "NASA Joint Altimetry Satellite Oceanography Network – 3"@en ;
    skos:topConceptOf cci-scheme:platform .

<http://vocab.ceda.ac.uk/collection/cci/platform/plat_landsat_1> a cci:platform,
        skos:Concept ;
    cci:hasSensor <http://vocab.ceda.ac.uk/collection/cci/sensor/sens_mss> ;
    rdfs:seeAlso <http://www.wmo-sat.info/oscar/satellites/view/219> ;
    skos:altLabel "Landsat ERTS"@en ;
    skos:broader <http://vocab.ceda.ac.uk/collection/cci/platformProg/plat_landsat> ;
    skos:definition "NASA Landsat"@en ;
    skos:inScheme cci-scheme:platform ;
    skos:prefLabel "Landsat-1"@en ;
    skos:scopeNote "NASA Landsat"@en ;
    skos:topConceptOf cci-scheme:platform .

<http://vocab.ceda.ac.uk/collection/cci/platform/plat_landsat_2> a cci:platform,
        skos:Concept ;
    cci:hasSensor <http://vocab.ceda.ac.uk/collection/cci/sensor/sens_mss> ;
    rdfs:seeAlso <http://www.wmo-sat.info/oscar/satellites/view/220> ;
    skos:broader <http://vocab.ceda.ac.uk/collection/cci/platformProg/plat_landsat> ;
    skos:definition "NASA Landsat"@en ;
    skos:inScheme cci-scheme:platform ;
    skos:prefLabel "Landsat-2"@en ;
    skos:scopeNote "NASA Landsat"@en ;
    skos:topConceptOf cci-scheme:platform .

<http://vocab.ceda.ac.uk/collection/cci/platform/plat_landsat_3> a cci:platform,
        skos:Concept ;
    cci:hasSensor <http://vocab.ceda.ac.uk/collection/cci/sensor/sens_mss> ;
    rdfs:seeAlso <http://www.wmo-sat.info/oscar/satellites/view/221> ;
    skos:broader <http://vocab.ceda.ac.uk/collection/cci/platformProg/plat_landsat> ;
    skos:definition "NASA Landsat"@en ;
    skos:inScheme cci-scheme:platform ;
    skos:prefLabel "Landsat-3"@en ;
    skos:scopeNote "NASA Landsat"@en ;
    skos:topConceptOf cci-scheme:platform .

<http://vocab.ceda.ac.uk/collection/cci/platform/plat_landsat_7> a cci:platform,
        skos:Concept ;
    cci:hasSensor <http://vocab.ceda.ac.uk/collection/cci/sensor/sens_tm> ;
    rdfs:seeAlso <http://www.wmo-sat.info/oscar/satellites/view/225> ;
    skos:broader <http://vocab.ceda.ac.uk/collection/cci/platformProg/plat_landsat> ;
    skos:definition "NASA Landsat"@en ;
    skos:inScheme cci-scheme:platform ;
    skos:prefLabel "Landsat-7"@en ;
    skos:scopeNote "NASA Landsat"@en ;
    skos:topConceptOf cci-scheme:platform .

<http://vocab.ceda.ac.uk/collection/cci/platform/plat_meteosat_1> a cci:platform,
        skos:Concept ;
    cci:hasSensor <http://vocab.ceda.ac.uk/collection/cci/sensor/sens_mviri> ;
    rdfs:seeAlso <https://www.wmo-sat.info/oscar/satellites/view/295> ;
    skos:broader <http://vocab.ceda.ac.uk/collection/cci/platformProg/plat_mfg_prog> ;
    skos:definition "EUMETSAT /ESA Meteosat-1"@en ;
    skos:inScheme cci-scheme:platform ;
    skos:prefLabel "Meteosat-1"@en ;
    skos:scopeNote "EUMETSAT /ESA Meteosat-1"@en ;
    skos:topConceptOf cci-scheme:platform .

<http://vocab.ceda.ac.uk/collection/cci/platform/plat_meteosat_10> a cci:platform,
        skos:Concept ;
    cci:hasSensor <http://vocab.ceda.ac.uk/collection/cci/sensor/sens_seviri> ;
    rdfs:seeAlso <http://www.wmo-sat.info/oscar/satellites/view/304> ;
    skos:altLabel "MSG-3"@en ;
    skos:broader <http://vocab.ceda.ac.uk/collection/cci/platformProg/plat_msg> ;
    skos:definition "ESA Meteosat-10"@en ;
    skos:inScheme cci-scheme:platform ;
    skos:prefLabel "Meteosat-10"@en ;
    skos:scopeNote "ESA Meteosat-10"@en ;
    skos:topConceptOf cci-scheme:platform .

<http://vocab.ceda.ac.uk/collection/cci/platform/plat_meteosat_11> a cci:platform,
        skos:Concept ;
    cci:hasSensor <http://vocab.ceda.ac.uk/collection/cci/sensor/sens_seviri> ;
    rdfs:seeAlso <http://www.wmo-sat.info/oscar/satellites/view/305> ;
    skos:altLabel "MSG-4"@en ;
    skos:broader <http://vocab.ceda.ac.uk/collection/cci/platformProg/plat_msg> ;
    skos:definition "ESA Meteosat-11"@en ;
    skos:inScheme cci-scheme:platform ;
    skos:prefLabel "Meteosat-11"@en ;
    skos:scopeNote "ESA Meteosat-11"@en ;
    skos:topConceptOf cci-scheme:platform .

<http://vocab.ceda.ac.uk/collection/cci/platform/plat_meteosat_2> a cci:platform,
        skos:Concept ;
    cci:hasSensor <http://vocab.ceda.ac.uk/collection/cci/sensor/sens_mviri> ;
    rdfs:seeAlso <https://www.wmo-sat.info/oscar/satellites/view/296> ;
    skos:broader <http://vocab.ceda.ac.uk/collection/cci/platformProg/plat_mfg_prog> ;
    skos:definition "EUMETSAT /ESA Meteosat-2"@en ;
    skos:inScheme cci-scheme:platform ;
    skos:prefLabel "Meteosat-2"@en ;
    skos:scopeNote "EUMETSAT /ESA Meteosat-2"@en ;
    skos:topConceptOf cci-scheme:platform .

<http://vocab.ceda.ac.uk/collection/cci/platform/plat_meteosat_3> a cci:platform,
        skos:Concept ;
    cci:hasSensor <http://vocab.ceda.ac.uk/collection/cci/sensor/sens_mviri> ;
    rdfs:seeAlso <https://www.wmo-sat.info/oscar/satellites/view/297> ;
    skos:broader <http://vocab.ceda.ac.uk/collection/cci/platformProg/plat_mfg_prog> ;
    skos:definition "EUMETSAT/ESA Meteosat-3"@en ;
    skos:inScheme cci-scheme:platform ;
    skos:prefLabel "Meteosat-3"@en ;
    skos:scopeNote "EUMETSAT/ESA Meteosat-3"@en ;
    skos:topConceptOf cci-scheme:platform .

<http://vocab.ceda.ac.uk/collection/cci/platform/plat_meteosat_3_adc> a cci:platform,
        skos:Concept ;
    cci:hasSensor <http://vocab.ceda.ac.uk/collection/cci/sensor/sens_mviri> ;
    rdfs:seeAlso <https://www.wmo-sat.info/oscar/satellites/view/531> ;
    skos:broader <http://vocab.ceda.ac.uk/collection/cci/platformProg/plat_mfg_prog> ;
    skos:definition "EUMETSAT/ ESA Meteosat-3 (Atlantic Data Coverage)"@en ;
    skos:inScheme cci-scheme:platform ;
    skos:prefLabel "Meteosat-3 (ADC)"@en ;
    skos:scopeNote "EUMETSAT/ ESA Meteosat-3 (Atlantic Data Coverage)"@en ;
    skos:topConceptOf cci-scheme:platform .

<http://vocab.ceda.ac.uk/collection/cci/platform/plat_meteosat_3_xadc> a cci:platform,
        skos:Concept ;
    cci:hasSensor <http://vocab.ceda.ac.uk/collection/cci/sensor/sens_mviri> ;
    rdfs:seeAlso <https://www.wmo-sat.info/oscar/satellites/view/532> ;
    skos:broader <http://vocab.ceda.ac.uk/collection/cci/platformProg/plat_mfg_prog> ;
    skos:definition "EUMETSAT/ESA Meteosat-3 (Extended Atlantic Data Coverage)"@en ;
    skos:inScheme cci-scheme:platform ;
    skos:prefLabel "Meteosat-3 (X-ADC)"@en ;
    skos:scopeNote "EUMETSAT/ESA Meteosat-3 (Extended Atlantic Data Coverage)"@en ;
    skos:topConceptOf cci-scheme:platform .

<http://vocab.ceda.ac.uk/collection/cci/platform/plat_meteosat_4> a cci:platform,
        skos:Concept ;
    cci:hasSensor <http://vocab.ceda.ac.uk/collection/cci/sensor/sens_mviri> ;
    rdfs:seeAlso <https://www.wmo-sat.info/oscar/satellites/view/298> ;
    skos:broader <http://vocab.ceda.ac.uk/collection/cci/platformProg/plat_mfg_prog> ;
    skos:definition "EUMETSAT/ESA Meteosat-4"@en ;
    skos:inScheme cci-scheme:platform ;
    skos:prefLabel "Meteosat-4"@en ;
    skos:scopeNote "EUMETSAT/ESA Meteosat-4"@en ;
    skos:topConceptOf cci-scheme:platform .

<http://vocab.ceda.ac.uk/collection/cci/platform/plat_meteosat_5> a cci:platform,
        skos:Concept ;
    cci:hasSensor <http://vocab.ceda.ac.uk/collection/cci/sensor/sens_mviri> ;
    rdfs:seeAlso <https://www.wmo-sat.info/oscar/satellites/view/299> ;
    skos:broader <http://vocab.ceda.ac.uk/collection/cci/platformProg/plat_mfg_prog> ;
    skos:definition "EUMETSAT/ESA Meteosat-5"@en ;
    skos:inScheme cci-scheme:platform ;
    skos:prefLabel "Meteosat-5"@en ;
    skos:scopeNote "EUMETSAT/ESA Meteosat-5"@en ;
    skos:topConceptOf cci-scheme:platform .

<http://vocab.ceda.ac.uk/collection/cci/platform/plat_meteosat_5_iodc> a cci:platform,
        skos:Concept ;
    cci:hasSensor <http://vocab.ceda.ac.uk/collection/cci/sensor/sens_mviri> ;
    rdfs:seeAlso <https://www.wmo-sat.info/oscar/satellites/view/533> ;
    skos:broader <http://vocab.ceda.ac.uk/collection/cci/platformProg/plat_mfg_prog> ;
    skos:definition "EUMETSAT/ESA Meteosat-5 (Indian Ocean Data Coverage)"@en ;
    skos:inScheme cci-scheme:platform ;
    skos:prefLabel "Meteosat-5 (IODC)"@en ;
    skos:scopeNote "EUMETSAT/ESA Meteosat-5 (Indian Ocean Data Coverage)"@en ;
    skos:topConceptOf cci-scheme:platform .

<http://vocab.ceda.ac.uk/collection/cci/platform/plat_meteosat_6> a cci:platform,
        skos:Concept ;
    cci:hasSensor <http://vocab.ceda.ac.uk/collection/cci/sensor/sens_mviri> ;
    rdfs:seeAlso <https://www.wmo-sat.info/oscar/satellites/view/300> ;
    skos:broader <http://vocab.ceda.ac.uk/collection/cci/platformProg/plat_mfg_prog> ;
    skos:definition "EUMETSAT/ESA Meteosat-6"@en ;
    skos:inScheme cci-scheme:platform ;
    skos:prefLabel "Meteosat-6"@en ;
    skos:scopeNote "EUMETSAT/ESA Meteosat-6"@en ;
    skos:topConceptOf cci-scheme:platform .

<http://vocab.ceda.ac.uk/collection/cci/platform/plat_meteosat_6_iodc> a cci:platform,
        skos:Concept ;
    cci:hasSensor <http://vocab.ceda.ac.uk/collection/cci/sensor/sens_mviri> ;
    rdfs:seeAlso <https://www.wmo-sat.info/oscar/satellites/view/534> ;
    skos:broader <http://vocab.ceda.ac.uk/collection/cci/platformProg/plat_mfg_prog> ;
    skos:definition "EUMETSAT/ESA Meteosat-6 (Indian Ocean Data Coverage)"@en ;
    skos:inScheme cci-scheme:platform ;
    skos:prefLabel "Meteosat-6 (IODC)"@en ;
    skos:scopeNote "EUMETSAT/ESA Meteosat-6 (Indian Ocean Data Coverage)"@en ;
    skos:topConceptOf cci-scheme:platform .

<http://vocab.ceda.ac.uk/collection/cci/platform/plat_meteosat_7> a cci:platform,
        skos:Concept ;
    cci:hasSensor <http://vocab.ceda.ac.uk/collection/cci/sensor/sens_mviri> ;
    rdfs:seeAlso <https://www.wmo-sat.info/oscar/satellites/view/535> ;
    skos:broader <http://vocab.ceda.ac.uk/collection/cci/platformProg/plat_mfg_prog> ;
    skos:definition "EUMETSAT/ESA Meteosat-7"@en ;
    skos:inScheme cci-scheme:platform ;
    skos:prefLabel "Meteosat-7"@en ;
    skos:scopeNote "EUMETSAT/ESA Meteosat-7"@en ;
    skos:topConceptOf cci-scheme:platform .

<http://vocab.ceda.ac.uk/collection/cci/platform/plat_meteosat_7_iodc> a cci:platform,
        skos:Concept ;
    cci:hasSensor <http://vocab.ceda.ac.uk/collection/cci/sensor/sens_mviri> ;
    rdfs:seeAlso <https://www.wmo-sat.info/oscar/satellites/view/301> ;
    skos:broader <http://vocab.ceda.ac.uk/collection/cci/platformProg/plat_mfg_prog> ;
    skos:definition "EUMETSAT/ESA Meteosat-7 (Indian Ocean Data Coverage)"@en ;
    skos:inScheme cci-scheme:platform ;
    skos:prefLabel "Meteosat-7 (IODC)"@en ;
    skos:scopeNote "EUMETSAT/ESA Meteosat-7 (Indian Ocean Data Coverage)"@en ;
    skos:topConceptOf cci-scheme:platform .

<http://vocab.ceda.ac.uk/collection/cci/platform/plat_meteosat_8> a cci:platform,
        skos:Concept ;
    cci:hasSensor <http://vocab.ceda.ac.uk/collection/cci/sensor/sens_seviri> ;
    rdfs:seeAlso <http://www.wmo-sat.info/oscar/satellites/view/302> ;
    skos:altLabel "MSG-1"@en ;
    skos:broader <http://vocab.ceda.ac.uk/collection/cci/platformProg/plat_msg> ;
    skos:definition "ESA Meteosat-8"@en ;
    skos:inScheme cci-scheme:platform ;
    skos:prefLabel "Meteosat-8"@en ;
    skos:scopeNote "ESA Meteosat-8"@en ;
    skos:topConceptOf cci-scheme:platform .

<http://vocab.ceda.ac.uk/collection/cci/platform/plat_meteosat_9> a cci:platform,
        skos:Concept ;
    cci:hasSensor <http://vocab.ceda.ac.uk/collection/cci/sensor/sens_seviri> ;
    rdfs:seeAlso <http://www.wmo-sat.info/oscar/satellites/view/303> ;
    skos:altLabel "MSG-2"@en ;
    skos:broader <http://vocab.ceda.ac.uk/collection/cci/platformProg/plat_msg> ;
    skos:definition "ESA Meteosat-9"@en ;
    skos:inScheme cci-scheme:platform ;
    skos:prefLabel "Meteosat-9"@en ;
    skos:scopeNote "ESA Meteosat-9"@en ;
    skos:topConceptOf cci-scheme:platform .

<http://vocab.ceda.ac.uk/collection/cci/platform/plat_nimbus5> a cci:platform,
        skos:Concept ;
    cci:hasSensor <http://vocab.ceda.ac.uk/collection/cci/sensor/sens_esmrNim5> ;
    rdfs:seeAlso <http://www.wmo-sat.info/oscar/satellites/view/319> ;
    skos:broader <http://vocab.ceda.ac.uk/collection/cci/platformProg/plat_nimbus> ;
    skos:definition "NASA Research-and-development satellite 5"@en ;
    skos:inScheme cci-scheme:platform ;
    skos:prefLabel "Nimbus-5"@en ;
    skos:scopeNote "NASA Research-and-development satellite 5"@en ;
    skos:topConceptOf cci-scheme:platform .

<http://vocab.ceda.ac.uk/collection/cci/platform/plat_nimbus7> a cci:platform,
        skos:Concept ;
    cci:hasSensor <http://vocab.ceda.ac.uk/collection/cci/sensor/sens_smmr>,
        <http://vocab.ceda.ac.uk/collection/cci/sensor/sens_toms> ;
    rdfs:seeAlso <http://www.wmo-sat.info/oscar/satellites/view/321> ;
    skos:broader <http://vocab.ceda.ac.uk/collection/cci/platformProg/plat_nimbus> ;
    skos:definition "NASA Research-and-development satellite 7"@en ;
    skos:inScheme cci-scheme:platform ;
    skos:prefLabel "Nimbus-7"@en ;
    skos:scopeNote "NASA Research-and-development satellite 7"@en ;
    skos:topConceptOf cci-scheme:platform .

<http://vocab.ceda.ac.uk/collection/cci/platform/plat_oco2> a cci:platform,
        skos:Concept ;
    cci:hasSensor <http://vocab.ceda.ac.uk/collection/cci/sensor/sens_oco> ;
    rdfs:seeAlso <https://www.wmo-sat.info/oscar/satellites/view/347> ;
    skos:broader <http://vocab.ceda.ac.uk/collection/cci/platformProg/plat_oco_prog> ;
    skos:definition "Orbiting Carbon Observatory – 2"@en ;
    skos:inScheme cci-scheme:platform ;
    skos:prefLabel "OCO-2"@en ;
    skos:scopeNote "Orbiting Carbon Observatory – 2"@en ;
    skos:topConceptOf cci-scheme:platform .

<http://vocab.ceda.ac.uk/collection/cci/platform/plat_orbview2> a cci:platform,
        skos:Concept ;
    cci:hasSensor <http://vocab.ceda.ac.uk/collection/cci/sensor/sens_seaWiFs> ;
    rdfs:seeAlso <http://www.wmo-sat.info/oscar/satellites/view/395> ;
    skos:altLabel "SeaStar"@en ;
    skos:broader <http://vocab.ceda.ac.uk/collection/cci/platformProg/plat_orbview2_prog> ;
    skos:definition "OIC USA Ocean Imaging satellite"@en ;
    skos:inScheme cci-scheme:platform ;
    skos:prefLabel "Orbview-2"@en ;
    skos:scopeNote "OIC USA Ocean Imaging satellite"@en ;
    skos:topConceptOf cci-scheme:platform .

<http://vocab.ceda.ac.uk/collection/cci/platform/plat_parasol> a cci:platform,
        skos:Concept ;
    cci:hasSensor <http://vocab.ceda.ac.uk/collection/cci/sensor/sens_polder> ;
    rdfs:seeAlso <http://www.wmo-sat.info/oscar/satellites/view/359> ;
    skos:broader <http://vocab.ceda.ac.uk/collection/cci/platformProg/plat_parasol_prog> ;
    skos:definition "CNES Polarization & Anisotropy of Reflectances for Atmospheric Sciences coupled with Observations from a Lidar"@en ;
    skos:inScheme cci-scheme:platform ;
    skos:prefLabel "PARASOL"@en ;
    skos:scopeNote "CNES Polarization & Anisotropy of Reflectances for Atmospheric Sciences coupled with Observations from a Lidar"@en ;
    skos:topConceptOf cci-scheme:platform .

<http://vocab.ceda.ac.uk/collection/cci/platform/plat_probaV> a cci:platform,
        skos:Concept ;
    cci:hasSensor <http://vocab.ceda.ac.uk/collection/cci/sensor/sens_vegetationP> ;
    rdfs:seeAlso <https://www.wmo-sat.info/oscar/satellites/view/562> ;
    skos:broader <http://vocab.ceda.ac.uk/collection/cci/platformProg/plat_proba_prog> ;
    skos:definition "Project for On-Board Autonomy – Végétation"@en ;
    skos:inScheme cci-scheme:platform ;
    skos:prefLabel "PROBA-V"@en ;
    skos:scopeNote "Project for On-Board Autonomy – Végétation"@en ;
    skos:topConceptOf cci-scheme:platform .

<http://vocab.ceda.ac.uk/collection/cci/platform/plat_sac_d> a cci:platform,
        skos:Concept ;
    cci:hasSensor <http://vocab.ceda.ac.uk/collection/cci/sensor/sens_aquarius> ;
    rdfs:seeAlso <https://www.wmo-sat.info/oscar/satellites/view/385> ;
    skos:broader <http://vocab.ceda.ac.uk/collection/cci/platformProg/plat_sac_prog> ;
    skos:definition "Satélite de Aplicaciones Cientificas - D"@en ;
    skos:inScheme cci-scheme:platform ;
    skos:prefLabel "SAC-D"@en ;
    skos:scopeNote "Satélite de Aplicaciones Cientificas - D"@en ;
    skos:topConceptOf cci-scheme:platform .

<http://vocab.ceda.ac.uk/collection/cci/platform/plat_saral> a cci:platform,
        skos:Concept ;
    cci:hasSensor <http://vocab.ceda.ac.uk/collection/cci/sensor/sens_altika> ;
    rdfs:seeAlso <https://www.wmo-sat.info/oscar/satellites/view/390> ;
    skos:broader <http://vocab.ceda.ac.uk/collection/cci/platformProg/plat_saral_prog> ;
    skos:definition "CNES Satellite with ARGOS and AltiKa"@en ;
    skos:inScheme cci-scheme:platform ;
    skos:prefLabel "SARAL"@en ;
    skos:scopeNote "CNES Satellite with ARGOS and AltiKa"@en ;
    skos:topConceptOf cci-scheme:platform .

<http://vocab.ceda.ac.uk/collection/cci/platform/plat_scisat> a cci:platform,
        skos:Concept ;
    cci:hasSensor <http://vocab.ceda.ac.uk/collection/cci/sensor/sens_aceFts> ;
    rdfs:seeAlso <http://www.wmo-sat.info/oscar/satellites/view/393> ;
    skos:broader <http://vocab.ceda.ac.uk/collection/cci/platformProg/plat_scisat_prog> ;
    skos:definition "CSA Science Satellite"@en ;
    skos:inScheme cci-scheme:platform ;
    skos:prefLabel "SCISAT-1"@en ;
    skos:scopeNote "CSA Science Satellite"@en ;
    skos:topConceptOf cci-scheme:platform .

<http://vocab.ceda.ac.uk/collection/cci/platform/plat_sentinel1a> a cci:platform,
        skos:Concept ;
    cci:hasSensor <http://vocab.ceda.ac.uk/collection/cci/sensor/sens_sarcS1> ;
    rdfs:seeAlso <https://www.wmo-sat.info/oscar/satellites/view/396> ;
    skos:broader <http://vocab.ceda.ac.uk/collection/cci/platformProg/plat_sentinel1_prog> ;
    skos:definition "Sentinel 1 programme, 1st flight"@en ;
    skos:inScheme cci-scheme:platform ;
    skos:prefLabel "Sentinel-1A"@en ;
    skos:scopeNote "Sentinel 1 programme, 1st flight"@en ;
    skos:topConceptOf cci-scheme:platform .

<http://vocab.ceda.ac.uk/collection/cci/platform/plat_sentinel1b> a cci:platform,
        skos:Concept ;
    cci:hasSensor <http://vocab.ceda.ac.uk/collection/cci/sensor/sens_sarcS1> ;
    rdfs:seeAlso <https://www.wmo-sat.info/oscar/satellites/view/397> ;
    skos:broader <http://vocab.ceda.ac.uk/collection/cci/platformProg/plat_sentinel1_prog> ;
    skos:definition "Sentinel 1 programme, 2nd flight"@en ;
    skos:inScheme cci-scheme:platform ;
    skos:prefLabel "Sentinel-1B"@en ;
    skos:scopeNote "Sentinel 1 programme, 2nd flight"@en ;
    skos:topConceptOf cci-scheme:platform .

<http://vocab.ceda.ac.uk/collection/cci/platform/plat_sentinel2a> a cci:platform,
        skos:Concept ;
    cci:hasSensor <http://vocab.ceda.ac.uk/collection/cci/sensor/sens_msi> ;
    rdfs:seeAlso <https://www.wmo-sat.info/oscar/satellites/view/398> ;
    skos:broader <http://vocab.ceda.ac.uk/collection/cci/platformProg/plat_sentinel2_prog> ;
    skos:definition "Sentinel 2 programme, 1st flight"@en ;
    skos:inScheme cci-scheme:platform ;
    skos:prefLabel "Sentinel-2A"@en ;
    skos:scopeNote "Sentinel 2 programme, 1st flight"@en ;
    skos:topConceptOf cci-scheme:platform .

<http://vocab.ceda.ac.uk/collection/cci/platform/plat_sentinel2b> a cci:platform,
        skos:Concept ;
    cci:hasSensor <http://vocab.ceda.ac.uk/collection/cci/sensor/sens_msi> ;
    rdfs:seeAlso <https://www.wmo-sat.info/oscar/satellites/view/399> ;
    skos:broader <http://vocab.ceda.ac.uk/collection/cci/platformProg/plat_sentinel2_prog> ;
    skos:definition "Sentinel 2 programme, 2nd flight"@en ;
    skos:inScheme cci-scheme:platform ;
    skos:prefLabel "Sentinel-2B"@en ;
    skos:scopeNote "Sentinel 2 programme, 2nd flight"@en ;
    skos:topConceptOf cci-scheme:platform .

<http://vocab.ceda.ac.uk/collection/cci/platform/plat_sentinel5p> a cci:platform,
        skos:Concept ;
    cci:hasSensor <http://vocab.ceda.ac.uk/collection/cci/sensor/sens_tropomi> ;
    rdfs:seeAlso <https://www.wmo-sat.info/oscar/satellites/view/402> ;
    skos:broader <http://vocab.ceda.ac.uk/collection/cci/platformProg/plat_s5p_prog> ;
    skos:definition "Sentinel-5 precursor"@en ;
    skos:inScheme cci-scheme:platform ;
    skos:prefLabel "Sentinel-5P"@en ;
    skos:scopeNote "Sentinel-5 precursor"@en ;
    skos:topConceptOf cci-scheme:platform .

<http://vocab.ceda.ac.uk/collection/cci/platform/plat_sentinel6a> a cci:platform,
        skos:Concept ;
    cci:hasSensor <http://vocab.ceda.ac.uk/collection/cci/sensor/sens_poseidon4> ;
    rdfs:seeAlso <https://space.oscar.wmo.int/satellites/view/sentinel_6a> ;
    skos:broader <http://vocab.ceda.ac.uk/collection/cci/platformProg/plat_sentinel6_prog> ;
    skos:definition "Sentinel 6 programme, 1st flight"@en ;
    skos:inScheme cci-scheme:platform ;
    skos:prefLabel "Sentinel-6A"@en ;
    skos:scopeNote "Sentinel 6 programme, 1st flight"@en ;
    skos:topConceptOf cci-scheme:platform .

<http://vocab.ceda.ac.uk/collection/cci/platform/plat_sentinel6b> a cci:platform,
        skos:Concept ;
    cci:hasSensor <http://vocab.ceda.ac.uk/collection/cci/sensor/sens_poseidon4> ;
    rdfs:seeAlso <https://space.oscar.wmo.int/satellites/view/sentinel_6b> ;
    skos:broader <http://vocab.ceda.ac.uk/collection/cci/platformProg/plat_sentinel6_prog> ;
    skos:definition "Sentinel 6 programme, 2nd flight"@en ;
    skos:inScheme cci-scheme:platform ;
    skos:prefLabel "Sentinel-6B"@en ;
    skos:scopeNote "Sentinel 6 programme, 2nd flight"@en ;
    skos:topConceptOf cci-scheme:platform .

<http://vocab.ceda.ac.uk/collection/cci/platform/plat_smap> a cci:platform,
        skos:Concept ;
    cci:hasSensor <http://vocab.ceda.ac.uk/collection/cci/sensor/sens_smap> ;
    rdfs:seeAlso <https://www.wmo-sat.info/oscar/satellites/view/406> ;
    skos:broader <http://vocab.ceda.ac.uk/collection/cci/platformProg/plat_smap_prog> ;
    skos:definition "Soil Moisture Active-Passive"@en ;
    skos:inScheme cci-scheme:platform ;
    skos:prefLabel "SMAP"@en ;
    skos:scopeNote "Soil Moisture Active-Passive"@en ;
    skos:topConceptOf cci-scheme:platform .

<http://vocab.ceda.ac.uk/collection/cci/platform/plat_smos> a cci:platform,
        skos:Concept ;
    cci:hasSensor <http://vocab.ceda.ac.uk/collection/cci/sensor/sens_miras> ;
    rdfs:seeAlso <https://www.wmo-sat.info/oscar/satellites/view/408> ;
    skos:broader <http://vocab.ceda.ac.uk/collection/cci/platformProg/plat_smos_prog> ;
    skos:definition "ESA Soil Moisture and Ocean Salinity Satellite"@en ;
    skos:inScheme cci-scheme:platform ;
    skos:prefLabel "SMOS"@en ;
    skos:scopeNote "ESA Soil Moisture and Ocean Salinity Satellite"@en ;
    skos:topConceptOf cci-scheme:platform .

<http://vocab.ceda.ac.uk/collection/cci/platform/plat_snpp> a cci:platform,
        skos:Concept ;
    cci:hasSensor <http://vocab.ceda.ac.uk/collection/cci/sensor/sens_viirs> ;
    rdfs:seeAlso <https://www.wmo-sat.info/oscar/satellites/view/342> ;
    skos:altLabel "Suomi NPP"@en ;
    skos:broader <http://vocab.ceda.ac.uk/collection/cci/platformProg/plat_jpss_prog> ;
    skos:definition "Suomi National Polar-orbiting Partnership"@en ;
    skos:inScheme cci-scheme:platform ;
    skos:prefLabel "SNPP"@en ;
    skos:scopeNote "Suomi National Polar-orbiting Partnership"@en ;
    skos:topConceptOf cci-scheme:platform .

<http://vocab.ceda.ac.uk/collection/cci/platform/plat_spot4> a cci:platform,
        skos:Concept ;
    cci:hasSensor <http://vocab.ceda.ac.uk/collection/cci/sensor/sens_vegetation> ;
    rdfs:seeAlso <http://www.wmo-sat.info/oscar/satellites/view/415> ;
    skos:broader <http://vocab.ceda.ac.uk/collection/cci/platformProg/plat_spot> ;
    skos:definition "CNES Satellite Pour l'Observation de la Terre 4"@en ;
    skos:inScheme cci-scheme:platform ;
    skos:prefLabel "SPOT-4"@en ;
    skos:scopeNote "CNES Satellite Pour l'Observation de la Terre 4"@en ;
    skos:topConceptOf cci-scheme:platform .

<http://vocab.ceda.ac.uk/collection/cci/platform/plat_tandem_X> a cci:platform,
        skos:Concept ;
    cci:hasSensor <http://vocab.ceda.ac.uk/collection/cci/sensor/sens_sarX> ;
    rdfs:seeAlso <http://www.wmo-sat.info/oscar/satellites/view/426> ;
    skos:broader <http://vocab.ceda.ac.uk/collection/cci/platformProg/plat_terraSAR> ;
    skos:definition "DLR TanDEM-X"@en ;
    skos:inScheme cci-scheme:platform ;
    skos:prefLabel "TanDEM-X"@en ;
    skos:scopeNote "DLR TanDEM-X"@en ;
    skos:topConceptOf cci-scheme:platform .

<http://vocab.ceda.ac.uk/collection/cci/platform/plat_terraSar_X> a cci:platform,
        skos:Concept ;
    cci:hasSensor <http://vocab.ceda.ac.uk/collection/cci/sensor/sens_sarX> ;
    rdfs:seeAlso <http://www.wmo-sat.info/oscar/satellites/view/427> ;
    skos:broader <http://vocab.ceda.ac.uk/collection/cci/platformProg/plat_terraSAR> ;
    skos:definition "DLR TerraSar-X"@en ;
    skos:inScheme cci-scheme:platform ;
    skos:prefLabel "TerraSar-X"@en ;
    skos:scopeNote "DLR TerraSar-X"@en ;
    skos:topConceptOf cci-scheme:platform .

<http://vocab.ceda.ac.uk/collection/cci/platform/plat_tiros_n> a cci:platform,
        skos:Concept ;
    cci:hasSensor <http://vocab.ceda.ac.uk/collection/cci/sensor/sens_hirs2> ;
    rdfs:seeAlso <https://www.wmo-sat.info/oscar/satellites/view/441> ;
    skos:broader <http://vocab.ceda.ac.uk/collection/cci/platformProg/plat_noaa_4th> ;
    skos:definition "Television and Infra-Red Observation Satellite - N"@en ;
    skos:inScheme cci-scheme:platform ;
    skos:prefLabel "TIROS-N"@en ;
    skos:scopeNote "Television and Infra-Red Observation Satellite - N"@en ;
    skos:topConceptOf cci-scheme:platform .

<http://vocab.ceda.ac.uk/collection/cci/platform/plat_trmm> a cci:platform,
        skos:Concept ;
    cci:hasSensor <http://vocab.ceda.ac.uk/collection/cci/sensor/sens_tmi> ;
    rdfs:seeAlso <http://www.wmo-sat.info/oscar/satellites/view/445> ;
    skos:broader <http://vocab.ceda.ac.uk/collection/cci/platformProg/plat_trmm_prog> ;
    skos:definition "NASA Tropical Rainfall Measuring Mission"@en ;
    skos:inScheme cci-scheme:platform ;
    skos:prefLabel "TRMM"@en ;
    skos:scopeNote "NASA Tropical Rainfall Measuring Mission"@en ;
    skos:topConceptOf cci-scheme:platform .

<http://vocab.ceda.ac.uk/collection/cci/platform/plat_tsx_ng> a cci:platform,
        skos:Concept ;
    cci:hasSensor <http://vocab.ceda.ac.uk/collection/cci/sensor/sens_sarX> ;
    rdfs:seeAlso <http://www.wmo-sat.info/oscar/satellites/view/428> ;
    skos:broader <http://vocab.ceda.ac.uk/collection/cci/platformProg/plat_terraSAR> ;
    skos:definition "DLR TSX-NG"@en ;
    skos:inScheme cci-scheme:platform ;
    skos:prefLabel "TSX-NG"@en ;
    skos:scopeNote "DLR TSX-NG"@en ;
    skos:topConceptOf cci-scheme:platform .

<http://vocab.ceda.ac.uk/collection/cci/platformProg/plat_ers> a cci:platformProg,
        skos:Concept ;
    rdfs:seeAlso <http://www.wmo-sat.info/oscar/satelliteprogrammes/view/47> ;
    skos:definition "ESA European Remote Sensing Satellite"@en ;
    skos:inScheme cci-scheme:platformProg ;
    skos:narrower <http://vocab.ceda.ac.uk/collection/cci/platform/plat_ers1>,
        <http://vocab.ceda.ac.uk/collection/cci/platform/plat_ers2> ;
    skos:prefLabel "ERS"@en ;
    skos:scopeNote "ESA European Remote Sensing Satellite"@en ;
    skos:topConceptOf cci-scheme:platformProg .

<http://vocab.ceda.ac.uk/collection/cci/platformProg/plat_geodetic> a cci:platformProg,
        skos:Concept ;
    rdfs:seeAlso <http://www.wmo-sat.info/oscar/satelliteprogrammes/view/59> ;
    skos:definition "NASA Geodetic Satellite"@en ;
    skos:inScheme cci-scheme:platformProg ;
    skos:narrower <http://vocab.ceda.ac.uk/collection/cci/platform/plat_geosat>,
        <http://vocab.ceda.ac.uk/collection/cci/platform/plat_gfo> ;
    skos:prefLabel "Geodetic"@en ;
    skos:scopeNote "NASA Geodetic Satellite"@en ;
    skos:topConceptOf cci-scheme:platformProg .

<http://vocab.ceda.ac.uk/collection/cci/platformProg/plat_gosat_prog> a cci:platformProg,
        skos:Concept ;
    rdfs:seeAlso <http://www.wmo-sat.info/oscar/satelliteprogrammes/view/66> ;
    skos:altLabel "GOSAT"@en ;
    skos:definition "JAXA Greenhouse gas Observing Satellite"@en ;
    skos:inScheme cci-scheme:platformProg ;
    skos:narrower <http://vocab.ceda.ac.uk/collection/cci/platform/plat_gosat>,
        <http://vocab.ceda.ac.uk/collection/cci/platform/plat_gosat-2> ;
    skos:prefLabel "GOSAT-Programme"@en ;
    skos:scopeNote "JAXA Greenhouse gas Observing Satellite"@en ;
    skos:topConceptOf cci-scheme:platformProg .

<http://vocab.ceda.ac.uk/collection/cci/platformProg/plat_himawari> a cci:platformProg,
        skos:Concept ;
    rdfs:seeAlso <http://www.wmo-sat.info/oscar/satelliteprogrammes/view/71> ;
    skos:definition "JMA Himawari 2nd generation (Multifunction Transport Satellite)"@en ;
    skos:inScheme cci-scheme:platformProg ;
    skos:narrower <http://vocab.ceda.ac.uk/collection/cci/platform/plat_himawari-6>,
        <http://vocab.ceda.ac.uk/collection/cci/platform/plat_himawari-7> ;
    skos:prefLabel "Himawari"@en ;
    skos:scopeNote "JMA Himawari 2nd generation (Multifunction Transport Satellite)"@en ;
    skos:topConceptOf cci-scheme:platformProg .

<http://vocab.ceda.ac.uk/collection/cci/platformProg/plat_icesat_prog> a cci:platformProg,
        skos:Concept ;
    rdfs:seeAlso <http://www.wmo-sat.info/oscar/satelliteprogrammes/view/77> ;
    skos:altLabel "ICESat"@en ;
    skos:definition "NASA Ice Cloud and land Elevation Satellite"@en ;
    skos:inScheme cci-scheme:platformProg ;
    skos:narrower <http://vocab.ceda.ac.uk/collection/cci/platform/plat_icesat>,
        <http://vocab.ceda.ac.uk/collection/cci/platform/plat_icesat-2> ;
    skos:prefLabel "ICESat Programme"@en ;
    skos:scopeNote "NASA Ice Cloud and land Elevation Satellite"@en ;
    skos:topConceptOf cci-scheme:platformProg .

<http://vocab.ceda.ac.uk/collection/cci/platformProg/plat_sentinel1_prog> a cci:platformProg,
        skos:Concept ;
    rdfs:seeAlso <https://www.wmo-sat.info/oscar/satelliteprogrammes/view/145> ;
    skos:definition "Sentinel 1 programme"@en ;
    skos:inScheme cci-scheme:platformProg ;
    skos:narrower <http://vocab.ceda.ac.uk/collection/cci/platform/plat_sentinel1a>,
        <http://vocab.ceda.ac.uk/collection/cci/platform/plat_sentinel1b> ;
    skos:prefLabel "Sentinel-1"@en ;
    skos:scopeNote "Sentinel 1 programme"@en ;
    skos:topConceptOf cci-scheme:platformProg .

<http://vocab.ceda.ac.uk/collection/cci/platformProg/plat_sentinel2_prog> a cci:platformProg,
        skos:Concept ;
    rdfs:seeAlso <https://www.wmo-sat.info/oscar/satelliteprogrammes/view/146> ;
    skos:definition "Sentinel 2 programme"@en ;
    skos:inScheme cci-scheme:platformProg ;
    skos:narrower <http://vocab.ceda.ac.uk/collection/cci/platform/plat_sentinel2a>,
        <http://vocab.ceda.ac.uk/collection/cci/platform/plat_sentinel2b> ;
    skos:prefLabel "Sentinel-2"@en ;
    skos:scopeNote "Sentinel 2 programme"@en ;
    skos:topConceptOf cci-scheme:platformProg .

<http://vocab.ceda.ac.uk/collection/cci/platformProg/plat_sentinel3_prog> a cci:platformProg,
        skos:Concept ;
    rdfs:seeAlso <https://www.wmo-sat.info/oscar/satelliteprogrammes/view/147> ;
    skos:definition "Sentinel 3 programme"@en ;
    skos:inScheme cci-scheme:platformProg ;
    skos:narrower <http://vocab.ceda.ac.uk/collection/cci/platform/plat_sentinel3a>,
        <http://vocab.ceda.ac.uk/collection/cci/platform/plat_sentinel3b> ;
    skos:prefLabel "Sentinel-3"@en ;
    skos:scopeNote "Sentinel 3 programme"@en ;
    skos:topConceptOf cci-scheme:platformProg .

<http://vocab.ceda.ac.uk/collection/cci/platformProg/plat_sentinel6_prog> a cci:platformProg,
        skos:Concept ;
    rdfs:seeAlso <https://space.oscar.wmo.int/satelliteprogrammes/view/sentinel_6> ;
    skos:definition "Sentinel 6 programme"@en ;
    skos:inScheme cci-scheme:platformProg ;
    skos:narrower <http://vocab.ceda.ac.uk/collection/cci/platform/plat_sentinel6a>,
        <http://vocab.ceda.ac.uk/collection/cci/platform/plat_sentinel6b> ;
    skos:prefLabel "Sentinel-6"@en ;
    skos:scopeNote "Sentinel 6 programme"@en ;
    skos:topConceptOf cci-scheme:platformProg .

<http://vocab.ceda.ac.uk/collection/cci/platformProg/plat_spot_prog_follow> a cci:platformProg,
        skos:Concept ;
    rdfs:seeAlso <https://www.wmo-sat.info/oscar/satelliteprogrammes/view/157> ;
    skos:definition "Satellite Pour l’Observation de la Terre - Follow-on"@en ;
    skos:inScheme cci-scheme:platformProg ;
    skos:narrower <http://vocab.ceda.ac.uk/collection/cci/platform/plat_spot6>,
        <http://vocab.ceda.ac.uk/collection/cci/platform/plat_spot7> ;
    skos:prefLabel "SPOT Follow-on"@en ;
    skos:scopeNote "Satellite Pour l’Observation de la Terre - Follow-on"@en ;
    skos:topConceptOf cci-scheme:platformProg .

<http://vocab.ceda.ac.uk/collection/cci/sensor/sens_abi> a cci:sensor,
        skos:Concept ;
    cci:hasPlatform <http://vocab.ceda.ac.uk/collection/cci/platform/plat_goes_16>,
        <http://vocab.ceda.ac.uk/collection/cci/platform/plat_goes_17> ;
    rdfs:seeAlso <https://space.oscar.wmo.int/instruments/view/abi> ;
    skos:definition "Advanced Baseline Imager"@en ;
    skos:inScheme cci-scheme:sensor ;
    skos:prefLabel "ABI"@en ;
    skos:scopeNote "Advanced Baseline Imager"@en ;
    skos:topConceptOf cci-scheme:sensor .

<http://vocab.ceda.ac.uk/collection/cci/sensor/sens_amisar> a cci:sensor,
        skos:Concept ;
    cci:hasPlatform <http://vocab.ceda.ac.uk/collection/cci/platform/plat_ers1>,
        <http://vocab.ceda.ac.uk/collection/cci/platform/plat_ers2> ;
    rdfs:seeAlso <http://www.wmo-sat.info/oscar/instruments/view/23> ;
    skos:definition "Active Microwave Instrument - Synthetic Aperture Antenna"@en ;
    skos:inScheme cci-scheme:sensor ;
    skos:prefLabel "AMI-SAR"@en ;
    skos:scopeNote "Active Microwave Instrument - Synthetic Aperture Antenna"@en ;
    skos:topConceptOf cci-scheme:sensor .

<http://vocab.ceda.ac.uk/collection/cci/sensor/sens_amiscat> a cci:sensor,
        skos:Concept ;
    cci:hasPlatform <http://vocab.ceda.ac.uk/collection/cci/platform/plat_ers1>,
        <http://vocab.ceda.ac.uk/collection/cci/platform/plat_ers2> ;
    rdfs:seeAlso <http://www.wmo-sat.info/oscar/instruments/view/24> ;
    skos:altLabel "AMI-WS"@en ;
    skos:definition "Active Microwave Instrument – Scatterometer"@en ;
    skos:inScheme cci-scheme:sensor ;
    skos:prefLabel "AMI-SCAT"@en ;
    skos:scopeNote "Active Microwave Instrument – Scatterometer"@en ;
    skos:topConceptOf cci-scheme:sensor .

<http://vocab.ceda.ac.uk/collection/cci/sensor/sens_modis> a cci:sensor,
        skos:Concept ;
    cci:hasPlatform <http://vocab.ceda.ac.uk/collection/cci/platform/plat_aqua>,
        <http://vocab.ceda.ac.uk/collection/cci/platform/plat_terra> ;
    rdfs:seeAlso <http://www.wmo-sat.info/oscar/instruments/view/296> ;
    skos:definition "Moderate Resolution Imaging Spectroradiometer"@en ;
    skos:inScheme cci-scheme:sensor ;
    skos:prefLabel "MODIS"@en ;
    skos:scopeNote "Moderate Resolution Imaging Spectroradiometer"@en ;
    skos:topConceptOf cci-scheme:sensor .

<http://vocab.ceda.ac.uk/collection/cci/sensor/sens_msi> a cci:sensor,
        skos:Concept ;
    cci:hasPlatform <http://vocab.ceda.ac.uk/collection/cci/platform/plat_sentinel2a>,
        <http://vocab.ceda.ac.uk/collection/cci/platform/plat_sentinel2b> ;
    rdfs:seeAlso <https://www.wmo-sat.info/oscar/instruments/view/312> ;
    skos:altLabel "MSI"@en ;
    skos:definition "Multi-Spectral Instrument (Sentinel-2)"@en ;
    skos:inScheme cci-scheme:sensor ;
    skos:prefLabel "MSI (Sentinel-2)"@en ;
    skos:scopeNote "Multi-Spectral Instrument (Sentinel-2)"@en ;
    skos:topConceptOf cci-scheme:sensor .

<http://vocab.ceda.ac.uk/collection/cci/sensor/sens_olci> a cci:sensor,
        skos:Concept ;
    cci:hasPlatform <http://vocab.ceda.ac.uk/collection/cci/platform/plat_sentinel3a>,
        <http://vocab.ceda.ac.uk/collection/cci/platform/plat_sentinel3b> ;
    rdfs:seeAlso <https://www.wmo-sat.info/oscar/instruments/view/374> ;
    skos:definition "Ocean and Land Colour Imager"@en ;
    skos:inScheme cci-scheme:sensor ;
    skos:prefLabel "OLCI"@en ;
    skos:scopeNote "Ocean and Land Colour Imager"@en ;
    skos:topConceptOf cci-scheme:sensor .

<http://vocab.ceda.ac.uk/collection/cci/sensor/sens_poseidon4> a cci:sensor,
        skos:Concept ;
    cci:hasPlatform <http://vocab.ceda.ac.uk/collection/cci/platform/plat_sentinel6a>,
        <http://vocab.ceda.ac.uk/collection/cci/platform/plat_sentinel6b> ;
    rdfs:seeAlso <https://space.oscar.wmo.int/instruments/view/poseidon_4> ;
    skos:definition "Poseidon-4"@en ;
    skos:inScheme cci-scheme:sensor ;
    skos:prefLabel "Poseidon-4"@en ;
    skos:scopeNote "Poseidon-4"@en ;
    skos:topConceptOf cci-scheme:sensor .

<http://vocab.ceda.ac.uk/collection/cci/sensor/sens_ra> a cci:sensor,
        skos:Concept ;
    cci:hasPlatform <http://vocab.ceda.ac.uk/collection/cci/platform/plat_ers1>,
        <http://vocab.ceda.ac.uk/collection/cci/platform/plat_ers2> ;
    rdfs:seeAlso <http://www.wmo-sat.info/oscar/instruments/view/415> ;
    skos:definition "Radar Altimeter"@en ;
    skos:inScheme cci-scheme:sensor ;
    skos:prefLabel "RA"@en ;
    skos:scopeNote "Radar Altimeter"@en ;
    skos:topConceptOf cci-scheme:sensor .

<http://vocab.ceda.ac.uk/collection/cci/sensor/sens_sarcS1> a cci:sensor,
        skos:Concept ;
    cci:hasPlatform <http://vocab.ceda.ac.uk/collection/cci/platform/plat_sentinel1a>,
        <http://vocab.ceda.ac.uk/collection/cci/platform/plat_sentinel1b> ;
    rdfs:seeAlso <https://www.wmo-sat.info/oscar/instruments/view/450> ;
    skos:definition "Synthetic Aperture Radar (C-band)"@en ;
    skos:inScheme cci-scheme:sensor ;
    skos:prefLabel "SAR-C (Sentinel-1)"@en ;
    skos:scopeNote "Synthetic Aperture Radar (C-band)"@en ;
    skos:topConceptOf cci-scheme:sensor .

<http://vocab.ceda.ac.uk/collection/cci/sensor/sens_slstr> a cci:sensor,
        skos:Concept ;
    cci:hasPlatform <http://vocab.ceda.ac.uk/collection/cci/platform/plat_sentinel3a>,
        <http://vocab.ceda.ac.uk/collection/cci/platform/plat_sentinel3b> ;
    rdfs:seeAlso <https://www.wmo-sat.info/oscar/instruments/view/518> ;
    skos:definition "Sea and Land Surface Temperature Radiometer"@en ;
    skos:inScheme cci-scheme:sensor ;
    skos:prefLabel "SLSTR"@en ;
    skos:scopeNote "Sea and Land Surface Temperature Radiometer"@en ;
    skos:topConceptOf cci-scheme:sensor .

<http://vocab.ceda.ac.uk/collection/cci/sensor/sens_sral> a cci:sensor,
        skos:Concept ;
    cci:hasPlatform <http://vocab.ceda.ac.uk/collection/cci/platform/plat_sentinel3a>,
        <http://vocab.ceda.ac.uk/collection/cci/platform/plat_sentinel3b> ;
    rdfs:seeAlso <https://www.wmo-sat.info/oscar/instruments/view/530> ;
    skos:definition "Synthetic Aperture Radar Altimeter"@en ;
    skos:inScheme cci-scheme:sensor ;
    skos:prefLabel "SRAL"@en ;
    skos:scopeNote "Synthetic Aperture Radar Altimeter"@en ;
    skos:topConceptOf cci-scheme:sensor .

<http://vocab.ceda.ac.uk/collection/cci/sensor/sens_vegetation> a cci:sensor,
        skos:Concept ;
    cci:hasPlatform <http://vocab.ceda.ac.uk/collection/cci/platform/plat_spot4>,
        <http://vocab.ceda.ac.uk/collection/cci/platform/plat_spot5> ;
    rdfs:seeAlso <http://www.wmo-sat.info/oscar/instruments/view/594> ;
    skos:altLabel "Végétation"@en ;
    skos:definition "Vegetation observation"@en ;
    skos:inScheme cci-scheme:sensor ;
    skos:prefLabel "VEGETATION"@en ;
    skos:scopeNote "Vegetation observation"@en ;
    skos:topConceptOf cci-scheme:sensor .

<http://vocab.ceda.ac.uk/collection/cci/platform/plat_FY-3A> a cci:platform,
        skos:Concept ;
    cci:hasSensor <http://vocab.ceda.ac.uk/collection/cci/sensor/sens_mwri>,
        <http://vocab.ceda.ac.uk/collection/cci/sensor/sens_virr> ;
    rdfs:seeAlso <http://www.wmo-sat.info/oscar/satellites/view/113> ;
    skos:altLabel "Feng-Yun - 3A"@en ;
    skos:broader <http://vocab.ceda.ac.uk/collection/cci/platformProg/plat_fengyun3> ;
    skos:definition "CMA Feng-Yun – 3A"@en ;
    skos:inScheme cci-scheme:platform ;
    skos:prefLabel "FY-3A"@en ;
    skos:scopeNote "CMA Feng-Yun – 3A"@en ;
    skos:topConceptOf cci-scheme:platform .

<http://vocab.ceda.ac.uk/collection/cci/platform/plat_FY-3B> a cci:platform,
        skos:Concept ;
    cci:hasSensor <http://vocab.ceda.ac.uk/collection/cci/sensor/sens_mwri>,
        <http://vocab.ceda.ac.uk/collection/cci/sensor/sens_virr> ;
    rdfs:seeAlso <http://www.wmo-sat.info/oscar/satellites/view/114> ;
    skos:altLabel "Feng-Yun - 3B"@en ;
    skos:broader <http://vocab.ceda.ac.uk/collection/cci/platformProg/plat_fengyun3> ;
    skos:definition "CMA Feng-Yun – 3B"@en ;
    skos:inScheme cci-scheme:platform ;
    skos:prefLabel "FY-3B"@en ;
    skos:scopeNote "CMA Feng-Yun – 3B"@en ;
    skos:topConceptOf cci-scheme:platform .

<http://vocab.ceda.ac.uk/collection/cci/platform/plat_FY-3C> a cci:platform,
        skos:Concept ;
    cci:hasSensor <http://vocab.ceda.ac.uk/collection/cci/sensor/sens_mwri>,
        <http://vocab.ceda.ac.uk/collection/cci/sensor/sens_virr> ;
    rdfs:seeAlso <http://www.wmo-sat.info/oscar/satellites/view/115> ;
    skos:altLabel "Feng-Yun - 3C"@en ;
    skos:broader <http://vocab.ceda.ac.uk/collection/cci/platformProg/plat_fengyun3> ;
    skos:definition "CMA Feng-Yun – 3C"@en ;
    skos:inScheme cci-scheme:platform ;
    skos:prefLabel "FY-3C"@en ;
    skos:scopeNote "CMA Feng-Yun – 3C"@en ;
    skos:topConceptOf cci-scheme:platform .

<http://vocab.ceda.ac.uk/collection/cci/platform/plat_gosat> a cci:platform,
        skos:Concept ;
    cci:hasSensor <http://vocab.ceda.ac.uk/collection/cci/sensor/sens_tansoCai>,
        <http://vocab.ceda.ac.uk/collection/cci/sensor/sens_tansoFts> ;
    rdfs:seeAlso <http://www.wmo-sat.info/oscar/satellites/view/154> ;
    skos:broader <http://vocab.ceda.ac.uk/collection/cci/platformProg/plat_gosat_prog> ;
    skos:definition "JAXA Greenhouse gas Observing Satellite"@en ;
    skos:inScheme cci-scheme:platform ;
    skos:prefLabel "GOSAT"@en ;
    skos:scopeNote "JAXA Greenhouse gas Observing Satellite"@en ;
    skos:topConceptOf cci-scheme:platform .

<http://vocab.ceda.ac.uk/collection/cci/platform/plat_landsat_4> a cci:platform,
        skos:Concept ;
    cci:hasSensor <http://vocab.ceda.ac.uk/collection/cci/sensor/sens_mss>,
        <http://vocab.ceda.ac.uk/collection/cci/sensor/sens_tm> ;
    rdfs:seeAlso <http://www.wmo-sat.info/oscar/satellites/view/222> ;
    skos:broader <http://vocab.ceda.ac.uk/collection/cci/platformProg/plat_landsat> ;
    skos:definition "NASA Landsat"@en ;
    skos:inScheme cci-scheme:platform ;
    skos:prefLabel "Landsat-4"@en ;
    skos:scopeNote "NASA Landsat"@en ;
    skos:topConceptOf cci-scheme:platform .

<http://vocab.ceda.ac.uk/collection/cci/platform/plat_landsat_5> a cci:platform,
        skos:Concept ;
    cci:hasSensor <http://vocab.ceda.ac.uk/collection/cci/sensor/sens_mss>,
        <http://vocab.ceda.ac.uk/collection/cci/sensor/sens_tm> ;
    rdfs:seeAlso <http://www.wmo-sat.info/oscar/satellites/view/223> ;
    skos:broader <http://vocab.ceda.ac.uk/collection/cci/platformProg/plat_landsat> ;
    skos:definition "NASA Landsat"@en ;
    skos:inScheme cci-scheme:platform ;
    skos:prefLabel "Landsat-5"@en ;
    skos:scopeNote "NASA Landsat"@en ;
    skos:topConceptOf cci-scheme:platform .

<http://vocab.ceda.ac.uk/collection/cci/platform/plat_landsat_8> a cci:platform,
        skos:Concept ;
    cci:hasSensor <http://vocab.ceda.ac.uk/collection/cci/sensor/sens_oli>,
        <http://vocab.ceda.ac.uk/collection/cci/sensor/sens_tirs> ;
    rdfs:seeAlso <http://www.wmo-sat.info/oscar/satellites/view/227> ;
    skos:broader <http://vocab.ceda.ac.uk/collection/cci/platformProg/plat_landsat_dcm> ;
    skos:definition "NASA Landsat"@en ;
    skos:inScheme cci-scheme:platform ;
    skos:prefLabel "Landsat-8"@en ;
    skos:scopeNote "NASA Landsat"@en ;
    skos:topConceptOf cci-scheme:platform .

<http://vocab.ceda.ac.uk/collection/cci/platform/plat_nimbus6> a cci:platform,
        skos:Concept ;
    cci:hasSensor <http://vocab.ceda.ac.uk/collection/cci/sensor/sens_esmrNim6>,
        <http://vocab.ceda.ac.uk/collection/cci/sensor/sens_hirs> ;
    rdfs:seeAlso <http://www.wmo-sat.info/oscar/satellites/view/320> ;
    skos:broader <http://vocab.ceda.ac.uk/collection/cci/platformProg/plat_nimbus> ;
    skos:definition "NASA Research-and-development satellite 6"@en ;
    skos:inScheme cci-scheme:platform ;
    skos:prefLabel "Nimbus-6"@en ;
    skos:scopeNote "NASA Research-and-development satellite 6"@en ;
    skos:topConceptOf cci-scheme:platform .

<http://vocab.ceda.ac.uk/collection/cci/platform/plat_noaa_10> a cci:platform,
        skos:Concept ;
    cci:hasSensor <http://vocab.ceda.ac.uk/collection/cci/sensor/sens_avhrr>,
        <http://vocab.ceda.ac.uk/collection/cci/sensor/sens_hirs2> ;
    rdfs:seeAlso <http://www.wmo-sat.info/oscar/satellites/view/332> ;
    skos:broader <http://vocab.ceda.ac.uk/collection/cci/platformProg/plat_noaa_4th> ;
    skos:definition "NASA NOAA Environmental satellite 10"@en ;
    skos:inScheme cci-scheme:platform ;
    skos:prefLabel "NOAA-10"@en ;
    skos:scopeNote "NASA NOAA Environmental satellite 10"@en ;
    skos:topConceptOf cci-scheme:platform .

<http://vocab.ceda.ac.uk/collection/cci/platform/plat_noaa_11> a cci:platform,
        skos:Concept ;
    cci:hasSensor <http://vocab.ceda.ac.uk/collection/cci/sensor/sens_avhrr2>,
        <http://vocab.ceda.ac.uk/collection/cci/sensor/sens_hirs2> ;
    rdfs:seeAlso <http://www.wmo-sat.info/oscar/satellites/view/333> ;
    skos:broader <http://vocab.ceda.ac.uk/collection/cci/platformProg/plat_noaa_4th> ;
    skos:definition "NASA NOAA Environmental satellite 11"@en ;
    skos:inScheme cci-scheme:platform ;
    skos:prefLabel "NOAA-11"@en ;
    skos:scopeNote "NASA NOAA Environmental satellite 11"@en ;
    skos:topConceptOf cci-scheme:platform .

<http://vocab.ceda.ac.uk/collection/cci/platform/plat_noaa_12> a cci:platform,
        skos:Concept ;
    cci:hasSensor <http://vocab.ceda.ac.uk/collection/cci/sensor/sens_avhrr2>,
        <http://vocab.ceda.ac.uk/collection/cci/sensor/sens_hirs2> ;
    rdfs:seeAlso <http://www.wmo-sat.info/oscar/satellites/view/334> ;
    skos:broader <http://vocab.ceda.ac.uk/collection/cci/platformProg/plat_noaa_4th> ;
    skos:definition "NASA NOAA Environmental satellite 12"@en ;
    skos:inScheme cci-scheme:platform ;
    skos:prefLabel "NOAA-12"@en ;
    skos:scopeNote "NASA NOAA Environmental satellite 12"@en ;
    skos:topConceptOf cci-scheme:platform .

<http://vocab.ceda.ac.uk/collection/cci/platform/plat_noaa_13> a cci:platform,
        skos:Concept ;
    cci:hasSensor <http://vocab.ceda.ac.uk/collection/cci/sensor/sens_avhrr2>,
        <http://vocab.ceda.ac.uk/collection/cci/sensor/sens_hirs2> ;
    rdfs:seeAlso <http://www.wmo-sat.info/oscar/satellites/view/335> ;
    skos:broader <http://vocab.ceda.ac.uk/collection/cci/platformProg/plat_noaa_4th> ;
    skos:definition "NASA NOAA Environmental satellite 13"@en ;
    skos:inScheme cci-scheme:platform ;
    skos:prefLabel "NOAA-13"@en ;
    skos:scopeNote "NASA NOAA Environmental satellite 13"@en ;
    skos:topConceptOf cci-scheme:platform .

<http://vocab.ceda.ac.uk/collection/cci/platform/plat_noaa_14> a cci:platform,
        skos:Concept ;
    cci:hasSensor <http://vocab.ceda.ac.uk/collection/cci/sensor/sens_avhrr2>,
        <http://vocab.ceda.ac.uk/collection/cci/sensor/sens_hirs2> ;
    rdfs:seeAlso <http://www.wmo-sat.info/oscar/satellites/view/336> ;
    skos:broader <http://vocab.ceda.ac.uk/collection/cci/platformProg/plat_noaa_4th> ;
    skos:definition "NASA NOAA Environmental satellite 14"@en ;
    skos:inScheme cci-scheme:platform ;
    skos:prefLabel "NOAA-14"@en ;
    skos:scopeNote "NASA NOAA Environmental satellite 14"@en ;
    skos:topConceptOf cci-scheme:platform .

<http://vocab.ceda.ac.uk/collection/cci/platform/plat_noaa_6> a cci:platform,
        skos:Concept ;
    cci:hasSensor <http://vocab.ceda.ac.uk/collection/cci/sensor/sens_avhrr>,
        <http://vocab.ceda.ac.uk/collection/cci/sensor/sens_hirs2> ;
    rdfs:seeAlso <http://www.wmo-sat.info/oscar/satellites/view/328> ;
    skos:broader <http://vocab.ceda.ac.uk/collection/cci/platformProg/plat_noaa_4th> ;
    skos:definition "NASA NOAA Environmental satellite 6"@en ;
    skos:inScheme cci-scheme:platform ;
    skos:prefLabel "NOAA-6"@en ;
    skos:scopeNote "NASA NOAA Environmental satellite 6"@en ;
    skos:topConceptOf cci-scheme:platform .

<http://vocab.ceda.ac.uk/collection/cci/platform/plat_noaa_7> a cci:platform,
        skos:Concept ;
    cci:hasSensor <http://vocab.ceda.ac.uk/collection/cci/sensor/sens_avhrr2>,
        <http://vocab.ceda.ac.uk/collection/cci/sensor/sens_hirs2> ;
    rdfs:seeAlso <http://www.wmo-sat.info/oscar/satellites/view/329> ;
    skos:broader <http://vocab.ceda.ac.uk/collection/cci/platformProg/plat_noaa_4th> ;
    skos:definition "NASA NOAA Environmental satellite 7"@en ;
    skos:inScheme cci-scheme:platform ;
    skos:prefLabel "NOAA-7"@en ;
    skos:scopeNote "NASA NOAA Environmental satellite 7"@en ;
    skos:topConceptOf cci-scheme:platform .

<http://vocab.ceda.ac.uk/collection/cci/platform/plat_noaa_8> a cci:platform,
        skos:Concept ;
    cci:hasSensor <http://vocab.ceda.ac.uk/collection/cci/sensor/sens_avhrr>,
        <http://vocab.ceda.ac.uk/collection/cci/sensor/sens_hirs2> ;
    rdfs:seeAlso <http://www.wmo-sat.info/oscar/satellites/view/330> ;
    skos:broader <http://vocab.ceda.ac.uk/collection/cci/platformProg/plat_noaa_4th> ;
    skos:definition "NASA NOAA Environmental satellite 8"@en ;
    skos:inScheme cci-scheme:platform ;
    skos:prefLabel "NOAA-8"@en ;
    skos:scopeNote "NASA NOAA Environmental satellite 8"@en ;
    skos:topConceptOf cci-scheme:platform .

<http://vocab.ceda.ac.uk/collection/cci/platform/plat_noaa_9> a cci:platform,
        skos:Concept ;
    cci:hasSensor <http://vocab.ceda.ac.uk/collection/cci/sensor/sens_avhrr2>,
        <http://vocab.ceda.ac.uk/collection/cci/sensor/sens_hirs2> ;
    rdfs:seeAlso <http://www.wmo-sat.info/oscar/satellites/view/331> ;
    skos:broader <http://vocab.ceda.ac.uk/collection/cci/platformProg/plat_noaa_4th> ;
    skos:definition "NASA NOAA Environmental satellite 9"@en ;
    skos:inScheme cci-scheme:platform ;
    skos:prefLabel "NOAA-9"@en ;
    skos:scopeNote "NASA NOAA Environmental satellite 9"@en ;
    skos:topConceptOf cci-scheme:platform .

<http://vocab.ceda.ac.uk/collection/cci/platform/plat_odin> a cci:platform,
        skos:Concept ;
    cci:hasSensor <http://vocab.ceda.ac.uk/collection/cci/sensor/sens_osiris>,
        <http://vocab.ceda.ac.uk/collection/cci/sensor/sens_smr> ;
    rdfs:seeAlso <http://www.wmo-sat.info/oscar/satellites/view/348> ;
    skos:broader <http://vocab.ceda.ac.uk/collection/cci/platformProg/plat_odin_prog> ;
    skos:definition "OHB Sweden Astrophysics and Aeronomy satellite"@en ;
    skos:inScheme cci-scheme:platform ;
    skos:prefLabel "ODIN"@en ;
    skos:scopeNote "OHB Sweden Astrophysics and Aeronomy satellite"@en ;
    skos:topConceptOf cci-scheme:platform .

<http://vocab.ceda.ac.uk/collection/cci/platform/plat_spot5> a cci:platform,
        skos:Concept ;
    cci:hasSensor <http://vocab.ceda.ac.uk/collection/cci/sensor/sens_hrs>,
        <http://vocab.ceda.ac.uk/collection/cci/sensor/sens_vegetation> ;
    rdfs:seeAlso <https://www.wmo-sat.info/oscar/satellites/view/416> ;
    skos:broader <http://vocab.ceda.ac.uk/collection/cci/platformProg/plat_spot> ;
    skos:definition "CNES Satellite Pour l'Observation de la Terre 5"@en ;
    skos:inScheme cci-scheme:platform ;
    skos:prefLabel "SPOT-5"@en ;
    skos:scopeNote "CNES Satellite Pour l'Observation de la Terre 5"@en ;
    skos:topConceptOf cci-scheme:platform .

<http://vocab.ceda.ac.uk/collection/cci/platform/plat_terra> a cci:platform,
        skos:Concept ;
    cci:hasSensor <http://vocab.ceda.ac.uk/collection/cci/sensor/sens_aster>,
        <http://vocab.ceda.ac.uk/collection/cci/sensor/sens_modis> ;
    rdfs:seeAlso <http://www.wmo-sat.info/oscar/satellites/view/81> ;
    skos:broader <http://vocab.ceda.ac.uk/collection/cci/platformProg/plat_eos> ;
    skos:definition "NASA Earth Observing System Satellite"@en ;
    skos:inScheme cci-scheme:platform ;
    skos:prefLabel "Terra"@en ;
    skos:scopeNote "NASA Earth Observing System Satellite"@en ;
    skos:topConceptOf cci-scheme:platform .

<http://vocab.ceda.ac.uk/collection/cci/platform/plat_topexPoseidon> a cci:platform,
        skos:Concept ;
    cci:hasSensor <http://vocab.ceda.ac.uk/collection/cci/sensor/sens_nra>,
        <http://vocab.ceda.ac.uk/collection/cci/sensor/sens_ssalt> ;
    rdfs:seeAlso <http://www.wmo-sat.info/oscar/satellites/view/443> ;
    skos:broader <http://vocab.ceda.ac.uk/collection/cci/platformProg/plat_topexPoseidon_prog> ;
    skos:definition "CNES/NASA Ocean surface topography satellite"@en ;
    skos:inScheme cci-scheme:platform ;
    skos:prefLabel "Topex/Poseidon"@en ;
    skos:scopeNote "CNES/NASA Ocean surface topography satellite"@en ;
    skos:topConceptOf cci-scheme:platform .

<http://vocab.ceda.ac.uk/collection/cci/platformGrp/plat_dmsp> a cci:platformGrp,
        skos:Concept ;
    skos:definition "US Defense Meteorological Satellite Program"@en ;
    skos:inScheme cci-scheme:platformGrp ;
    skos:narrower <http://vocab.ceda.ac.uk/collection/cci/platformProg/plat_dmsp_5D1>,
        <http://vocab.ceda.ac.uk/collection/cci/platformProg/plat_dmsp_5D2>,
        <http://vocab.ceda.ac.uk/collection/cci/platformProg/plat_dmsp_5D3> ;
    skos:prefLabel "DMSP"@en ;
    skos:scopeNote "US Defense Meteorological Satellite Program"@en ;
    skos:topConceptOf cci-scheme:platformGrp .

<http://vocab.ceda.ac.uk/collection/cci/platformGrp/plat_goes> a cci:platformGrp,
        skos:Concept ;
    skos:definition "NASA NESDIS Geostationary Operational Environmental Satellite system"@en ;
    skos:inScheme cci-scheme:platformGrp ;
    skos:narrower <http://vocab.ceda.ac.uk/collection/cci/platformProg/plat_goes_1st>,
        <http://vocab.ceda.ac.uk/collection/cci/platformProg/plat_goes_2nd>,
        <http://vocab.ceda.ac.uk/collection/cci/platformProg/plat_goes_3rd> ;
    skos:prefLabel "GOES"@en ;
    skos:scopeNote "NASA NESDIS Geostationary Operational Environmental Satellite system"@en ;
    skos:topConceptOf cci-scheme:platformGrp .

<http://vocab.ceda.ac.uk/collection/cci/platformGrp/plat_noaa> a cci:platformGrp,
        skos:Concept ;
    skos:definition "NASA NOAA Environmental satellite programme"@en ;
    skos:inScheme cci-scheme:platformGrp ;
    skos:narrower <http://vocab.ceda.ac.uk/collection/cci/platformProg/plat_noaa_3rd>,
        <http://vocab.ceda.ac.uk/collection/cci/platformProg/plat_noaa_4th>,
        <http://vocab.ceda.ac.uk/collection/cci/platformProg/plat_noaa_5th> ;
    skos:prefLabel "NOAA"@en ;
    skos:scopeNote "NASA NOAA Environmental satellite programme"@en ;
    skos:topConceptOf cci-scheme:platformGrp .

<http://vocab.ceda.ac.uk/collection/cci/platformProg/plat_alos_prog> a cci:platformProg,
        skos:Concept ;
    rdfs:seeAlso <http://www.wmo-sat.info/oscar/satelliteprogrammes/view/7> ;
    skos:altLabel "ALOS"@en ;
    skos:definition "JAXA Advanced Land Observation Satellite Programme"@en ;
    skos:inScheme cci-scheme:platformProg ;
    skos:narrower <http://vocab.ceda.ac.uk/collection/cci/platform/plat_alos>,
        <http://vocab.ceda.ac.uk/collection/cci/platform/plat_alos-2>,
        <http://vocab.ceda.ac.uk/collection/cci/platform/plat_alos-3> ;
    skos:prefLabel "ALOS Programme"@en ;
    skos:scopeNote "JAXA Advanced Land Observation Satellite Programme"@en ;
    skos:topConceptOf cci-scheme:platformProg .

<http://vocab.ceda.ac.uk/collection/cci/platformProg/plat_eos> a cci:platformProg,
        skos:Concept ;
    rdfs:seeAlso <http://www.wmo-sat.info/oscar/satelliteprogrammes/view/43> ;
    skos:definition "NASA A-Train  Earth Observing System Satellite"@en ;
    skos:inScheme cci-scheme:platformProg ;
    skos:narrower <http://vocab.ceda.ac.uk/collection/cci/platform/plat_aqua>,
        <http://vocab.ceda.ac.uk/collection/cci/platform/plat_aura>,
        <http://vocab.ceda.ac.uk/collection/cci/platform/plat_terra> ;
    skos:prefLabel "EOS"@en ;
    skos:scopeNote "NASA A-Train  Earth Observing System Satellite"@en ;
    skos:topConceptOf cci-scheme:platformProg .

<http://vocab.ceda.ac.uk/collection/cci/platformProg/plat_gcom> a cci:platformProg,
        skos:Concept ;
    rdfs:seeAlso <http://www.wmo-sat.info/oscar/satelliteprogrammes/view/57> ;
    skos:definition "NASA Global Change Observation Mission for Water (\"Shizuku\")"@en ;
    skos:inScheme cci-scheme:platformProg ;
    skos:narrower <http://vocab.ceda.ac.uk/collection/cci/platform/plat_gcomW1>,
        <http://vocab.ceda.ac.uk/collection/cci/platform/plat_gcomW2>,
        <http://vocab.ceda.ac.uk/collection/cci/platform/plat_gcomW3> ;
    skos:prefLabel "GCOM"@en ;
    skos:scopeNote "NASA Global Change Observation Mission for Water (\"Shizuku\")"@en ;
    skos:topConceptOf cci-scheme:platformProg .

<http://vocab.ceda.ac.uk/collection/cci/platformProg/plat_jason> a cci:platformProg,
        skos:Concept ;
    rdfs:seeAlso <http://www.wmo-sat.info/oscar/satelliteprogrammes/view/85> ;
    skos:definition "NASA Joint Altimetry Satellite Oceanography Network"@en ;
    skos:inScheme cci-scheme:platformProg ;
    skos:narrower <http://vocab.ceda.ac.uk/collection/cci/platform/plat_jason1>,
        <http://vocab.ceda.ac.uk/collection/cci/platform/plat_jason2>,
        <http://vocab.ceda.ac.uk/collection/cci/platform/plat_jason3> ;
    skos:prefLabel "JASON"@en ;
    skos:scopeNote "NASA Joint Altimetry Satellite Oceanography Network"@en ;
    skos:topConceptOf cci-scheme:platformProg .

<http://vocab.ceda.ac.uk/collection/cci/platformProg/plat_metop> a cci:platformProg,
        skos:Concept ;
    rdfs:seeAlso <http://www.wmo-sat.info/oscar/satelliteprogrammes/view/44> ;
    skos:definition "ESA/EUMETSAT Meteorological operational Polar System satellite"@en ;
    skos:inScheme cci-scheme:platformProg ;
    skos:narrower <http://vocab.ceda.ac.uk/collection/cci/platform/plat_metOpA>,
        <http://vocab.ceda.ac.uk/collection/cci/platform/plat_metOpB>,
        <http://vocab.ceda.ac.uk/collection/cci/platform/plat_metOpC> ;
    skos:prefLabel "Metop"@en ;
    skos:scopeNote "ESA/EUMETSAT Meteorological operational Polar System satellite"@en ;
    skos:topConceptOf cci-scheme:platformProg .

<http://vocab.ceda.ac.uk/collection/cci/procLev/proc_level1> a cci:procLev,
        skos:Concept ;
    skos:altLabel "L1"@en ;
    skos:inScheme cci-scheme:procLev ;
    skos:narrower <http://vocab.ceda.ac.uk/collection/cci/procLev/proc_level1A>,
        <http://vocab.ceda.ac.uk/collection/cci/procLev/proc_level1B>,
        <http://vocab.ceda.ac.uk/collection/cci/procLev/proc_level1C> ;
    skos:prefLabel "Level 1"@en ;
    skos:topConceptOf cci-scheme:procLev .

<http://vocab.ceda.ac.uk/collection/cci/procLev/proc_level3> a cci:procLev,
        skos:Concept ;
    rdfs:seeAlso <https://www.ghrsst.org/> ;
    skos:altLabel "L3"@en ;
    skos:definition "Level 2 variables mapped on a defined grid with reduced requirements for ancillary data. Three types of L3 products are defined."@en ;
    skos:inScheme cci-scheme:procLev ;
    skos:narrower <http://vocab.ceda.ac.uk/collection/cci/procLev/proc_level3C>,
        <http://vocab.ceda.ac.uk/collection/cci/procLev/proc_level3S>,
        <http://vocab.ceda.ac.uk/collection/cci/procLev/proc_level3U> ;
    skos:prefLabel "Level 3"@en ;
    skos:scopeNote "Level 2 variables mapped on a defined grid with reduced requirements for ancillary data. Three types of L3 products are defined."@en ;
    skos:topConceptOf cci-scheme:procLev .

<http://vocab.ceda.ac.uk/collection/cci/sensor/sens_amsr2> a cci:sensor,
        skos:Concept ;
    cci:hasPlatform <http://vocab.ceda.ac.uk/collection/cci/platform/plat_gcomW1>,
        <http://vocab.ceda.ac.uk/collection/cci/platform/plat_gcomW2>,
        <http://vocab.ceda.ac.uk/collection/cci/platform/plat_gcomW3> ;
    rdfs:seeAlso <http://www.wmo-sat.info/oscar/instruments/view/28> ;
    skos:definition "Advanced Microwave Scanning Radiometer"@en ;
    skos:inScheme cci-scheme:sensor ;
    skos:prefLabel "AMSR2"@en ;
    skos:scopeNote "Advanced Microwave Scanning Radiometer"@en ;
    skos:topConceptOf cci-scheme:sensor .

<http://vocab.ceda.ac.uk/collection/cci/sensor/sens_amsub> a cci:sensor,
        skos:Concept ;
    cci:hasPlatform <http://vocab.ceda.ac.uk/collection/cci/platform/plat_noaa_15>,
        <http://vocab.ceda.ac.uk/collection/cci/platform/plat_noaa_16>,
        <http://vocab.ceda.ac.uk/collection/cci/platform/plat_noaa_17> ;
    rdfs:seeAlso <http://www.wmo-sat.info/oscar/instruments/view/33> ;
    skos:definition "Advanced microwave sounding unit – B"@en ;
    skos:inScheme cci-scheme:sensor ;
    skos:prefLabel "AMSU-B"@en ;
    skos:scopeNote "Advanced microwave sounding unit – B"@en ;
    skos:topConceptOf cci-scheme:sensor .

<http://vocab.ceda.ac.uk/collection/cci/sensor/sens_ascat> a cci:sensor,
        skos:Concept ;
    cci:hasPlatform <http://vocab.ceda.ac.uk/collection/cci/platform/plat_metOpA>,
        <http://vocab.ceda.ac.uk/collection/cci/platform/plat_metOpB>,
        <http://vocab.ceda.ac.uk/collection/cci/platform/plat_metOpC> ;
    rdfs:seeAlso <http://www.wmo-sat.info/oscar/instruments/view/47> ;
    skos:definition "Advanced SCATterometer"@en ;
    skos:inScheme cci-scheme:sensor ;
    skos:prefLabel "ASCAT"@en ;
    skos:scopeNote "Advanced SCATterometer"@en ;
    skos:topConceptOf cci-scheme:sensor .

<http://vocab.ceda.ac.uk/collection/cci/sensor/sens_avhrr> a cci:sensor,
        skos:Concept ;
    cci:hasPlatform <http://vocab.ceda.ac.uk/collection/cci/platform/plat_noaa_10>,
        <http://vocab.ceda.ac.uk/collection/cci/platform/plat_noaa_6>,
        <http://vocab.ceda.ac.uk/collection/cci/platform/plat_noaa_8> ;
    rdfs:seeAlso <http://www.wmo-sat.info/oscar/instruments/view/60> ;
    skos:definition "Advanced Very High Resolution Radiometer"@en ;
    skos:inScheme cci-scheme:sensor ;
    skos:prefLabel "AVHRR"@en ;
    skos:scopeNote "Advanced Very High Resolution Radiometer"@en ;
    skos:topConceptOf cci-scheme:sensor .

<http://vocab.ceda.ac.uk/collection/cci/sensor/sens_gome2> a cci:sensor,
        skos:Concept ;
    cci:hasPlatform <http://vocab.ceda.ac.uk/collection/cci/platform/plat_metOpA>,
        <http://vocab.ceda.ac.uk/collection/cci/platform/plat_metOpB>,
        <http://vocab.ceda.ac.uk/collection/cci/platform/plat_metOpC> ;
    rdfs:seeAlso <http://www.wmo-sat.info/oscar/instruments/view/167> ;
    skos:definition "Global Monitoring of Atmospheric Ozone 2"@en ;
    skos:inScheme cci-scheme:sensor ;
    skos:prefLabel "GOME-2"@en ;
    skos:scopeNote "Global Monitoring of Atmospheric Ozone 2"@en ;
    skos:topConceptOf cci-scheme:sensor .

<http://vocab.ceda.ac.uk/collection/cci/sensor/sens_hirs3> a cci:sensor,
        skos:Concept ;
    cci:hasPlatform <http://vocab.ceda.ac.uk/collection/cci/platform/plat_noaa_15>,
        <http://vocab.ceda.ac.uk/collection/cci/platform/plat_noaa_16>,
        <http://vocab.ceda.ac.uk/collection/cci/platform/plat_noaa_17> ;
    rdfs:seeAlso <https://www.wmo-sat.info/oscar/instruments/view/183> ;
    skos:definition "High-Resolution Infra-Red Sounder / 3"@en ;
    skos:inScheme cci-scheme:sensor ;
    skos:prefLabel "HIRS/3"@en ;
    skos:scopeNote "High-Resolution Infra-Red Sounder / 3"@en ;
    skos:topConceptOf cci-scheme:sensor .

<http://vocab.ceda.ac.uk/collection/cci/sensor/sens_iasi> a cci:sensor,
        skos:Concept ;
    cci:hasPlatform <http://vocab.ceda.ac.uk/collection/cci/platform/plat_metOpA>,
        <http://vocab.ceda.ac.uk/collection/cci/platform/plat_metOpB>,
        <http://vocab.ceda.ac.uk/collection/cci/platform/plat_metOpC> ;
    rdfs:seeAlso <http://www.wmo-sat.info/oscar/instruments/view/207> ;
    skos:definition "Infra-Red Atmospheric Sounding Interferometer"@en ;
    skos:inScheme cci-scheme:sensor ;
    skos:prefLabel "IASI"@en ;
    skos:scopeNote "Infra-Red Atmospheric Sounding Interferometer"@en ;
    skos:topConceptOf cci-scheme:sensor .

<http://vocab.ceda.ac.uk/collection/cci/sensor/sens_sarX> a cci:sensor,
        skos:Concept ;
    cci:hasPlatform <http://vocab.ceda.ac.uk/collection/cci/platform/plat_tandem_X>,
        <http://vocab.ceda.ac.uk/collection/cci/platform/plat_terraSar_X>,
        <http://vocab.ceda.ac.uk/collection/cci/platform/plat_tsx_ng> ;
    rdfs:seeAlso <http://www.wmo-sat.info/oscar/instruments/view/459> ;
    skos:definition "Synthetic Aperture Radar X-band"@en ;
    skos:inScheme cci-scheme:sensor ;
    skos:prefLabel "SAR-X"@en ;
    skos:scopeNote "Synthetic Aperture Radar X-band"@en ;
    skos:topConceptOf cci-scheme:sensor .

<http://vocab.ceda.ac.uk/collection/cci/sensor/sens_tm> a cci:sensor,
        skos:Concept ;
    cci:hasPlatform <http://vocab.ceda.ac.uk/collection/cci/platform/plat_landsat_4>,
        <http://vocab.ceda.ac.uk/collection/cci/platform/plat_landsat_5>,
        <http://vocab.ceda.ac.uk/collection/cci/platform/plat_landsat_7> ;
    rdfs:seeAlso <http://www.wmo-sat.info/oscar/instruments/view/568> ;
    skos:definition "Thematic Mapper"@en ;
    skos:inScheme cci-scheme:sensor ;
    skos:prefLabel "TM"@en ;
    skos:scopeNote "Thematic Mapper"@en ;
    skos:topConceptOf cci-scheme:sensor .

<http://vocab.ceda.ac.uk/collection/cci/sensor/sens_virr> a cci:sensor,
        skos:Concept ;
    cci:hasPlatform <http://vocab.ceda.ac.uk/collection/cci/platform/plat_FY-3A>,
        <http://vocab.ceda.ac.uk/collection/cci/platform/plat_FY-3B>,
        <http://vocab.ceda.ac.uk/collection/cci/platform/plat_FY-3C> ;
    rdfs:seeAlso <https://www.wmo-sat.info/oscar/instruments/view/virr_fy_3> ;
    skos:altLabel "VIRR (FY-3)"@en ;
    skos:definition "Visible and Infra-Red Radiometer"@en ;
    skos:inScheme cci-scheme:sensor ;
    skos:prefLabel "VIRR"@en ;
    skos:scopeNote "Visible and Infra-Red Radiometer"@en ;
    skos:topConceptOf cci-scheme:sensor .

<http://vocab.ceda.ac.uk/collection/cci/platform/plat_noaa_18> a cci:platform,
        skos:Concept ;
    cci:hasSensor <http://vocab.ceda.ac.uk/collection/cci/sensor/sens_amsua>,
        <http://vocab.ceda.ac.uk/collection/cci/sensor/sens_avhrr3>,
        <http://vocab.ceda.ac.uk/collection/cci/sensor/sens_hirs4> ;
    rdfs:seeAlso <http://www.wmo-sat.info/oscar/satellites/view/340> ;
    skos:broader <http://vocab.ceda.ac.uk/collection/cci/platformProg/plat_noaa_5th> ;
    skos:definition "NASA NOAA Environmental satellite 18"@en ;
    skos:inScheme cci-scheme:platform ;
    skos:prefLabel "NOAA-18"@en ;
    skos:scopeNote "NASA NOAA Environmental satellite 18"@en ;
    skos:topConceptOf cci-scheme:platform .

<http://vocab.ceda.ac.uk/collection/cci/platform/plat_noaa_19> a cci:platform,
        skos:Concept ;
    cci:hasSensor <http://vocab.ceda.ac.uk/collection/cci/sensor/sens_amsua>,
        <http://vocab.ceda.ac.uk/collection/cci/sensor/sens_avhrr3>,
        <http://vocab.ceda.ac.uk/collection/cci/sensor/sens_hirs4> ;
    rdfs:seeAlso <http://www.wmo-sat.info/oscar/satellites/view/341> ;
    skos:broader <http://vocab.ceda.ac.uk/collection/cci/platformProg/plat_noaa_5th> ;
    skos:definition "NASA NOAA Environmental satellite 19"@en ;
    skos:inScheme cci-scheme:platform ;
    skos:prefLabel "NOAA-19"@en ;
    skos:scopeNote "NASA NOAA Environmental satellite 19"@en ;
    skos:topConceptOf cci-scheme:platform .

<http://vocab.ceda.ac.uk/collection/cci/platform/plat_sentinel3a> a cci:platform,
        skos:Concept ;
    cci:hasSensor <http://vocab.ceda.ac.uk/collection/cci/sensor/sens_olci>,
        <http://vocab.ceda.ac.uk/collection/cci/sensor/sens_slstr>,
        <http://vocab.ceda.ac.uk/collection/cci/sensor/sens_sral> ;
    rdfs:seeAlso <https://www.wmo-sat.info/oscar/satellites/view/400> ;
    skos:broader <http://vocab.ceda.ac.uk/collection/cci/platformProg/plat_sentinel3_prog> ;
    skos:definition "Sentinel 3 programme, 1st flight"@en ;
    skos:inScheme cci-scheme:platform ;
    skos:prefLabel "Sentinel-3A"@en ;
    skos:scopeNote "Sentinel 3 programme, 1st flight"@en ;
    skos:topConceptOf cci-scheme:platform .

<http://vocab.ceda.ac.uk/collection/cci/platform/plat_sentinel3b> a cci:platform,
        skos:Concept ;
    cci:hasSensor <http://vocab.ceda.ac.uk/collection/cci/sensor/sens_olci>,
        <http://vocab.ceda.ac.uk/collection/cci/sensor/sens_slstr>,
        <http://vocab.ceda.ac.uk/collection/cci/sensor/sens_sral> ;
    rdfs:seeAlso <https://www.wmo-sat.info/oscar/satellites/view/401> ;
    skos:broader <http://vocab.ceda.ac.uk/collection/cci/platformProg/plat_sentinel3_prog> ;
    skos:definition "Sentinel 3 programme, 2nd flight"@en ;
    skos:inScheme cci-scheme:platform ;
    skos:prefLabel "Sentinel-3B"@en ;
    skos:scopeNote "Sentinel 3 programme, 2nd flight"@en ;
    skos:topConceptOf cci-scheme:platform .

<http://vocab.ceda.ac.uk/collection/cci/platformProg/plat_csk_prog> a cci:platformProg,
        skos:Concept ;
    rdfs:seeAlso <https://www.wmo-sat.info/oscar/satelliteprogrammes/view/27> ;
    skos:definition "COSMO-SkyMed programme"@en ;
    skos:inScheme cci-scheme:platformProg ;
    skos:narrower <http://vocab.ceda.ac.uk/collection/cci/platform/plat_csk1>,
        <http://vocab.ceda.ac.uk/collection/cci/platform/plat_csk2>,
        <http://vocab.ceda.ac.uk/collection/cci/platform/plat_csk3>,
        <http://vocab.ceda.ac.uk/collection/cci/platform/plat_csk4> ;
    skos:prefLabel "COSMO-SkyMed"@en ;
    skos:scopeNote "COSMO-SkyMed programme"@en ;
    skos:topConceptOf cci-scheme:platformProg .

<http://vocab.ceda.ac.uk/collection/cci/platformProg/plat_msg> a cci:platformProg,
        skos:Concept ;
    rdfs:seeAlso <http://www.wmo-sat.info/oscar/satelliteprogrammes/view/102> ;
    skos:definition "ESA Meteosat Second Generation"@en ;
    skos:inScheme cci-scheme:platformProg ;
    skos:narrower <http://vocab.ceda.ac.uk/collection/cci/platform/plat_meteosat_10>,
        <http://vocab.ceda.ac.uk/collection/cci/platform/plat_meteosat_11>,
        <http://vocab.ceda.ac.uk/collection/cci/platform/plat_meteosat_8>,
        <http://vocab.ceda.ac.uk/collection/cci/platform/plat_meteosat_9> ;
    skos:prefLabel "MSG"@en ;
    skos:scopeNote "ESA Meteosat Second Generation"@en ;
    skos:topConceptOf cci-scheme:platformProg .

<http://vocab.ceda.ac.uk/collection/cci/platformProg/plat_terraSAR> a cci:platformProg,
        skos:Concept ;
    rdfs:seeAlso <http://www.wmo-sat.info/oscar/satelliteprogrammes/view/164> ;
    skos:definition "DLR X-band SAR programme"@en ;
    skos:inScheme cci-scheme:platformProg ;
    skos:narrower <http://vocab.ceda.ac.uk/collection/cci/platform/plat_hrws_sar>,
        <http://vocab.ceda.ac.uk/collection/cci/platform/plat_tandem_X>,
        <http://vocab.ceda.ac.uk/collection/cci/platform/plat_terraSar_X>,
        <http://vocab.ceda.ac.uk/collection/cci/platform/plat_tsx_ng> ;
    skos:prefLabel "TerraSAR"@en ;
    skos:scopeNote "DLR X-band SAR programme"@en ;
    skos:topConceptOf cci-scheme:platformProg .

<http://vocab.ceda.ac.uk/collection/cci/sensor/sens_hirs4> a cci:sensor,
        skos:Concept ;
    cci:hasPlatform <http://vocab.ceda.ac.uk/collection/cci/platform/plat_metOpA>,
        <http://vocab.ceda.ac.uk/collection/cci/platform/plat_metOpB>,
        <http://vocab.ceda.ac.uk/collection/cci/platform/plat_noaa_18>,
        <http://vocab.ceda.ac.uk/collection/cci/platform/plat_noaa_19> ;
    rdfs:seeAlso <https://www.wmo-sat.info/oscar/instruments/view/184> ;
    skos:definition "High-Resolution Infra-Red Sounder /4"@en ;
    skos:inScheme cci-scheme:sensor ;
    skos:prefLabel "HIRS/4"@en ;
    skos:scopeNote "High-Resolution Infra-Red Sounder /4"@en ;
    skos:topConceptOf cci-scheme:sensor .

<http://vocab.ceda.ac.uk/collection/cci/sensor/sens_sar2000> a cci:sensor,
        skos:Concept ;
    cci:hasPlatform <http://vocab.ceda.ac.uk/collection/cci/platform/plat_csk1>,
        <http://vocab.ceda.ac.uk/collection/cci/platform/plat_csk2>,
        <http://vocab.ceda.ac.uk/collection/cci/platform/plat_csk3>,
        <http://vocab.ceda.ac.uk/collection/cci/platform/plat_csk4> ;
    rdfs:seeAlso <https://www.wmo-sat.info/oscar/instruments/view/447> ;
    skos:definition "Synthetic Aperture Radar 2000 (X-band)"@en ;
    skos:inScheme cci-scheme:sensor ;
    skos:prefLabel "SAR-2000"@en ;
    skos:scopeNote "Synthetic Aperture Radar 2000 (X-band)"@en ;
    skos:topConceptOf cci-scheme:sensor .

<http://vocab.ceda.ac.uk/collection/cci/sensor/sens_seviri> a cci:sensor,
        skos:Concept ;
    cci:hasPlatform <http://vocab.ceda.ac.uk/collection/cci/platform/plat_meteosat_10>,
        <http://vocab.ceda.ac.uk/collection/cci/platform/plat_meteosat_11>,
        <http://vocab.ceda.ac.uk/collection/cci/platform/plat_meteosat_8>,
        <http://vocab.ceda.ac.uk/collection/cci/platform/plat_meteosat_9> ;
    rdfs:seeAlso <http://www.wmo-sat.info/oscar/instruments/view/503> ;
    skos:definition "Spinning Enhanced Visible and Infrared Imager"@en ;
    skos:inScheme cci-scheme:sensor ;
    skos:prefLabel "SEVIRI"@en ;
    skos:scopeNote "Spinning Enhanced Visible and Infrared Imager"@en ;
    skos:topConceptOf cci-scheme:sensor .

<http://vocab.ceda.ac.uk/collection/cci/platform/plat_aqua> a cci:platform,
        skos:Concept ;
    cci:hasSensor <http://vocab.ceda.ac.uk/collection/cci/sensor/sens_airs>,
        <http://vocab.ceda.ac.uk/collection/cci/sensor/sens_amsre>,
        <http://vocab.ceda.ac.uk/collection/cci/sensor/sens_amsua>,
        <http://vocab.ceda.ac.uk/collection/cci/sensor/sens_modis> ;
    rdfs:seeAlso <http://www.wmo-sat.info/oscar/satellites/view/79> ;
    skos:broader <http://vocab.ceda.ac.uk/collection/cci/platformProg/plat_eos> ;
    skos:definition "NASA Earth Observing System Satellite"@en ;
    skos:inScheme cci-scheme:platform ;
    skos:prefLabel "Aqua"@en ;
    skos:scopeNote "NASA Earth Observing System Satellite"@en ;
    skos:topConceptOf cci-scheme:platform .

<http://vocab.ceda.ac.uk/collection/cci/platform/plat_ers1> a cci:platform,
        skos:Concept ;
    cci:hasSensor <http://vocab.ceda.ac.uk/collection/cci/sensor/sens_amisar>,
        <http://vocab.ceda.ac.uk/collection/cci/sensor/sens_amiscat>,
        <http://vocab.ceda.ac.uk/collection/cci/sensor/sens_atsr>,
        <http://vocab.ceda.ac.uk/collection/cci/sensor/sens_ra> ;
    rdfs:seeAlso <http://www.wmo-sat.info/oscar/satellites/view/89> ;
    skos:broader <http://vocab.ceda.ac.uk/collection/cci/platformProg/plat_ers> ;
    skos:definition "ESA European Remote Sensing Satellite 1"@en ;
    skos:inScheme cci-scheme:platform ;
    skos:prefLabel "ERS-1"@en ;
    skos:scopeNote "ESA European Remote Sensing Satellite 1"@en ;
    skos:topConceptOf cci-scheme:platform .

<http://vocab.ceda.ac.uk/collection/cci/platform/plat_noaa_15> a cci:platform,
        skos:Concept ;
    cci:hasSensor <http://vocab.ceda.ac.uk/collection/cci/sensor/sens_amsua>,
        <http://vocab.ceda.ac.uk/collection/cci/sensor/sens_amsub>,
        <http://vocab.ceda.ac.uk/collection/cci/sensor/sens_avhrr3>,
        <http://vocab.ceda.ac.uk/collection/cci/sensor/sens_hirs3> ;
    rdfs:seeAlso <http://www.wmo-sat.info/oscar/satellites/view/337> ;
    skos:broader <http://vocab.ceda.ac.uk/collection/cci/platformProg/plat_noaa_5th> ;
    skos:definition "NASA NOAA Environmental satellite 15"@en ;
    skos:inScheme cci-scheme:platform ;
    skos:prefLabel "NOAA-15"@en ;
    skos:scopeNote "NASA NOAA Environmental satellite 15"@en ;
    skos:topConceptOf cci-scheme:platform .

<http://vocab.ceda.ac.uk/collection/cci/platform/plat_noaa_16> a cci:platform,
        skos:Concept ;
    cci:hasSensor <http://vocab.ceda.ac.uk/collection/cci/sensor/sens_amsua>,
        <http://vocab.ceda.ac.uk/collection/cci/sensor/sens_amsub>,
        <http://vocab.ceda.ac.uk/collection/cci/sensor/sens_avhrr3>,
        <http://vocab.ceda.ac.uk/collection/cci/sensor/sens_hirs3> ;
    rdfs:seeAlso <http://www.wmo-sat.info/oscar/satellites/view/338> ;
    skos:broader <http://vocab.ceda.ac.uk/collection/cci/platformProg/plat_noaa_5th> ;
    skos:definition "NASA NOAA Environmental satellite 16"@en ;
    skos:inScheme cci-scheme:platform ;
    skos:prefLabel "NOAA-16"@en ;
    skos:scopeNote "NASA NOAA Environmental satellite 16"@en ;
    skos:topConceptOf cci-scheme:platform .

<http://vocab.ceda.ac.uk/collection/cci/platform/plat_noaa_17> a cci:platform,
        skos:Concept ;
    cci:hasSensor <http://vocab.ceda.ac.uk/collection/cci/sensor/sens_amsua>,
        <http://vocab.ceda.ac.uk/collection/cci/sensor/sens_amsub>,
        <http://vocab.ceda.ac.uk/collection/cci/sensor/sens_avhrr3>,
        <http://vocab.ceda.ac.uk/collection/cci/sensor/sens_hirs3> ;
    rdfs:seeAlso <http://www.wmo-sat.info/oscar/satellites/view/339> ;
    skos:broader <http://vocab.ceda.ac.uk/collection/cci/platformProg/plat_noaa_5th> ;
    skos:definition "NASA NOAA Environmental satellite 17"@en ;
    skos:inScheme cci-scheme:platform ;
    skos:prefLabel "NOAA-17"@en ;
    skos:scopeNote "NASA NOAA Environmental satellite 17"@en ;
    skos:topConceptOf cci-scheme:platform .

<http://vocab.ceda.ac.uk/collection/cci/platformProg/plat_goes_3rd> a cci:platformProg,
        skos:Concept ;
    rdfs:seeAlso <http://www.wmo-sat.info/oscar/satelliteprogrammes/view/65> ;
    skos:broader <http://vocab.ceda.ac.uk/collection/cci/platformGrp/plat_goes> ;
    skos:definition "NASA Geostationary Operational Environmental Satellite - 3rd generation"@en ;
    skos:inScheme cci-scheme:platformProg ;
    skos:narrower <http://vocab.ceda.ac.uk/collection/cci/platform/plat_goes_16>,
        <http://vocab.ceda.ac.uk/collection/cci/platform/plat_goes_17>,
        <http://vocab.ceda.ac.uk/collection/cci/platform/plat_goes_T>,
        <http://vocab.ceda.ac.uk/collection/cci/platform/plat_goes_U> ;
    skos:prefLabel "GOES 3rd Gen"@en ;
    skos:scopeNote "NASA Geostationary Operational Environmental Satellite - 3rd generation"@en ;
    skos:topConceptOf cci-scheme:platformProg .

<http://vocab.ceda.ac.uk/collection/cci/platformProg/plat_spot> a cci:platformProg,
        skos:Concept ;
    rdfs:seeAlso <http://www.wmo-sat.info/oscar/satelliteprogrammes/view/156> ;
    skos:definition "Satellite Pour l’Observation de la Terre"@en ;
    skos:inScheme cci-scheme:platformProg ;
    skos:narrower <http://vocab.ceda.ac.uk/collection/cci/platform/plat_spot1>,
        <http://vocab.ceda.ac.uk/collection/cci/platform/plat_spot2>,
        <http://vocab.ceda.ac.uk/collection/cci/platform/plat_spot3>,
        <http://vocab.ceda.ac.uk/collection/cci/platform/plat_spot4>,
        <http://vocab.ceda.ac.uk/collection/cci/platform/plat_spot5> ;
    skos:prefLabel "SPOT"@en ;
    skos:scopeNote "Satellite Pour l’Observation de la Terre"@en ;
    skos:topConceptOf cci-scheme:platformProg .

<http://vocab.ceda.ac.uk/collection/cci/sensor/sens_goesImager1215> a cci:sensor,
        skos:Concept ;
    cci:hasPlatform <http://vocab.ceda.ac.uk/collection/cci/platform/plat_goes_12>,
        <http://vocab.ceda.ac.uk/collection/cci/platform/plat_goes_12_SA>,
        <http://vocab.ceda.ac.uk/collection/cci/platform/plat_goes_13>,
        <http://vocab.ceda.ac.uk/collection/cci/platform/plat_goes_14>,
        <http://vocab.ceda.ac.uk/collection/cci/platform/plat_goes_15> ;
    rdfs:seeAlso <http://www.wmo-sat.info/oscar/instruments/view/879> ;
    skos:definition "GOES IMAGER (12-15)"@en ;
    skos:inScheme cci-scheme:sensor ;
    skos:prefLabel "GOES-Imager-12-15"@en ;
    skos:scopeNote "GOES IMAGER (12-15)"@en ;
    skos:topConceptOf cci-scheme:sensor .

<http://vocab.ceda.ac.uk/collection/cci/sensor/sens_mss> a cci:sensor,
        skos:Concept ;
    cci:hasPlatform <http://vocab.ceda.ac.uk/collection/cci/platform/plat_landsat_1>,
        <http://vocab.ceda.ac.uk/collection/cci/platform/plat_landsat_2>,
        <http://vocab.ceda.ac.uk/collection/cci/platform/plat_landsat_3>,
        <http://vocab.ceda.ac.uk/collection/cci/platform/plat_landsat_4>,
        <http://vocab.ceda.ac.uk/collection/cci/platform/plat_landsat_5> ;
    rdfs:seeAlso <http://www.wmo-sat.info/oscar/instruments/view/316> ;
    skos:definition "Multi-Spectral Scanner"@en ;
    skos:inScheme cci-scheme:sensor ;
    skos:prefLabel "MSS"@en ;
    skos:scopeNote "Multi-Spectral Scanner"@en ;
    skos:topConceptOf cci-scheme:sensor .

<http://vocab.ceda.ac.uk/collection/cci/sensor/sens_mwri> a cci:sensor,
        skos:Concept ;
    cci:hasPlatform <http://vocab.ceda.ac.uk/collection/cci/platform/plat_FY-3A>,
        <http://vocab.ceda.ac.uk/collection/cci/platform/plat_FY-3B>,
        <http://vocab.ceda.ac.uk/collection/cci/platform/plat_FY-3C>,
        <http://vocab.ceda.ac.uk/collection/cci/platform/plat_FY-3D>,
        <http://vocab.ceda.ac.uk/collection/cci/platform/plat_FY-3F> ;
    rdfs:seeAlso <http://www.wmo-sat.info/oscar/instruments/view/350> ;
    skos:definition "Micro-Wave Radiation Imager"@en ;
    skos:inScheme cci-scheme:sensor ;
    skos:prefLabel "MWRI"@en ;
    skos:scopeNote "Micro-Wave Radiation Imager"@en ;
    skos:topConceptOf cci-scheme:sensor .

cci-scheme:platformGrp a skos:ConceptScheme ;
    dc:creator "Science and Technology Facilities Council" ;
    dc:date "2025-01-23" ;
    dc:description "<p>The CCI concept schemes are used to define concepts within an element of a Directory Reference Scheme. There are currently eight concept schemes defined: <a href=../dataType>data type</a>, <a href=..//ecv>ecv</a>, <a href=../scheme/cci/freq>frequency</a>, <a href=../org>institutes</a>, <a href=../platform>platforms</a>, <a href=../procLev>processing levels</a>, <a href=../product>products</a>, and <a href=../sensor>sensors</a>. The use of a concept scheme allows easy navigation up and down the tree.</p><h5>SKOS Navigation Down the Concept Scheme</h5><img src=conceptSchemeDown.svg /><h5>SKOS Navigation Up the Concept Scheme</h5><img src=conceptSchemeUp.svg /><p>As well as being concepts the the concepts are also named individuals of the <a href=../../../ontology/cci>CCI Ontology</a> classes.<h5>OWL Classes</h5><img src=classes.svg /><p></p>" ;
    dc:publisher "STFC"@en ;
    dc:rights "This work is licensed under a BSD license."@en ;
    dc:title "Platform Group" ;
    rdfs:comment "This concept scheme represents the platforms used by the CCI project" ;
    owl:versionInfo "0.0.1" ;
    skos:definition "The platform groups that have been used in the collection of data for the ESA Climate Change Initiative (CCI). A group consists of a number of <a href=#platformPrg>programmes</a>"@en ;
    skos:hasTopConcept <http://vocab.ceda.ac.uk/collection/cci/platformGrp/plat_dmsp>,
        <http://vocab.ceda.ac.uk/collection/cci/platformGrp/plat_goes>,
        <http://vocab.ceda.ac.uk/collection/cci/platformGrp/plat_noaa> ;
    skos:prefLabel "Platform Group"@en .

<http://vocab.ceda.ac.uk/collection/cci/platform/plat_ers2> a cci:platform,
        skos:Concept ;
    cci:hasSensor <http://vocab.ceda.ac.uk/collection/cci/sensor/sens_amisar>,
        <http://vocab.ceda.ac.uk/collection/cci/sensor/sens_amiscat>,
        <http://vocab.ceda.ac.uk/collection/cci/sensor/sens_atsr2>,
        <http://vocab.ceda.ac.uk/collection/cci/sensor/sens_gome>,
        <http://vocab.ceda.ac.uk/collection/cci/sensor/sens_ra> ;
    rdfs:seeAlso <http://www.wmo-sat.info/oscar/satellites/view/90> ;
    skos:broader <http://vocab.ceda.ac.uk/collection/cci/platformProg/plat_ers> ;
    skos:definition "ESA European Remote Sensing Satellite 2"@en ;
    skos:inScheme cci-scheme:platform ;
    skos:prefLabel "ERS-2"@en ;
    skos:scopeNote "ESA European Remote Sensing Satellite 2"@en ;
    skos:topConceptOf cci-scheme:platform .

<http://vocab.ceda.ac.uk/collection/cci/platform/plat_metOpC> a cci:platform,
        skos:Concept ;
    cci:hasSensor <http://vocab.ceda.ac.uk/collection/cci/sensor/sens_amsua>,
        <http://vocab.ceda.ac.uk/collection/cci/sensor/sens_ascat>,
        <http://vocab.ceda.ac.uk/collection/cci/sensor/sens_avhrr3>,
        <http://vocab.ceda.ac.uk/collection/cci/sensor/sens_gome2>,
        <http://vocab.ceda.ac.uk/collection/cci/sensor/sens_iasi> ;
    rdfs:seeAlso <http://www.wmo-sat.info/oscar/satellites/view/308> ;
    skos:broader <http://vocab.ceda.ac.uk/collection/cci/platformProg/plat_metop> ;
    skos:definition "ESA/EUMETSAT Meteorological operational Polar System satellite – C"@en ;
    skos:inScheme cci-scheme:platform ;
    skos:prefLabel "Metop-C"@en ;
    skos:scopeNote "ESA/EUMETSAT Meteorological operational Polar System satellite – C"@en ;
    skos:topConceptOf cci-scheme:platform .

<http://vocab.ceda.ac.uk/collection/cci/platformProg/plat_dmsp_5D1> a cci:platformProg,
        skos:Concept ;
    rdfs:seeAlso <http://www.wmo-sat.info/oscar/satelliteprogrammes/view/33> ;
    skos:broader <http://vocab.ceda.ac.uk/collection/cci/platformGrp/plat_dmsp> ;
    skos:definition "US Defense Meteorological Satellite Program Block 5D-1"@en ;
    skos:inScheme cci-scheme:platformProg ;
    skos:narrower <http://vocab.ceda.ac.uk/collection/cci/platform/plat_dmsp_F01>,
        <http://vocab.ceda.ac.uk/collection/cci/platform/plat_dmsp_F02>,
        <http://vocab.ceda.ac.uk/collection/cci/platform/plat_dmsp_F03>,
        <http://vocab.ceda.ac.uk/collection/cci/platform/plat_dmsp_F04>,
        <http://vocab.ceda.ac.uk/collection/cci/platform/plat_dmsp_F05> ;
    skos:prefLabel "DMSP Block 5D-1"@en ;
    skos:scopeNote "US Defense Meteorological Satellite Program Block 5D-1"@en ;
    skos:topConceptOf cci-scheme:platformProg .

<http://vocab.ceda.ac.uk/collection/cci/platformProg/plat_noaa_3rd> a cci:platformProg,
        skos:Concept ;
    rdfs:seeAlso <http://www.wmo-sat.info/oscar/satelliteprogrammes/view/110> ;
    skos:broader <http://vocab.ceda.ac.uk/collection/cci/platformGrp/plat_noaa> ;
    skos:definition "NASA NOAA Environmental satellites 3rd Generation"@en ;
    skos:inScheme cci-scheme:platformProg ;
    skos:narrower <http://vocab.ceda.ac.uk/collection/cci/platform/plat_noaa_1>,
        <http://vocab.ceda.ac.uk/collection/cci/platform/plat_noaa_2>,
        <http://vocab.ceda.ac.uk/collection/cci/platform/plat_noaa_3>,
        <http://vocab.ceda.ac.uk/collection/cci/platform/plat_noaa_4>,
        <http://vocab.ceda.ac.uk/collection/cci/platform/plat_noaa_5> ;
    skos:prefLabel "NOAA-3rd"@en ;
    skos:scopeNote "NASA NOAA Environmental satellites 3rd Generation"@en ;
    skos:topConceptOf cci-scheme:platformProg .

<http://vocab.ceda.ac.uk/collection/cci/platformProg/plat_noaa_5th> a cci:platformProg,
        skos:Concept ;
    rdfs:seeAlso <http://www.wmo-sat.info/oscar/satelliteprogrammes/view/112> ;
    skos:broader <http://vocab.ceda.ac.uk/collection/cci/platformGrp/plat_noaa> ;
    skos:definition "NASA NOAA Environmental satellites 5th Generation"@en ;
    skos:inScheme cci-scheme:platformProg ;
    skos:narrower <http://vocab.ceda.ac.uk/collection/cci/platform/plat_noaa_15>,
        <http://vocab.ceda.ac.uk/collection/cci/platform/plat_noaa_16>,
        <http://vocab.ceda.ac.uk/collection/cci/platform/plat_noaa_17>,
        <http://vocab.ceda.ac.uk/collection/cci/platform/plat_noaa_18>,
        <http://vocab.ceda.ac.uk/collection/cci/platform/plat_noaa_19> ;
    skos:prefLabel "NOAA-5th"@en ;
    skos:scopeNote "NASA NOAA Environmental satellites 5th Generation"@en ;
    skos:topConceptOf cci-scheme:platformProg .

<http://vocab.ceda.ac.uk/collection/cci/sensor/sens_avhrr2> a cci:sensor,
        skos:Concept ;
    cci:hasPlatform <http://vocab.ceda.ac.uk/collection/cci/platform/plat_noaa_11>,
        <http://vocab.ceda.ac.uk/collection/cci/platform/plat_noaa_12>,
        <http://vocab.ceda.ac.uk/collection/cci/platform/plat_noaa_13>,
        <http://vocab.ceda.ac.uk/collection/cci/platform/plat_noaa_14>,
        <http://vocab.ceda.ac.uk/collection/cci/platform/plat_noaa_7>,
        <http://vocab.ceda.ac.uk/collection/cci/platform/plat_noaa_9> ;
    rdfs:seeAlso <http://www.wmo-sat.info/oscar/instruments/view/61> ;
    skos:definition "Advanced Very High Resolution Radiometer / 2"@en ;
    skos:inScheme cci-scheme:sensor ;
    skos:prefLabel "AVHRR-2"@en ;
    skos:scopeNote "Advanced Very High Resolution Radiometer / 2"@en ;
    skos:topConceptOf cci-scheme:sensor .

<http://vocab.ceda.ac.uk/collection/cci/sensor/sens_goesImager811> a cci:sensor,
        skos:Concept ;
    cci:hasPlatform <http://vocab.ceda.ac.uk/collection/cci/platform/plat_goes_08>,
        <http://vocab.ceda.ac.uk/collection/cci/platform/plat_goes_09>,
        <http://vocab.ceda.ac.uk/collection/cci/platform/plat_goes_09_bk>,
        <http://vocab.ceda.ac.uk/collection/cci/platform/plat_goes_10>,
        <http://vocab.ceda.ac.uk/collection/cci/platform/plat_goes_10_SA>,
        <http://vocab.ceda.ac.uk/collection/cci/platform/plat_goes_11> ;
    rdfs:seeAlso <http://www.wmo-sat.info/oscar/instruments/view/217> ;
    skos:definition "GOES IMAGER (8-11)"@en ;
    skos:inScheme cci-scheme:sensor ;
    skos:prefLabel "GOES-Imager-8-11"@en ;
    skos:scopeNote "GOES IMAGER (8-11)"@en ;
    skos:topConceptOf cci-scheme:sensor .

<http://vocab.ceda.ac.uk/collection/cci/platform/plat_metOpA> a cci:platform,
        skos:Concept ;
    cci:hasSensor <http://vocab.ceda.ac.uk/collection/cci/sensor/sens_amsua>,
        <http://vocab.ceda.ac.uk/collection/cci/sensor/sens_ascat>,
        <http://vocab.ceda.ac.uk/collection/cci/sensor/sens_avhrr3>,
        <http://vocab.ceda.ac.uk/collection/cci/sensor/sens_gome2>,
        <http://vocab.ceda.ac.uk/collection/cci/sensor/sens_hirs4>,
        <http://vocab.ceda.ac.uk/collection/cci/sensor/sens_iasi> ;
    rdfs:seeAlso <http://www.wmo-sat.info/oscar/satellites/view/306> ;
    skos:broader <http://vocab.ceda.ac.uk/collection/cci/platformProg/plat_metop> ;
    skos:definition "ESA/EUMETSAT Meteorological operational Polar System satellite - A"@en ;
    skos:inScheme cci-scheme:platform ;
    skos:prefLabel "Metop-A"@en ;
    skos:scopeNote "ESA/EUMETSAT Meteorological operational Polar System satellite - A"@en ;
    skos:topConceptOf cci-scheme:platform .

<http://vocab.ceda.ac.uk/collection/cci/platform/plat_metOpB> a cci:platform,
        skos:Concept ;
    cci:hasSensor <http://vocab.ceda.ac.uk/collection/cci/sensor/sens_amsua>,
        <http://vocab.ceda.ac.uk/collection/cci/sensor/sens_ascat>,
        <http://vocab.ceda.ac.uk/collection/cci/sensor/sens_avhrr3>,
        <http://vocab.ceda.ac.uk/collection/cci/sensor/sens_gome2>,
        <http://vocab.ceda.ac.uk/collection/cci/sensor/sens_hirs4>,
        <http://vocab.ceda.ac.uk/collection/cci/sensor/sens_iasi> ;
    rdfs:seeAlso <http://www.wmo-sat.info/oscar/satellites/view/307> ;
    skos:broader <http://vocab.ceda.ac.uk/collection/cci/platformProg/plat_metop> ;
    skos:definition "ESA/EUMETSAT Meteorological operational Polar System satellite – B"@en ;
    skos:inScheme cci-scheme:platform ;
    skos:prefLabel "Metop-B"@en ;
    skos:scopeNote "ESA/EUMETSAT Meteorological operational Polar System satellite – B"@en ;
    skos:topConceptOf cci-scheme:platform .

<http://vocab.ceda.ac.uk/collection/cci/platformProg/plat_dmsp_5D3> a cci:platformProg,
        skos:Concept ;
    rdfs:seeAlso <http://www.wmo-sat.info/oscar/satelliteprogrammes/view/35> ;
    skos:broader <http://vocab.ceda.ac.uk/collection/cci/platformGrp/plat_dmsp> ;
    skos:definition "US Defense Meteorological Satellite Program Block 5D-3"@en ;
    skos:inScheme cci-scheme:platformProg ;
    skos:narrower <http://vocab.ceda.ac.uk/collection/cci/platform/plat_dmsp_F15>,
        <http://vocab.ceda.ac.uk/collection/cci/platform/plat_dmsp_F16>,
        <http://vocab.ceda.ac.uk/collection/cci/platform/plat_dmsp_F17>,
        <http://vocab.ceda.ac.uk/collection/cci/platform/plat_dmsp_F18>,
        <http://vocab.ceda.ac.uk/collection/cci/platform/plat_dmsp_F19>,
        <http://vocab.ceda.ac.uk/collection/cci/platform/plat_dmsp_S20> ;
    skos:prefLabel "DMSP Block 5D-3"@en ;
    skos:scopeNote "US Defense Meteorological Satellite Program Block 5D-3"@en ;
    skos:topConceptOf cci-scheme:platformProg .

<http://vocab.ceda.ac.uk/collection/cci/platformProg/plat_fengyun3> a cci:platformProg,
        skos:Concept ;
    rdfs:seeAlso <http://www.wmo-sat.info/oscar/satelliteprogrammes/view/53> ;
    skos:altLabel "Fengyun"@en ;
    skos:definition "CMA Feng-Yun - 3"@en ;
    skos:inScheme cci-scheme:platformProg ;
    skos:narrower <http://vocab.ceda.ac.uk/collection/cci/platform/plat_FY-3A>,
        <http://vocab.ceda.ac.uk/collection/cci/platform/plat_FY-3B>,
        <http://vocab.ceda.ac.uk/collection/cci/platform/plat_FY-3C>,
        <http://vocab.ceda.ac.uk/collection/cci/platform/plat_FY-3D>,
        <http://vocab.ceda.ac.uk/collection/cci/platform/plat_FY-3E>,
        <http://vocab.ceda.ac.uk/collection/cci/platform/plat_FY-3F>,
        <http://vocab.ceda.ac.uk/collection/cci/platform/plat_FY-3G> ;
    skos:prefLabel "Feng-Yun 3"@en ;
    skos:scopeNote "CMA Feng-Yun - 3"@en ;
    skos:topConceptOf cci-scheme:platformProg .

<http://vocab.ceda.ac.uk/collection/cci/platformProg/plat_landsat> a cci:platformProg,
        skos:Concept ;
    rdfs:seeAlso <http://www.wmo-sat.info/oscar/satelliteprogrammes/view/92> ;
    skos:definition "NASA/USGS Satellite imagery of Earth"@en ;
    skos:inScheme cci-scheme:platformProg ;
    skos:narrower <http://vocab.ceda.ac.uk/collection/cci/platform/plat_landsat_1>,
        <http://vocab.ceda.ac.uk/collection/cci/platform/plat_landsat_2>,
        <http://vocab.ceda.ac.uk/collection/cci/platform/plat_landsat_3>,
        <http://vocab.ceda.ac.uk/collection/cci/platform/plat_landsat_4>,
        <http://vocab.ceda.ac.uk/collection/cci/platform/plat_landsat_5>,
        <http://vocab.ceda.ac.uk/collection/cci/platform/plat_landsat_6>,
        <http://vocab.ceda.ac.uk/collection/cci/platform/plat_landsat_7> ;
    skos:prefLabel "Landsat"@en ;
    skos:scopeNote "NASA/USGS Satellite imagery of Earth"@en ;
    skos:topConceptOf cci-scheme:platformProg .

<http://vocab.ceda.ac.uk/collection/cci/platformProg/plat_nimbus> a cci:platformProg,
        skos:Concept ;
    rdfs:seeAlso <http://www.wmo-sat.info/oscar/satelliteprogrammes/view/108> ;
    skos:definition "NASA Nimbus Research-and-development satellite programme"@en ;
    skos:inScheme cci-scheme:platformProg ;
    skos:narrower <http://vocab.ceda.ac.uk/collection/cci/platform/plat_nimbus1>,
        <http://vocab.ceda.ac.uk/collection/cci/platform/plat_nimbus2>,
        <http://vocab.ceda.ac.uk/collection/cci/platform/plat_nimbus3>,
        <http://vocab.ceda.ac.uk/collection/cci/platform/plat_nimbus4>,
        <http://vocab.ceda.ac.uk/collection/cci/platform/plat_nimbus5>,
        <http://vocab.ceda.ac.uk/collection/cci/platform/plat_nimbus6>,
        <http://vocab.ceda.ac.uk/collection/cci/platform/plat_nimbus7> ;
    skos:prefLabel "Nimbus"@en ;
    skos:scopeNote "NASA Nimbus Research-and-development satellite programme"@en ;
    skos:topConceptOf cci-scheme:platformProg .

<http://vocab.ceda.ac.uk/collection/cci/sensor/sens_ssmI> a cci:sensor,
        skos:Concept ;
    cci:hasPlatform <http://vocab.ceda.ac.uk/collection/cci/platform/plat_dmsp_F08>,
        <http://vocab.ceda.ac.uk/collection/cci/platform/plat_dmsp_F10>,
        <http://vocab.ceda.ac.uk/collection/cci/platform/plat_dmsp_F11>,
        <http://vocab.ceda.ac.uk/collection/cci/platform/plat_dmsp_F12>,
        <http://vocab.ceda.ac.uk/collection/cci/platform/plat_dmsp_F13>,
        <http://vocab.ceda.ac.uk/collection/cci/platform/plat_dmsp_F14>,
        <http://vocab.ceda.ac.uk/collection/cci/platform/plat_dmsp_F15> ;
    rdfs:seeAlso <http://www.wmo-sat.info/oscar/instruments/view/533> ;
    skos:altLabel "SSMI"@en ;
    skos:definition "Special Sensor Microwave Imager"@en ;
    skos:inScheme cci-scheme:sensor ;
    skos:prefLabel "SSM/I"@en ;
    skos:scopeNote "Special Sensor Microwave Imager"@en ;
    skos:topConceptOf cci-scheme:sensor .

<http://vocab.ceda.ac.uk/collection/cci/platform/plat_envisat> a cci:platform,
        skos:Concept ;
    cci:hasSensor <http://vocab.ceda.ac.uk/collection/cci/sensor/sens_aatsr>,
        <http://vocab.ceda.ac.uk/collection/cci/sensor/sens_asar>,
        <http://vocab.ceda.ac.uk/collection/cci/sensor/sens_gomos>,
        <http://vocab.ceda.ac.uk/collection/cci/sensor/sens_meris>,
        <http://vocab.ceda.ac.uk/collection/cci/sensor/sens_mipas>,
        <http://vocab.ceda.ac.uk/collection/cci/sensor/sens_ra2>,
        <http://vocab.ceda.ac.uk/collection/cci/sensor/sens_sciamachy> ;
    rdfs:seeAlso <http://www.wmo-sat.info/oscar/satellites/view/78> ;
    skos:broader <http://vocab.ceda.ac.uk/collection/cci/platformProg/plat_envisat_prog> ;
    skos:definition "ESA Environmental Satellite"@en ;
    skos:inScheme cci-scheme:platform ;
    skos:prefLabel "Envisat"@en ;
    skos:scopeNote "ESA Environmental Satellite"@en ;
    skos:topConceptOf cci-scheme:platform .

<http://vocab.ceda.ac.uk/collection/cci/platformProg/plat_goes_1st> a cci:platformProg,
        skos:Concept ;
    rdfs:seeAlso <http://www.wmo-sat.info/oscar/satelliteprogrammes/view/63> ;
    skos:broader <http://vocab.ceda.ac.uk/collection/cci/platformGrp/plat_goes> ;
    skos:definition "NASA Geostationary Operational Environmental Satellite - 1st generation"@en ;
    skos:inScheme cci-scheme:platformProg ;
    skos:narrower <http://vocab.ceda.ac.uk/collection/cci/platform/plat_goes_01>,
        <http://vocab.ceda.ac.uk/collection/cci/platform/plat_goes_02>,
        <http://vocab.ceda.ac.uk/collection/cci/platform/plat_goes_03>,
        <http://vocab.ceda.ac.uk/collection/cci/platform/plat_goes_04>,
        <http://vocab.ceda.ac.uk/collection/cci/platform/plat_goes_05>,
        <http://vocab.ceda.ac.uk/collection/cci/platform/plat_goes_06>,
        <http://vocab.ceda.ac.uk/collection/cci/platform/plat_goes_07> ;
    skos:prefLabel "GOES 1st Gen"@en ;
    skos:scopeNote "NASA Geostationary Operational Environmental Satellite - 1st generation"@en ;
    skos:topConceptOf cci-scheme:platformProg .

<http://vocab.ceda.ac.uk/collection/cci/sensor/sens_avhrr3> a cci:sensor,
        skos:Concept ;
    cci:hasPlatform <http://vocab.ceda.ac.uk/collection/cci/platform/plat_metOpA>,
        <http://vocab.ceda.ac.uk/collection/cci/platform/plat_metOpB>,
        <http://vocab.ceda.ac.uk/collection/cci/platform/plat_metOpC>,
        <http://vocab.ceda.ac.uk/collection/cci/platform/plat_noaa_15>,
        <http://vocab.ceda.ac.uk/collection/cci/platform/plat_noaa_16>,
        <http://vocab.ceda.ac.uk/collection/cci/platform/plat_noaa_17>,
        <http://vocab.ceda.ac.uk/collection/cci/platform/plat_noaa_18>,
        <http://vocab.ceda.ac.uk/collection/cci/platform/plat_noaa_19> ;
    rdfs:seeAlso <http://www.wmo-sat.info/oscar/instruments/view/62> ;
    skos:definition "Advanced Very High Resolution Radiometer / 3"@en ;
    skos:inScheme cci-scheme:sensor ;
    skos:prefLabel "AVHRR-3"@en ;
    skos:scopeNote "Advanced Very High Resolution Radiometer / 3"@en ;
    skos:topConceptOf cci-scheme:sensor .

<http://vocab.ceda.ac.uk/collection/cci/sensor/sens_amsua> a cci:sensor,
        skos:Concept ;
    cci:hasPlatform <http://vocab.ceda.ac.uk/collection/cci/platform/plat_aqua>,
        <http://vocab.ceda.ac.uk/collection/cci/platform/plat_metOpA>,
        <http://vocab.ceda.ac.uk/collection/cci/platform/plat_metOpB>,
        <http://vocab.ceda.ac.uk/collection/cci/platform/plat_metOpC>,
        <http://vocab.ceda.ac.uk/collection/cci/platform/plat_noaa_15>,
        <http://vocab.ceda.ac.uk/collection/cci/platform/plat_noaa_16>,
        <http://vocab.ceda.ac.uk/collection/cci/platform/plat_noaa_17>,
        <http://vocab.ceda.ac.uk/collection/cci/platform/plat_noaa_18>,
        <http://vocab.ceda.ac.uk/collection/cci/platform/plat_noaa_19> ;
    rdfs:seeAlso <http://www.wmo-sat.info/oscar/instruments/view/30> ;
    skos:definition "Advanced microwave sounding unit – A"@en ;
    skos:inScheme cci-scheme:sensor ;
    skos:prefLabel "AMSU-A"@en ;
    skos:scopeNote "Advanced microwave sounding unit – A"@en ;
    skos:topConceptOf cci-scheme:sensor .

cci: a owl:Ontology,
        skos:ConceptScheme ;
    rdfs:label "CCI Ontology" ;
    vann:preferredNamespaceUri <http://vocab.ceda.ac.uk/ontology/cci#> ;
    vann:preferredNamespacePrefix "cci" ;
    dc:creator "Science and Technology Facilities Council" ;
    dc:date "2025-01-23" ;
    dc:description "<h4>OWL Classes</h4>There are currently eight classes in the ontology, each of which represents an entry in the DRS as well a two object properties to link sensors and platforms.<h5>OWL Classes</h5><p><img src=classes.svg><p></p><h4>Concept Schemes</h4><p>The named individuals of each class are also represented as concepts in SKOS concept schemes: <a href=../../../scheme/cci/dataType>data type</a>, <a href=../../../scheme/cci/ecv>ecv</a>, <a href=../../../scheme/cci/freq>frequency</a>, <a href=../../../scheme/cci/org>institutes</a>, <a href=../../../scheme/cci/platform>platforms</a>, <a href=../../../scheme/cci/procLev>processing levels</a>, <a href=../../../scheme/cci/product>products</a>, and <a href=../../../scheme/cci/sensor>sensors</a>. The use of a concept scheme allows easy navigation up and down the tree as well as providing relationships to concepts from other DRS. As well as relationships between sensors and platforms, each ECV concept is related to one or more data type concepts.</p><h5>SKOS Navigation Down the Concept Scheme</h5><img src=../../../scheme/cci/conceptSchemeDown.svg /><h5>SKOS Navigation Up the Concept Scheme</h5><img src=../../../scheme/cci/conceptSchemeUp.svg /><h4>Collections</h4><p>The named individuals of each class are also represented as members in SKOS collections: <a href=../../../collection/cci/dataType>data type</a>, <a href=../../../collection/cci/ecv>ecv</a>, <a href=../../../collection/cci/freq>frequency</a>, <a href=../../../collection/cci/org>institutes</a>, <a href=../../../collection/cci/platform>platforms</a>, <a href=../../../collection/cci/procLev>processing levels</a>, <a href=../../../collection/cci/product>products</a>, and <a href=../../../collection/cci/sensor>sensors</a>. As well as relationships between sensors and platforms, each ECV concept is related to one or more data type concepts.</p><h5>SKOS Collections</h5><img src=../../../collection/cci/collection.svg />" ;
    dc:publisher "STFC"@en ;
    dc:rights "This work is licensed under a BSD license."@en ;
    dc:title "The CCI Ontology" ;
    rdfs:comment "This ontology represents the Directory Reference Scheme (DRS) used by the ESA Climate Change Initiative <a href=http://cci.esa.int/>CCI project</a>." ;
    owl:versionInfo "0.0.1" ;
    skos:hasTopConcept cci-scheme:dataType,
        cci-scheme:ecv,
        cci-scheme:freq,
        cci-scheme:org,
        cci-scheme:platform,
        cci-scheme:platformGrp,
        cci-scheme:platformProg,
        cci-scheme:procLev,
        cci-scheme:product,
        cci-scheme:project,
        cci-scheme:sensor .

<http://vocab.ceda.ac.uk/collection/cci/platformProg/plat_dmsp_5D2> a cci:platformProg,
        skos:Concept ;
    rdfs:seeAlso <http://www.wmo-sat.info/oscar/satelliteprogrammes/view/34> ;
    skos:broader <http://vocab.ceda.ac.uk/collection/cci/platformGrp/plat_dmsp> ;
    skos:definition "US Defense Meteorological Satellite Program Block 5D-2"@en ;
    skos:inScheme cci-scheme:platformProg ;
    skos:narrower <http://vocab.ceda.ac.uk/collection/cci/platform/plat_dmsp_F06>,
        <http://vocab.ceda.ac.uk/collection/cci/platform/plat_dmsp_F07>,
        <http://vocab.ceda.ac.uk/collection/cci/platform/plat_dmsp_F08>,
        <http://vocab.ceda.ac.uk/collection/cci/platform/plat_dmsp_F09>,
        <http://vocab.ceda.ac.uk/collection/cci/platform/plat_dmsp_F10>,
        <http://vocab.ceda.ac.uk/collection/cci/platform/plat_dmsp_F11>,
        <http://vocab.ceda.ac.uk/collection/cci/platform/plat_dmsp_F12>,
        <http://vocab.ceda.ac.uk/collection/cci/platform/plat_dmsp_F13>,
        <http://vocab.ceda.ac.uk/collection/cci/platform/plat_dmsp_F14> ;
    skos:prefLabel "DMSP Block 5D-2"@en ;
    skos:scopeNote "US Defense Meteorological Satellite Program Block 5D-2"@en ;
    skos:topConceptOf cci-scheme:platformProg .

<http://vocab.ceda.ac.uk/collection/cci/sensor/sens_hirs2> a cci:sensor,
        skos:Concept ;
    cci:hasPlatform <http://vocab.ceda.ac.uk/collection/cci/platform/plat_noaa_10>,
        <http://vocab.ceda.ac.uk/collection/cci/platform/plat_noaa_11>,
        <http://vocab.ceda.ac.uk/collection/cci/platform/plat_noaa_12>,
        <http://vocab.ceda.ac.uk/collection/cci/platform/plat_noaa_13>,
        <http://vocab.ceda.ac.uk/collection/cci/platform/plat_noaa_14>,
        <http://vocab.ceda.ac.uk/collection/cci/platform/plat_noaa_6>,
        <http://vocab.ceda.ac.uk/collection/cci/platform/plat_noaa_7>,
        <http://vocab.ceda.ac.uk/collection/cci/platform/plat_noaa_8>,
        <http://vocab.ceda.ac.uk/collection/cci/platform/plat_noaa_9>,
        <http://vocab.ceda.ac.uk/collection/cci/platform/plat_tiros_n> ;
    rdfs:seeAlso <https://www.wmo-sat.info/oscar/instruments/view/182> ;
    skos:definition "High-Resolution Infra-Red Sounder / 2"@en ;
    skos:inScheme cci-scheme:sensor ;
    skos:prefLabel "HIRS/2"@en ;
    skos:scopeNote "High-Resolution Infra-Red Sounder / 2"@en ;
    skos:topConceptOf cci-scheme:sensor .

<http://vocab.ceda.ac.uk/collection/cci/platformProg/plat_noaa_4th> a cci:platformProg,
        skos:Concept ;
    rdfs:seeAlso <http://www.wmo-sat.info/oscar/satelliteprogrammes/view/111> ;
    skos:broader <http://vocab.ceda.ac.uk/collection/cci/platformGrp/plat_noaa> ;
    skos:definition "NASA NOAA Environmental satellites 4th Generation"@en ;
    skos:inScheme cci-scheme:platformProg ;
    skos:narrower <http://vocab.ceda.ac.uk/collection/cci/platform/plat_noaa_10>,
        <http://vocab.ceda.ac.uk/collection/cci/platform/plat_noaa_11>,
        <http://vocab.ceda.ac.uk/collection/cci/platform/plat_noaa_12>,
        <http://vocab.ceda.ac.uk/collection/cci/platform/plat_noaa_13>,
        <http://vocab.ceda.ac.uk/collection/cci/platform/plat_noaa_14>,
        <http://vocab.ceda.ac.uk/collection/cci/platform/plat_noaa_6>,
        <http://vocab.ceda.ac.uk/collection/cci/platform/plat_noaa_7>,
        <http://vocab.ceda.ac.uk/collection/cci/platform/plat_noaa_8>,
        <http://vocab.ceda.ac.uk/collection/cci/platform/plat_noaa_9>,
        <http://vocab.ceda.ac.uk/collection/cci/platform/plat_tiros_n> ;
    skos:prefLabel "NOAA-4th"@en ;
    skos:scopeNote "NASA NOAA Environmental satellites 4th Generation"@en ;
    skos:topConceptOf cci-scheme:platformProg .

<http://vocab.ceda.ac.uk/collection/cci/platformProg/plat_goes_2nd> a cci:platformProg,
        skos:Concept ;
    rdfs:seeAlso <http://www.wmo-sat.info/oscar/satelliteprogrammes/view/64> ;
    skos:broader <http://vocab.ceda.ac.uk/collection/cci/platformGrp/plat_goes> ;
    skos:definition "NASA Geostationary Operational Environmental Satellite - 2nd generation"@en ;
    skos:inScheme cci-scheme:platformProg ;
    skos:narrower <http://vocab.ceda.ac.uk/collection/cci/platform/plat_goes_08>,
        <http://vocab.ceda.ac.uk/collection/cci/platform/plat_goes_09>,
        <http://vocab.ceda.ac.uk/collection/cci/platform/plat_goes_09_bk>,
        <http://vocab.ceda.ac.uk/collection/cci/platform/plat_goes_10>,
        <http://vocab.ceda.ac.uk/collection/cci/platform/plat_goes_10_SA>,
        <http://vocab.ceda.ac.uk/collection/cci/platform/plat_goes_11>,
        <http://vocab.ceda.ac.uk/collection/cci/platform/plat_goes_12>,
        <http://vocab.ceda.ac.uk/collection/cci/platform/plat_goes_12_SA>,
        <http://vocab.ceda.ac.uk/collection/cci/platform/plat_goes_13>,
        <http://vocab.ceda.ac.uk/collection/cci/platform/plat_goes_14>,
        <http://vocab.ceda.ac.uk/collection/cci/platform/plat_goes_15> ;
    skos:prefLabel "GOES 2nd Gen"@en ;
    skos:scopeNote "NASA Geostationary Operational Environmental Satellite - 2nd generation"@en ;
    skos:topConceptOf cci-scheme:platformProg .

<http://vocab.ceda.ac.uk/collection/cci/platformProg/plat_mfg_prog> a cci:platformProg,
        skos:Concept ;
    rdfs:seeAlso <https://www.wmo-sat.info/oscar/satelliteprogrammes/view/101> ;
    skos:definition "EUMETSAT/ ESA Meteosat First Generation"@en ;
    skos:inScheme cci-scheme:platformProg ;
    skos:narrower <http://vocab.ceda.ac.uk/collection/cci/platform/plat_meteosat_1>,
        <http://vocab.ceda.ac.uk/collection/cci/platform/plat_meteosat_2>,
        <http://vocab.ceda.ac.uk/collection/cci/platform/plat_meteosat_3>,
        <http://vocab.ceda.ac.uk/collection/cci/platform/plat_meteosat_3_adc>,
        <http://vocab.ceda.ac.uk/collection/cci/platform/plat_meteosat_3_xadc>,
        <http://vocab.ceda.ac.uk/collection/cci/platform/plat_meteosat_4>,
        <http://vocab.ceda.ac.uk/collection/cci/platform/plat_meteosat_5>,
        <http://vocab.ceda.ac.uk/collection/cci/platform/plat_meteosat_5_iodc>,
        <http://vocab.ceda.ac.uk/collection/cci/platform/plat_meteosat_6>,
        <http://vocab.ceda.ac.uk/collection/cci/platform/plat_meteosat_6_iodc>,
        <http://vocab.ceda.ac.uk/collection/cci/platform/plat_meteosat_7>,
        <http://vocab.ceda.ac.uk/collection/cci/platform/plat_meteosat_7_iodc> ;
    skos:prefLabel "Meteosat First Generation"@en ;
    skos:scopeNote "EUMETSAT/ ESA Meteosat First Generation"@en ;
    skos:topConceptOf cci-scheme:platformProg .

<http://vocab.ceda.ac.uk/collection/cci/sensor/sens_mviri> a cci:sensor,
        skos:Concept ;
    cci:hasPlatform <http://vocab.ceda.ac.uk/collection/cci/platform/plat_meteosat_1>,
        <http://vocab.ceda.ac.uk/collection/cci/platform/plat_meteosat_2>,
        <http://vocab.ceda.ac.uk/collection/cci/platform/plat_meteosat_3>,
        <http://vocab.ceda.ac.uk/collection/cci/platform/plat_meteosat_3_adc>,
        <http://vocab.ceda.ac.uk/collection/cci/platform/plat_meteosat_3_xadc>,
        <http://vocab.ceda.ac.uk/collection/cci/platform/plat_meteosat_4>,
        <http://vocab.ceda.ac.uk/collection/cci/platform/plat_meteosat_5>,
        <http://vocab.ceda.ac.uk/collection/cci/platform/plat_meteosat_5_iodc>,
        <http://vocab.ceda.ac.uk/collection/cci/platform/plat_meteosat_6>,
        <http://vocab.ceda.ac.uk/collection/cci/platform/plat_meteosat_6_iodc>,
        <http://vocab.ceda.ac.uk/collection/cci/platform/plat_meteosat_7>,
        <http://vocab.ceda.ac.uk/collection/cci/platform/plat_meteosat_7_iodc> ;
    rdfs:seeAlso <https://www.wmo-sat.info/oscar/instruments/view/337> ;
    skos:definition "Meteosat Visible Infra-red Imager"@en ;
    skos:inScheme cci-scheme:sensor ;
    skos:prefLabel "MVIRI"@en ;
    skos:scopeNote "Meteosat Visible Infra-red Imager"@en ;
    skos:topConceptOf cci-scheme:sensor .

cci:procLev a owl:Class ;
    rdfs:label "Processing Level" ;
    dc:description "The different processing levels of satellite observational data that are used within the ESA Climate Change Initiative (CCI)." ;
    rdfs:isDefinedBy <http://vocab.ceda.ac.uk/ontology/cci#> .

cci:freq a owl:Class ;
    rdfs:label "Frequency" ;
    dc:description "Temporal frequencies of data from the ESA Climate Change Initiative (CCI)." ;
    rdfs:isDefinedBy <http://vocab.ceda.ac.uk/ontology/cci#> .

cci:ecv a owl:Class ;
    rdfs:label "ECV" ;
    dc:description "The Essential Climate Variable (ECVs) in the ESA Climate Change Initiative (<a href=http://cci.esa.int/> CCI </a>)." ;
    rdfs:isDefinedBy <http://vocab.ceda.ac.uk/ontology/cci#> .

cci:project a owl:Class ;
    rdfs:label "Project" ;
    dc:description "The different projects within the ESA Climate Change Initiative (CCI)." ;
    rdfs:isDefinedBy <http://vocab.ceda.ac.uk/ontology/cci#> .

cci-scheme:procLev a skos:ConceptScheme ;
    dc:creator "Science and Technology Facilities Council" ;
    dc:date "2025-01-23" ;
    dc:description "<p>The CCI concept schemes are used to define concepts within an element of a Directory Reference Scheme. There are currently eight concept schemes defined: <a href=../dataType>data type</a>, <a href=..//ecv>ecv</a>, <a href=../scheme/cci/freq>frequency</a>, <a href=../org>institutes</a>, <a href=../platform>platforms</a>, <a href=../procLev>processing levels</a>, <a href=../product>products</a>, and <a href=../sensor>sensors</a>. The use of a concept scheme allows easy navigation up and down the tree.</p><h5>SKOS Navigation Down the Concept Scheme</h5><img src=conceptSchemeDown.svg /><h5>SKOS Navigation Up the Concept Scheme</h5><img src=conceptSchemeUp.svg /><p>As well as being concepts the the concepts are also named individuals of the <a href=../../../ontology/cci>CCI Ontology</a> classes.<h5>OWL Classes</h5><img src=classes.svg /><p></p>" ;
    dc:publisher "STFC"@en ;
    dc:rights "This work is licensed under a BSD license."@en ;
    dc:title "Processing Level" ;
    rdfs:comment "This concept scheme represents the processing levels used by the CCI project" ;
    owl:versionInfo "0.0.1" ;
    skos:definition "The different processing levels of satellite observational data that are used within the ESA Climate Change Initiative (CCI)."@en ;
    skos:hasTopConcept <http://vocab.ceda.ac.uk/collection/cci/procLev/proc_ind>,
        <http://vocab.ceda.ac.uk/collection/cci/procLev/proc_level0>,
        <http://vocab.ceda.ac.uk/collection/cci/procLev/proc_level1>,
        <http://vocab.ceda.ac.uk/collection/cci/procLev/proc_level1A>,
        <http://vocab.ceda.ac.uk/collection/cci/procLev/proc_level1B>,
        <http://vocab.ceda.ac.uk/collection/cci/procLev/proc_level1C>,
        <http://vocab.ceda.ac.uk/collection/cci/procLev/proc_level2>,
        <http://vocab.ceda.ac.uk/collection/cci/procLev/proc_level2P>,
        <http://vocab.ceda.ac.uk/collection/cci/procLev/proc_level3>,
        <http://vocab.ceda.ac.uk/collection/cci/procLev/proc_level3C>,
        <http://vocab.ceda.ac.uk/collection/cci/procLev/proc_level3S>,
        <http://vocab.ceda.ac.uk/collection/cci/procLev/proc_level3U>,
        <http://vocab.ceda.ac.uk/collection/cci/procLev/proc_level4>,
        <http://vocab.ceda.ac.uk/collection/cci/procLev/proc_unspecified> ;
    skos:prefLabel "Processing Level"@en .

cci-scheme:freq a skos:ConceptScheme ;
    dc:creator "Science and Technology Facilities Council" ;
    dc:date "2025-01-23" ;
    dc:description "<p>The CCI concept schemes are used to define concepts within an element of a Directory Reference Scheme. There are currently eight concept schemes defined: <a href=../dataType>data type</a>, <a href=..//ecv>ecv</a>, <a href=../scheme/cci/freq>frequency</a>, <a href=../org>institutes</a>, <a href=../platform>platforms</a>, <a href=../procLev>processing levels</a>, <a href=../product>products</a>, and <a href=../sensor>sensors</a>. The use of a concept scheme allows easy navigation up and down the tree.</p><h5>SKOS Navigation Down the Concept Scheme</h5><img src=conceptSchemeDown.svg /><h5>SKOS Navigation Up the Concept Scheme</h5><img src=conceptSchemeUp.svg /><p>As well as being concepts the the concepts are also named individuals of the <a href=../../../ontology/cci>CCI Ontology</a> classes.<h5>OWL Classes</h5><img src=classes.svg /><p></p>" ;
    dc:publisher "STFC"@en ;
    dc:rights "This work is licensed under a BSD license."@en ;
    dc:title "Frequency" ;
    rdfs:comment "This concept scheme represents the frequencies used by the CCI project" ;
    owl:versionInfo "0.0.1" ;
    skos:definition "Temporal frequencies of data from the ESA Climate Change Initiative (CCI)."@en ;
    skos:hasTopConcept <http://vocab.ceda.ac.uk/collection/cci/freq/feq_min>,
        <http://vocab.ceda.ac.uk/collection/cci/freq/freq_10day>,
        <http://vocab.ceda.ac.uk/collection/cci/freq/freq_13yr>,
        <http://vocab.ceda.ac.uk/collection/cci/freq/freq_15day>,
        <http://vocab.ceda.ac.uk/collection/cci/freq/freq_3hr>,
        <http://vocab.ceda.ac.uk/collection/cci/freq/freq_5day>,
        <http://vocab.ceda.ac.uk/collection/cci/freq/freq_5yr>,
        <http://vocab.ceda.ac.uk/collection/cci/freq/freq_8day>,
        <http://vocab.ceda.ac.uk/collection/cci/freq/freq_clim>,
        <http://vocab.ceda.ac.uk/collection/cci/freq/freq_day>,
        <http://vocab.ceda.ac.uk/collection/cci/freq/freq_hr>,
        <http://vocab.ceda.ac.uk/collection/cci/freq/freq_mon>,
        <http://vocab.ceda.ac.uk/collection/cci/freq/freq_sat_orb>,
        <http://vocab.ceda.ac.uk/collection/cci/freq/freq_sec>,
        <http://vocab.ceda.ac.uk/collection/cci/freq/freq_unspecified>,
        <http://vocab.ceda.ac.uk/collection/cci/freq/freq_week>,
        <http://vocab.ceda.ac.uk/collection/cci/freq/freq_yr> ;
    skos:prefLabel "Frequency"@en .

cci-scheme:ecv a skos:ConceptScheme ;
    dc:creator "Science and Technology Facilities Council" ;
    dc:date "2025-01-23" ;
    dc:description "<p>The CCI concept schemes are used to define concepts within an element of a Directory Reference Scheme. There are currently eight concept schemes defined: <a href=../dataType>data type</a>, <a href=..//ecv>ecv</a>, <a href=../scheme/cci/freq>frequency</a>, <a href=../org>institutes</a>, <a href=../platform>platforms</a>, <a href=../procLev>processing levels</a>, <a href=../product>products</a>, and <a href=../sensor>sensors</a>. The use of a concept scheme allows easy navigation up and down the tree.</p><h5>SKOS Navigation Down the Concept Scheme</h5><img src=conceptSchemeDown.svg /><h5>SKOS Navigation Up the Concept Scheme</h5><img src=conceptSchemeUp.svg /><p>As well as being concepts the the concepts are also named individuals of the <a href=../../../ontology/cci>CCI Ontology</a> classes.<h5>OWL Classes</h5><img src=classes.svg /><p></p>" ;
    dc:publisher "STFC"@en ;
    dc:rights "This work is licensed under a BSD license."@en ;
    dc:title "ECV" ;
    rdfs:comment "This concept scheme represents the ECVs used by the CCI project" ;
    owl:versionInfo "0.0.1" ;
    skos:definition "The Essential Climate Variable (ECVs) in the ESA Climate Change Initiative (<a href=http://cci.esa.int/> CCI </a>)."@en ;
    skos:hasTopConcept <http://vocab.ceda.ac.uk/collection/cci/ecv/cciecv_aerosol>,
        <http://vocab.ceda.ac.uk/collection/cci/ecv/cciecv_biomass>,
        <http://vocab.ceda.ac.uk/collection/cci/ecv/cciecv_cloud>,
        <http://vocab.ceda.ac.uk/collection/cci/ecv/cciecv_fire>,
        <http://vocab.ceda.ac.uk/collection/cci/ecv/cciecv_ghg>,
        <http://vocab.ceda.ac.uk/collection/cci/ecv/cciecv_glaciers>,
        <http://vocab.ceda.ac.uk/collection/cci/ecv/cciecv_iceSheet>,
        <http://vocab.ceda.ac.uk/collection/cci/ecv/cciecv_lakes>,
        <http://vocab.ceda.ac.uk/collection/cci/ecv/cciecv_landCov>,
        <http://vocab.ceda.ac.uk/collection/cci/ecv/cciecv_landSurfTemp>,
        <http://vocab.ceda.ac.uk/collection/cci/ecv/cciecv_oceanCol>,
        <http://vocab.ceda.ac.uk/collection/cci/ecv/cciecv_ozone>,
        <http://vocab.ceda.ac.uk/collection/cci/ecv/cciecv_permafrost>,
        <http://vocab.ceda.ac.uk/collection/cci/ecv/cciecv_riverDischarge>,
        <http://vocab.ceda.ac.uk/collection/cci/ecv/cciecv_salinity>,
        <http://vocab.ceda.ac.uk/collection/cci/ecv/cciecv_seaIce>,
        <http://vocab.ceda.ac.uk/collection/cci/ecv/cciecv_seaLevel>,
        <http://vocab.ceda.ac.uk/collection/cci/ecv/cciecv_seaState>,
        <http://vocab.ceda.ac.uk/collection/cci/ecv/cciecv_snow>,
        <http://vocab.ceda.ac.uk/collection/cci/ecv/cciecv_soilMst>,
        <http://vocab.ceda.ac.uk/collection/cci/ecv/cciecv_sst>,
        <http://vocab.ceda.ac.uk/collection/cci/ecv/cciecv_vegParam>,
        <http://vocab.ceda.ac.uk/collection/cci/ecv/cciecv_waterVapour> ;
    skos:prefLabel "ECV"@en .

cci-scheme:project a skos:ConceptScheme ;
    dc:creator "Science and Technology Facilities Council" ;
    dc:date "2025-01-23" ;
    dc:description "<p>The CCI concept schemes are used to define concepts within an element of a Directory Reference Scheme. There are currently eight concept schemes defined: <a href=../dataType>data type</a>, <a href=..//ecv>ecv</a>, <a href=../scheme/cci/freq>frequency</a>, <a href=../org>institutes</a>, <a href=../platform>platforms</a>, <a href=../procLev>processing levels</a>, <a href=../product>products</a>, and <a href=../sensor>sensors</a>. The use of a concept scheme allows easy navigation up and down the tree.</p><h5>SKOS Navigation Down the Concept Scheme</h5><img src=conceptSchemeDown.svg /><h5>SKOS Navigation Up the Concept Scheme</h5><img src=conceptSchemeUp.svg /><p>As well as being concepts the the concepts are also named individuals of the <a href=../../../ontology/cci>CCI Ontology</a> classes.<h5>OWL Classes</h5><img src=classes.svg /><p></p>" ;
    dc:publisher "STFC"@en ;
    dc:rights "This work is licensed under a BSD license."@en ;
    dc:title "Project" ;
    rdfs:comment "This concept scheme represents the projects used by the CCI project" ;
    owl:versionInfo "0.0.1" ;
    skos:definition "The different projects within the ESA Climate Change Initiative (CCI)."@en ;
    skos:hasTopConcept <http://vocab.ceda.ac.uk/collection/cci/project/cciproject_aerosol>,
        <http://vocab.ceda.ac.uk/collection/cci/project/cciproject_biomass>,
        <http://vocab.ceda.ac.uk/collection/cci/project/cciproject_cloud>,
        <http://vocab.ceda.ac.uk/collection/cci/project/cciproject_fire>,
        <http://vocab.ceda.ac.uk/collection/cci/project/cciproject_ghg>,
        <http://vocab.ceda.ac.uk/collection/cci/project/cciproject_glaciers>,
        <http://vocab.ceda.ac.uk/collection/cci/project/cciproject_iceSheet>,
        <http://vocab.ceda.ac.uk/collection/cci/project/cciproject_lakes>,
        <http://vocab.ceda.ac.uk/collection/cci/project/cciproject_landCov>,
        <http://vocab.ceda.ac.uk/collection/cci/project/cciproject_landSurfTemp>,
        <http://vocab.ceda.ac.uk/collection/cci/project/cciproject_oceanCol>,
        <http://vocab.ceda.ac.uk/collection/cci/project/cciproject_ozone>,
        <http://vocab.ceda.ac.uk/collection/cci/project/cciproject_permafrost>,
        <http://vocab.ceda.ac.uk/collection/cci/project/cciproject_riverDischarge>,
        <http://vocab.ceda.ac.uk/collection/cci/project/cciproject_salinity>,
        <http://vocab.ceda.ac.uk/collection/cci/project/cciproject_seaIce>,
        <http://vocab.ceda.ac.uk/collection/cci/project/cciproject_seaLevel>,
        <http://vocab.ceda.ac.uk/collection/cci/project/cciproject_seaState>,
        <http://vocab.ceda.ac.uk/collection/cci/project/cciproject_snow>,
        <http://vocab.ceda.ac.uk/collection/cci/project/cciproject_soilMst>,
        <http://vocab.ceda.ac.uk/collection/cci/project/cciproject_sst>,
        <http://vocab.ceda.ac.uk/collection/cci/project/cciproject_vegParam>,
        <http://vocab.ceda.ac.uk/collection/cci/project/cciproject_waterVapour> ;
    skos:prefLabel "Project"@en .

cci:platformProg a owl:Class ;
    rdfs:label "Platform Programme" ;
    dc:description "The platform programmes that have been used in the collection of data for the ESA Climate Change Initiative (CCI). A programme consists of a number of <a href=#platform>platforms</a>" ;
    rdfs:isDefinedBy <http://vocab.ceda.ac.uk/ontology/cci#> .

cci:dataType a owl:Class ;
    rdfs:label "Geophysical Quantity" ;
    dc:description "The main data type in a data set used by the ESA Climate Change Initiative (CCI)." ;
    rdfs:isDefinedBy <http://vocab.ceda.ac.uk/ontology/cci#> .

cci:sensor a owl:Class ;
    rdfs:label "Sensor" ;
    dc:description "The sensors that have been used in the collection of the data for the ESA Climate Change Initiative (CCI)." ;
    rdfs:isDefinedBy <http://vocab.ceda.ac.uk/ontology/cci#> .

cci:org a owl:Class ;
    rdfs:label "Institute" ;
    dc:description "Organisations (institutions) that are involved in production of data for the ESA Climate Change Initiative (CCI)." ;
    rdfs:isDefinedBy <http://vocab.ceda.ac.uk/ontology/cci#> .

cci-scheme:platformProg a skos:ConceptScheme ;
    dc:creator "Science and Technology Facilities Council" ;
    dc:date "2025-01-23" ;
    dc:description "<p>The CCI concept schemes are used to define concepts within an element of a Directory Reference Scheme. There are currently eight concept schemes defined: <a href=../dataType>data type</a>, <a href=..//ecv>ecv</a>, <a href=../scheme/cci/freq>frequency</a>, <a href=../org>institutes</a>, <a href=../platform>platforms</a>, <a href=../procLev>processing levels</a>, <a href=../product>products</a>, and <a href=../sensor>sensors</a>. The use of a concept scheme allows easy navigation up and down the tree.</p><h5>SKOS Navigation Down the Concept Scheme</h5><img src=conceptSchemeDown.svg /><h5>SKOS Navigation Up the Concept Scheme</h5><img src=conceptSchemeUp.svg /><p>As well as being concepts the the concepts are also named individuals of the <a href=../../../ontology/cci>CCI Ontology</a> classes.<h5>OWL Classes</h5><img src=classes.svg /><p></p>" ;
    dc:publisher "STFC"@en ;
    dc:rights "This work is licensed under a BSD license."@en ;
    dc:title "Platform Programme" ;
    rdfs:comment "This concept scheme represents the platforms used by the CCI project" ;
    owl:versionInfo "0.0.1" ;
    skos:definition "The platform programmes that have been used in the collection of data for the ESA Climate Change Initiative (CCI). A programme consists of a number of <a href=#platform>platforms</a>"@en ;
    skos:hasTopConcept <http://vocab.ceda.ac.uk/collection/cci/platformProg/plat_alos_prog>,
        <http://vocab.ceda.ac.uk/collection/cci/platformProg/plat_coriolis_prog>,
        <http://vocab.ceda.ac.uk/collection/cci/platformProg/plat_cryosat_prog>,
        <http://vocab.ceda.ac.uk/collection/cci/platformProg/plat_csk_prog>,
        <http://vocab.ceda.ac.uk/collection/cci/platformProg/plat_dmsp_5D1>,
        <http://vocab.ceda.ac.uk/collection/cci/platformProg/plat_dmsp_5D2>,
        <http://vocab.ceda.ac.uk/collection/cci/platformProg/plat_dmsp_5D3>,
        <http://vocab.ceda.ac.uk/collection/cci/platformProg/plat_envisat_prog>,
        <http://vocab.ceda.ac.uk/collection/cci/platformProg/plat_eos>,
        <http://vocab.ceda.ac.uk/collection/cci/platformProg/plat_ers>,
        <http://vocab.ceda.ac.uk/collection/cci/platformProg/plat_fengyun3>,
        <http://vocab.ceda.ac.uk/collection/cci/platformProg/plat_gcom>,
        <http://vocab.ceda.ac.uk/collection/cci/platformProg/plat_geodetic>,
        <http://vocab.ceda.ac.uk/collection/cci/platformProg/plat_goes_1st>,
        <http://vocab.ceda.ac.uk/collection/cci/platformProg/plat_goes_2nd>,
        <http://vocab.ceda.ac.uk/collection/cci/platformProg/plat_goes_3rd>,
        <http://vocab.ceda.ac.uk/collection/cci/platformProg/plat_gosat_prog>,
        <http://vocab.ceda.ac.uk/collection/cci/platformProg/plat_gpm_prog>,
        <http://vocab.ceda.ac.uk/collection/cci/platformProg/plat_grace_prog>,
        <http://vocab.ceda.ac.uk/collection/cci/platformProg/plat_himawari>,
        <http://vocab.ceda.ac.uk/collection/cci/platformProg/plat_icesat_prog>,
        <http://vocab.ceda.ac.uk/collection/cci/platformProg/plat_jason>,
        <http://vocab.ceda.ac.uk/collection/cci/platformProg/plat_jpss_prog>,
        <http://vocab.ceda.ac.uk/collection/cci/platformProg/plat_landsat>,
        <http://vocab.ceda.ac.uk/collection/cci/platformProg/plat_landsat_dcm>,
        <http://vocab.ceda.ac.uk/collection/cci/platformProg/plat_metop>,
        <http://vocab.ceda.ac.uk/collection/cci/platformProg/plat_mfg_prog>,
        <http://vocab.ceda.ac.uk/collection/cci/platformProg/plat_msg>,
        <http://vocab.ceda.ac.uk/collection/cci/platformProg/plat_nimbus>,
        <http://vocab.ceda.ac.uk/collection/cci/platformProg/plat_noaa_3rd>,
        <http://vocab.ceda.ac.uk/collection/cci/platformProg/plat_noaa_4th>,
        <http://vocab.ceda.ac.uk/collection/cci/platformProg/plat_noaa_5th>,
        <http://vocab.ceda.ac.uk/collection/cci/platformProg/plat_oco_prog>,
        <http://vocab.ceda.ac.uk/collection/cci/platformProg/plat_odin_prog>,
        <http://vocab.ceda.ac.uk/collection/cci/platformProg/plat_orbview2_prog>,
        <http://vocab.ceda.ac.uk/collection/cci/platformProg/plat_parasol_prog>,
        <http://vocab.ceda.ac.uk/collection/cci/platformProg/plat_proba_prog>,
        <http://vocab.ceda.ac.uk/collection/cci/platformProg/plat_radarsat_prog>,
        <http://vocab.ceda.ac.uk/collection/cci/platformProg/plat_s5p_prog>,
        <http://vocab.ceda.ac.uk/collection/cci/platformProg/plat_sac_prog>,
        <http://vocab.ceda.ac.uk/collection/cci/platformProg/plat_saral_prog>,
        <http://vocab.ceda.ac.uk/collection/cci/platformProg/plat_scisat_prog>,
        <http://vocab.ceda.ac.uk/collection/cci/platformProg/plat_sentinel1_prog>,
        <http://vocab.ceda.ac.uk/collection/cci/platformProg/plat_sentinel2_prog>,
        <http://vocab.ceda.ac.uk/collection/cci/platformProg/plat_sentinel3_prog>,
        <http://vocab.ceda.ac.uk/collection/cci/platformProg/plat_sentinel6_prog>,
        <http://vocab.ceda.ac.uk/collection/cci/platformProg/plat_smap_prog>,
        <http://vocab.ceda.ac.uk/collection/cci/platformProg/plat_smos_prog>,
        <http://vocab.ceda.ac.uk/collection/cci/platformProg/plat_spot>,
        <http://vocab.ceda.ac.uk/collection/cci/platformProg/plat_spot_prog_follow>,
        <http://vocab.ceda.ac.uk/collection/cci/platformProg/plat_terraSAR>,
        <http://vocab.ceda.ac.uk/collection/cci/platformProg/plat_topexPoseidon_prog>,
        <http://vocab.ceda.ac.uk/collection/cci/platformProg/plat_trmm_prog> ;
    skos:prefLabel "Platform Programme"@en .

cci:platform a owl:Class ;
    rdfs:label "Platform" ;
    dc:description "The platforms that have been used in the collection of data for the ESA Climate Change Initiative (CCI)." ;
    rdfs:isDefinedBy <http://vocab.ceda.ac.uk/ontology/cci#> .

cci-scheme:dataType a skos:ConceptScheme ;
    dc:creator "Science and Technology Facilities Council" ;
    dc:date "2025-01-23" ;
    dc:description "<p>The CCI concept schemes are used to define concepts within an element of a Directory Reference Scheme. There are currently eight concept schemes defined: <a href=../dataType>data type</a>, <a href=..//ecv>ecv</a>, <a href=../scheme/cci/freq>frequency</a>, <a href=../org>institutes</a>, <a href=../platform>platforms</a>, <a href=../procLev>processing levels</a>, <a href=../product>products</a>, and <a href=../sensor>sensors</a>. The use of a concept scheme allows easy navigation up and down the tree.</p><h5>SKOS Navigation Down the Concept Scheme</h5><img src=conceptSchemeDown.svg /><h5>SKOS Navigation Up the Concept Scheme</h5><img src=conceptSchemeUp.svg /><p>As well as being concepts the the concepts are also named individuals of the <a href=../../../ontology/cci>CCI Ontology</a> classes.<h5>OWL Classes</h5><img src=classes.svg /><p></p>" ;
    dc:publisher "STFC"@en ;
    dc:rights "This work is licensed under a BSD license."@en ;
    dc:title "Geophysical Quantity" ;
    rdfs:comment "This concept scheme represents the data types used by the CCI project" ;
    owl:versionInfo "0.0.1" ;
    skos:definition "The main data type in a data set used by the ESA Climate Change Initiative (CCI)."@en ;
    skos:hasTopConcept <http://vocab.ceda.ac.uk/collection/cci/dataType/dtype_aai>,
        <http://vocab.ceda.ac.uk/collection/cci/dataType/dtype_adg>,
        <http://vocab.ceda.ac.uk/collection/cci/dataType/dtype_adt>,
        <http://vocab.ceda.ac.uk/collection/cci/dataType/dtype_aerProd>,
        <http://vocab.ceda.ac.uk/collection/cci/dataType/dtype_aex>,
        <http://vocab.ceda.ac.uk/collection/cci/dataType/dtype_agb>,
        <http://vocab.ceda.ac.uk/collection/cci/dataType/dtype_alb>,
        <http://vocab.ceda.ac.uk/collection/cci/dataType/dtype_all>,
        <http://vocab.ceda.ac.uk/collection/cci/dataType/dtype_alt>,
        <http://vocab.ceda.ac.uk/collection/cci/dataType/dtype_aod>,
        <http://vocab.ceda.ac.uk/collection/cci/dataType/dtype_aph>,
        <http://vocab.ceda.ac.uk/collection/cci/dataType/dtype_atot>,
        <http://vocab.ceda.ac.uk/collection/cci/dataType/dtype_aty>,
        <http://vocab.ceda.ac.uk/collection/cci/dataType/dtype_ba>,
        <http://vocab.ceda.ac.uk/collection/cci/dataType/dtype_bb>,
        <http://vocab.ceda.ac.uk/collection/cci/dataType/dtype_cer>,
        <http://vocab.ceda.ac.uk/collection/cci/dataType/dtype_cfc>,
        <http://vocab.ceda.ac.uk/collection/cci/dataType/dtype_cfl>,
        <http://vocab.ceda.ac.uk/collection/cci/dataType/dtype_ch4>,
        <http://vocab.ceda.ac.uk/collection/cci/dataType/dtype_chlorA>,
        <http://vocab.ceda.ac.uk/collection/cci/dataType/dtype_cldProd>,
        <http://vocab.ceda.ac.uk/collection/cci/dataType/dtype_co2>,
        <http://vocab.ceda.ac.uk/collection/cci/dataType/dtype_cot>,
        <http://vocab.ceda.ac.uk/collection/cci/dataType/dtype_cth>,
        <http://vocab.ceda.ac.uk/collection/cci/dataType/dtype_ctp>,
        <http://vocab.ceda.ac.uk/collection/cci/dataType/dtype_ctt>,
        <http://vocab.ceda.ac.uk/collection/cci/dataType/dtype_ga>,
        <http://vocab.ceda.ac.uk/collection/cci/dataType/dtype_gll>,
        <http://vocab.ceda.ac.uk/collection/cci/dataType/dtype_gmb>,
        <http://vocab.ceda.ac.uk/collection/cci/dataType/dtype_gtd>,
        <http://vocab.ceda.ac.uk/collection/cci/dataType/dtype_iop>,
        <http://vocab.ceda.ac.uk/collection/cci/dataType/dtype_iv>,
        <http://vocab.ceda.ac.uk/collection/cci/dataType/dtype_iwp>,
        <http://vocab.ceda.ac.uk/collection/cci/dataType/dtype_jch>,
        <http://vocab.ceda.ac.uk/collection/cci/dataType/dtype_k_490>,
        <http://vocab.ceda.ac.uk/collection/cci/dataType/dtype_lai>,
        <http://vocab.ceda.ac.uk/collection/cci/dataType/dtype_lcchange>,
        <http://vocab.ceda.ac.uk/collection/cci/dataType/dtype_lccs>,
        <http://vocab.ceda.ac.uk/collection/cci/dataType/dtype_lkProds>,
        <http://vocab.ceda.ac.uk/collection/cci/dataType/dtype_lp>,
        <http://vocab.ceda.ac.uk/collection/cci/dataType/dtype_lst>,
        <http://vocab.ceda.ac.uk/collection/cci/dataType/dtype_lwp>,
        <http://vocab.ceda.ac.uk/collection/cci/dataType/dtype_map>,
        <http://vocab.ceda.ac.uk/collection/cci/dataType/dtype_msl>,
        <http://vocab.ceda.ac.uk/collection/cci/dataType/dtype_msla>,
        <http://vocab.ceda.ac.uk/collection/cci/dataType/dtype_mslamph>,
        <http://vocab.ceda.ac.uk/collection/cci/dataType/dtype_msltr>,
        <http://vocab.ceda.ac.uk/collection/cci/dataType/dtype_ndvi>,
        <http://vocab.ceda.ac.uk/collection/cci/dataType/dtype_nlw>,
        <http://vocab.ceda.ac.uk/collection/cci/dataType/dtype_np>,
        <http://vocab.ceda.ac.uk/collection/cci/dataType/dtype_ocProd>,
        <http://vocab.ceda.ac.uk/collection/cci/dataType/dtype_pfr>,
        <http://vocab.ceda.ac.uk/collection/cci/dataType/dtype_pft>,
        <http://vocab.ceda.ac.uk/collection/cci/dataType/dtype_rrs>,
        <http://vocab.ceda.ac.uk/collection/cci/dataType/dtype_scfg>,
        <http://vocab.ceda.ac.uk/collection/cci/dataType/dtype_scfv>,
        <http://vocab.ceda.ac.uk/collection/cci/dataType/dtype_sec>,
        <http://vocab.ceda.ac.uk/collection/cci/dataType/dtype_sic>,
        <http://vocab.ceda.ac.uk/collection/cci/dataType/dtype_sie>,
        <http://vocab.ceda.ac.uk/collection/cci/dataType/dtype_sit>,
        <http://vocab.ceda.ac.uk/collection/cci/dataType/dtype_sla>,
        <http://vocab.ceda.ac.uk/collection/cci/dataType/dtype_snow>,
        <http://vocab.ceda.ac.uk/collection/cci/dataType/dtype_sr>,
        <http://vocab.ceda.ac.uk/collection/cci/dataType/dtype_ssh>,
        <http://vocab.ceda.ac.uk/collection/cci/dataType/dtype_ssms>,
        <http://vocab.ceda.ac.uk/collection/cci/dataType/dtype_ssmsa>,
        <http://vocab.ceda.ac.uk/collection/cci/dataType/dtype_ssmv>,
        <http://vocab.ceda.ac.uk/collection/cci/dataType/dtype_ssmva>,
        <http://vocab.ceda.ac.uk/collection/cci/dataType/dtype_sss>,
        <http://vocab.ceda.ac.uk/collection/cci/dataType/dtype_sstDepth>,
        <http://vocab.ceda.ac.uk/collection/cci/dataType/dtype_sstFnd>,
        <http://vocab.ceda.ac.uk/collection/cci/dataType/dtype_sstInt>,
        <http://vocab.ceda.ac.uk/collection/cci/dataType/dtype_sstSkin>,
        <http://vocab.ceda.ac.uk/collection/cci/dataType/dtype_sstSubsk>,
        <http://vocab.ceda.ac.uk/collection/cci/dataType/dtype_swe>,
        <http://vocab.ceda.ac.uk/collection/cci/dataType/dtype_swh>,
        <http://vocab.ceda.ac.uk/collection/cci/dataType/dtype_swis>,
        <http://vocab.ceda.ac.uk/collection/cci/dataType/dtype_swisa>,
        <http://vocab.ceda.ac.uk/collection/cci/dataType/dtype_swiv>,
        <http://vocab.ceda.ac.uk/collection/cci/dataType/dtype_swiva>,
        <http://vocab.ceda.ac.uk/collection/cci/dataType/dtype_tc>,
        <http://vocab.ceda.ac.uk/collection/cci/dataType/dtype_tcwv>,
        <http://vocab.ceda.ac.uk/collection/cci/dataType/dtype_uncert>,
        <http://vocab.ceda.ac.uk/collection/cci/dataType/dtype_unspecified>,
        <http://vocab.ceda.ac.uk/collection/cci/dataType/dtype_v>,
        <http://vocab.ceda.ac.uk/collection/cci/dataType/dtype_vp>,
        <http://vocab.ceda.ac.uk/collection/cci/dataType/dtype_wb>,
        <http://vocab.ceda.ac.uk/collection/cci/dataType/dtype_wl> ;
    skos:prefLabel "Geophysical Quantity"@en .

cci-scheme:sensor a skos:ConceptScheme ;
    dc:creator "Science and Technology Facilities Council" ;
    dc:date "2025-01-23" ;
    dc:description "<p>The CCI concept schemes are used to define concepts within an element of a Directory Reference Scheme. There are currently eight concept schemes defined: <a href=../dataType>data type</a>, <a href=..//ecv>ecv</a>, <a href=../scheme/cci/freq>frequency</a>, <a href=../org>institutes</a>, <a href=../platform>platforms</a>, <a href=../procLev>processing levels</a>, <a href=../product>products</a>, and <a href=../sensor>sensors</a>. The use of a concept scheme allows easy navigation up and down the tree.</p><h5>SKOS Navigation Down the Concept Scheme</h5><img src=conceptSchemeDown.svg /><h5>SKOS Navigation Up the Concept Scheme</h5><img src=conceptSchemeUp.svg /><p>As well as being concepts the the concepts are also named individuals of the <a href=../../../ontology/cci>CCI Ontology</a> classes.<h5>OWL Classes</h5><img src=classes.svg /><p></p>" ;
    dc:publisher "STFC"@en ;
    dc:rights "This work is licensed under a BSD license."@en ;
    dc:title "Sensor" ;
    rdfs:comment "This concept scheme represents the sensors used by the CCI project" ;
    owl:versionInfo "0.0.1" ;
    skos:definition "The sensors that have been used in the collection of the data for the ESA Climate Change Initiative (CCI)."@en ;
    skos:hasTopConcept <http://vocab.ceda.ac.uk/collection/cci/sensor/sens_aatsr>,
        <http://vocab.ceda.ac.uk/collection/cci/sensor/sens_abi>,
        <http://vocab.ceda.ac.uk/collection/cci/sensor/sens_aceFts>,
        <http://vocab.ceda.ac.uk/collection/cci/sensor/sens_airs>,
        <http://vocab.ceda.ac.uk/collection/cci/sensor/sens_altika>,
        <http://vocab.ceda.ac.uk/collection/cci/sensor/sens_amisar>,
        <http://vocab.ceda.ac.uk/collection/cci/sensor/sens_amiscat>,
        <http://vocab.ceda.ac.uk/collection/cci/sensor/sens_amsr2>,
        <http://vocab.ceda.ac.uk/collection/cci/sensor/sens_amsre>,
        <http://vocab.ceda.ac.uk/collection/cci/sensor/sens_amsua>,
        <http://vocab.ceda.ac.uk/collection/cci/sensor/sens_amsub>,
        <http://vocab.ceda.ac.uk/collection/cci/sensor/sens_aquarius>,
        <http://vocab.ceda.ac.uk/collection/cci/sensor/sens_asar>,
        <http://vocab.ceda.ac.uk/collection/cci/sensor/sens_ascat>,
        <http://vocab.ceda.ac.uk/collection/cci/sensor/sens_aster>,
        <http://vocab.ceda.ac.uk/collection/cci/sensor/sens_atsr>,
        <http://vocab.ceda.ac.uk/collection/cci/sensor/sens_atsr2>,
        <http://vocab.ceda.ac.uk/collection/cci/sensor/sens_avhrr>,
        <http://vocab.ceda.ac.uk/collection/cci/sensor/sens_avhrr2>,
        <http://vocab.ceda.ac.uk/collection/cci/sensor/sens_avhrr3>,
        <http://vocab.ceda.ac.uk/collection/cci/sensor/sens_esmrNim5>,
        <http://vocab.ceda.ac.uk/collection/cci/sensor/sens_esmrNim6>,
        <http://vocab.ceda.ac.uk/collection/cci/sensor/sens_etmplus>,
        <http://vocab.ceda.ac.uk/collection/cci/sensor/sens_gfora>,
        <http://vocab.ceda.ac.uk/collection/cci/sensor/sens_glas>,
        <http://vocab.ceda.ac.uk/collection/cci/sensor/sens_gmi>,
        <http://vocab.ceda.ac.uk/collection/cci/sensor/sens_goesImager1215>,
        <http://vocab.ceda.ac.uk/collection/cci/sensor/sens_goesImager811>,
        <http://vocab.ceda.ac.uk/collection/cci/sensor/sens_gome>,
        <http://vocab.ceda.ac.uk/collection/cci/sensor/sens_gome2>,
        <http://vocab.ceda.ac.uk/collection/cci/sensor/sens_gomos>,
        <http://vocab.ceda.ac.uk/collection/cci/sensor/sens_grace>,
        <http://vocab.ceda.ac.uk/collection/cci/sensor/sens_hirs>,
        <http://vocab.ceda.ac.uk/collection/cci/sensor/sens_hirs2>,
        <http://vocab.ceda.ac.uk/collection/cci/sensor/sens_hirs3>,
        <http://vocab.ceda.ac.uk/collection/cci/sensor/sens_hirs4>,
        <http://vocab.ceda.ac.uk/collection/cci/sensor/sens_hrs>,
        <http://vocab.ceda.ac.uk/collection/cci/sensor/sens_iasi>,
        <http://vocab.ceda.ac.uk/collection/cci/sensor/sens_imagerMtsat2>,
        <http://vocab.ceda.ac.uk/collection/cci/sensor/sens_jami>,
        <http://vocab.ceda.ac.uk/collection/cci/sensor/sens_meris>,
        <http://vocab.ceda.ac.uk/collection/cci/sensor/sens_mipas>,
        <http://vocab.ceda.ac.uk/collection/cci/sensor/sens_miras>,
        <http://vocab.ceda.ac.uk/collection/cci/sensor/sens_modis>,
        <http://vocab.ceda.ac.uk/collection/cci/sensor/sens_msi>,
        <http://vocab.ceda.ac.uk/collection/cci/sensor/sens_mss>,
        <http://vocab.ceda.ac.uk/collection/cci/sensor/sens_mviri>,
        <http://vocab.ceda.ac.uk/collection/cci/sensor/sens_mwri>,
        <http://vocab.ceda.ac.uk/collection/cci/sensor/sens_nra>,
        <http://vocab.ceda.ac.uk/collection/cci/sensor/sens_oco>,
        <http://vocab.ceda.ac.uk/collection/cci/sensor/sens_olci>,
        <http://vocab.ceda.ac.uk/collection/cci/sensor/sens_oli>,
        <http://vocab.ceda.ac.uk/collection/cci/sensor/sens_omi>,
        <http://vocab.ceda.ac.uk/collection/cci/sensor/sens_osiris>,
        <http://vocab.ceda.ac.uk/collection/cci/sensor/sens_palsar>,
        <http://vocab.ceda.ac.uk/collection/cci/sensor/sens_palsar2>,
        <http://vocab.ceda.ac.uk/collection/cci/sensor/sens_polder>,
        <http://vocab.ceda.ac.uk/collection/cci/sensor/sens_poseidon2>,
        <http://vocab.ceda.ac.uk/collection/cci/sensor/sens_poseidon3>,
        <http://vocab.ceda.ac.uk/collection/cci/sensor/sens_poseidon3b>,
        <http://vocab.ceda.ac.uk/collection/cci/sensor/sens_poseidon4>,
        <http://vocab.ceda.ac.uk/collection/cci/sensor/sens_ra>,
        <http://vocab.ceda.ac.uk/collection/cci/sensor/sens_ra2>,
        <http://vocab.ceda.ac.uk/collection/cci/sensor/sens_sar2000>,
        <http://vocab.ceda.ac.uk/collection/cci/sensor/sens_sarRadarSat2>,
        <http://vocab.ceda.ac.uk/collection/cci/sensor/sens_sarX>,
        <http://vocab.ceda.ac.uk/collection/cci/sensor/sens_sarcS1>,
        <http://vocab.ceda.ac.uk/collection/cci/sensor/sens_sciamachy>,
        <http://vocab.ceda.ac.uk/collection/cci/sensor/sens_seaWiFs>,
        <http://vocab.ceda.ac.uk/collection/cci/sensor/sens_seviri>,
        <http://vocab.ceda.ac.uk/collection/cci/sensor/sens_siral>,
        <http://vocab.ceda.ac.uk/collection/cci/sensor/sens_slstr>,
        <http://vocab.ceda.ac.uk/collection/cci/sensor/sens_smap>,
        <http://vocab.ceda.ac.uk/collection/cci/sensor/sens_smmr>,
        <http://vocab.ceda.ac.uk/collection/cci/sensor/sens_smr>,
        <http://vocab.ceda.ac.uk/collection/cci/sensor/sens_sral>,
        <http://vocab.ceda.ac.uk/collection/cci/sensor/sens_ssalt>,
        <http://vocab.ceda.ac.uk/collection/cci/sensor/sens_ssmI>,
        <http://vocab.ceda.ac.uk/collection/cci/sensor/sens_ssmiS>,
        <http://vocab.ceda.ac.uk/collection/cci/sensor/sens_tansoCai>,
        <http://vocab.ceda.ac.uk/collection/cci/sensor/sens_tansoFts>,
        <http://vocab.ceda.ac.uk/collection/cci/sensor/sens_tansoFts2>,
        <http://vocab.ceda.ac.uk/collection/cci/sensor/sens_tirs>,
        <http://vocab.ceda.ac.uk/collection/cci/sensor/sens_tm>,
        <http://vocab.ceda.ac.uk/collection/cci/sensor/sens_tmi>,
        <http://vocab.ceda.ac.uk/collection/cci/sensor/sens_toms>,
        <http://vocab.ceda.ac.uk/collection/cci/sensor/sens_tropomi>,
        <http://vocab.ceda.ac.uk/collection/cci/sensor/sens_unspecified>,
        <http://vocab.ceda.ac.uk/collection/cci/sensor/sens_vegetation>,
        <http://vocab.ceda.ac.uk/collection/cci/sensor/sens_vegetationP>,
        <http://vocab.ceda.ac.uk/collection/cci/sensor/sens_viirs>,
        <http://vocab.ceda.ac.uk/collection/cci/sensor/sens_virr>,
        <http://vocab.ceda.ac.uk/collection/cci/sensor/sens_windSat> ;
    skos:prefLabel "Sensor"@en .

cci:product a owl:Class ;
    rdfs:label "Product" ;
    dc:description "The different products that are produced within the ESA Climate Change Initiative (CCI)." ;
    rdfs:isDefinedBy <http://vocab.ceda.ac.uk/ontology/cci#> .

cci-scheme:org a skos:ConceptScheme ;
    dc:creator "Science and Technology Facilities Council" ;
    dc:date "2025-01-23" ;
    dc:description "<p>The CCI concept schemes are used to define concepts within an element of a Directory Reference Scheme. There are currently eight concept schemes defined: <a href=../dataType>data type</a>, <a href=..//ecv>ecv</a>, <a href=../scheme/cci/freq>frequency</a>, <a href=../org>institutes</a>, <a href=../platform>platforms</a>, <a href=../procLev>processing levels</a>, <a href=../product>products</a>, and <a href=../sensor>sensors</a>. The use of a concept scheme allows easy navigation up and down the tree.</p><h5>SKOS Navigation Down the Concept Scheme</h5><img src=conceptSchemeDown.svg /><h5>SKOS Navigation Up the Concept Scheme</h5><img src=conceptSchemeUp.svg /><p>As well as being concepts the the concepts are also named individuals of the <a href=../../../ontology/cci>CCI Ontology</a> classes.<h5>OWL Classes</h5><img src=classes.svg /><p></p>" ;
    dc:publisher "STFC"@en ;
    dc:rights "This work is licensed under a BSD license."@en ;
    dc:title "Institute" ;
    rdfs:comment "This concept scheme represents the organisations in the CCI project" ;
    owl:versionInfo "0.0.1" ;
    skos:definition "Organisations (institutions) that are involved in production of data for the ESA Climate Change Initiative (CCI)."@en ;
    skos:hasTopConcept <http://vocab.ceda.ac.uk/collection/cci/org/org01>,
        <http://vocab.ceda.ac.uk/collection/cci/org/org02>,
        <http://vocab.ceda.ac.uk/collection/cci/org/org03>,
        <http://vocab.ceda.ac.uk/collection/cci/org/org04>,
        <http://vocab.ceda.ac.uk/collection/cci/org/org05>,
        <http://vocab.ceda.ac.uk/collection/cci/org/org06>,
        <http://vocab.ceda.ac.uk/collection/cci/org/org07>,
        <http://vocab.ceda.ac.uk/collection/cci/org/org08>,
        <http://vocab.ceda.ac.uk/collection/cci/org/org09>,
        <http://vocab.ceda.ac.uk/collection/cci/org/org10>,
        <http://vocab.ceda.ac.uk/collection/cci/org/org100>,
        <http://vocab.ceda.ac.uk/collection/cci/org/org101>,
        <http://vocab.ceda.ac.uk/collection/cci/org/org102>,
        <http://vocab.ceda.ac.uk/collection/cci/org/org103>,
        <http://vocab.ceda.ac.uk/collection/cci/org/org104>,
        <http://vocab.ceda.ac.uk/collection/cci/org/org105>,
        <http://vocab.ceda.ac.uk/collection/cci/org/org106>,
        <http://vocab.ceda.ac.uk/collection/cci/org/org107>,
        <http://vocab.ceda.ac.uk/collection/cci/org/org11>,
        <http://vocab.ceda.ac.uk/collection/cci/org/org12>,
        <http://vocab.ceda.ac.uk/collection/cci/org/org13>,
        <http://vocab.ceda.ac.uk/collection/cci/org/org14>,
        <http://vocab.ceda.ac.uk/collection/cci/org/org15>,
        <http://vocab.ceda.ac.uk/collection/cci/org/org16>,
        <http://vocab.ceda.ac.uk/collection/cci/org/org17>,
        <http://vocab.ceda.ac.uk/collection/cci/org/org18>,
        <http://vocab.ceda.ac.uk/collection/cci/org/org19>,
        <http://vocab.ceda.ac.uk/collection/cci/org/org20>,
        <http://vocab.ceda.ac.uk/collection/cci/org/org21>,
        <http://vocab.ceda.ac.uk/collection/cci/org/org22>,
        <http://vocab.ceda.ac.uk/collection/cci/org/org23>,
        <http://vocab.ceda.ac.uk/collection/cci/org/org24>,
        <http://vocab.ceda.ac.uk/collection/cci/org/org25>,
        <http://vocab.ceda.ac.uk/collection/cci/org/org26>,
        <http://vocab.ceda.ac.uk/collection/cci/org/org27>,
        <http://vocab.ceda.ac.uk/collection/cci/org/org28>,
        <http://vocab.ceda.ac.uk/collection/cci/org/org29>,
        <http://vocab.ceda.ac.uk/collection/cci/org/org30>,
        <http://vocab.ceda.ac.uk/collection/cci/org/org31>,
        <http://vocab.ceda.ac.uk/collection/cci/org/org32>,
        <http://vocab.ceda.ac.uk/collection/cci/org/org33>,
        <http://vocab.ceda.ac.uk/collection/cci/org/org34>,
        <http://vocab.ceda.ac.uk/collection/cci/org/org35>,
        <http://vocab.ceda.ac.uk/collection/cci/org/org36>,
        <http://vocab.ceda.ac.uk/collection/cci/org/org37>,
        <http://vocab.ceda.ac.uk/collection/cci/org/org38>,
        <http://vocab.ceda.ac.uk/collection/cci/org/org39>,
        <http://vocab.ceda.ac.uk/collection/cci/org/org40>,
        <http://vocab.ceda.ac.uk/collection/cci/org/org41>,
        <http://vocab.ceda.ac.uk/collection/cci/org/org42>,
        <http://vocab.ceda.ac.uk/collection/cci/org/org43>,
        <http://vocab.ceda.ac.uk/collection/cci/org/org44>,
        <http://vocab.ceda.ac.uk/collection/cci/org/org45>,
        <http://vocab.ceda.ac.uk/collection/cci/org/org46>,
        <http://vocab.ceda.ac.uk/collection/cci/org/org47>,
        <http://vocab.ceda.ac.uk/collection/cci/org/org48>,
        <http://vocab.ceda.ac.uk/collection/cci/org/org49>,
        <http://vocab.ceda.ac.uk/collection/cci/org/org50>,
        <http://vocab.ceda.ac.uk/collection/cci/org/org51>,
        <http://vocab.ceda.ac.uk/collection/cci/org/org52>,
        <http://vocab.ceda.ac.uk/collection/cci/org/org53>,
        <http://vocab.ceda.ac.uk/collection/cci/org/org54>,
        <http://vocab.ceda.ac.uk/collection/cci/org/org55>,
        <http://vocab.ceda.ac.uk/collection/cci/org/org56>,
        <http://vocab.ceda.ac.uk/collection/cci/org/org57>,
        <http://vocab.ceda.ac.uk/collection/cci/org/org58>,
        <http://vocab.ceda.ac.uk/collection/cci/org/org59>,
        <http://vocab.ceda.ac.uk/collection/cci/org/org60>,
        <http://vocab.ceda.ac.uk/collection/cci/org/org61>,
        <http://vocab.ceda.ac.uk/collection/cci/org/org62>,
        <http://vocab.ceda.ac.uk/collection/cci/org/org63>,
        <http://vocab.ceda.ac.uk/collection/cci/org/org64>,
        <http://vocab.ceda.ac.uk/collection/cci/org/org65>,
        <http://vocab.ceda.ac.uk/collection/cci/org/org66>,
        <http://vocab.ceda.ac.uk/collection/cci/org/org67>,
        <http://vocab.ceda.ac.uk/collection/cci/org/org68>,
        <http://vocab.ceda.ac.uk/collection/cci/org/org69>,
        <http://vocab.ceda.ac.uk/collection/cci/org/org70>,
        <http://vocab.ceda.ac.uk/collection/cci/org/org71>,
        <http://vocab.ceda.ac.uk/collection/cci/org/org72>,
        <http://vocab.ceda.ac.uk/collection/cci/org/org73>,
        <http://vocab.ceda.ac.uk/collection/cci/org/org74>,
        <http://vocab.ceda.ac.uk/collection/cci/org/org75>,
        <http://vocab.ceda.ac.uk/collection/cci/org/org76>,
        <http://vocab.ceda.ac.uk/collection/cci/org/org77>,
        <http://vocab.ceda.ac.uk/collection/cci/org/org78>,
        <http://vocab.ceda.ac.uk/collection/cci/org/org79>,
        <http://vocab.ceda.ac.uk/collection/cci/org/org80>,
        <http://vocab.ceda.ac.uk/collection/cci/org/org81>,
        <http://vocab.ceda.ac.uk/collection/cci/org/org82>,
        <http://vocab.ceda.ac.uk/collection/cci/org/org83>,
        <http://vocab.ceda.ac.uk/collection/cci/org/org84>,
        <http://vocab.ceda.ac.uk/collection/cci/org/org85>,
        <http://vocab.ceda.ac.uk/collection/cci/org/org86>,
        <http://vocab.ceda.ac.uk/collection/cci/org/org87>,
        <http://vocab.ceda.ac.uk/collection/cci/org/org88>,
        <http://vocab.ceda.ac.uk/collection/cci/org/org89>,
        <http://vocab.ceda.ac.uk/collection/cci/org/org90>,
        <http://vocab.ceda.ac.uk/collection/cci/org/org91>,
        <http://vocab.ceda.ac.uk/collection/cci/org/org92>,
        <http://vocab.ceda.ac.uk/collection/cci/org/org93>,
        <http://vocab.ceda.ac.uk/collection/cci/org/org94>,
        <http://vocab.ceda.ac.uk/collection/cci/org/org95>,
        <http://vocab.ceda.ac.uk/collection/cci/org/org96>,
        <http://vocab.ceda.ac.uk/collection/cci/org/org97>,
        <http://vocab.ceda.ac.uk/collection/cci/org/org98>,
        <http://vocab.ceda.ac.uk/collection/cci/org/org99> ;
    skos:prefLabel "Institute"@en .

cci-scheme:platform a skos:ConceptScheme ;
    dc:creator "Science and Technology Facilities Council" ;
    dc:date "2025-01-23" ;
    dc:description "<p>The CCI concept schemes are used to define concepts within an element of a Directory Reference Scheme. There are currently eight concept schemes defined: <a href=../dataType>data type</a>, <a href=..//ecv>ecv</a>, <a href=../scheme/cci/freq>frequency</a>, <a href=../org>institutes</a>, <a href=../platform>platforms</a>, <a href=../procLev>processing levels</a>, <a href=../product>products</a>, and <a href=../sensor>sensors</a>. The use of a concept scheme allows easy navigation up and down the tree.</p><h5>SKOS Navigation Down the Concept Scheme</h5><img src=conceptSchemeDown.svg /><h5>SKOS Navigation Up the Concept Scheme</h5><img src=conceptSchemeUp.svg /><p>As well as being concepts the the concepts are also named individuals of the <a href=../../../ontology/cci>CCI Ontology</a> classes.<h5>OWL Classes</h5><img src=classes.svg /><p></p>" ;
    dc:publisher "STFC"@en ;
    dc:rights "This work is licensed under a BSD license."@en ;
    dc:title "Platform" ;
    rdfs:comment "This concept scheme represents the platforms used by the CCI project" ;
    owl:versionInfo "0.0.1" ;
    skos:definition "The platforms that have been used in the collection of data for the ESA Climate Change Initiative (CCI)."@en ;
    skos:hasTopConcept <http://vocab.ceda.ac.uk/collection/cci/platform/plat_FY-3A>,
        <http://vocab.ceda.ac.uk/collection/cci/platform/plat_FY-3B>,
        <http://vocab.ceda.ac.uk/collection/cci/platform/plat_FY-3C>,
        <http://vocab.ceda.ac.uk/collection/cci/platform/plat_FY-3D>,
        <http://vocab.ceda.ac.uk/collection/cci/platform/plat_FY-3E>,
        <http://vocab.ceda.ac.uk/collection/cci/platform/plat_FY-3F>,
        <http://vocab.ceda.ac.uk/collection/cci/platform/plat_FY-3G>,
        <http://vocab.ceda.ac.uk/collection/cci/platform/plat_alos>,
        <http://vocab.ceda.ac.uk/collection/cci/platform/plat_alos-2>,
        <http://vocab.ceda.ac.uk/collection/cci/platform/plat_alos-3>,
        <http://vocab.ceda.ac.uk/collection/cci/platform/plat_aqua>,
        <http://vocab.ceda.ac.uk/collection/cci/platform/plat_aura>,
        <http://vocab.ceda.ac.uk/collection/cci/platform/plat_coriolis>,
        <http://vocab.ceda.ac.uk/collection/cci/platform/plat_cryosat2>,
        <http://vocab.ceda.ac.uk/collection/cci/platform/plat_csk1>,
        <http://vocab.ceda.ac.uk/collection/cci/platform/plat_csk2>,
        <http://vocab.ceda.ac.uk/collection/cci/platform/plat_csk3>,
        <http://vocab.ceda.ac.uk/collection/cci/platform/plat_csk4>,
        <http://vocab.ceda.ac.uk/collection/cci/platform/plat_dmsp_F01>,
        <http://vocab.ceda.ac.uk/collection/cci/platform/plat_dmsp_F02>,
        <http://vocab.ceda.ac.uk/collection/cci/platform/plat_dmsp_F03>,
        <http://vocab.ceda.ac.uk/collection/cci/platform/plat_dmsp_F04>,
        <http://vocab.ceda.ac.uk/collection/cci/platform/plat_dmsp_F05>,
        <http://vocab.ceda.ac.uk/collection/cci/platform/plat_dmsp_F06>,
        <http://vocab.ceda.ac.uk/collection/cci/platform/plat_dmsp_F07>,
        <http://vocab.ceda.ac.uk/collection/cci/platform/plat_dmsp_F08>,
        <http://vocab.ceda.ac.uk/collection/cci/platform/plat_dmsp_F09>,
        <http://vocab.ceda.ac.uk/collection/cci/platform/plat_dmsp_F10>,
        <http://vocab.ceda.ac.uk/collection/cci/platform/plat_dmsp_F11>,
        <http://vocab.ceda.ac.uk/collection/cci/platform/plat_dmsp_F12>,
        <http://vocab.ceda.ac.uk/collection/cci/platform/plat_dmsp_F13>,
        <http://vocab.ceda.ac.uk/collection/cci/platform/plat_dmsp_F14>,
        <http://vocab.ceda.ac.uk/collection/cci/platform/plat_dmsp_F15>,
        <http://vocab.ceda.ac.uk/collection/cci/platform/plat_dmsp_F16>,
        <http://vocab.ceda.ac.uk/collection/cci/platform/plat_dmsp_F17>,
        <http://vocab.ceda.ac.uk/collection/cci/platform/plat_dmsp_F18>,
        <http://vocab.ceda.ac.uk/collection/cci/platform/plat_dmsp_F19>,
        <http://vocab.ceda.ac.uk/collection/cci/platform/plat_dmsp_S20>,
        <http://vocab.ceda.ac.uk/collection/cci/platform/plat_envisat>,
        <http://vocab.ceda.ac.uk/collection/cci/platform/plat_ers1>,
        <http://vocab.ceda.ac.uk/collection/cci/platform/plat_ers2>,
        <http://vocab.ceda.ac.uk/collection/cci/platform/plat_gcomW1>,
        <http://vocab.ceda.ac.uk/collection/cci/platform/plat_gcomW2>,
        <http://vocab.ceda.ac.uk/collection/cci/platform/plat_gcomW3>,
        <http://vocab.ceda.ac.uk/collection/cci/platform/plat_geosat>,
        <http://vocab.ceda.ac.uk/collection/cci/platform/plat_gfo>,
        <http://vocab.ceda.ac.uk/collection/cci/platform/plat_goes_01>,
        <http://vocab.ceda.ac.uk/collection/cci/platform/plat_goes_02>,
        <http://vocab.ceda.ac.uk/collection/cci/platform/plat_goes_03>,
        <http://vocab.ceda.ac.uk/collection/cci/platform/plat_goes_04>,
        <http://vocab.ceda.ac.uk/collection/cci/platform/plat_goes_05>,
        <http://vocab.ceda.ac.uk/collection/cci/platform/plat_goes_06>,
        <http://vocab.ceda.ac.uk/collection/cci/platform/plat_goes_07>,
        <http://vocab.ceda.ac.uk/collection/cci/platform/plat_goes_08>,
        <http://vocab.ceda.ac.uk/collection/cci/platform/plat_goes_09>,
        <http://vocab.ceda.ac.uk/collection/cci/platform/plat_goes_09_bk>,
        <http://vocab.ceda.ac.uk/collection/cci/platform/plat_goes_10>,
        <http://vocab.ceda.ac.uk/collection/cci/platform/plat_goes_10_SA>,
        <http://vocab.ceda.ac.uk/collection/cci/platform/plat_goes_11>,
        <http://vocab.ceda.ac.uk/collection/cci/platform/plat_goes_12>,
        <http://vocab.ceda.ac.uk/collection/cci/platform/plat_goes_12_SA>,
        <http://vocab.ceda.ac.uk/collection/cci/platform/plat_goes_13>,
        <http://vocab.ceda.ac.uk/collection/cci/platform/plat_goes_14>,
        <http://vocab.ceda.ac.uk/collection/cci/platform/plat_goes_15>,
        <http://vocab.ceda.ac.uk/collection/cci/platform/plat_goes_16>,
        <http://vocab.ceda.ac.uk/collection/cci/platform/plat_goes_17>,
        <http://vocab.ceda.ac.uk/collection/cci/platform/plat_goes_T>,
        <http://vocab.ceda.ac.uk/collection/cci/platform/plat_goes_U>,
        <http://vocab.ceda.ac.uk/collection/cci/platform/plat_gosat>,
        <http://vocab.ceda.ac.uk/collection/cci/platform/plat_gosat-2>,
        <http://vocab.ceda.ac.uk/collection/cci/platform/plat_gpm>,
        <http://vocab.ceda.ac.uk/collection/cci/platform/plat_grace>,
        <http://vocab.ceda.ac.uk/collection/cci/platform/plat_himawari-6>,
        <http://vocab.ceda.ac.uk/collection/cci/platform/plat_himawari-7>,
        <http://vocab.ceda.ac.uk/collection/cci/platform/plat_hrws_sar>,
        <http://vocab.ceda.ac.uk/collection/cci/platform/plat_icesat>,
        <http://vocab.ceda.ac.uk/collection/cci/platform/plat_icesat-2>,
        <http://vocab.ceda.ac.uk/collection/cci/platform/plat_jason1>,
        <http://vocab.ceda.ac.uk/collection/cci/platform/plat_jason2>,
        <http://vocab.ceda.ac.uk/collection/cci/platform/plat_jason3>,
        <http://vocab.ceda.ac.uk/collection/cci/platform/plat_landsat_1>,
        <http://vocab.ceda.ac.uk/collection/cci/platform/plat_landsat_2>,
        <http://vocab.ceda.ac.uk/collection/cci/platform/plat_landsat_3>,
        <http://vocab.ceda.ac.uk/collection/cci/platform/plat_landsat_4>,
        <http://vocab.ceda.ac.uk/collection/cci/platform/plat_landsat_5>,
        <http://vocab.ceda.ac.uk/collection/cci/platform/plat_landsat_6>,
        <http://vocab.ceda.ac.uk/collection/cci/platform/plat_landsat_7>,
        <http://vocab.ceda.ac.uk/collection/cci/platform/plat_landsat_8>,
        <http://vocab.ceda.ac.uk/collection/cci/platform/plat_metOpA>,
        <http://vocab.ceda.ac.uk/collection/cci/platform/plat_metOpB>,
        <http://vocab.ceda.ac.uk/collection/cci/platform/plat_metOpC>,
        <http://vocab.ceda.ac.uk/collection/cci/platform/plat_meteosat_1>,
        <http://vocab.ceda.ac.uk/collection/cci/platform/plat_meteosat_10>,
        <http://vocab.ceda.ac.uk/collection/cci/platform/plat_meteosat_11>,
        <http://vocab.ceda.ac.uk/collection/cci/platform/plat_meteosat_2>,
        <http://vocab.ceda.ac.uk/collection/cci/platform/plat_meteosat_3>,
        <http://vocab.ceda.ac.uk/collection/cci/platform/plat_meteosat_3_adc>,
        <http://vocab.ceda.ac.uk/collection/cci/platform/plat_meteosat_3_xadc>,
        <http://vocab.ceda.ac.uk/collection/cci/platform/plat_meteosat_4>,
        <http://vocab.ceda.ac.uk/collection/cci/platform/plat_meteosat_5>,
        <http://vocab.ceda.ac.uk/collection/cci/platform/plat_meteosat_5_iodc>,
        <http://vocab.ceda.ac.uk/collection/cci/platform/plat_meteosat_6>,
        <http://vocab.ceda.ac.uk/collection/cci/platform/plat_meteosat_6_iodc>,
        <http://vocab.ceda.ac.uk/collection/cci/platform/plat_meteosat_7>,
        <http://vocab.ceda.ac.uk/collection/cci/platform/plat_meteosat_7_iodc>,
        <http://vocab.ceda.ac.uk/collection/cci/platform/plat_meteosat_8>,
        <http://vocab.ceda.ac.uk/collection/cci/platform/plat_meteosat_9>,
        <http://vocab.ceda.ac.uk/collection/cci/platform/plat_nimbus1>,
        <http://vocab.ceda.ac.uk/collection/cci/platform/plat_nimbus2>,
        <http://vocab.ceda.ac.uk/collection/cci/platform/plat_nimbus3>,
        <http://vocab.ceda.ac.uk/collection/cci/platform/plat_nimbus4>,
        <http://vocab.ceda.ac.uk/collection/cci/platform/plat_nimbus5>,
        <http://vocab.ceda.ac.uk/collection/cci/platform/plat_nimbus6>,
        <http://vocab.ceda.ac.uk/collection/cci/platform/plat_nimbus7>,
        <http://vocab.ceda.ac.uk/collection/cci/platform/plat_noaa_1>,
        <http://vocab.ceda.ac.uk/collection/cci/platform/plat_noaa_10>,
        <http://vocab.ceda.ac.uk/collection/cci/platform/plat_noaa_11>,
        <http://vocab.ceda.ac.uk/collection/cci/platform/plat_noaa_12>,
        <http://vocab.ceda.ac.uk/collection/cci/platform/plat_noaa_13>,
        <http://vocab.ceda.ac.uk/collection/cci/platform/plat_noaa_14>,
        <http://vocab.ceda.ac.uk/collection/cci/platform/plat_noaa_15>,
        <http://vocab.ceda.ac.uk/collection/cci/platform/plat_noaa_16>,
        <http://vocab.ceda.ac.uk/collection/cci/platform/plat_noaa_17>,
        <http://vocab.ceda.ac.uk/collection/cci/platform/plat_noaa_18>,
        <http://vocab.ceda.ac.uk/collection/cci/platform/plat_noaa_19>,
        <http://vocab.ceda.ac.uk/collection/cci/platform/plat_noaa_2>,
        <http://vocab.ceda.ac.uk/collection/cci/platform/plat_noaa_3>,
        <http://vocab.ceda.ac.uk/collection/cci/platform/plat_noaa_4>,
        <http://vocab.ceda.ac.uk/collection/cci/platform/plat_noaa_5>,
        <http://vocab.ceda.ac.uk/collection/cci/platform/plat_noaa_6>,
        <http://vocab.ceda.ac.uk/collection/cci/platform/plat_noaa_7>,
        <http://vocab.ceda.ac.uk/collection/cci/platform/plat_noaa_8>,
        <http://vocab.ceda.ac.uk/collection/cci/platform/plat_noaa_9>,
        <http://vocab.ceda.ac.uk/collection/cci/platform/plat_oco2>,
        <http://vocab.ceda.ac.uk/collection/cci/platform/plat_odin>,
        <http://vocab.ceda.ac.uk/collection/cci/platform/plat_orbview2>,
        <http://vocab.ceda.ac.uk/collection/cci/platform/plat_parasol>,
        <http://vocab.ceda.ac.uk/collection/cci/platform/plat_probaV>,
        <http://vocab.ceda.ac.uk/collection/cci/platform/plat_radarsat2>,
        <http://vocab.ceda.ac.uk/collection/cci/platform/plat_sac_d>,
        <http://vocab.ceda.ac.uk/collection/cci/platform/plat_saral>,
        <http://vocab.ceda.ac.uk/collection/cci/platform/plat_scisat>,
        <http://vocab.ceda.ac.uk/collection/cci/platform/plat_sentinel1a>,
        <http://vocab.ceda.ac.uk/collection/cci/platform/plat_sentinel1b>,
        <http://vocab.ceda.ac.uk/collection/cci/platform/plat_sentinel2a>,
        <http://vocab.ceda.ac.uk/collection/cci/platform/plat_sentinel2b>,
        <http://vocab.ceda.ac.uk/collection/cci/platform/plat_sentinel3a>,
        <http://vocab.ceda.ac.uk/collection/cci/platform/plat_sentinel3b>,
        <http://vocab.ceda.ac.uk/collection/cci/platform/plat_sentinel5p>,
        <http://vocab.ceda.ac.uk/collection/cci/platform/plat_sentinel6a>,
        <http://vocab.ceda.ac.uk/collection/cci/platform/plat_sentinel6b>,
        <http://vocab.ceda.ac.uk/collection/cci/platform/plat_smap>,
        <http://vocab.ceda.ac.uk/collection/cci/platform/plat_smos>,
        <http://vocab.ceda.ac.uk/collection/cci/platform/plat_snpp>,
        <http://vocab.ceda.ac.uk/collection/cci/platform/plat_spot1>,
        <http://vocab.ceda.ac.uk/collection/cci/platform/plat_spot2>,
        <http://vocab.ceda.ac.uk/collection/cci/platform/plat_spot3>,
        <http://vocab.ceda.ac.uk/collection/cci/platform/plat_spot4>,
        <http://vocab.ceda.ac.uk/collection/cci/platform/plat_spot5>,
        <http://vocab.ceda.ac.uk/collection/cci/platform/plat_spot6>,
        <http://vocab.ceda.ac.uk/collection/cci/platform/plat_spot7>,
        <http://vocab.ceda.ac.uk/collection/cci/platform/plat_tandem_X>,
        <http://vocab.ceda.ac.uk/collection/cci/platform/plat_terra>,
        <http://vocab.ceda.ac.uk/collection/cci/platform/plat_terraSar_X>,
        <http://vocab.ceda.ac.uk/collection/cci/platform/plat_tiros_n>,
        <http://vocab.ceda.ac.uk/collection/cci/platform/plat_topexPoseidon>,
        <http://vocab.ceda.ac.uk/collection/cci/platform/plat_trmm>,
        <http://vocab.ceda.ac.uk/collection/cci/platform/plat_tsx_ng>,
        <http://vocab.ceda.ac.uk/collection/cci/platform/plat_unspecified> ;
    skos:prefLabel "Platform"@en .

cci-scheme:product a skos:ConceptScheme ;
    dc:creator "Science and Technology Facilities Council" ;
    dc:date "2025-01-23" ;
    dc:description "<p>The CCI concept schemes are used to define concepts within an element of a Directory Reference Scheme. There are currently eight concept schemes defined: <a href=../dataType>data type</a>, <a href=..//ecv>ecv</a>, <a href=../scheme/cci/freq>frequency</a>, <a href=../org>institutes</a>, <a href=../platform>platforms</a>, <a href=../procLev>processing levels</a>, <a href=../product>products</a>, and <a href=../sensor>sensors</a>. The use of a concept scheme allows easy navigation up and down the tree.</p><h5>SKOS Navigation Down the Concept Scheme</h5><img src=conceptSchemeDown.svg /><h5>SKOS Navigation Up the Concept Scheme</h5><img src=conceptSchemeUp.svg /><p>As well as being concepts the the concepts are also named individuals of the <a href=../../../ontology/cci>CCI Ontology</a> classes.<h5>OWL Classes</h5><img src=classes.svg /><p></p>" ;
    dc:publisher "STFC"@en ;
    dc:rights "This work is licensed under a BSD license."@en ;
    dc:title "Product" ;
    rdfs:comment "This concept scheme represents the products used by the CCI project" ;
    owl:versionInfo "0.0.1" ;
    skos:definition "The different products that are produced within the ESA Climate Change Initiative (CCI)."@en ;
    skos:hasTopConcept <http://vocab.ceda.ac.uk/collection/cci/product/prod_AvhrMa>,
        <http://vocab.ceda.ac.uk/collection/cci/product/prod_AvhrrMetopA>,
        <http://vocab.ceda.ac.uk/collection/cci/product/prod_AvhrrMetopB>,
        <http://vocab.ceda.ac.uk/collection/cci/product/prod_AvhrrMetopC>,
        <http://vocab.ceda.ac.uk/collection/cci/product/prod_AvhrrNoaa10>,
        <http://vocab.ceda.ac.uk/collection/cci/product/prod_AvhrrNoaa11>,
        <http://vocab.ceda.ac.uk/collection/cci/product/prod_AvhrrNoaa12>,
        <http://vocab.ceda.ac.uk/collection/cci/product/prod_AvhrrNoaa14>,
        <http://vocab.ceda.ac.uk/collection/cci/product/prod_AvhrrNoaa16>,
        <http://vocab.ceda.ac.uk/collection/cci/product/prod_AvhrrNoaa17>,
        <http://vocab.ceda.ac.uk/collection/cci/product/prod_AvhrrNoaa18>,
        <http://vocab.ceda.ac.uk/collection/cci/product/prod_AvhrrNoaa19>,
        <http://vocab.ceda.ac.uk/collection/cci/product/prod_AvhrrNoaa6>,
        <http://vocab.ceda.ac.uk/collection/cci/product/prod_AvhrrNoaa7>,
        <http://vocab.ceda.ac.uk/collection/cci/product/prod_AvhrrNoaa8>,
        <http://vocab.ceda.ac.uk/collection/cci/product/prod_AvhrrNoaa9>,
        <http://vocab.ceda.ac.uk/collection/cci/product/prod_AvhrrTirosN>,
        <http://vocab.ceda.ac.uk/collection/cci/product/prod_CL02A01>,
        <http://vocab.ceda.ac.uk/collection/cci/product/prod_CL02A01Mos>,
        <http://vocab.ceda.ac.uk/collection/cci/product/prod_CL02A02>,
        <http://vocab.ceda.ac.uk/collection/cci/product/prod_CL02A02Mos>,
        <http://vocab.ceda.ac.uk/collection/cci/product/prod_CL02A03>,
        <http://vocab.ceda.ac.uk/collection/cci/product/prod_CL02A03Mos>,
        <http://vocab.ceda.ac.uk/collection/cci/product/prod_CryoSat2>,
        <http://vocab.ceda.ac.uk/collection/cci/product/prod_Diff>,
        <http://vocab.ceda.ac.uk/collection/cci/product/prod_GlobMerg7day>,
        <http://vocab.ceda.ac.uk/collection/cci/product/prod_GlobMergCent>,
        <http://vocab.ceda.ac.uk/collection/cci/product/prod_HRLC10A01>,
        <http://vocab.ceda.ac.uk/collection/cci/product/prod_HRLC10A02>,
        <http://vocab.ceda.ac.uk/collection/cci/product/prod_HRLC10A03>,
        <http://vocab.ceda.ac.uk/collection/cci/product/prod_HRLC30A01>,
        <http://vocab.ceda.ac.uk/collection/cci/product/prod_HRLC30A02>,
        <http://vocab.ceda.ac.uk/collection/cci/product/prod_HRLC30A03>,
        <http://vocab.ceda.ac.uk/collection/cci/product/prod_HRLCC30A01>,
        <http://vocab.ceda.ac.uk/collection/cci/product/prod_HRLCC30A02>,
        <http://vocab.ceda.ac.uk/collection/cci/product/prod_HRLCC30A03>,
        <http://vocab.ceda.ac.uk/collection/cci/product/prod_IQIXA01>,
        <http://vocab.ceda.ac.uk/collection/cci/product/prod_IQIXA01Mos>,
        <http://vocab.ceda.ac.uk/collection/cci/product/prod_IQIXA02>,
        <http://vocab.ceda.ac.uk/collection/cci/product/prod_IQIXA02Mos>,
        <http://vocab.ceda.ac.uk/collection/cci/product/prod_IQIXA03>,
        <http://vocab.ceda.ac.uk/collection/cci/product/prod_IQIXA03Mos>,
        <http://vocab.ceda.ac.uk/collection/cci/product/prod_Jason1>,
        <http://vocab.ceda.ac.uk/collection/cci/product/prod_Jason2>,
        <http://vocab.ceda.ac.uk/collection/cci/product/prod_Jason3>,
        <http://vocab.ceda.ac.uk/collection/cci/product/prod_PS01A01>,
        <http://vocab.ceda.ac.uk/collection/cci/product/prod_PS01A01Mos>,
        <http://vocab.ceda.ac.uk/collection/cci/product/prod_PS01A02>,
        <http://vocab.ceda.ac.uk/collection/cci/product/prod_PS01A02Mos>,
        <http://vocab.ceda.ac.uk/collection/cci/product/prod_PS01A03>,
        <http://vocab.ceda.ac.uk/collection/cci/product/prod_PS01A03Mos>,
        <http://vocab.ceda.ac.uk/collection/cci/product/prod_PS02A01>,
        <http://vocab.ceda.ac.uk/collection/cci/product/prod_PS02A01Mos>,
        <http://vocab.ceda.ac.uk/collection/cci/product/prod_PS02A02>,
        <http://vocab.ceda.ac.uk/collection/cci/product/prod_PS02A02Mos>,
        <http://vocab.ceda.ac.uk/collection/cci/product/prod_PS02A03>,
        <http://vocab.ceda.ac.uk/collection/cci/product/prod_PS02A03Mos>,
        <http://vocab.ceda.ac.uk/collection/cci/product/prod_PolMerg7dayNh>,
        <http://vocab.ceda.ac.uk/collection/cci/product/prod_PolMerg7daySh>,
        <http://vocab.ceda.ac.uk/collection/cci/product/prod_PolMergCentNH>,
        <http://vocab.ceda.ac.uk/collection/cci/product/prod_PolMergCentSH>,
        <http://vocab.ceda.ac.uk/collection/cci/product/prod_aFS>,
        <http://vocab.ceda.ac.uk/collection/cci/product/prod_aatsr>,
        <http://vocab.ceda.ac.uk/collection/cci/product/prod_aatsrEn>,
        <http://vocab.ceda.ac.uk/collection/cci/product/prod_aatsrEns>,
        <http://vocab.ceda.ac.uk/collection/cci/product/prod_aatsrEnsannual>,
        <http://vocab.ceda.ac.uk/collection/cci/product/prod_aatsrEnsdaily>,
        <http://vocab.ceda.ac.uk/collection/cci/product/prod_aatsrEnsmonthly>,
        <http://vocab.ceda.ac.uk/collection/cci/product/prod_active>,
        <http://vocab.ceda.ac.uk/collection/cci/product/prod_adv>,
        <http://vocab.ceda.ac.uk/collection/cci/product/prod_aergom>,
        <http://vocab.ceda.ac.uk/collection/cci/product/prod_alamo>,
        <http://vocab.ceda.ac.uk/collection/cci/product/prod_amsr>,
        <http://vocab.ceda.ac.uk/collection/cci/product/prod_amsr25E>,
        <http://vocab.ceda.ac.uk/collection/cci/product/prod_amsr50E>,
        <http://vocab.ceda.ac.uk/collection/cci/product/prod_atsr1>,
        <http://vocab.ceda.ac.uk/collection/cci/product/prod_atsr2>,
        <http://vocab.ceda.ac.uk/collection/cci/product/prod_atsr2Aatsr>,
        <http://vocab.ceda.ac.uk/collection/cci/product/prod_atsr2Er2>,
        <http://vocab.ceda.ac.uk/collection/cci/product/prod_atsr2ens>,
        <http://vocab.ceda.ac.uk/collection/cci/product/prod_atsr2ensannual>,
        <http://vocab.ceda.ac.uk/collection/cci/product/prod_atsr2ensdaily>,
        <http://vocab.ceda.ac.uk/collection/cci/product/prod_atsr2ensmonthly>,
        <http://vocab.ceda.ac.uk/collection/cci/product/prod_atsr3>,
        <http://vocab.ceda.ac.uk/collection/cci/product/prod_atsr_2>,
        <http://vocab.ceda.ac.uk/collection/cci/product/prod_avhrr07G>,
        <http://vocab.ceda.ac.uk/collection/cci/product/prod_avhrr09G>,
        <http://vocab.ceda.ac.uk/collection/cci/product/prod_avhrr11G>,
        <http://vocab.ceda.ac.uk/collection/cci/product/prod_avhrr12G>,
        <http://vocab.ceda.ac.uk/collection/cci/product/prod_avhrr14G>,
        <http://vocab.ceda.ac.uk/collection/cci/product/prod_avhrr15G>,
        <http://vocab.ceda.ac.uk/collection/cci/product/prod_avhrr16G>,
        <http://vocab.ceda.ac.uk/collection/cci/product/prod_avhrr17G>,
        <http://vocab.ceda.ac.uk/collection/cci/product/prod_avhrr18G>,
        <http://vocab.ceda.ac.uk/collection/cci/product/prod_avhrr19G>,
        <http://vocab.ceda.ac.uk/collection/cci/product/prod_avhrrAm>,
        <http://vocab.ceda.ac.uk/collection/cci/product/prod_avhrrLtdr>,
        <http://vocab.ceda.ac.uk/collection/cci/product/prod_avhrrMg>,
        <http://vocab.ceda.ac.uk/collection/cci/product/prod_avhrrNoaa>,
        <http://vocab.ceda.ac.uk/collection/cci/product/prod_avhrrPm>,
        <http://vocab.ceda.ac.uk/collection/cci/product/prod_avhrrmtag>,
        <http://vocab.ceda.ac.uk/collection/cci/product/prod_besd>,
        <http://vocab.ceda.ac.uk/collection/cci/product/prod_change>,
        <http://vocab.ceda.ac.uk/collection/cci/product/prod_cl01A01>,
        <http://vocab.ceda.ac.uk/collection/cci/product/prod_cl01A01Mos>,
        <http://vocab.ceda.ac.uk/collection/cci/product/prod_cl01A02>,
        <http://vocab.ceda.ac.uk/collection/cci/product/prod_cl01A02Mos>,
        <http://vocab.ceda.ac.uk/collection/cci/product/prod_cl01A03>,
        <http://vocab.ceda.ac.uk/collection/cci/product/prod_cl01A03Mos>,
        <http://vocab.ceda.ac.uk/collection/cci/product/prod_clim>,
        <http://vocab.ceda.ac.uk/collection/cci/product/prod_comb>,
        <http://vocab.ceda.ac.uk/collection/cci/product/prod_combAdj>,
        <http://vocab.ceda.ac.uk/collection/cci/product/prod_emma>,
        <http://vocab.ceda.ac.uk/collection/cci/product/prod_envisat>,
        <http://vocab.ceda.ac.uk/collection/cci/product/prod_eraModBias>,
        <http://vocab.ceda.ac.uk/collection/cci/product/prod_ers1>,
        <http://vocab.ceda.ac.uk/collection/cci/product/prod_ers2>,
        <http://vocab.ceda.ac.uk/collection/cci/product/prod_focal>,
        <http://vocab.ceda.ac.uk/collection/cci/product/prod_gfo>,
        <http://vocab.ceda.ac.uk/collection/cci/product/prod_gmp>,
        <http://vocab.ceda.ac.uk/collection/cci/product/prod_gmpe>,
        <http://vocab.ceda.ac.uk/collection/cci/product/prod_gomEn>,
        <http://vocab.ceda.ac.uk/collection/cci/product/prod_gosat>,
        <http://vocab.ceda.ac.uk/collection/cci/product/prod_iasDLRImars>,
        <http://vocab.ceda.ac.uk/collection/cci/product/prod_iasiLMDaero>,
        <http://vocab.ceda.ac.uk/collection/cci/product/prod_iasiMAPIR>,
        <http://vocab.ceda.ac.uk/collection/cci/product/prod_iasiULB>,
        <http://vocab.ceda.ac.uk/collection/cci/product/prod_imap>,
        <http://vocab.ceda.ac.uk/collection/cci/product/prod_ircdr>,
        <http://vocab.ceda.ac.uk/collection/cci/product/prod_irmgp>,
        <http://vocab.ceda.ac.uk/collection/cci/product/prod_map>,
        <http://vocab.ceda.ac.uk/collection/cci/product/prod_meAaEn>,
        <http://vocab.ceda.ac.uk/collection/cci/product/prod_medSea>,
        <http://vocab.ceda.ac.uk/collection/cci/product/prod_merg7dayDaily>,
        <http://vocab.ceda.ac.uk/collection/cci/product/prod_mergMon15day25km>,
        <http://vocab.ceda.ac.uk/collection/cci/product/prod_merged>,
        <http://vocab.ceda.ac.uk/collection/cci/product/prod_merris>,
        <http://vocab.ceda.ac.uk/collection/cci/product/prod_merris_envisat>,
        <http://vocab.ceda.ac.uk/collection/cci/product/prod_miEn>,
        <http://vocab.ceda.ac.uk/collection/cci/product/prod_modA>,
        <http://vocab.ceda.ac.uk/collection/cci/product/prod_modAqu>,
        <http://vocab.ceda.ac.uk/collection/cci/product/prod_modMg>,
        <http://vocab.ceda.ac.uk/collection/cci/product/prod_modT>,
        <http://vocab.ceda.ac.uk/collection/cci/product/prod_modTe>,
        <http://vocab.ceda.ac.uk/collection/cci/product/prod_modis>,
        <http://vocab.ceda.ac.uk/collection/cci/product/prod_modlstCryo>,
        <http://vocab.ceda.ac.uk/collection/cci/product/prod_msUvai>,
        <http://vocab.ceda.ac.uk/collection/cci/product/prod_msaai>,
        <http://vocab.ceda.ac.uk/collection/cci/product/prod_msi>,
        <http://vocab.ceda.ac.uk/collection/cci/product/prod_multi1d>,
        <http://vocab.ceda.ac.uk/collection/cci/product/prod_multi1m>,
        <http://vocab.ceda.ac.uk/collection/cci/product/prod_mzm>,
        <http://vocab.ceda.ac.uk/collection/cci/product/prod_nInd>,
        <http://vocab.ceda.ac.uk/collection/cci/product/prod_neAtl>,
        <http://vocab.ceda.ac.uk/collection/cci/product/prod_nh>,
        <http://vocab.ceda.ac.uk/collection/cci/product/prod_nh25kmease2>,
        <http://vocab.ceda.ac.uk/collection/cci/product/prod_nimEsmrNH>,
        <http://vocab.ceda.ac.uk/collection/cci/product/prod_nimEsmrSH>,
        <http://vocab.ceda.ac.uk/collection/cci/product/prod_ocfp>,
        <http://vocab.ceda.ac.uk/collection/cci/product/prod_ocpr>,
        <http://vocab.ceda.ac.uk/collection/cci/product/prod_opera>,
        <http://vocab.ceda.ac.uk/collection/cci/product/prod_orac>,
        <http://vocab.ceda.ac.uk/collection/cci/product/prod_osOd>,
        <http://vocab.ceda.ac.uk/collection/cci/product/prod_ostia>,
        <http://vocab.ceda.ac.uk/collection/cci/product/prod_parGrasp>,
        <http://vocab.ceda.ac.uk/collection/cci/product/prod_passive>,
        <http://vocab.ceda.ac.uk/collection/cci/product/prod_reSSMINH>,
        <http://vocab.ceda.ac.uk/collection/cci/product/prod_reSSMISH>,
        <http://vocab.ceda.ac.uk/collection/cci/product/prod_sAust>,
        <http://vocab.ceda.ac.uk/collection/cci/product/prod_saral>,
        <http://vocab.ceda.ac.uk/collection/cci/product/prod_sciam>,
        <http://vocab.ceda.ac.uk/collection/cci/product/prod_sciamEn>,
        <http://vocab.ceda.ac.uk/collection/cci/product/prod_seAsia>,
        <http://vocab.ceda.ac.uk/collection/cci/product/prod_sh>,
        <http://vocab.ceda.ac.uk/collection/cci/product/prod_sh50kmease2>,
        <http://vocab.ceda.ac.uk/collection/cci/product/prod_slstrA>,
        <http://vocab.ceda.ac.uk/collection/cci/product/prod_slstrB>,
        <http://vocab.ceda.ac.uk/collection/cci/product/prod_smm>,
        <http://vocab.ceda.ac.uk/collection/cci/product/prod_smrOd>,
        <http://vocab.ceda.ac.uk/collection/cci/product/prod_srfp>,
        <http://vocab.ceda.ac.uk/collection/cci/product/prod_srpr>,
        <http://vocab.ceda.ac.uk/collection/cci/product/prod_ssmi>,
        <http://vocab.ceda.ac.uk/collection/cci/product/prod_ssmiS>,
        <http://vocab.ceda.ac.uk/collection/cci/product/prod_su>,
        <http://vocab.ceda.ac.uk/collection/cci/product/prod_syn>,
        <http://vocab.ceda.ac.uk/collection/cci/product/prod_tcwvLand005>,
        <http://vocab.ceda.ac.uk/collection/cci/product/prod_tcwvLand05>,
        <http://vocab.ceda.ac.uk/collection/cci/product/prod_topexPos>,
        <http://vocab.ceda.ac.uk/collection/cci/product/prod_unspecified>,
        <http://vocab.ceda.ac.uk/collection/cci/product/prod_var>,
        <http://vocab.ceda.ac.uk/collection/cci/product/prod_wAfrica>,
        <http://vocab.ceda.ac.uk/collection/cci/product/prod_wfmd> ;
    skos:prefLabel "Product"@en .

