@prefix cci: <https://vocab.ceda.ac.uk/ontology/cci#> .
@prefix cci-scheme: <https://vocab.ceda.ac.uk/scheme/cci/> .
@prefix dc: <http://purl.org/dc/elements/1.1/> .
@prefix owl: <http://www.w3.org/2002/07/owl#> .
@prefix rdfs: <http://www.w3.org/2000/01/rdf-schema#> .
@prefix skos: <http://www.w3.org/2004/02/skos/core#> .

<https://vocab.ceda.ac.uk/collection/cci/platformGrp/plat_dmsp> a skos:Concept,
        cci:platformGrp ;
    skos:definition "US Defense Meteorological Satellite Program"@en ;
    skos:inScheme cci-scheme:platformGrp ;
    skos:narrower <https://vocab.ceda.ac.uk/collection/cci/platformProg/plat_dmsp_5D1>,
        <https://vocab.ceda.ac.uk/collection/cci/platformProg/plat_dmsp_5D2>,
        <https://vocab.ceda.ac.uk/collection/cci/platformProg/plat_dmsp_5D3> ;
    skos:prefLabel "DMSP"@en ;
    skos:scopeNote "US Defense Meteorological Satellite Program"@en ;
    skos:topConceptOf cci-scheme:platformGrp .

<https://vocab.ceda.ac.uk/collection/cci/platformGrp/plat_goes> a skos:Concept,
        cci:platformGrp ;
    skos:definition "NASA NESDIS Geostationary Operational Environmental Satellite system"@en ;
    skos:inScheme cci-scheme:platformGrp ;
    skos:narrower <https://vocab.ceda.ac.uk/collection/cci/platformProg/plat_goes_1st>,
        <https://vocab.ceda.ac.uk/collection/cci/platformProg/plat_goes_2nd>,
        <https://vocab.ceda.ac.uk/collection/cci/platformProg/plat_goes_3rd> ;
    skos:prefLabel "GOES"@en ;
    skos:scopeNote "NASA NESDIS Geostationary Operational Environmental Satellite system"@en ;
    skos:topConceptOf cci-scheme:platformGrp .

<https://vocab.ceda.ac.uk/collection/cci/platformGrp/plat_noaa> a skos:Concept,
        cci:platformGrp ;
    skos:definition "NASA NOAA Environmental satellite programme"@en ;
    skos:inScheme cci-scheme:platformGrp ;
    skos:narrower <https://vocab.ceda.ac.uk/collection/cci/platformProg/plat_noaa_3rd>,
        <https://vocab.ceda.ac.uk/collection/cci/platformProg/plat_noaa_4th>,
        <https://vocab.ceda.ac.uk/collection/cci/platformProg/plat_noaa_5th> ;
    skos:prefLabel "NOAA"@en ;
    skos:scopeNote "NASA NOAA Environmental satellite programme"@en ;
    skos:topConceptOf cci-scheme:platformGrp .

cci-scheme:platformGrp a skos:ConceptScheme ;
    dc:creator "Science and Technology Facilities Council" ;
    dc:date "2025-09-12" ;
    dc:description "<p>The CCI concept schemes are used to define concepts within an element of a Directory Reference Scheme. There are currently 11 concept schemes defined: <a href=../dataType>data type</a>, <a href=..//ecv>ecv</a>, <a href=../scheme/cci/freq>frequency</a>, <a href=../org>institutes</a>, <a href=../platform>platforms</a>, <a href=../platformGrp>platform groups</a>, <a href=../platformProg>platform programmes</a>, <a href=../procLev>processing levels</a>, <a href=../product>products</a>, <a href=../project>projects</a>,  and <a href=../sensor>sensors</a>. The use of a concept scheme allows easy navigation up and down the tree.</p><p>As well as being concepts, all of the concepts are also named individuals of the <a href=../../../ontology/cci>CCI Ontology</a> classes.</p>" ;
    dc:publisher "STFC"@en ;
    dc:rights "This work is licensed under a BSD license."@en ;
    dc:title "Platform Group" ;
    rdfs:comment "This concept scheme represents the platforms used by the CCI project" ;
    owl:versionInfo "0.0.1" ;
    skos:definition "The platform groups that have been used in the collection of data for the ESA Climate Change Initiative (CCI). A group consists of a number of <a href=#platformPrg>programmes</a>"@en ;
    skos:hasTopConcept <https://vocab.ceda.ac.uk/collection/cci/platformGrp/plat_dmsp>,
        <https://vocab.ceda.ac.uk/collection/cci/platformGrp/plat_goes>,
        <https://vocab.ceda.ac.uk/collection/cci/platformGrp/plat_noaa> ;
    skos:prefLabel "Platform Group"@en .

