@prefix cci: <http://vocab.ceda.ac.uk/ontology/cci#> .
@prefix cci-scheme: <http://vocab.ceda.ac.uk/scheme/cci/> .
@prefix dc: <http://purl.org/dc/elements/1.1/> .
@prefix owl: <http://www.w3.org/2002/07/owl#> .
@prefix rdfs: <http://www.w3.org/2000/01/rdf-schema#> .
@prefix skos: <http://www.w3.org/2004/02/skos/core#> .

<http://vocab.ceda.ac.uk/collection/cci/project/cciproject_aerosol> a cci:project,
        skos:Concept ;
    skos:altLabel "AEROSOL"@en ;
    skos:definition "The European Space Agency (ESA) Climate Change Initiative (CCI) Aerosol project"@en ;
    skos:inScheme cci-scheme:project ;
    skos:prefLabel "aerosol"@en ;
    skos:scopeNote "The European Space Agency (ESA) Climate Change Initiative (CCI) Aerosol project"@en ;
    skos:topConceptOf cci-scheme:project .

<http://vocab.ceda.ac.uk/collection/cci/project/cciproject_biomass> a cci:project,
        skos:Concept ;
    skos:altLabel "BIOMASS"@en ;
    skos:definition "The European Space Agency (ESA) Climate Change Initiative (CCI) Biomass project"@en ;
    skos:inScheme cci-scheme:project ;
    skos:prefLabel "above-ground biomass"@en ;
    skos:scopeNote "The European Space Agency (ESA) Climate Change Initiative (CCI) Biomass project"@en ;
    skos:topConceptOf cci-scheme:project .

<http://vocab.ceda.ac.uk/collection/cci/project/cciproject_cloud> a cci:project,
        skos:Concept ;
    skos:altLabel "CLOUD"@en ;
    skos:definition "The European Space Agency (ESA) Climate Change Initiative (CCI) Cloud project"@en ;
    skos:inScheme cci-scheme:project ;
    skos:prefLabel "cloud"@en ;
    skos:scopeNote "The European Space Agency (ESA) Climate Change Initiative (CCI) Cloud project"@en ;
    skos:topConceptOf cci-scheme:project .

<http://vocab.ceda.ac.uk/collection/cci/project/cciproject_fire> a cci:project,
        skos:Concept ;
    skos:altLabel "FIRE"@en ;
    skos:definition "The European Space Agency (ESA) Climate Change Initiative (CCI) Fire project"@en ;
    skos:inScheme cci-scheme:project ;
    skos:prefLabel "fire"@en ;
    skos:scopeNote "The European Space Agency (ESA) Climate Change Initiative (CCI) Fire project"@en ;
    skos:topConceptOf cci-scheme:project .

<http://vocab.ceda.ac.uk/collection/cci/project/cciproject_ghg> a cci:project,
        skos:Concept ;
    skos:altLabel "GHG"@en ;
    skos:definition "The European Space Agency (ESA) Climate Change Initiative (CCI) Greenhouse gases project"@en ;
    skos:inScheme cci-scheme:project ;
    skos:prefLabel "greenhouse gases"@en ;
    skos:scopeNote "The European Space Agency (ESA) Climate Change Initiative (CCI) Greenhouse gases project"@en ;
    skos:topConceptOf cci-scheme:project .

<http://vocab.ceda.ac.uk/collection/cci/project/cciproject_glaciers> a cci:project,
        skos:Concept ;
    skos:altLabel "GLACIERS"@en ;
    skos:definition "The European Space Agency (ESA) Climate Change Initiative (CCI) Glaciers project"@en ;
    skos:inScheme cci-scheme:project ;
    skos:prefLabel "glaciers"@en ;
    skos:scopeNote "The European Space Agency (ESA) Climate Change Initiative (CCI) Glaciers project"@en ;
    skos:topConceptOf cci-scheme:project .

<http://vocab.ceda.ac.uk/collection/cci/project/cciproject_iceSheet> a cci:project,
        skos:Concept ;
    skos:altLabel "ICESHEETS"@en ;
    skos:definition "The European Space Agency (ESA) Climate Change Initiative (CCI) Ice Sheets project"@en ;
    skos:inScheme cci-scheme:project ;
    skos:prefLabel "ice sheets"@en ;
    skos:scopeNote "The European Space Agency (ESA) Climate Change Initiative (CCI) Ice Sheets project"@en ;
    skos:topConceptOf cci-scheme:project .

<http://vocab.ceda.ac.uk/collection/cci/project/cciproject_lakes> a cci:project,
        skos:Concept ;
    skos:altLabel "LAKES"@en ;
    skos:definition "The European Space Agency (ESA) Climate Change Initiative (CCI) Lakes project"@en ;
    skos:inScheme cci-scheme:project ;
    skos:prefLabel "lakes"@en ;
    skos:scopeNote "The European Space Agency (ESA) Climate Change Initiative (CCI) Lakes project"@en ;
    skos:topConceptOf cci-scheme:project .

<http://vocab.ceda.ac.uk/collection/cci/project/cciproject_landCov> a cci:project,
        skos:Concept ;
    skos:altLabel "LC"@en ;
    skos:definition "The European Space Agency (ESA) Climate Change Initiative (CCI) Land Cover project"@en ;
    skos:inScheme cci-scheme:project ;
    skos:prefLabel "land cover"@en ;
    skos:scopeNote "The European Space Agency (ESA) Climate Change Initiative (CCI) Land Cover project"@en ;
    skos:topConceptOf cci-scheme:project .

<http://vocab.ceda.ac.uk/collection/cci/project/cciproject_landSurfTemp> a cci:project,
        skos:Concept ;
    skos:altLabel "LST"@en ;
    skos:definition "The European Space Agency (ESA) Climate Change Initiative (CCI) Land Surface Temperature project"@en ;
    skos:inScheme cci-scheme:project ;
    skos:prefLabel "land surface temperature"@en ;
    skos:scopeNote "The European Space Agency (ESA) Climate Change Initiative (CCI) Land Surface Temperature project"@en ;
    skos:topConceptOf cci-scheme:project .

<http://vocab.ceda.ac.uk/collection/cci/project/cciproject_oceanCol> a cci:project,
        skos:Concept ;
    skos:altLabel "OC"@en ;
    skos:definition "Ocean colour climate data record produced from satellite data as part of the European Space Agency (ESA) Climate Change Initiative (CCI)"@en ;
    skos:inScheme cci-scheme:project ;
    skos:prefLabel "ocean colour"@en ;
    skos:scopeNote "Ocean colour climate data record produced from satellite data as part of the European Space Agency (ESA) Climate Change Initiative (CCI)"@en ;
    skos:topConceptOf cci-scheme:project .

<http://vocab.ceda.ac.uk/collection/cci/project/cciproject_ozone> a cci:project,
        skos:Concept ;
    skos:altLabel "OZONE"@en ;
    skos:definition "The European Space Agency (ESA) Climate Change Initiative (CCI) Sea Level project"@en ;
    skos:inScheme cci-scheme:project ;
    skos:prefLabel "ozone"@en ;
    skos:scopeNote "The European Space Agency (ESA) Climate Change Initiative (CCI) Sea Level project"@en ;
    skos:topConceptOf cci-scheme:project .

<http://vocab.ceda.ac.uk/collection/cci/project/cciproject_permafrost> a cci:project,
        skos:Concept ;
    skos:altLabel "PERMAFROST"@en ;
    skos:definition "The European Space Agency (ESA) Climate Change Initiative (CCI) Permafrost project"@en ;
    skos:inScheme cci-scheme:project ;
    skos:prefLabel "permafrost"@en ;
    skos:scopeNote "The European Space Agency (ESA) Climate Change Initiative (CCI) Permafrost project"@en ;
    skos:topConceptOf cci-scheme:project .

<http://vocab.ceda.ac.uk/collection/cci/project/cciproject_reccap2> a cci:project,
        skos:Concept ;
    skos:altLabel "RECCAP-2"@en ;
    skos:definition "The European Space Agency (ESA) Climate Change Initiative (CCI) RECCAP-2 project"@en ;
    skos:inScheme cci-scheme:project ;
    skos:prefLabel "RECCAP2"@en ;
    skos:scopeNote "The European Space Agency (ESA) Climate Change Initiative (CCI) RECCAP-2 project"@en ;
    skos:topConceptOf cci-scheme:project .

<http://vocab.ceda.ac.uk/collection/cci/project/cciproject_riverDischarge> a cci:project,
        skos:Concept ;
    skos:altLabel "RD"@en ;
    skos:definition "The European Space Agency (ESA) Climate Change Initiative (CCI) River Discharge project"@en ;
    skos:inScheme cci-scheme:project ;
    skos:prefLabel "river discharge"@en ;
    skos:scopeNote "The European Space Agency (ESA) Climate Change Initiative (CCI) River Discharge project"@en ;
    skos:topConceptOf cci-scheme:project .

<http://vocab.ceda.ac.uk/collection/cci/project/cciproject_salinity> a cci:project,
        skos:Concept ;
    skos:altLabel "SEASURFACESALINITY"@en ;
    skos:definition "The European Space Agency (ESA) Climate Change Initiative (CCI) Salinity project"@en ;
    skos:inScheme cci-scheme:project ;
    skos:prefLabel "sea surface salinity"@en ;
    skos:scopeNote "The European Space Agency (ESA) Climate Change Initiative (CCI) Salinity project"@en ;
    skos:topConceptOf cci-scheme:project .

<http://vocab.ceda.ac.uk/collection/cci/project/cciproject_seaIce> a cci:project,
        skos:Concept ;
    skos:altLabel "SEAICE"@en ;
    skos:definition "The European Space Agency (ESA) Climate Change Initiative (CCI) Sea Ice project"@en ;
    skos:inScheme cci-scheme:project ;
    skos:prefLabel "sea ice"@en ;
    skos:scopeNote "The European Space Agency (ESA) Climate Change Initiative (CCI) Sea Ice project"@en ;
    skos:topConceptOf cci-scheme:project .

<http://vocab.ceda.ac.uk/collection/cci/project/cciproject_seaLevel> a cci:project,
        skos:Concept ;
    skos:altLabel "SEALEVEL"@en ;
    skos:definition "Sea level climate data record produced from satellite data as part of the European Space Agency (ESA) Climate Change Initiative (CCI)"@en ;
    skos:inScheme cci-scheme:project ;
    skos:prefLabel "sea level"@en ;
    skos:scopeNote "Sea level climate data record produced from satellite data as part of the European Space Agency (ESA) Climate Change Initiative (CCI)"@en ;
    skos:topConceptOf cci-scheme:project .

<http://vocab.ceda.ac.uk/collection/cci/project/cciproject_seaLevelBudgetClos> a cci:project,
        skos:Concept ;
    skos:altLabel "SLBC"@en ;
    skos:definition "The European Space Agency (ESA) Climate Change Initiative (CCI) Sea Level budget closure"@en ;
    skos:inScheme cci-scheme:project ;
    skos:prefLabel "sea level budget closure"@en ;
    skos:scopeNote "The European Space Agency (ESA) Climate Change Initiative (CCI) Sea Level budget closure"@en ;
    skos:topConceptOf cci-scheme:project .

<http://vocab.ceda.ac.uk/collection/cci/project/cciproject_seaState> a cci:project,
        skos:Concept ;
    skos:altLabel "SEASTATE"@en ;
    skos:definition "The European Space Agency (ESA) Climate Change Initiative (CCI) Sea State project"@en ;
    skos:inScheme cci-scheme:project ;
    skos:prefLabel "sea state"@en ;
    skos:scopeNote "The European Space Agency (ESA) Climate Change Initiative (CCI) Sea State project"@en ;
    skos:topConceptOf cci-scheme:project .

<http://vocab.ceda.ac.uk/collection/cci/project/cciproject_snow> a cci:project,
        skos:Concept ;
    skos:altLabel "SNOW"@en ;
    skos:definition "The European Space Agency (ESA) Climate Change Initiative (CCI) Snow project"@en ;
    skos:inScheme cci-scheme:project ;
    skos:prefLabel "snow"@en ;
    skos:scopeNote "The European Space Agency (ESA) Climate Change Initiative (CCI) Snow project"@en ;
    skos:topConceptOf cci-scheme:project .

<http://vocab.ceda.ac.uk/collection/cci/project/cciproject_soilMst> a cci:project,
        skos:Concept ;
    skos:altLabel "SOILMOISTURE"@en ;
    skos:definition "The European Space Agency (ESA) Climate Change Initiative (CCI) Soil Moisture project"@en ;
    skos:inScheme cci-scheme:project ;
    skos:prefLabel "soil moisture"@en ;
    skos:scopeNote "The European Space Agency (ESA) Climate Change Initiative (CCI) Soil Moisture project"@en ;
    skos:topConceptOf cci-scheme:project .

<http://vocab.ceda.ac.uk/collection/cci/project/cciproject_sst> a cci:project,
        skos:Concept ;
    skos:altLabel "SST"@en ;
    skos:definition "The European Space Agency (ESA) Climate Change Initiative (CCI) Sea Surface Temperature project"@en ;
    skos:inScheme cci-scheme:project ;
    skos:prefLabel "sea surface temperature"@en ;
    skos:scopeNote "The European Space Agency (ESA) Climate Change Initiative (CCI) Sea Surface Temperature project"@en ;
    skos:topConceptOf cci-scheme:project .

<http://vocab.ceda.ac.uk/collection/cci/project/cciproject_vegParam> a cci:project,
        skos:Concept ;
    skos:altLabel "VEGETATION"@en ;
    skos:definition "The European Space Agency (ESA) Climate Change Initiative (CCI) Vegetation Parameters project"@en ;
    skos:inScheme cci-scheme:project ;
    skos:prefLabel "vegetation parameters"@en ;
    skos:scopeNote "The European Space Agency (ESA) Climate Change Initiative (CCI) Vegetation Parameters project"@en ;
    skos:topConceptOf cci-scheme:project .

<http://vocab.ceda.ac.uk/collection/cci/project/cciproject_waterVapour> a cci:project,
        skos:Concept ;
    skos:altLabel "WATERVAPOUR"@en ;
    skos:definition "The European Space Agency (ESA) Climate Change Initiative (CCI) Water Vapour project"@en ;
    skos:inScheme cci-scheme:project ;
    skos:prefLabel "water vapour"@en ;
    skos:scopeNote "The European Space Agency (ESA) Climate Change Initiative (CCI) Water Vapour project"@en ;
    skos:topConceptOf cci-scheme:project .

cci-scheme:project a skos:ConceptScheme ;
    dc:creator "Science and Technology Facilities Council" ;
    dc:date "2025-05-30" ;
    dc:description "<p>The CCI concept schemes are used to define concepts within an element of a Directory Reference Scheme. There are currently 11 concept schemes defined: <a href=../dataType>data type</a>, <a href=..//ecv>ecv</a>, <a href=../scheme/cci/freq>frequency</a>, <a href=../org>institutes</a>, <a href=../platform>platforms</a>, <a href=../platformGrp>platform groups</a>, <a href=../platformProg>platform programmes</a>, <a href=../procLev>processing levels</a>, <a href=../product>products</a>, <a href=../project>projects</a>,  and <a href=../sensor>sensors</a>. The use of a concept scheme allows easy navigation up and down the tree.</p><p>As well as being concepts, all of the concepts are also named individuals of the <a href=../../../ontology/cci>CCI Ontology</a> classes.</p>" ;
    dc:publisher "STFC"@en ;
    dc:rights "This work is licensed under a BSD license."@en ;
    dc:title "Project" ;
    rdfs:comment "This concept scheme represents the projects in the CCI project" ;
    owl:versionInfo "0.0.1" ;
    skos:definition "The different projects within the ESA Climate Change Initiative (CCI)."@en ;
    skos:hasTopConcept <http://vocab.ceda.ac.uk/collection/cci/project/cciproject_aerosol>,
        <http://vocab.ceda.ac.uk/collection/cci/project/cciproject_biomass>,
        <http://vocab.ceda.ac.uk/collection/cci/project/cciproject_cloud>,
        <http://vocab.ceda.ac.uk/collection/cci/project/cciproject_fire>,
        <http://vocab.ceda.ac.uk/collection/cci/project/cciproject_ghg>,
        <http://vocab.ceda.ac.uk/collection/cci/project/cciproject_glaciers>,
        <http://vocab.ceda.ac.uk/collection/cci/project/cciproject_iceSheet>,
        <http://vocab.ceda.ac.uk/collection/cci/project/cciproject_lakes>,
        <http://vocab.ceda.ac.uk/collection/cci/project/cciproject_landCov>,
        <http://vocab.ceda.ac.uk/collection/cci/project/cciproject_landSurfTemp>,
        <http://vocab.ceda.ac.uk/collection/cci/project/cciproject_oceanCol>,
        <http://vocab.ceda.ac.uk/collection/cci/project/cciproject_ozone>,
        <http://vocab.ceda.ac.uk/collection/cci/project/cciproject_permafrost>,
        <http://vocab.ceda.ac.uk/collection/cci/project/cciproject_reccap2>,
        <http://vocab.ceda.ac.uk/collection/cci/project/cciproject_riverDischarge>,
        <http://vocab.ceda.ac.uk/collection/cci/project/cciproject_salinity>,
        <http://vocab.ceda.ac.uk/collection/cci/project/cciproject_seaIce>,
        <http://vocab.ceda.ac.uk/collection/cci/project/cciproject_seaLevel>,
        <http://vocab.ceda.ac.uk/collection/cci/project/cciproject_seaLevelBudgetClos>,
        <http://vocab.ceda.ac.uk/collection/cci/project/cciproject_seaState>,
        <http://vocab.ceda.ac.uk/collection/cci/project/cciproject_snow>,
        <http://vocab.ceda.ac.uk/collection/cci/project/cciproject_soilMst>,
        <http://vocab.ceda.ac.uk/collection/cci/project/cciproject_sst>,
        <http://vocab.ceda.ac.uk/collection/cci/project/cciproject_vegParam>,
        <http://vocab.ceda.ac.uk/collection/cci/project/cciproject_waterVapour> ;
    skos:prefLabel "Project"@en .

